# baseURI: http://toop.eu/organization
# imports: file:///C:/Users/veerrjjd/TBCMEWorkspace/TopBraid/SKOS/skos-core.ttl.tbc
# imports: http://spinrdf.org/spin
# imports: https://www.w3.org/2009/08/skos-reference/skos.rdf
# prefix: toop

@prefix adms: <http://www.w3.org/ns/adms#> .
@prefix dc: <http://purl.org/dc/elements/1.1/> .
@prefix dcam: <http://purl.org/dc/dcam/> .
@prefix dcat: <http://www.w3.org/ns/dcat#> .
@prefix dct: <http://purl.org/dc/terms/> .
@prefix dcterms: <http://purl.org/dc/terms/> .
@prefix elobr: <http://example.register.elo/elonia-business-register#> .
@prefix foaf: <http://xmlns.com/foaf/0.1/> .
@prefix freebr: <http://example.register.fre/freedonia-business-register#> .
@prefix gr: <http://purl.org/goodrelations/v1#> .
@prefix nhr: <http://example.register.nl/nationaalhandelsregister#> .
@prefix org: <http://www.w3.org/ns/org#> .
@prefix owl: <http://www.w3.org/2002/07/owl#> .
@prefix owlTime: <http://www.w3.org/2006/time#> .
@prefix prov: <http://www.w3.org/ns/prov#> .
@prefix rdf: <http://www.w3.org/1999/02/22-rdf-syntax-ns#> .
@prefix rdfs: <http://www.w3.org/2000/01/rdf-schema#> .
@prefix rov: <http://www.w3.org/ns/regorg#> .
@prefix schema: <http://schema.org/> .
@prefix skos: <http://www.w3.org/2004/02/skos/core#> .
@prefix skosxl: <http://www.w3.org/2008/05/skos-xl#> .
@prefix sp: <http://spinrdf.org/sp#> .
@prefix spin: <http://spinrdf.org/spin#> .
@prefix toop: <http://toop.eu/organization#> .
@prefix vann: <http://purl.org/vocab/vann/> .
@prefix vcard: <http://www.w3.org/2006/vcard/ns#> .
@prefix voaf: <http://purl.org/vocommons/voaf#> .
@prefix vs: <http://www.w3.org/2003/06/sw-vocab-status/ns#> .
@prefix wdrs: <http://www.w3.org/2007/05/powder-s#> .
@prefix wgs: <http://www.w3.org/2003/01/geo/wgs84_pos#> .
@prefix wot: <http://xmlns.com/wot/0.1/> .
@prefix xml: <http://www.w3.org/XML/1998/namespace> .
@prefix xsd: <http://www.w3.org/2001/XMLSchema#> .

<http://andrea-perego.name/>
  rdf:type schema:CreativeWork ;
  rdf:type foaf:Document ;
  foaf:primaryTopic _:b937381 ;
  foaf:primaryTopic _:b937505 ;
  foaf:primaryTopic _:b937610 ;
  foaf:primaryTopic _:b938234 ;
  foaf:topic _:b937381 ;
  foaf:topic _:b937505 ;
  foaf:topic _:b937610 ;
  foaf:topic _:b938234 ;
.
<http://example.register.elo/elonia-business-register>
  owl:versionInfo "Created with TopBraid Composer" ;
.
elobr:Company
  rdf:type owl:Class ;
  rdfs:comment "A company is an organisation with a business character with a goal to make profit by producing products or providing services."@en ;
  rdfs:label "Company"@en ;
  rdfs:subClassOf skos:Concept ;
  rdfs:subClassOf _:b213787 ;
  rdfs:subClassOf _:b772676 ;
.
elobr:EloniaActivityDeclaration
  rdf:type owl:ObjectProperty ;
  rdfs:comment "The description of the main activity of the company as free text description recorded on the registry. This tag should be used to give a description of the company activity in the local language. This should be used in conjunction with the CompanyNaceCode."@en ;
  rdfs:label "Elonia activity declaration"@en ;
  rdfs:subPropertyOf dc:description ;
  rdfs:subPropertyOf dcterms:description ;
  owl:equivalentProperty freebr:FreedoniaActivityDeclaration ;
  owl:equivalentProperty toop:activityDeclaration ;
.
elobr:EloniaAddress
  rdf:type owl:Class ;
  rdfs:comment "The postal address and/or the visiting address of a physical site of the company, or, an virtual address, i.e., an URL."@en ;
  rdfs:label "Company address"@en ;
  rdfs:subClassOf owl:Thing ;
  owl:equivalentClass freebr:FreedoniaAddress ;
  owl:equivalentClass toop:Address ;
  owl:equivalentClass vcard:Address ;
  owl:equivalentClass _:b49042 ;
.
elobr:EloniaBusinessCode
  rdf:type rdfs:Class ;
  rdfs:comment "The unique official company identifier_"@en ;
  rdfs:label "Elonia business code" ;
  rdfs:label "Elonia business code"@en ;
  rdfs:subClassOf toop:CompanyCode ;
  owl:equivalentClass freebr:FreedoniaBusinessCode ;
  owl:equivalentClass toop:CompanyCode ;
  skos:prefLabel "Elonia business code" ;
.
elobr:EloniaCompanyNaceCode
  rdf:type owl:ObjectProperty ;
  rdfs:comment "The description of the main activity of the company as free text description recorded on the registry. This tag should be used to give a description of the company activity in the local language. This should be used in conjunction with the CompanyNaceCode"@en ;
  rdfs:domain dcterms:Agent ;
  rdfs:domain owl:Thing ;
  rdfs:domain org:Organization ;
  rdfs:domain foaf:Agent ;
  rdfs:domain foaf:Organization ;
  rdfs:domain _:b420951 ;
  rdfs:domain _:b421075 ;
  rdfs:domain _:b421664 ;
  rdfs:domain _:b421928 ;
  rdfs:domain _:b937877 ;
  rdfs:domain _:b938265 ;
  rdfs:label "Elonia company NACE Code"@en ;
  rdfs:range owl:Thing ;
  rdfs:range skos:Concept ;
  rdfs:range _:b327858 ;
  rdfs:subPropertyOf org:classification ;
  rdfs:subPropertyOf rov:orgActivity ;
  owl:equivalentProperty freebr:FreedoniaCompanyNaceCode ;
  owl:equivalentProperty toop:companyNaceCode ;
.
elobr:EloniaCompanyName
  rdf:type owl:DatatypeProperty ;
  rdfs:comment "All companies have to provide an Elonia company name upon registration at the Elonia business register." ;
  rdfs:domain elobr:Company ;
  rdfs:domain freebr:Company ;
  rdfs:domain dcterms:Agent ;
  rdfs:domain owl:Thing ;
  rdfs:domain skos:Concept ;
  rdfs:domain org:FormalOrganization ;
  rdfs:domain org:Organization ;
  rdfs:domain foaf:Agent ;
  rdfs:domain foaf:Organization ;
  rdfs:domain _:b156576 ;
  rdfs:domain _:b213787 ;
  rdfs:domain _:b327858 ;
  rdfs:domain _:b420951 ;
  rdfs:domain _:b421075 ;
  rdfs:domain _:b421664 ;
  rdfs:domain _:b421928 ;
  rdfs:domain _:b772676 ;
  rdfs:domain _:b883411 ;
  rdfs:domain _:b937877 ;
  rdfs:domain _:b938265 ;
  rdfs:label "company name"@en ;
  rdfs:range rdfs:Literal ;
  rdfs:range xsd:string ;
  rdfs:subPropertyOf toop:companyName ;
  rdfs:subPropertyOf rov:legalName ;
  owl:equivalentProperty freebr:FreedoniaCompanyName ;
  owl:equivalentProperty toop:companyName ;
  skos:prefLabel "company name"@en ;
.
elobr:EloniaCompanyType
  rdf:type owl:ObjectProperty ;
  rdfs:comment "The legal type of the company_"@en ;
  rdfs:domain elobr:Company ;
  rdfs:domain freebr:Company ;
  rdfs:domain dcterms:Agent ;
  rdfs:domain toop:RegisteredOrganization ;
  rdfs:domain owl:Thing ;
  rdfs:domain skos:Concept ;
  rdfs:domain org:FormalOrganization ;
  rdfs:domain org:Organization ;
  rdfs:domain rov:RegisteredOrganization ;
  rdfs:domain foaf:Agent ;
  rdfs:domain foaf:Organization ;
  rdfs:domain _:b156576 ;
  rdfs:domain _:b180769 ;
  rdfs:domain _:b213787 ;
  rdfs:domain _:b254570 ;
  rdfs:domain _:b327858 ;
  rdfs:domain _:b420951 ;
  rdfs:domain _:b421075 ;
  rdfs:domain _:b421664 ;
  rdfs:domain _:b421928 ;
  rdfs:domain _:b454254 ;
  rdfs:domain _:b772676 ;
  rdfs:domain _:b826282 ;
  rdfs:domain _:b826680 ;
  rdfs:domain _:b883411 ;
  rdfs:domain _:b937877 ;
  rdfs:domain _:b938265 ;
  rdfs:label "company type"@en ;
  rdfs:range owl:Thing ;
  rdfs:range skos:Concept ;
  rdfs:range _:b327858 ;
  rdfs:range _:b875853 ;
  rdfs:subPropertyOf org:classification ;
  owl:equivalentProperty freebr:FreedoniaCompanyType ;
  owl:equivalentProperty toop:companyType ;
  owl:equivalentProperty rov:orgType ;
.
elobr:EloniaLegalStatus
  rdf:type owl:ObjectProperty ;
  rdfs:comment "The legal status of the company"@en ;
  rdfs:domain elobr:Company ;
  rdfs:domain elobr:EloniaBusinessCode ;
  rdfs:domain freebr:Company ;
  rdfs:domain freebr:FreedoniaBusinessCode ;
  rdfs:domain dcterms:Agent ;
  rdfs:domain toop:CompanyCode ;
  rdfs:domain owl:Thing ;
  rdfs:domain skos:Concept ;
  rdfs:domain adms:Identifier ;
  rdfs:domain org:Organization ;
  rdfs:domain foaf:Agent ;
  rdfs:domain foaf:Organization ;
  rdfs:domain _:b156576 ;
  rdfs:domain _:b213787 ;
  rdfs:domain _:b327858 ;
  rdfs:domain _:b420951 ;
  rdfs:domain _:b421075 ;
  rdfs:domain _:b421664 ;
  rdfs:domain _:b421928 ;
  rdfs:domain _:b772676 ;
  rdfs:domain _:b883411 ;
  rdfs:domain _:b937877 ;
  rdfs:domain _:b938265 ;
  rdfs:label "company legal status"@en ;
  rdfs:range owl:Thing ;
  rdfs:range skos:Concept ;
  rdfs:range _:b327858 ;
  rdfs:subPropertyOf org:classification ;
  owl:equivalentProperty freebr:FreedoniaLegalStatus ;
  owl:equivalentProperty toop:legalStatus ;
  owl:equivalentProperty rov:orgStatus ;
.
elobr:EloniaLegalStatusEffectiveDate
  rdf:type owl:ObjectProperty ;
  rdfs:comment "The date at which the current legal status became effective_"@en ;
  rdfs:domain elobr:Company ;
  rdfs:domain elobr:EloniaBusinessCode ;
  rdfs:domain freebr:Company ;
  rdfs:domain freebr:FreedoniaBusinessCode ;
  rdfs:domain toop:CompanyCode ;
  rdfs:domain owl:Thing ;
  rdfs:domain skos:Concept ;
  rdfs:domain adms:Identifier ;
  rdfs:domain _:b156576 ;
  rdfs:domain _:b213787 ;
  rdfs:domain _:b327858 ;
  rdfs:domain _:b772676 ;
  rdfs:domain _:b883411 ;
  rdfs:label "Elonia legal status effective date"@en ;
  rdfs:range rdfs:Literal ;
  rdfs:subPropertyOf dc:date ;
  rdfs:subPropertyOf dcterms:date ;
  rdfs:subPropertyOf dcterms:issued ;
  owl:equivalentProperty freebr:FreedoniaLegalStatusEffectiveDate ;
  owl:equivalentProperty toop:legalStatusEffectiveDate ;
.
elobr:EloniaRegistrationAuthority
  rdf:type owl:ObjectProperty ;
  rdfs:comment "The reference to the official register that has registered the company"@en ;
  rdfs:domain elobr:EloniaBusinessCode ;
  rdfs:domain freebr:FreedoniaBusinessCode ;
  rdfs:domain toop:CompanyCode ;
  rdfs:domain owl:Thing ;
  rdfs:domain adms:Identifier ;
  rdfs:label "registration authority"@en ;
  rdfs:range dcterms:Agent ;
  rdfs:range owl:Thing ;
  rdfs:range foaf:Agent ;
  rdfs:range _:b420951 ;
  rdfs:range _:b421075 ;
  rdfs:range _:b421664 ;
  rdfs:range _:b421928 ;
  rdfs:range _:b937877 ;
  rdfs:range _:b938265 ;
  rdfs:subPropertyOf dc:contributor ;
  rdfs:subPropertyOf dc:creator ;
  rdfs:subPropertyOf dcterms:contributor ;
  owl:equivalentProperty freebr:FreedoniaRegistrationAuthority ;
  owl:equivalentProperty dcterms:creator ;
  owl:equivalentProperty toop:registrationAuthority ;
  owl:equivalentProperty foaf:maker ;
.
elobr:EloniaRegistrationDate
  rdf:type owl:DatatypeProperty ;
  rdfs:comment "Represents the date at which the company started."@en ;
  rdfs:domain toop:Registration ;
  rdfs:domain owl:Thing ;
  rdfs:domain org:ChangeEvent ;
  rdfs:domain prov:Activity ;
  rdfs:domain _:b53184 ;
  rdfs:domain _:b170340 ;
  rdfs:domain _:b399839 ;
  rdfs:domain _:b715640 ;
  rdfs:domain _:b895567 ;
  rdfs:domain _:b897711 ;
  rdfs:label "Elonia registration date"@en ;
  rdfs:range xsd:date ;
  rdfs:range xsd:dateTime ;
  rdfs:range _:b115973 ;
  rdfs:range _:b148299 ;
  rdfs:range _:b671381 ;
  rdfs:range _:b719479 ;
  rdfs:subPropertyOf prov:startedAtTime ;
  owl:equivalentProperty freebr:FreedoniaRegistrationDate ;
  owl:equivalentProperty toop:registrationDate ;
.
elobr:EloniaRegistrationNumber
  rdf:type owl:DatatypeProperty ;
  rdfs:comment "The number of the company as recorded on the register. In some jurisdictions, the number on the register may be different from the official company number. This field must be populated in all service requests even when the RegistrationNumber is the same as the CompanyCode"@en ;
  rdfs:domain dcterms:Agent ;
  rdfs:domain owl:Thing ;
  rdfs:domain org:Organization ;
  rdfs:domain foaf:Agent ;
  rdfs:domain foaf:Organization ;
  rdfs:domain _:b420951 ;
  rdfs:domain _:b421075 ;
  rdfs:domain _:b421664 ;
  rdfs:domain _:b421928 ;
  rdfs:domain _:b937877 ;
  rdfs:domain _:b938265 ;
  rdfs:label "Elonia registration number"@en ;
  rdfs:subPropertyOf skos:notation ;
  owl:equivalentProperty freebr:FreedoniaRegistrationNumber ;
  owl:equivalentProperty toop:registrationNumber ;
  owl:equivalentProperty org:identifier ;
.
elobr:EloniaSSNumber
  rdf:type rdfs:Class ;
  rdfs:comment "The social security number of the company_"@en ;
  rdfs:label "Social security number"@en ;
  rdfs:subClassOf rdfs:Resource ;
  owl:equivalentClass freebr:FreedoniaSSNumber ;
  owl:equivalentClass toop:SSNumber ;
.
elobr:EloniaVATNumber
  rdf:type rdfs:Class ;
  rdfs:comment "The value added tax number of the company"@en ;
  rdfs:label "VAT number"@en ;
  rdfs:subClassOf rdfs:Resource ;
  owl:equivalentClass freebr:FreedoniaVATNumber ;
  owl:equivalentClass toop:VATNumber ;
.
elobr:hasBusinessCode
  rdf:type owl:ObjectProperty ;
  rdfs:comment "All companies get an Elonia Business Code uponregistration at the Elonia business register." ;
  rdfs:domain elobr:Company ;
  rdfs:domain dcterms:Agent ;
  rdfs:domain owl:Thing ;
  rdfs:domain skos:Concept ;
  rdfs:domain org:FormalOrganization ;
  rdfs:domain org:Organization ;
  rdfs:domain rov:RegisteredOrganization ;
  rdfs:domain foaf:Agent ;
  rdfs:domain foaf:Organization ;
  rdfs:domain _:b213787 ;
  rdfs:domain _:b327858 ;
  rdfs:domain _:b420951 ;
  rdfs:domain _:b421075 ;
  rdfs:domain _:b421664 ;
  rdfs:domain _:b421928 ;
  rdfs:domain _:b772676 ;
  rdfs:domain _:b937877 ;
  rdfs:domain _:b938265 ;
  rdfs:label "has business code"@en ;
  rdfs:range elobr:EloniaBusinessCode ;
  rdfs:range freebr:FreedoniaBusinessCode ;
  rdfs:range toop:CompanyCode ;
  rdfs:range owl:Thing ;
  rdfs:range adms:Identifier ;
  rdfs:subPropertyOf toop:hasCompanyCode ;
  rdfs:subPropertyOf adms:identifier ;
  rdfs:subPropertyOf rov:registration ;
  skos:prefLabel "has business code"@en ;
.
<http://example.register.fre/freedonia-business-register>
  owl:versionInfo "Created with TopBraid Composer" ;
.
freebr:Company
  rdf:type owl:Class ;
  rdfs:comment "A company is an organisation with a business character with a goal to make profit by producing products or providing services."@en ;
  rdfs:label "Company"@en ;
  rdfs:subClassOf skos:Concept ;
  rdfs:subClassOf _:b156576 ;
  rdfs:subClassOf _:b883411 ;
.
freebr:FreedoniaActivityDeclaration
  rdf:type owl:ObjectProperty ;
  rdfs:comment "The description of the main activity of the company as free text description recorded on the registry. This tag should be used to give a description of the company activity in the local language. This should be used in conjunction with the CompanyNaceCode."@en ;
  rdfs:label "Freedonia activity declaration"@en ;
  rdfs:subPropertyOf dc:description ;
  rdfs:subPropertyOf dcterms:description ;
  owl:equivalentProperty elobr:EloniaActivityDeclaration ;
  owl:equivalentProperty toop:activityDeclaration ;
.
freebr:FreedoniaAddress
  rdf:type owl:Class ;
  rdfs:comment "The postal address and/or the visiting address of a physical site of the company, or, an virtual address, i.e., an URL."@en ;
  rdfs:label "Company address"@en ;
  rdfs:subClassOf owl:Thing ;
  owl:equivalentClass elobr:EloniaAddress ;
  owl:equivalentClass toop:Address ;
  owl:equivalentClass vcard:Address ;
  owl:equivalentClass _:b49042 ;
.
freebr:FreedoniaBusinessCode
  rdf:type rdfs:Class ;
  rdfs:comment "The unique official company identifier_"@en ;
  rdfs:label "Elonia business code"@en ;
  rdfs:label "Freedonia business code" ;
  rdfs:subClassOf toop:CompanyCode ;
  owl:equivalentClass elobr:EloniaBusinessCode ;
  owl:equivalentClass toop:CompanyCode ;
  skos:prefLabel "Freedonia business code" ;
.
freebr:FreedoniaCompanyNaceCode
  rdf:type owl:ObjectProperty ;
  rdfs:comment "The description of the main activity of the company as free text description recorded on the registry. This tag should be used to give a description of the company activity in the local language. This should be used in conjunction with the CompanyNaceCode"@en ;
  rdfs:domain dcterms:Agent ;
  rdfs:domain owl:Thing ;
  rdfs:domain org:Organization ;
  rdfs:domain foaf:Agent ;
  rdfs:domain foaf:Organization ;
  rdfs:domain _:b420951 ;
  rdfs:domain _:b421075 ;
  rdfs:domain _:b421664 ;
  rdfs:domain _:b421928 ;
  rdfs:domain _:b937877 ;
  rdfs:domain _:b938265 ;
  rdfs:label "Freedonia company NACE code"@en ;
  rdfs:range owl:Thing ;
  rdfs:range skos:Concept ;
  rdfs:range _:b327858 ;
  rdfs:subPropertyOf org:classification ;
  rdfs:subPropertyOf rov:orgActivity ;
  owl:equivalentProperty elobr:EloniaCompanyNaceCode ;
  owl:equivalentProperty toop:companyNaceCode ;
.
freebr:FreedoniaCompanyName
  rdf:type owl:DatatypeProperty ;
  rdfs:comment "All companies have to provide an Freedonia company name upon registration at the Frreedonia business register." ;
  rdfs:domain elobr:Company ;
  rdfs:domain freebr:Company ;
  rdfs:domain dcterms:Agent ;
  rdfs:domain owl:Thing ;
  rdfs:domain skos:Concept ;
  rdfs:domain org:FormalOrganization ;
  rdfs:domain org:Organization ;
  rdfs:domain foaf:Agent ;
  rdfs:domain foaf:Organization ;
  rdfs:domain _:b156576 ;
  rdfs:domain _:b213787 ;
  rdfs:domain _:b327858 ;
  rdfs:domain _:b420951 ;
  rdfs:domain _:b421075 ;
  rdfs:domain _:b421664 ;
  rdfs:domain _:b421928 ;
  rdfs:domain _:b772676 ;
  rdfs:domain _:b883411 ;
  rdfs:domain _:b937877 ;
  rdfs:domain _:b938265 ;
  rdfs:label "company name"@en ;
  rdfs:range rdfs:Literal ;
  rdfs:range xsd:string ;
  rdfs:subPropertyOf toop:companyName ;
  rdfs:subPropertyOf rov:legalName ;
  owl:equivalentProperty elobr:EloniaCompanyName ;
  owl:equivalentProperty toop:companyName ;
.
freebr:FreedoniaCompanyType
  rdf:type owl:ObjectProperty ;
  rdfs:comment "The legal type of the company_"@en ;
  rdfs:domain elobr:Company ;
  rdfs:domain freebr:Company ;
  rdfs:domain dcterms:Agent ;
  rdfs:domain toop:RegisteredOrganization ;
  rdfs:domain owl:Thing ;
  rdfs:domain skos:Concept ;
  rdfs:domain org:FormalOrganization ;
  rdfs:domain org:Organization ;
  rdfs:domain rov:RegisteredOrganization ;
  rdfs:domain foaf:Agent ;
  rdfs:domain foaf:Organization ;
  rdfs:domain _:b156576 ;
  rdfs:domain _:b180769 ;
  rdfs:domain _:b213787 ;
  rdfs:domain _:b254570 ;
  rdfs:domain _:b327858 ;
  rdfs:domain _:b420951 ;
  rdfs:domain _:b421075 ;
  rdfs:domain _:b421664 ;
  rdfs:domain _:b421928 ;
  rdfs:domain _:b454254 ;
  rdfs:domain _:b772676 ;
  rdfs:domain _:b826282 ;
  rdfs:domain _:b826680 ;
  rdfs:domain _:b883411 ;
  rdfs:domain _:b937877 ;
  rdfs:domain _:b938265 ;
  rdfs:label "company type"@en ;
  rdfs:range owl:Thing ;
  rdfs:range skos:Concept ;
  rdfs:range _:b327858 ;
  rdfs:range _:b875853 ;
  rdfs:subPropertyOf org:classification ;
  owl:equivalentProperty elobr:EloniaCompanyType ;
  owl:equivalentProperty toop:companyType ;
  owl:equivalentProperty rov:orgType ;
.
freebr:FreedoniaLegalStatus
  rdf:type owl:ObjectProperty ;
  rdfs:comment "The legal status of the company"@en ;
  rdfs:domain elobr:Company ;
  rdfs:domain elobr:EloniaBusinessCode ;
  rdfs:domain freebr:Company ;
  rdfs:domain freebr:FreedoniaBusinessCode ;
  rdfs:domain dcterms:Agent ;
  rdfs:domain toop:CompanyCode ;
  rdfs:domain owl:Thing ;
  rdfs:domain skos:Concept ;
  rdfs:domain adms:Identifier ;
  rdfs:domain org:Organization ;
  rdfs:domain foaf:Agent ;
  rdfs:domain foaf:Organization ;
  rdfs:domain _:b156576 ;
  rdfs:domain _:b213787 ;
  rdfs:domain _:b327858 ;
  rdfs:domain _:b420951 ;
  rdfs:domain _:b421075 ;
  rdfs:domain _:b421664 ;
  rdfs:domain _:b421928 ;
  rdfs:domain _:b772676 ;
  rdfs:domain _:b883411 ;
  rdfs:domain _:b937877 ;
  rdfs:domain _:b938265 ;
  rdfs:label "company legal status"@en ;
  rdfs:range owl:Thing ;
  rdfs:range skos:Concept ;
  rdfs:range _:b327858 ;
  rdfs:subPropertyOf org:classification ;
  owl:equivalentProperty elobr:EloniaLegalStatus ;
  owl:equivalentProperty toop:legalStatus ;
  owl:equivalentProperty rov:orgStatus ;
.
freebr:FreedoniaLegalStatusEffectiveDate
  rdf:type owl:ObjectProperty ;
  rdfs:comment "The date at which the current legal status became effective_"@en ;
  rdfs:domain elobr:Company ;
  rdfs:domain elobr:EloniaBusinessCode ;
  rdfs:domain freebr:Company ;
  rdfs:domain freebr:FreedoniaBusinessCode ;
  rdfs:domain toop:CompanyCode ;
  rdfs:domain owl:Thing ;
  rdfs:domain skos:Concept ;
  rdfs:domain adms:Identifier ;
  rdfs:domain _:b156576 ;
  rdfs:domain _:b213787 ;
  rdfs:domain _:b327858 ;
  rdfs:domain _:b772676 ;
  rdfs:domain _:b883411 ;
  rdfs:label "Freedonia legal status effective date"@en ;
  rdfs:range rdfs:Literal ;
  rdfs:subPropertyOf dc:date ;
  rdfs:subPropertyOf dcterms:date ;
  rdfs:subPropertyOf dcterms:issued ;
  owl:equivalentProperty elobr:EloniaLegalStatusEffectiveDate ;
  owl:equivalentProperty toop:legalStatusEffectiveDate ;
.
freebr:FreedoniaRegistrationAuthority
  rdf:type owl:ObjectProperty ;
  rdfs:comment "The reference to the official register that has registered the company"@en ;
  rdfs:domain elobr:EloniaBusinessCode ;
  rdfs:domain freebr:FreedoniaBusinessCode ;
  rdfs:domain toop:CompanyCode ;
  rdfs:domain owl:Thing ;
  rdfs:domain adms:Identifier ;
  rdfs:label "registration authority"@en ;
  rdfs:range dcterms:Agent ;
  rdfs:range owl:Thing ;
  rdfs:range foaf:Agent ;
  rdfs:range _:b420951 ;
  rdfs:range _:b421075 ;
  rdfs:range _:b421664 ;
  rdfs:range _:b421928 ;
  rdfs:range _:b937877 ;
  rdfs:range _:b938265 ;
  rdfs:subPropertyOf dc:contributor ;
  rdfs:subPropertyOf dc:creator ;
  rdfs:subPropertyOf dcterms:contributor ;
  owl:equivalentProperty elobr:EloniaRegistrationAuthority ;
  owl:equivalentProperty dcterms:creator ;
  owl:equivalentProperty toop:registrationAuthority ;
  owl:equivalentProperty foaf:maker ;
.
freebr:FreedoniaRegistrationDate
  rdf:type owl:DatatypeProperty ;
  rdfs:comment "Represents the date at which the company started."@en ;
  rdfs:domain toop:Registration ;
  rdfs:domain owl:Thing ;
  rdfs:domain org:ChangeEvent ;
  rdfs:domain prov:Activity ;
  rdfs:domain _:b53184 ;
  rdfs:domain _:b170340 ;
  rdfs:domain _:b399839 ;
  rdfs:domain _:b715640 ;
  rdfs:domain _:b895567 ;
  rdfs:domain _:b897711 ;
  rdfs:label "Freedonia registration date"@en ;
  rdfs:range xsd:date ;
  rdfs:range xsd:dateTime ;
  rdfs:range _:b115973 ;
  rdfs:range _:b148299 ;
  rdfs:range _:b671381 ;
  rdfs:range _:b719479 ;
  rdfs:subPropertyOf prov:startedAtTime ;
  owl:equivalentProperty elobr:EloniaRegistrationDate ;
  owl:equivalentProperty toop:registrationDate ;
.
freebr:FreedoniaRegistrationNumber
  rdf:type owl:DatatypeProperty ;
  rdfs:comment "The number of the company as recorded on the register. In some jurisdictions, the number on the register may be different from the official company number. This field must be populated in all service requests even when the RegistrationNumber is the same as the CompanyCode"@en ;
  rdfs:domain dcterms:Agent ;
  rdfs:domain owl:Thing ;
  rdfs:domain org:Organization ;
  rdfs:domain foaf:Agent ;
  rdfs:domain foaf:Organization ;
  rdfs:domain _:b420951 ;
  rdfs:domain _:b421075 ;
  rdfs:domain _:b421664 ;
  rdfs:domain _:b421928 ;
  rdfs:domain _:b937877 ;
  rdfs:domain _:b938265 ;
  rdfs:label "Freeodina registration number"@en ;
  rdfs:subPropertyOf skos:notation ;
  owl:equivalentProperty elobr:EloniaRegistrationNumber ;
  owl:equivalentProperty toop:registrationNumber ;
  owl:equivalentProperty org:identifier ;
.
freebr:FreedoniaSSNumber
  rdf:type rdfs:Class ;
  rdfs:comment "The social security number of the company_"@en ;
  rdfs:label "Social security number"@en ;
  rdfs:subClassOf rdfs:Resource ;
  owl:equivalentClass elobr:EloniaSSNumber ;
  owl:equivalentClass toop:SSNumber ;
.
freebr:FreedoniaVATNumber
  rdf:type rdfs:Class ;
  rdfs:comment "The value added tax number of the company"@en ;
  rdfs:label "VAT number"@en ;
  rdfs:subClassOf rdfs:Resource ;
  owl:equivalentClass elobr:EloniaVATNumber ;
  owl:equivalentClass toop:VATNumber ;
.
freebr:hasBusinessCode
  rdf:type owl:ObjectProperty ;
  rdfs:comment "All companies get an Freedonia Business Code uponregistration at the Freedonia business register." ;
  rdfs:domain freebr:Company ;
  rdfs:domain dcterms:Agent ;
  rdfs:domain owl:Thing ;
  rdfs:domain skos:Concept ;
  rdfs:domain org:FormalOrganization ;
  rdfs:domain org:Organization ;
  rdfs:domain rov:RegisteredOrganization ;
  rdfs:domain foaf:Agent ;
  rdfs:domain foaf:Organization ;
  rdfs:domain _:b156576 ;
  rdfs:domain _:b327858 ;
  rdfs:domain _:b420951 ;
  rdfs:domain _:b421075 ;
  rdfs:domain _:b421664 ;
  rdfs:domain _:b421928 ;
  rdfs:domain _:b883411 ;
  rdfs:domain _:b937877 ;
  rdfs:domain _:b938265 ;
  rdfs:label "has business code"@en ;
  rdfs:range elobr:EloniaBusinessCode ;
  rdfs:range freebr:FreedoniaBusinessCode ;
  rdfs:range toop:CompanyCode ;
  rdfs:range owl:Thing ;
  rdfs:range adms:Identifier ;
  rdfs:subPropertyOf toop:hasCompanyCode ;
  rdfs:subPropertyOf adms:identifier ;
  rdfs:subPropertyOf rov:registration ;
  skos:prefLabel "has business code"@en ;
.
<http://example.register.nl/nationaalhandelsregister>
  owl:versionInfo "Created with TopBraid Composer" ;
.
nhr:Adres
  rdf:type owl:Class ;
  rdfs:comment "Het adres van een locatie."@nl ;
  rdfs:label "Adres"@nl ;
  rdfs:subClassOf toop:Address ;
  rdfs:subClassOf skos:Concept ;
  skos:prefLabel "Adres"@nl ;
.
nhr:BeslotenVennootschap
  rdf:type owl:Class ;
  rdf:type _:b875853 ;
  rdfs:comment "Juridische rechtsvorm die eigen rechtspersoonlijkheid heeft en waarvan het eigen vermogen is opgebouwd uit aandelen die in handen zijn van de vennoten (daarom heten die aandeelhouders). De aandeelhouders kunnen voor niet meer dan hun aandeel in het eigen vermogen van de vennootschap aansprakelijk gesteld worden voor de financiële verplichtingen van de onderneming."@nl ;
  rdfs:label "BV"@nl ;
  rdfs:label "Besloten Vennootschap"@nl ;
  rdfs:subClassOf skos:Concept ;
  skos:altLabel "BV"@nl ;
  skos:inScheme nhr:RechtsvormRechtspersoon ;
  skos:prefLabel "Besloten Vennootschap"@nl ;
.
nhr:Bestuurder
  rdf:type owl:Class ;
  rdf:type _:b875853 ;
  rdfs:comment "De bestuurder van een rechtspersoon."@nl ;
  rdfs:label "Bestuurder"@nl ;
  rdfs:subClassOf skos:Concept ;
  skos:inScheme nhr:TypeBestuurder ;
  skos:prefLabel "Bestuurder"@nl ;
.
nhr:BestuurderSETU
  rdf:type nhr:Bestuurder ;
  rdf:type nhr:Functievervulling ;
  rdf:type _:b327858 ;
  nhr:doorPersoon nhr:NatuurlijkPersoon_1 ;
  rdfs:comment "De bestuurder van SETU."@nl ;
  rdfs:label "Bestuurder SETU"@nl ;
  skos:prefLabel "Bestuurder SETU"@nl ;
.
nhr:Bestuursfunctie
  rdf:type owl:Class ;
  rdfs:comment "De functionaris die als bestuurder werkzaam is bij een privaatrechtelijke {Rechtspersoon}."@nl ;
  rdfs:label "Bestuursfunctie"@nl ;
  rdfs:subClassOf nhr:Functievervulling ;
  skos:prefLabel "Bestuursfunctie"@nl ;
.
nhr:BezoekadresABU
  rdf:type elobr:EloniaAddress ;
  rdf:type freebr:FreedoniaAddress ;
  rdf:type nhr:BinnenlandsAdres ;
  rdf:type vcard:Address ;
  rdf:type _:b49042 ;
  rdf:type _:b83024 ;
  rdf:type _:b327858 ;
  rdf:type _:b401324 ;
  rdf:type _:b541374 ;
  rdf:type _:b583853 ;
  rdf:type _:b652026 ;
  rdf:type _:b763315 ;
  rdf:type _:b955705 ;
  nhr:huisnummer 74 ;
  nhr:plaats "Lijnden" ;
  nhr:postcode "1175RA" ;
  nhr:straatnaam "Singaporestraat" ;
  toop:locality "Lijnden" ;
  toop:postalCode "1175RA" ;
  rdfs:comment "Het bezoekadres van ABU."@nl ;
  rdfs:label "Bezoekadres ABU"@nl ;
  skos:prefLabel "Bezoekadres ABU"@nl ;
  vcard:locality "Lijnden" ;
  vcard:postal-code "1175RA" ;
.
nhr:BezoeklocatieABU
  rdf:type nhr:Locatie-Vestiging ;
  rdf:type _:b327858 ;
  nhr:heeftVolledigAdres nhr:BezoekadresABU ;
  rdfs:comment "De bezoeklocatie van ABU."@nl ;
  rdfs:label "Bezoeklocatie ABU"@nl ;
  skos:prefLabel "Bezoeklocatie ABU"@nl ;
.
nhr:BinnenlandsAdres
  rdf:type owl:Class ;
  rdfs:comment "Een adres in Nederland."@nl ;
  rdfs:label "Binnenlands adres"@nl ;
  rdfs:subClassOf nhr:Adres ;
  rdfs:subClassOf _:b329657 ;
  rdfs:subClassOf _:b593574 ;
  owl:disjointWith nhr:BuitenlandsAdres ;
  skos:prefLabel "Binnenlands adres"@nl ;
.
nhr:BinnenlandseNietNatuurlijkPersoon
  rdf:type owl:Class ;
  rdfs:comment "Een {BinnenlandseNietNatuurlijkPersoon} is een {NietNatuurlijkPersoon} die is opgericht naar Nederlands recht."@nl ;
  rdfs:label "Binnenlandse niet natuurlijk persoon"@nl ;
  rdfs:subClassOf nhr:NietNatuurlijkPersoon ;
  skos:prefLabel "Binnenlandse niet natuurlijk persoon"@nl ;
.
nhr:BuitenlandsAdres
  rdf:type owl:Class ;
  rdfs:comment "Een adres buiten Nederland."@nl ;
  rdfs:label "Buitenlands adres"@nl ;
  rdfs:subClassOf nhr:Adres ;
  rdfs:subClassOf _:b229905 ;
  rdfs:subClassOf _:b302287 ;
  rdfs:subClassOf _:b918886 ;
  owl:disjointWith nhr:BinnenlandsAdres ;
  skos:prefLabel "Buitenlands adres"@nl ;
.
nhr:BuitenlandseVennootschap
  rdf:type owl:Class ;
  rdfs:comment "Een {BuitenlandseVennootschap} is opgericht naar buitenlands recht."@nl ;
  rdfs:label "Buitenlandse vennootschap"@nl ;
  rdfs:subClassOf nhr:NietNatuurlijkPersoon ;
  skos:prefLabel "Buitenlandse vennootschap"@nl ;
.
nhr:CommanditaireVennootschap
  rdf:type owl:Class ;
  rdf:type _:b875853 ;
  rdfs:comment "Samenwerkingsverband tussen twee of meer personen waarbij een of meer personen uitsluitend als geldverschaffer optreden (de commanditaire of stille vennoot)."@nl ;
  rdfs:label "CV"@nl ;
  rdfs:label "Commanditaire Vennootschap"@nl ;
  rdfs:subClassOf skos:Concept ;
  skos:altLabel "CV"@nl ;
  skos:inScheme nhr:RechtsvormSamenwerkingsverband ;
  skos:prefLabel "Commanditaire Vennootschap"@nl ;
.
nhr:Communicatiegegeven
  rdf:type owl:Class ;
  rdfs:comment "De communicatiegegevens."@nl ;
  rdfs:label "Communicatiegegeven"@nl ;
  rdfs:subClassOf skos:Concept ;
  skos:prefLabel "Communicatiegegeven"@nl ;
.
nhr:Communicatiegegeven-MaatschappelijkeActiviteit
  rdf:type owl:Class ;
  rdfs:comment "Een Communicatiegegeven die bij een MaatschappelijkeActiviteit hoort."@nl ;
  rdfs:label "Communicatiegegeven Maatschappelijke activiteit"@nl ;
  rdfs:subClassOf nhr:Communicatiegegeven ;
  skos:prefLabel "Communicatiegegeven Maatschappelijke activiteit"@nl ;
.
nhr:Communicatiegegeven-Rechtspersoon
  rdf:type owl:Class ;
  rdfs:comment "Een Communicatiegegeven die bij een Rechtspersoon hoort."@nl ;
  rdfs:label "Communicatiegegeven Rechtspersoon"@nl ;
  rdfs:subClassOf nhr:Communicatiegegeven ;
  skos:prefLabel "Communicatiegegeven Rechtspersoon"@nl ;
.
nhr:Communicatiegegeven-Vestiging
  rdf:type owl:Class ;
  rdfs:comment "Een Communicatiegegeven die bij een Vestiging hoort."@nl ;
  rdfs:label "Communicatiegegeven Vestiging"@nl ;
  rdfs:subClassOf nhr:Communicatiegegeven ;
  skos:prefLabel "Communicatiegegeven Vestiging"@nl ;
.
nhr:CommunicatiegegevensSETU
  rdf:type nhr:Communicatiegegeven-MaatschappelijkeActiviteit ;
  rdf:type _:b327858 ;
  nhr:heeftEmailAdres nhr:EmailAdresSETU ;
  rdfs:comment "De communicatiegegevens van SETU."@nl ;
  rdfs:label "Communicatiegegevens SETU"@nl ;
  skos:prefLabel "Communicatiegegevens SETU"@nl ;
.
nhr:Communicatienummer
  rdf:type owl:Class ;
  rdfs:comment "Het telefoon- of faxnummer."@nl ;
  rdfs:label "Communicatienummer"@nl ;
  rdfs:subClassOf skos:Concept ;
  rdfs:subClassOf _:b18002 ;
  rdfs:subClassOf _:b767375 ;
  rdfs:subClassOf _:b770826 ;
  skos:prefLabel "Communicatienummer"@nl ;
.
nhr:CommunicatienummerSETU
  rdf:type nhr:Communicatienummer ;
  rdf:type _:b327858 ;
  nhr:nummerCommunicatienummer "0800-SETU" ;
  nhr:soortCommunicatienummer "T" ;
  nhr:toegangscodeCommunicatienummer "031" ;
  rdfs:comment "Het communicatienummer van SETU."@nl ;
  rdfs:label "Communicatienummer SETU"@nl ;
  skos:prefLabel "Communicatienummer SETU"@nl ;
.
nhr:Coöperatie
  rdf:type owl:Class ;
  rdf:type _:b875853 ;
  rdfs:comment "Een vorm van economische samenwerking die een gedeelte van hun bedrijfsactiviteiten (in de regel de marktfunctie) voor gezamenlijke rekening en risico - blijvend - uitvoeren, met behoud van de zelfstandigheid van de overige activiteiten."@nl ;
  rdfs:label "COP"@nl ;
  rdfs:label "Coöperatie"@nl ;
  rdfs:subClassOf skos:Concept ;
  skos:altLabel "COP"@nl ;
  skos:inScheme nhr:RechtsvormRechtspersoon ;
  skos:prefLabel "Coöperatie"@nl ;
.
nhr:Domeinnaam
  rdf:type owl:Class ;
  rdfs:comment "De domeinnaam is de naam waaronder de betrokkene zaken doet of informatie verschaft op het internet."@nl ;
  rdfs:label "Domeinnaam"@nl ;
  rdfs:subClassOf skos:Concept ;
  rdfs:subClassOf _:b627138 ;
  skos:prefLabel "Domeinnaam"@nl ;
.
nhr:DomeinnaamSETU
  rdf:type nhr:Domeinnaam ;
  rdf:type _:b327858 ;
  nhr:naamDomeinnaam "www.setu.nl" ;
  rdfs:comment "De domeinnaam van SETU."@nl ;
  rdfs:label "Domeinnaam SETU"@nl ;
  skos:prefLabel "Domeinnaam SETU"@nl ;
.
nhr:EenmanszaakMetMeerdereEigenaren
  rdf:type owl:Class ;
  rdfs:comment "Een eenmanszaak met onverdeelde boedel."@nl ;
  rdfs:label "Eenmanszaak met meerdere eigenaren"@nl ;
  rdfs:subClassOf nhr:BinnenlandseNietNatuurlijkPersoon ;
  skos:prefLabel "Eenmanszaak met meerdere eigenaren"@nl ;
.
nhr:EmailAdres
  rdf:type owl:Class ;
  rdfs:comment "Het e-mail adres dat de betrokkene open heeft gesteld voor communicatie."@nl ;
  rdfs:label "Email adres"@nl ;
  rdfs:subClassOf skos:Concept ;
  rdfs:subClassOf _:b813138 ;
  skos:prefLabel "Email adres"@nl ;
.
nhr:EmailAdresSETU
  rdf:type nhr:EmailAdres ;
  rdf:type _:b327858 ;
  nhr:adresEmailAdres "info@setu.nl" ;
  rdfs:comment "Het emailadres van SETU."@nl ;
  rdfs:label "Email adres SETU"@nl ;
  skos:prefLabel "Email adres SETU"@nl ;
.
nhr:EuropeesEconomischSamenwerkingsverband
  rdf:type owl:Class ;
  rdf:type _:b875853 ;
  rdfs:comment "Samenwerkingsverband (volgens Europees recht) van verschillende, binnen de Europese Unie gevestigde ondernemingen, waarbij dat samenwerkingsverband een eigen Europees-rechterlijke rechtspersoonlijkheid heeft."@nl ;
  rdfs:label "EESV"@nl ;
  rdfs:label "Europees Economisch Samenwerkingsverband"@nl ;
  rdfs:subClassOf skos:Concept ;
  skos:altLabel "EESV"@nl ;
  skos:inScheme nhr:RechtsvormRechtspersoon ;
  skos:prefLabel "Europees Economisch Samenwerkingsverband"@nl ;
.
nhr:EuropeseCoöperatieveVennootschap
  rdf:type owl:Class ;
  rdf:type _:b875853 ;
  rdfs:comment """De Europese coöperatieve vennootschap (Societas Cooperativa Europaea, SCE) is een Europese rechtsvorm met kenmerken van de coöperatie en de nv. Net als de Europese naamloze vennootschap (SE) is de SCE niet gebonden aan een EUlidstaat. Daardoor is het mogelijk de statutaire zetel naar een ander land te verplaatsen. 
Het kapitaal is de SCE is verdeeld in aandelen. Het minimum geplaatste kapitaal van de leden is 30.000 euro."""@nl ;
  rdfs:label "Europese Coöperatieve Vennootschap"@nl ;
  rdfs:label "SCE"@nl ;
  rdfs:subClassOf skos:Concept ;
  skos:altLabel "SCE"@nl ;
  skos:inScheme nhr:RechtsvormRechtspersoon ;
  skos:prefLabel "Europese Coöperatieve Vennootschap"@nl ;
.
nhr:EuropeseNaamlozeVennootschap
  rdf:type owl:Class ;
  rdf:type _:b875853 ;
  rdfs:comment """De Europese naamloze vennootschap (Societas Europaea, SE) is een rechtsvorm voor vennootschappen met internationale activiteiten, die in alle landen van de EU bestaat. Alleen rechtspersonen kunnen een SE oprichten.
Het minimumkapitaal bij oprichting is 120.000 euro."""@nl ;
  rdfs:label "Europese Naamloze Vennootschap"@nl ;
  rdfs:label "SE"@nl ;
  rdfs:subClassOf skos:Concept ;
  skos:altLabel "SE"@nl ;
  skos:inScheme nhr:RechtsvormRechtspersoon ;
  skos:prefLabel "Europese Naamloze Vennootschap"@nl ;
.
nhr:Functievervulling
  rdf:type owl:Class ;
  rdfs:comment "Een {Functievervulling} is een vervulling door een {Persoon} van een functie voor een {Persoon}."@nl ;
  rdfs:label "Functievervulling"@nl ;
  rdfs:subClassOf skos:Concept ;
  skos:prefLabel "Functievervulling"@nl ;
.
nhr:Kerkgenootschap
  rdf:type owl:Class ;
  rdf:type _:b875853 ;
  rdfs:comment "Kerkelijke organisatie die door een eigen statuut wordt geregeerd en rechtspersoonlijkheid bezit."@nl ;
  rdfs:label "KG"@nl ;
  rdfs:label "Kerkgenootschap"@nl ;
  rdfs:subClassOf skos:Concept ;
  skos:altLabel "KG"@nl ;
  skos:inScheme nhr:RechtsvormRechtspersoon ;
  skos:prefLabel "Kerkgenootschap"@nl ;
.
nhr:LidVanHetBesturendOrgaan
  rdf:type owl:Class ;
  rdf:type _:b875853 ;
  rdfs:comment "Een persoon die een bestuursfunctie heeft bij een Europese naamloze vennootschap (SE) of Europese coöperatieve vennootschap (SCE) indien de SE of SCE is ingericht volgens het monistisch stelsel."@nl ;
  rdfs:label "Lid van het besturend orgaan"@nl ;
  rdfs:subClassOf skos:Concept ;
  skos:inScheme nhr:TypeBestuurder ;
  skos:prefLabel "Lid van het besturend orgaan"@nl ;
.
nhr:LidVanHetLeidinggevendOrgaan
  rdf:type owl:Class ;
  rdf:type _:b875853 ;
  rdfs:comment "Een persoon die een bestuursfunctie heeft bij een Europese naamloze vennootschap (SE) of Europese coöperatieve vennootschap (SCE) indien de SE of SCE is ingericht volgens het dualistisch stelsel."@nl ;
  rdfs:label "Lid van het leidinggevend orgaan"@nl ;
  rdfs:subClassOf skos:Concept ;
  skos:inScheme nhr:TypeBestuurder ;
  skos:prefLabel "Lid van het leidinggevend orgaan"@nl ;
.
nhr:Locatie
  rdf:type owl:Class ;
  rdfs:comment "Een locatie is een aanwijsbare plek op aarde."@nl ;
  rdfs:label "Locatie"@nl ;
  rdfs:subClassOf skos:Concept ;
  skos:prefLabel "Locatie"@nl ;
.
nhr:Locatie-BuitenlandseVennootschap
  rdf:type owl:Class ;
  rdfs:comment "Een locatie die bij een BuitenlandseNietNatuurlijkPersoon hoort."@nl ;
  rdfs:label "Locatie-Buitenlandse vennootschap"@nl ;
  rdfs:subClassOf nhr:Locatie ;
  owl:disjointWith nhr:Locatie-MaatschappelijkeActiviteit ;
  owl:disjointWith nhr:Locatie-NaamPersoon ;
  owl:disjointWith nhr:Locatie-NatuurlijkPersoon ;
  owl:disjointWith nhr:Locatie-Persoon ;
  owl:disjointWith nhr:Locatie-Rechtspersoon ;
  owl:disjointWith nhr:Locatie-Vestiging ;
  skos:prefLabel "Locatie-Buitenlandse vennootschap"@nl ;
.
nhr:Locatie-MaatschappelijkeActiviteit
  rdf:type owl:Class ;
  rdfs:comment "Een locatie die bij een MaatschappelijkeActiviteit hoort."@nl ;
  rdfs:label "Locatie-Maatschappelijke activiteit"@nl ;
  rdfs:subClassOf nhr:Locatie ;
  owl:disjointWith nhr:Locatie-BuitenlandseVennootschap ;
  owl:disjointWith nhr:Locatie-NaamPersoon ;
  owl:disjointWith nhr:Locatie-NatuurlijkPersoon ;
  owl:disjointWith nhr:Locatie-Persoon ;
  owl:disjointWith nhr:Locatie-Rechtspersoon ;
  owl:disjointWith nhr:Locatie-Vestiging ;
  skos:prefLabel "Locatie-Maatschappelijke activiteit"@nl ;
.
nhr:Locatie-NaamPersoon
  rdf:type owl:Class ;
  rdfs:comment "Een locatie die bij een NaamPersoon hoort."@nl ;
  rdfs:label "Locatie-Naam persoon"@nl ;
  rdfs:subClassOf nhr:Locatie ;
  owl:disjointWith nhr:Locatie-BuitenlandseVennootschap ;
  owl:disjointWith nhr:Locatie-MaatschappelijkeActiviteit ;
  owl:disjointWith nhr:Locatie-NatuurlijkPersoon ;
  owl:disjointWith nhr:Locatie-Persoon ;
  owl:disjointWith nhr:Locatie-Rechtspersoon ;
  owl:disjointWith nhr:Locatie-Vestiging ;
  skos:prefLabel "Locatie-Naam persoon"@nl ;
.
nhr:Locatie-NatuurlijkPersoon
  rdf:type owl:Class ;
  rdfs:comment "Een locatie die bij een NatuurlijkPersoon hoort."@nl ;
  rdfs:label "Locatie-Natuurlijk persoon"@nl ;
  rdfs:subClassOf nhr:Locatie ;
  owl:disjointWith nhr:Locatie-BuitenlandseVennootschap ;
  owl:disjointWith nhr:Locatie-MaatschappelijkeActiviteit ;
  owl:disjointWith nhr:Locatie-NaamPersoon ;
  owl:disjointWith nhr:Locatie-Persoon ;
  owl:disjointWith nhr:Locatie-Rechtspersoon ;
  owl:disjointWith nhr:Locatie-Vestiging ;
  skos:prefLabel "Locatie-Natuurlijk persoon"@nl ;
.
nhr:Locatie-Persoon
  rdf:type owl:Class ;
  rdfs:comment "Een locatie die bij een Persoon hoort."@nl ;
  rdfs:label "Locatie-Persoon"@nl ;
  rdfs:subClassOf nhr:Locatie ;
  owl:disjointWith nhr:Locatie-BuitenlandseVennootschap ;
  owl:disjointWith nhr:Locatie-MaatschappelijkeActiviteit ;
  owl:disjointWith nhr:Locatie-NaamPersoon ;
  owl:disjointWith nhr:Locatie-NatuurlijkPersoon ;
  owl:disjointWith nhr:Locatie-Rechtspersoon ;
  owl:disjointWith nhr:Locatie-Vestiging ;
  skos:prefLabel "Locatie-Persoon"@nl ;
.
nhr:Locatie-Rechtspersoon
  rdf:type owl:Class ;
  rdfs:comment "Een locatie die bij een Rechtspersoon hoort."@nl ;
  rdfs:label "Locatie-Rechtspersoon"@nl ;
  rdfs:subClassOf nhr:Locatie ;
  owl:disjointWith nhr:Locatie-BuitenlandseVennootschap ;
  owl:disjointWith nhr:Locatie-MaatschappelijkeActiviteit ;
  owl:disjointWith nhr:Locatie-NaamPersoon ;
  owl:disjointWith nhr:Locatie-NatuurlijkPersoon ;
  owl:disjointWith nhr:Locatie-Persoon ;
  owl:disjointWith nhr:Locatie-Vestiging ;
  skos:prefLabel "Locatie-Rechtspersoon"@nl ;
.
nhr:Locatie-Vestiging
  rdf:type owl:Class ;
  rdfs:comment "Een locatie die bij een Vestiging hoort."@nl ;
  rdfs:label "Locatie-Vestiging"@nl ;
  rdfs:subClassOf nhr:Locatie ;
  owl:disjointWith nhr:Locatie-BuitenlandseVennootschap ;
  owl:disjointWith nhr:Locatie-MaatschappelijkeActiviteit ;
  owl:disjointWith nhr:Locatie-NaamPersoon ;
  owl:disjointWith nhr:Locatie-NatuurlijkPersoon ;
  owl:disjointWith nhr:Locatie-Persoon ;
  owl:disjointWith nhr:Locatie-Rechtspersoon ;
  skos:prefLabel "Locatie-Vestiging"@nl ;
.
nhr:Maatschap
  rdf:type owl:Class ;
  rdf:type _:b875853 ;
  rdfs:comment "Een maatschap is een samenwerkingsverband waarin de maten pro rata (ieder naar zijn/haar aandeel) participeren. Er wordt voor gezamenlijke rekening en risico belegd in (commercieel) onroerend goed met als doel het behalen van exploitatie- en/of verkoopwinst."@nl ;
  rdfs:label "MA"@nl ;
  rdfs:label "Maatschap"@nl ;
  rdfs:subClassOf skos:Concept ;
  skos:altLabel "MA"@nl ;
  skos:inScheme nhr:RechtsvormSamenwerkingsverband ;
  skos:prefLabel "Maatschap"@nl ;
.
nhr:MaatschappelijkeActiviteit
  rdf:type owl:Class ;
  rdfs:comment "Een MaatschappelijkeActiviteit is een organisatie zonder winstoogmerk maar met een missie die gericht is op het verbeteren of instandhouden van aktiviteiten of bezit met maatschappelijk karakter. "@nl ;
  rdfs:label "Maatschappelijke activiteit"@nl ;
  rdfs:subClassOf skos:Concept ;
  rdfs:subClassOf _:b407513 ;
  rdfs:subClassOf _:b809403 ;
.
nhr:NaamPersoon
  rdf:type owl:Class ;
  rdfs:comment "Een {NaamPersoon} bevat de naam van een {NatuurlijkPersoon} of {NietNatuurlijkPersoon} die niet inschrijfplichtig is, maar wel een functie vervult in het handelsregister."@nl ;
  rdfs:label "Naam persoon"@nl ;
  rdfs:subClassOf nhr:Persoon ;
  skos:prefLabel "Naam persoon"@nl ;
.
nhr:NaamlozeVennootschap
  rdf:type owl:Class ;
  rdf:type _:b875853 ;
  rdfs:comment "De naamloze vennootschap (afgekort tot N.V.) is een rechtspersoon waarvan het maatschappelijk kapitaal verdeeld is in aandelen die in beginsel vrij overdraagbaar zijn. De naamloze vennootschap is 'naamloos' omdat er bij de nv geen verplichting bestaat tot het houden van een register van aandeelhouders. De vennoten blijven als het ware buiten beeld; zij zijn anoniem."@nl ;
  rdfs:label "NV"@nl ;
  rdfs:label "Naamloze Vennootschap"@nl ;
  rdfs:subClassOf skos:Concept ;
  skos:altLabel "NV"@nl ;
  skos:inScheme nhr:RechtsvormRechtspersoon ;
  skos:prefLabel "Naamloze Vennootschap"@nl ;
.
nhr:NatuurlijkPersoon
  rdf:type owl:Class ;
  rdfs:comment "Een {NatuurlijkPersoon} is een mens."@nl ;
  rdfs:label "Natuurlijk persoon"@nl ;
  rdfs:subClassOf nhr:Persoon ;
  rdfs:subClassOf toop:Person ;
  rdfs:subClassOf _:b546250 ;
  rdfs:subClassOf _:b839515 ;
  skos:prefLabel "Natuurlijk persoon"@nl ;
.
nhr:NatuurlijkPersoon_1
  rdf:type nhr:NatuurlijkPersoon ;
  rdf:type dcterms:Agent ;
  rdf:type schema:Person ;
  rdf:type <http://www.w3.org/2000/10/swap/pim/contact#Person> ;
  rdf:type foaf:Person ;
  rdf:type _:b327858 ;
  rdf:type _:b420951 ;
  rdf:type _:b421075 ;
  rdf:type _:b421168 ;
  rdf:type _:b421447 ;
  rdf:type _:b421664 ;
  rdf:type _:b421928 ;
  rdf:type _:b642226 ;
  rdf:type _:b937877 ;
  rdf:type _:b938265 ;
  nhr:geboortedatum "1995-04-02"^^xsd:date ;
  nhr:geslachtsnaam "Veer" ;
  nhr:heeftVolledigeNaam "Robin de Veer" ;
  nhr:isEigenaarVan nhr:SETU_Standaarden ;
  nhr:voornamen "Robin Jacob Johannes" ;
  rdfs:comment "De naam van Natuurlijk Persoon 1."@nl ;
  rdfs:label "Natuurlijk persoon 1"@nl ;
  skos:prefLabel "Natuurlijk persoon 1"@nl ;
.
nhr:NietNatuurlijkPersoon
  rdf:type owl:Class ;
  rdfs:comment "Een {NietNatuurlijkPersoon} is een {Persoon} met rechten en plichten die geen {NatuurlijkPersoon} is."@nl ;
  rdfs:label "Niet natuurlijk persoon"@nl ;
  rdfs:subClassOf nhr:Persoon ;
  skos:prefLabel "Niet natuurlijk persoon"@nl ;
.
nhr:OnderlingeWaarborgMaatschappij
  rdf:type owl:Class ;
  rdf:type _:b875853 ;
  rdfs:comment "Een bij notariële akte als onderlinge waarborgmaatschappij opgerichte vereniging, die zich blijkens haar statuten ten doel stelt met haar leden overeenkomsten van verzekering te sluiten respectievelijk om leden en mogelijk anderen in het kader van een wettelijke regeling verzekerd te houden."@nl ;
  rdfs:label "OWM"@nl ;
  rdfs:label "Onderlinge Waarborg Maatschappij"@nl ;
  rdfs:subClassOf skos:Concept ;
  skos:altLabel "OWM"@nl ;
  skos:inScheme nhr:RechtsvormRechtspersoon ;
  skos:prefLabel "Onderlinge Waarborg Maatschappij"@nl ;
.
nhr:Onderneming
  rdf:type owl:Class ;
  rdfs:comment "Een Onderderming is een organisatie met winstoogmerk. "@nl ;
  rdfs:label "Onderneming"@nl ;
  rdfs:subClassOf nhr:MaatschappelijkeActiviteit ;
.
nhr:OverigePrivaatrechtelijkeRechtspersoon
  rdf:type owl:Class ;
  rdf:type _:b875853 ;
  rdfs:comment "Een privaatrechtelijke rechtspersoon die commerciële activiteiten uitoefent, zoals Boermarke, Hofje, Funcatie, Gilde of Buurtschap."@nl ;
  rdfs:label "OPR"@nl ;
  rdfs:label "Overige Privaatrechtelijke Rechtspersoon"@nl ;
  rdfs:subClassOf skos:Concept ;
  skos:altLabel "OPR"@nl ;
  skos:inScheme nhr:RechtsvormRechtspersoon ;
  skos:prefLabel "Overige Privaatrechtelijke Rechtspersoon"@nl ;
.
nhr:Persoon
  rdf:type owl:Class ;
  rdfs:comment "Een Persoon is een ieder die rechten en plichten kan hebben."@nl ;
  rdfs:label "Persoon"@nl ;
  rdfs:subClassOf skos:Concept ;
  skos:prefLabel "Persoon"@nl ;
.
nhr:PersoonKrachtensStatuten
  rdf:type owl:Class ;
  rdf:type _:b875853 ;
  rdfs:comment "De persoon die namens het bestuur optreedt indien het bestuur belet is haar bestuursfunctie uit te oefenen."@nl ;
  rdfs:label "Persoon krachtens statuten bevoegd bij ontstentenis belet van de bestuurders"@nl ;
  rdfs:subClassOf skos:Concept ;
  skos:inScheme nhr:TypeBestuurder ;
  skos:prefLabel "Persoon krachtens statuten bevoegd bij ontstentenis belet van de bestuurders"@nl ;
.
nhr:PostadresABU
  rdf:type elobr:EloniaAddress ;
  rdf:type freebr:FreedoniaAddress ;
  rdf:type nhr:BinnenlandsAdres ;
  rdf:type vcard:Address ;
  rdf:type _:b49042 ;
  rdf:type _:b83024 ;
  rdf:type _:b327858 ;
  rdf:type _:b401324 ;
  rdf:type _:b541374 ;
  rdf:type _:b583853 ;
  rdf:type _:b652026 ;
  rdf:type _:b763315 ;
  rdf:type _:b955705 ;
  nhr:plaats "Badhoevedorp" ;
  nhr:postbusnummer 144 ;
  nhr:postcode "1170AC" ;
  toop:locality "Badhoevedorp" ;
  toop:postalCode "1170AC" ;
  rdfs:comment "Het postadres van ABU."@nl ;
  rdfs:label "Postadres ABU"@nl ;
  skos:prefLabel "Postadres ABU"@nl ;
  vcard:locality "Badhoevedorp" ;
  vcard:postal-code "1170AC" ;
.
nhr:PostlocatieABU
  rdf:type nhr:Locatie-Vestiging ;
  rdf:type _:b327858 ;
  rdfs:comment "De postlocatie van ABU."@nl ;
  rdfs:label "Postlocatie ABU"@nl ;
  skos:prefLabel "Postlocatie ABU"@nl ;
.
nhr:PubliekrechtelijkeRechtspersoon
  rdf:type owl:Class ;
  rdf:type _:b875853 ;
  rdfs:comment "Een lichaam dat een bepaalde overheidstaak opgedragen heeft gekregen, bijvoorbeeld het Rijk, de provincie en de gemeente."@nl ;
  rdfs:label "PR"@nl ;
  rdfs:label "Publiekrechtelijke Rechtspersoon"@nl ;
  rdfs:subClassOf skos:Concept ;
  skos:altLabel "PR"@nl ;
  skos:inScheme nhr:RechtsvormRechtspersoon ;
  skos:prefLabel "Publiekrechtelijke Rechtspersoon"@nl ;
.
nhr:Rechtspersoon
  rdf:type owl:Class ;
  rdfs:comment "Een {Rechtspersoon} is een door de wet mogelijk gemaakt rechtssubject, welke drager van rechten en plichten is."@nl ;
  rdfs:label "Rechtspersoon"@nl ;
  rdfs:subClassOf nhr:BinnenlandseNietNatuurlijkPersoon ;
  rdfs:subClassOf _:b333528 ;
  skos:prefLabel "Rechtspersoon"@nl ;
.
nhr:RechtspersoonInOprichting
  rdf:type owl:Class ;
  rdfs:comment "Een {Rechtspersoon} die in oprichting is."@nl ;
  rdfs:label "Rechtspersoon in oprichting"@nl ;
  rdfs:subClassOf nhr:BinnenlandseNietNatuurlijkPersoon ;
  skos:prefLabel "Rechtspersoon in oprichting"@nl ;
.
nhr:RechtsvormRechtspersoon
  rdf:type toop:CompanyTypeScheme ;
  rdf:type owl:Class ;
  rdf:type skos:ConceptScheme ;
  rdfs:comment "De privaatrechtelijke rechtspersoon is de rechtspersoon."@nl ;
  rdfs:label "Rechtsvorm rechtspersoon"@nl ;
  rdfs:subClassOf skos:ConceptScheme ;
  skos:prefLabel "Rechtsvorm rechtspersoon"@nl ;
.
nhr:RechtsvormSamenwerkingsverband
  rdf:type toop:CompanyTypeScheme ;
  rdf:type owl:Class ;
  rdf:type skos:ConceptScheme ;
  rdfs:comment "Een fiscaal transparante rechtsvorm, waarin voor rekening voor meerdere personen een onderneming wordt gedreven."@nl ;
  rdfs:label "Rechtsvorm samenwerkingsverband"@nl ;
  rdfs:subClassOf skos:ConceptScheme ;
  skos:prefLabel "Rechtsvorm samenwerkingsverband"@nl ;
.
nhr:Rederij
  rdf:type owl:Class ;
  rdf:type _:b875853 ;
  rdfs:comment "Een rechtspersoon welke eigenaar is van één of meerdere schepen."@nl ;
  rdfs:label "RED"@nl ;
  rdfs:label "Rederij"@nl ;
  rdfs:subClassOf skos:Concept ;
  skos:altLabel "RED"@nl ;
  skos:inScheme nhr:RechtsvormSamenwerkingsverband ;
  skos:prefLabel "Rederij"@nl ;
.
nhr:SETU_Standaarden
  rdf:type elobr:Company ;
  rdf:type freebr:Company ;
  rdf:type nhr:MaatschappelijkeActiviteit ;
  rdf:type nhr:Rechtspersoon ;
  rdf:type nhr:Vestiging ;
  rdf:type dcterms:Agent ;
  rdf:type toop:RegisteredOrganization ;
  rdf:type _:b327858 ;
  rdf:type _:b420951 ;
  rdf:type _:b421075 ;
  rdf:type _:b421168 ;
  rdf:type _:b421447 ;
  rdf:type _:b421664 ;
  rdf:type _:b421928 ;
  rdf:type _:b642226 ;
  rdf:type _:b937877 ;
  rdf:type _:b938265 ;
  elobr:EloniaCompanyName "SETU Standaarden"@nl ;
  freebr:FreedoniaCompanyName "SETU Standaarden"@nl ;
  nhr:heeftBezoekadres nhr:BezoeklocatieABU ;
  nhr:heeftCommunicatiegegevens nhr:CommunicatiegegevensSETU ;
  nhr:heeftPostadres nhr:PostlocatieABU ;
  nhr:isActiviteitVan nhr:Stichting_SETU ;
  nhr:kvkNummer "34279048" ;
  nhr:naamMaatschappelijkeActiviteit "SETU Standaarden"@nl ;
  nhr:wordtGeleidVanuit nhr:VestigingABU ;
  toop:companyName "SETU Standaarden"@nl ;
  toop:hasMainSite nhr:VestigingABU ;
  org:hasPrimarySite nhr:VestigingABU ;
  org:hasSite nhr:VestigingABU ;
  rov:legalName "SETU Standaarden"@nl ;
.
nhr:Samenwerkingsverband
  rdf:type owl:Class ;
  rdfs:comment "Een Samenwerkingsverband is een groep van natuurlijke personen, rechtspersonen, samenwerkingsverbanden (of een combinatie hiervan) aan wie een {Onderneming} toebehoort."@nl ;
  rdfs:label "Samenwerkingsverband"@nl ;
  rdfs:subClassOf nhr:BinnenlandseNietNatuurlijkPersoon ;
  rdfs:subClassOf [
      rdf:type owl:Restriction ;
      owl:onDataRange nhr:RechtsvormSamenwerkingsverband ;
      owl:onProperty nhr:heeftRechtsvorm ;
      owl:qualifiedCardinality "1"^^xsd:nonNegativeInteger ;
    ] ;
  skos:prefLabel "Samenwerkingsverband"@nl ;
.
nhr:Stichting
  rdf:type nhr:RechtsvormRechtspersoon ;
  rdf:type toop:CompanyTypeScheme ;
  rdf:type owl:Class ;
  rdf:type skos:Concept ;
  rdf:type _:b327858 ;
  rdf:type _:b875853 ;
  rdfs:comment "Een bij notariële akte opgerichte organisatie (meestal zonder winstoogmerk), met een afgezonderd vermogen, die streeft naar een in de statuten genoemd doel."@nl ;
  rdfs:label "ST"@nl ;
  rdfs:label "Stichting"@nl ;
  rdfs:subClassOf skos:Concept ;
  skos:altLabel "ST"@nl ;
  skos:inScheme nhr:RechtsvormRechtspersoon ;
  skos:prefLabel "Stichting"@nl ;
.
nhr:Stichting_SETU
  rdf:type elobr:Company ;
  rdf:type freebr:Company ;
  rdf:type nhr:Rechtspersoon ;
  rdf:type dcterms:Agent ;
  rdf:type toop:RegisteredOrganization ;
  rdf:type _:b327858 ;
  rdf:type _:b420951 ;
  rdf:type _:b421075 ;
  rdf:type _:b421168 ;
  rdf:type _:b421447 ;
  rdf:type _:b421664 ;
  rdf:type _:b421928 ;
  rdf:type _:b642226 ;
  rdf:type _:b937877 ;
  rdf:type _:b938265 ;
  elobr:EloniaCompanyType nhr:Stichting ;
  freebr:FreedoniaCompanyType nhr:Stichting ;
  nhr:heeftFunctievervulling nhr:BestuurderSETU ;
  nhr:heeftRechtsvorm nhr:Stichting ;
  nhr:heeftVolledigeNaam "Stichting Elektronische Transacties Uitzendbranche"@nl ;
  toop:companyType nhr:Stichting ;
  rdfs:comment "Stichting SETU zorgt voor standaardisatie van elektronisch berichtenverkeer in de branche voor flexibele arbeid."@nl ;
  org:classification nhr:Stichting ;
  rov:orgType nhr:Stichting ;
.
nhr:TypeBestuurder
  rdf:type toop:CompanyTypeScheme ;
  rdf:type owl:Class ;
  rdf:type skos:ConceptScheme ;
  rdfs:comment "De opsomming van de bestuursfuncties die mogelijk zijn bij een rechtspersoon."@nl ;
  rdfs:label "Type bestuurder"@nl ;
  rdfs:subClassOf skos:ConceptScheme ;
  skos:prefLabel "Type bestuurder"@nl ;
.
nhr:VennootschapOnderFirma
  rdf:type owl:Class ;
  rdf:type _:b875853 ;
  rdfs:comment "Een vof is een vennootschap waarbij onder een gemeenschappelijke naam koophandel wordt gedreven. Een vof kan bij onderhandse akte worden opgericht. De aandelen in een vof zijn niet eenzijdig overdraagbaar. Wel zijn alle vennoten hoofdelijk en onbeperkt aansprakelijk voor de schulden van de vennootschap."@nl ;
  rdfs:label "VOF"@nl ;
  rdfs:label "Vennootschap Onder Firma"@nl ;
  rdfs:subClassOf skos:Concept ;
  skos:altLabel "VOF"@nl ;
  skos:inScheme nhr:RechtsvormSamenwerkingsverband ;
  skos:prefLabel "Vennootschap Onder Firma"@nl ;
.
nhr:Vereffenaar
  rdf:type owl:Class ;
  rdf:type _:b875853 ;
  rdfs:comment "De persoon die bevoegd is de baten te vereffenen tijdens de liquidatie van een rechtspersoon."@nl ;
  rdfs:label "Vereffenaar"@nl ;
  rdfs:subClassOf skos:Concept ;
  skos:inScheme nhr:TypeBestuurder ;
  skos:prefLabel "Vereffenaar"@nl ;
.
nhr:Vereniging
  rdf:type owl:Class ;
  rdf:type _:b875853 ;
  rdfs:comment "Een samenwerkingsvorm waarbij meerdere personen op voet van gelijkheid trachten een bepaald doel te verwezenlijken of een bepaalde activiteit te ontplooien, meestal zonder dat hieraan commerciële belangen ten grondslag liggen."@nl ;
  rdfs:label "VER"@nl ;
  rdfs:label "Vereniging"@nl ;
  rdfs:subClassOf skos:Concept ;
  skos:altLabel "VER"@nl ;
  skos:inScheme nhr:RechtsvormRechtspersoon ;
  skos:prefLabel "Vereniging"@nl ;
.
nhr:VerenigingVanEigenaars
  rdf:type owl:Class ;
  rdf:type _:b875853 ;
  rdfs:comment "Een Vereniging van Eigenaars (VvE) is in Nederland een vereniging van de eigenaren van de appartementsrechten van de woningen die tot een appartementencomplex behoren. De VvE zorgt voor het regelen van het onderhoud van het appartementsgebouw en alle andere gemeenschappelijke belangen van de eigenaren."@nl ;
  rdfs:label "Vereniging van Eigenaars"@nl ;
  rdfs:label "VvE"@nl ;
  rdfs:subClassOf skos:Concept ;
  skos:altLabel "VvE"@nl ;
  skos:inScheme nhr:RechtsvormRechtspersoon ;
  skos:prefLabel "Vereniging van Eigenaars"@nl ;
.
nhr:VertegenwoordigerBestuurderRechtspersoon
  rdf:type owl:Class ;
  rdf:type _:b875853 ;
  rdfs:comment "" ;
  rdfs:label "Vertegenwoordiger bestuurder rechtspersoon"@nl ;
  rdfs:subClassOf skos:Concept ;
  skos:inScheme nhr:TypeBestuurder ;
  skos:prefLabel "Vertegenwoordiger bestuurder rechtspersoon"@nl ;
.
nhr:Vestiging
  rdf:type owl:Class ;
  rdfs:comment """Een Vestiging is gebouw of een complex van gebouwen waar duurzame uitoefening van activiteiten van een
Onderneming of Rechtspersoon plaatsvindt."""@nl ;
  rdfs:label "Vestiging"@nl ;
  rdfs:subClassOf skos:Concept ;
  skos:prefLabel "Vestiging"@nl ;
.
nhr:VestigingABU
  rdf:type nhr:MaatschappelijkeActiviteit ;
  rdf:type nhr:Vestiging ;
  rdf:type toop:MainSite ;
  rdf:type _:b327858 ;
  nhr:heeftBezoekadres nhr:BezoeklocatieABU ;
  nhr:heeftPostadres nhr:PostlocatieABU ;
  toop:siteOf nhr:SETU_Standaarden ;
  rdfs:comment "De vestiging van de ABU."@nl ;
  rdfs:label "Vestiging ABU"@nl ;
  skos:prefLabel "Vestiging ABU"@nl ;
  org:siteOf nhr:SETU_Standaarden ;
.
nhr:aanduidingBijHuisnummer
  rdf:type owl:DatatypeProperty ;
  rdfs:comment "De aanduiding die wordt gebruikt voor adressen die niet zijn voorzien van de gebruikelijke straatnaam en huisnummeraanduidingen. Mogelijke waarden zijn o.a.: bij, tegenover."@nl ;
  rdfs:domain elobr:EloniaAddress ;
  rdfs:domain freebr:FreedoniaAddress ;
  rdfs:domain nhr:Adres ;
  rdfs:domain nhr:BinnenlandsAdres ;
  rdfs:domain toop:Address ;
  rdfs:domain owl:Thing ;
  rdfs:domain skos:Concept ;
  rdfs:domain vcard:Address ;
  rdfs:domain _:b49042 ;
  rdfs:domain _:b83024 ;
  rdfs:domain _:b157701 ;
  rdfs:domain _:b168676 ;
  rdfs:domain _:b327858 ;
  rdfs:domain _:b329657 ;
  rdfs:domain _:b396249 ;
  rdfs:domain _:b401324 ;
  rdfs:domain _:b499218 ;
  rdfs:domain _:b541374 ;
  rdfs:domain _:b583853 ;
  rdfs:domain _:b593574 ;
  rdfs:domain _:b652026 ;
  rdfs:domain _:b726818 ;
  rdfs:domain _:b763315 ;
  rdfs:domain _:b787338 ;
  rdfs:domain _:b926654 ;
  rdfs:domain _:b955705 ;
  rdfs:label "aanduiding bij huisnummer"@nl ;
  rdfs:range xsd:string ;
  skos:prefLabel "aanduiding bij huisnummer"@nl ;
.
nhr:activiteitenGestaaktPer
  rdf:type owl:DatatypeProperty ;
  rdfs:comment "Datum waarop de activiteiten van de onderneming zijn gestaakt."@nl ;
  rdfs:domain nhr:BinnenlandseNietNatuurlijkPersoon ;
  rdfs:domain nhr:NietNatuurlijkPersoon ;
  rdfs:domain nhr:Persoon ;
  rdfs:domain nhr:Rechtspersoon ;
  rdfs:domain owl:Thing ;
  rdfs:domain skos:Concept ;
  rdfs:domain _:b327858 ;
  rdfs:domain _:b333528 ;
  rdfs:domain _:b421168 ;
  rdfs:domain _:b421447 ;
  rdfs:domain _:b642226 ;
  rdfs:label "activiteiten gestaakt per"@nl ;
  rdfs:range xsd:date ;
  rdfs:range _:b115973 ;
  rdfs:range _:b148299 ;
  skos:prefLabel "activiteiten gestaakt per"@nl ;
.
nhr:adresEmailAdres
  rdf:type owl:DatatypeProperty ;
  rdfs:comment "Het e-mail adres waarop de ondernemer gemaild kan worden."@nl ;
  rdfs:domain nhr:EmailAdres ;
  rdfs:domain owl:Thing ;
  rdfs:domain skos:Concept ;
  rdfs:domain _:b327858 ;
  rdfs:domain _:b813138 ;
  rdfs:label "adres email adres"@nl ;
  rdfs:range xsd:string ;
  skos:prefLabel "adres email adres"@nl ;
.
nhr:doorPersoon
  rdf:type owl:ObjectProperty ;
  rdfs:comment "Een Functievervulling door een Persoon."@nl ;
  rdfs:domain nhr:Functievervulling ;
  rdfs:domain owl:Thing ;
  rdfs:domain skos:Concept ;
  rdfs:domain _:b327858 ;
  rdfs:label "door persoon"@nl ;
  rdfs:range nhr:Persoon ;
  rdfs:range owl:Thing ;
  rdfs:range skos:Concept ;
  rdfs:range _:b327858 ;
  skos:prefLabel "door persoon"@nl ;
.
nhr:functie
  rdf:type owl:ObjectProperty ;
  rdfs:comment "Een nadere aanduiding van de {Bestuurder}."@nl ;
  rdfs:domain nhr:Bestuursfunctie ;
  rdfs:domain nhr:Functievervulling ;
  rdfs:domain owl:Thing ;
  rdfs:domain skos:Concept ;
  rdfs:domain _:b327858 ;
  rdfs:label "functie {@nl]" ;
  rdfs:label "functie"@nl ;
  rdfs:range nhr:TypeBestuurder ;
  rdfs:range toop:CompanyTypeScheme ;
  rdfs:range owl:Thing ;
  rdfs:range skos:ConceptScheme ;
  skos:prefLabel "functie {@nl]" ;
.
nhr:geboortedatum
  rdf:type owl:DatatypeProperty ;
  rdfs:comment "Geboortedatum van de {NatuurlijkPersoon}."@nl ;
  rdfs:domain nhr:NatuurlijkPersoon ;
  rdfs:domain nhr:Persoon ;
  rdfs:domain dcterms:Agent ;
  rdfs:domain schema:Person ;
  rdfs:domain toop:Person ;
  rdfs:domain <http://www.w3.org/2000/10/swap/pim/contact#Person> ;
  rdfs:domain owl:Thing ;
  rdfs:domain wgs:SpatialThing ;
  rdfs:domain skos:Concept ;
  rdfs:domain foaf:Agent ;
  rdfs:domain foaf:Person ;
  rdfs:domain _:b327858 ;
  rdfs:domain _:b420951 ;
  rdfs:domain _:b421075 ;
  rdfs:domain _:b421168 ;
  rdfs:domain _:b421447 ;
  rdfs:domain _:b421664 ;
  rdfs:domain _:b421928 ;
  rdfs:domain _:b546250 ;
  rdfs:domain _:b642226 ;
  rdfs:domain _:b839515 ;
  rdfs:domain _:b937877 ;
  rdfs:domain _:b938265 ;
  rdfs:label "geboortedatum"@nl ;
  rdfs:range xsd:date ;
  rdfs:range _:b115973 ;
  rdfs:range _:b148299 ;
  skos:prefLabel "geboortedatum"@nl ;
.
nhr:geslachtsnaam
  rdf:type owl:DatatypeProperty ;
  rdfs:comment "De geslachtsnaam van de {NatuurlijkPersoon}."@nl ;
  rdfs:domain nhr:NatuurlijkPersoon ;
  rdfs:domain nhr:Persoon ;
  rdfs:domain dcterms:Agent ;
  rdfs:domain schema:Person ;
  rdfs:domain toop:Person ;
  rdfs:domain <http://www.w3.org/2000/10/swap/pim/contact#Person> ;
  rdfs:domain owl:Thing ;
  rdfs:domain wgs:SpatialThing ;
  rdfs:domain skos:Concept ;
  rdfs:domain foaf:Agent ;
  rdfs:domain foaf:Person ;
  rdfs:domain _:b327858 ;
  rdfs:domain _:b420951 ;
  rdfs:domain _:b421075 ;
  rdfs:domain _:b421168 ;
  rdfs:domain _:b421447 ;
  rdfs:domain _:b421664 ;
  rdfs:domain _:b421928 ;
  rdfs:domain _:b546250 ;
  rdfs:domain _:b642226 ;
  rdfs:domain _:b839515 ;
  rdfs:domain _:b937877 ;
  rdfs:domain _:b938265 ;
  rdfs:label "geslachtsnaam"@nl ;
  rdfs:range xsd:string ;
  skos:prefLabel "geslachtsnaam"@nl ;
.
nhr:heeftBezoekadres
  rdf:type owl:ObjectProperty ;
  rdfs:comment "Geeft het bezoekadres van de MaatschappelijkeActiviteit."@nl ;
  rdfs:domain nhr:MaatschappelijkeActiviteit ;
  rdfs:domain nhr:Vestiging ;
  rdfs:domain owl:Thing ;
  rdfs:domain skos:Concept ;
  rdfs:domain _:b327858 ;
  rdfs:domain _:b407513 ;
  rdfs:domain _:b809403 ;
  rdfs:label "heeft bezoekadres"@nl ;
  rdfs:range nhr:Locatie ;
  rdfs:range owl:Thing ;
  rdfs:range skos:Concept ;
  rdfs:range _:b327858 ;
  skos:prefLabel "heeft bezoekadres"@nl ;
.
nhr:heeftCommunicatiegegevens
  rdf:type owl:ObjectProperty ;
  rdfs:comment "De communicatiegegevens van een MaatschappelijkeActiviteit, Rechtspersoon of Vestiging."@nl ;
  rdfs:domain nhr:BinnenlandseNietNatuurlijkPersoon ;
  rdfs:domain nhr:MaatschappelijkeActiviteit ;
  rdfs:domain nhr:NietNatuurlijkPersoon ;
  rdfs:domain nhr:Persoon ;
  rdfs:domain nhr:Rechtspersoon ;
  rdfs:domain owl:Thing ;
  rdfs:domain skos:Concept ;
  rdfs:domain _:b327858 ;
  rdfs:domain _:b333528 ;
  rdfs:domain _:b407513 ;
  rdfs:domain _:b421168 ;
  rdfs:domain _:b421447 ;
  rdfs:domain _:b642226 ;
  rdfs:domain _:b809403 ;
  rdfs:label "heeft communicatiegegevens"@nl ;
  rdfs:range nhr:Communicatiegegeven ;
  rdfs:range owl:Thing ;
  rdfs:range skos:Concept ;
  rdfs:range _:b327858 ;
  skos:prefLabel "heeft communicatiegegevens"@nl ;
.
nhr:heeftCommunicatienummer
  rdf:type owl:ObjectProperty ;
  rdfs:comment "" ;
  rdfs:domain nhr:Communicatiegegeven ;
  rdfs:domain owl:Thing ;
  rdfs:domain skos:Concept ;
  rdfs:domain _:b327858 ;
  rdfs:label "heeft communicatienummer"@nl ;
  rdfs:range nhr:Communicatienummer ;
  rdfs:range owl:Thing ;
  rdfs:range skos:Concept ;
  rdfs:range _:b18002 ;
  rdfs:range _:b327858 ;
  rdfs:range _:b767375 ;
  rdfs:range _:b770826 ;
  skos:prefLabel "heeft communicatienummer"@nl ;
.
nhr:heeftDomeinnaam
  rdf:type owl:ObjectProperty ;
  rdfs:comment "" ;
  rdfs:domain nhr:Communicatiegegeven ;
  rdfs:domain owl:Thing ;
  rdfs:domain skos:Concept ;
  rdfs:domain _:b327858 ;
  rdfs:label "heeft domeinnaam"@nl ;
  rdfs:range nhr:Domeinnaam ;
  rdfs:range owl:Thing ;
  rdfs:range skos:Concept ;
  rdfs:range _:b327858 ;
  rdfs:range _:b627138 ;
  skos:prefLabel "heeft domeinnaam"@nl ;
.
nhr:heeftEmailAdres
  rdf:type owl:ObjectProperty ;
  rdfs:comment "" ;
  rdfs:domain nhr:Communicatiegegeven ;
  rdfs:domain owl:Thing ;
  rdfs:domain skos:Concept ;
  rdfs:domain _:b327858 ;
  rdfs:label "heeft email adres {2nl}" ;
  rdfs:label "heeft email adres"@nl ;
  rdfs:range nhr:EmailAdres ;
  rdfs:range owl:Thing ;
  rdfs:range skos:Concept ;
  rdfs:range _:b327858 ;
  rdfs:range _:b813138 ;
  skos:prefLabel "heeft email adres {2nl}" ;
.
nhr:heeftFunctievervulling
  rdf:type owl:ObjectProperty ;
  rdfs:comment "Een Persoon heeft een Functievervulling."@nl ;
  rdfs:domain nhr:Persoon ;
  rdfs:domain owl:Thing ;
  rdfs:domain skos:Concept ;
  rdfs:domain _:b327858 ;
  rdfs:label "heeft functievervulling"@nl ;
  rdfs:range nhr:Functievervulling ;
  rdfs:range owl:Thing ;
  rdfs:range skos:Concept ;
  rdfs:range _:b327858 ;
  skos:prefLabel "heeft functievervulling"@nl ;
.
nhr:heeftPostadres
  rdf:type owl:ObjectProperty ;
  rdfs:comment "Geeft het postadres van de MaatschappelijkeActiviteit."@nl ;
  rdfs:domain nhr:MaatschappelijkeActiviteit ;
  rdfs:domain nhr:Vestiging ;
  rdfs:domain owl:Thing ;
  rdfs:domain skos:Concept ;
  rdfs:domain _:b327858 ;
  rdfs:domain _:b407513 ;
  rdfs:domain _:b809403 ;
  rdfs:label "heeft postadres"@nl ;
  rdfs:range nhr:Locatie ;
  rdfs:range owl:Thing ;
  rdfs:range skos:Concept ;
  rdfs:range _:b327858 ;
  skos:prefLabel "heeft postadres"@nl ;
.
nhr:heeftRechtsvorm
  rdf:type owl:ObjectProperty ;
  rdfs:comment "De rechtsvorm van de rechtspersoon."@nl ;
  rdfs:domain elobr:Company ;
  rdfs:domain freebr:Company ;
  rdfs:domain nhr:BinnenlandseNietNatuurlijkPersoon ;
  rdfs:domain nhr:NietNatuurlijkPersoon ;
  rdfs:domain nhr:Persoon ;
  rdfs:domain nhr:Rechtspersoon ;
  rdfs:domain dcterms:Agent ;
  rdfs:domain toop:RegisteredOrganization ;
  rdfs:domain owl:Thing ;
  rdfs:domain skos:Concept ;
  rdfs:domain org:FormalOrganization ;
  rdfs:domain org:Organization ;
  rdfs:domain rov:RegisteredOrganization ;
  rdfs:domain foaf:Agent ;
  rdfs:domain foaf:Organization ;
  rdfs:domain _:b156576 ;
  rdfs:domain _:b180769 ;
  rdfs:domain _:b213787 ;
  rdfs:domain _:b254570 ;
  rdfs:domain _:b327858 ;
  rdfs:domain _:b333528 ;
  rdfs:domain _:b420951 ;
  rdfs:domain _:b421075 ;
  rdfs:domain _:b421168 ;
  rdfs:domain _:b421447 ;
  rdfs:domain _:b421664 ;
  rdfs:domain _:b421928 ;
  rdfs:domain _:b454254 ;
  rdfs:domain _:b642226 ;
  rdfs:domain _:b772676 ;
  rdfs:domain _:b826282 ;
  rdfs:domain _:b826680 ;
  rdfs:domain _:b883411 ;
  rdfs:domain _:b937877 ;
  rdfs:domain _:b938265 ;
  rdfs:label "heeft rechtsvorm"@nl ;
  rdfs:range nhr:RechtsvormRechtspersoon ;
  rdfs:range toop:CompanyTypeScheme ;
  rdfs:range owl:Thing ;
  rdfs:range skos:Concept ;
  rdfs:range skos:ConceptScheme ;
  rdfs:range _:b327858 ;
  rdfs:range _:b875853 ;
  rdfs:subPropertyOf elobr:EloniaCompanyType ;
  rdfs:subPropertyOf freebr:FreedoniaCompanyType ;
  rdfs:subPropertyOf toop:companyType ;
  rdfs:subPropertyOf org:classification ;
  rdfs:subPropertyOf rov:orgType ;
  skos:prefLabel "heeft rechtsvorm"@nl ;
.
nhr:heeftVolledigAdres
  rdf:type owl:ObjectProperty ;
  rdfs:comment "Samengesteld adres."@nl ;
  rdfs:domain nhr:Locatie ;
  rdfs:domain owl:Thing ;
  rdfs:domain skos:Concept ;
  rdfs:domain _:b327858 ;
  rdfs:label "heeft volledig adres"@nl ;
  rdfs:range elobr:EloniaAddress ;
  rdfs:range freebr:FreedoniaAddress ;
  rdfs:range nhr:Adres ;
  rdfs:range toop:Address ;
  rdfs:range owl:Thing ;
  rdfs:range skos:Concept ;
  rdfs:range vcard:Address ;
  rdfs:range _:b49042 ;
  rdfs:range _:b83024 ;
  rdfs:range _:b157701 ;
  rdfs:range _:b168676 ;
  rdfs:range _:b327858 ;
  rdfs:range _:b396249 ;
  rdfs:range _:b401324 ;
  rdfs:range _:b499218 ;
  rdfs:range _:b541374 ;
  rdfs:range _:b583853 ;
  rdfs:range _:b652026 ;
  rdfs:range _:b726818 ;
  rdfs:range _:b763315 ;
  rdfs:range _:b787338 ;
  rdfs:range _:b926654 ;
  rdfs:range _:b955705 ;
  skos:prefLabel "heeft volledig adres"@nl ;
.
nhr:heeftVolledigeNaam
  rdf:type owl:DatatypeProperty ;
  rdfs:comment "Volledige naam van de persoon."@nl ;
  rdfs:domain nhr:Persoon ;
  rdfs:domain owl:Thing ;
  rdfs:domain skos:Concept ;
  rdfs:domain _:b327858 ;
  rdfs:label "heeft volledige naam"@nl ;
  rdfs:range xsd:string ;
  skos:prefLabel "heeft volledige naam"@nl ;
.
nhr:huisletter
  rdf:type owl:DatatypeProperty ;
  rdfs:comment "De huisletter die door gemeente is toegekend aan het huisnummer."@nl ;
  rdfs:domain elobr:EloniaAddress ;
  rdfs:domain freebr:FreedoniaAddress ;
  rdfs:domain nhr:Adres ;
  rdfs:domain nhr:BinnenlandsAdres ;
  rdfs:domain toop:Address ;
  rdfs:domain owl:Thing ;
  rdfs:domain skos:Concept ;
  rdfs:domain vcard:Address ;
  rdfs:domain _:b49042 ;
  rdfs:domain _:b83024 ;
  rdfs:domain _:b157701 ;
  rdfs:domain _:b168676 ;
  rdfs:domain _:b327858 ;
  rdfs:domain _:b329657 ;
  rdfs:domain _:b396249 ;
  rdfs:domain _:b401324 ;
  rdfs:domain _:b499218 ;
  rdfs:domain _:b541374 ;
  rdfs:domain _:b583853 ;
  rdfs:domain _:b593574 ;
  rdfs:domain _:b652026 ;
  rdfs:domain _:b726818 ;
  rdfs:domain _:b763315 ;
  rdfs:domain _:b787338 ;
  rdfs:domain _:b926654 ;
  rdfs:domain _:b955705 ;
  rdfs:label "huisletter"@nl ;
  rdfs:range xsd:string ;
  skos:prefLabel "huisletter"@nl ;
.
nhr:huisnummer
  rdf:type owl:DatatypeProperty ;
  rdfs:comment "Het huisnummer van het adres."@nl ;
  rdfs:domain elobr:EloniaAddress ;
  rdfs:domain freebr:FreedoniaAddress ;
  rdfs:domain nhr:Adres ;
  rdfs:domain nhr:BinnenlandsAdres ;
  rdfs:domain toop:Address ;
  rdfs:domain owl:Thing ;
  rdfs:domain skos:Concept ;
  rdfs:domain vcard:Address ;
  rdfs:domain _:b49042 ;
  rdfs:domain _:b83024 ;
  rdfs:domain _:b157701 ;
  rdfs:domain _:b168676 ;
  rdfs:domain _:b327858 ;
  rdfs:domain _:b329657 ;
  rdfs:domain _:b396249 ;
  rdfs:domain _:b401324 ;
  rdfs:domain _:b499218 ;
  rdfs:domain _:b541374 ;
  rdfs:domain _:b583853 ;
  rdfs:domain _:b593574 ;
  rdfs:domain _:b652026 ;
  rdfs:domain _:b726818 ;
  rdfs:domain _:b763315 ;
  rdfs:domain _:b787338 ;
  rdfs:domain _:b926654 ;
  rdfs:domain _:b955705 ;
  rdfs:label "huisnummer"@nl ;
  rdfs:range xsd:integer ;
  skos:prefLabel "huisnummer"@nl ;
.
nhr:huisnummerToevoeging
  rdf:type owl:DatatypeProperty ;
  rdfs:comment "Een toevoeging van het adres bijvoorbeeld rood, bis, etc."@nl ;
  rdfs:domain elobr:EloniaAddress ;
  rdfs:domain freebr:FreedoniaAddress ;
  rdfs:domain nhr:Adres ;
  rdfs:domain nhr:BinnenlandsAdres ;
  rdfs:domain toop:Address ;
  rdfs:domain owl:Thing ;
  rdfs:domain skos:Concept ;
  rdfs:domain vcard:Address ;
  rdfs:domain _:b49042 ;
  rdfs:domain _:b83024 ;
  rdfs:domain _:b157701 ;
  rdfs:domain _:b168676 ;
  rdfs:domain _:b327858 ;
  rdfs:domain _:b329657 ;
  rdfs:domain _:b396249 ;
  rdfs:domain _:b401324 ;
  rdfs:domain _:b499218 ;
  rdfs:domain _:b541374 ;
  rdfs:domain _:b583853 ;
  rdfs:domain _:b593574 ;
  rdfs:domain _:b652026 ;
  rdfs:domain _:b726818 ;
  rdfs:domain _:b763315 ;
  rdfs:domain _:b787338 ;
  rdfs:domain _:b926654 ;
  rdfs:domain _:b955705 ;
  rdfs:label "huisnummer toevoeging"@nl ;
  rdfs:range xsd:string ;
  skos:prefLabel "huisnummer toevoeging"@nl ;
.
nhr:isActiviteitVan
  rdf:type owl:ObjectProperty ;
  rdfs:comment "Een {Maatschappelijke Activiteit} is de activiteit van een {Natuurlijk persoon} of {Niet-natuurlijk persoon}."@nl ;
  rdfs:domain nhr:MaatschappelijkeActiviteit ;
  rdfs:domain owl:Thing ;
  rdfs:domain skos:Concept ;
  rdfs:domain _:b327858 ;
  rdfs:domain _:b407513 ;
  rdfs:domain _:b809403 ;
  rdfs:label "is activiteit van"@nl ;
  rdfs:range nhr:Persoon ;
  rdfs:range owl:Thing ;
  rdfs:range skos:Concept ;
  rdfs:range _:b327858 ;
  skos:prefLabel "is activiteit van"@nl ;
.
nhr:isEigenaarVan
  rdf:type owl:ObjectProperty ;
  rdfs:comment "Een Persoon is eigenaar van een MaatschappelijkeActiviteit."@nl ;
  rdfs:domain nhr:Persoon ;
  rdfs:domain owl:Thing ;
  rdfs:domain skos:Concept ;
  rdfs:domain _:b327858 ;
  rdfs:label "is eigenaar van"@nl ;
  rdfs:range nhr:MaatschappelijkeActiviteit ;
  rdfs:range owl:Thing ;
  rdfs:range skos:Concept ;
  rdfs:range _:b327858 ;
  rdfs:range _:b407513 ;
  rdfs:range _:b809403 ;
  skos:prefLabel "is eigenaar van"@nl ;
.
nhr:kvkNummer
  rdf:type owl:DatatypeProperty ;
  rdfs:comment "Alle bedrijven krijgen bij inschrijving bij de Kamer van Koophandel een KvK-nummer. Bij een bedrijfsoverdracht krijgen ondernemingen een nieuw KvK-nummer, zodat het duidelijk is dat er sprake is van een nieuwe eigenaar. U moet het nieuwe KvK-nummer vermelden op uw bedrijfscorrespondentie, zoals brieven, orders, facturen en offertes. "@nl ;
  rdfs:domain nhr:MaatschappelijkeActiviteit ;
  rdfs:domain owl:Thing ;
  rdfs:domain skos:Concept ;
  rdfs:domain _:b327858 ;
  rdfs:domain _:b407513 ;
  rdfs:domain _:b809403 ;
  rdfs:label "kvk nummer"@nl ;
  rdfs:range rdfs:Literal ;
  skos:prefLabel "kvk nummer"@nl ;
.
nhr:land
  rdf:type owl:DatatypeProperty ;
  rdfs:comment "De naam van het land waar het adres zich bevindt."@nl ;
  rdfs:domain elobr:EloniaAddress ;
  rdfs:domain freebr:FreedoniaAddress ;
  rdfs:domain nhr:Adres ;
  rdfs:domain nhr:BuitenlandsAdres ;
  rdfs:domain toop:Address ;
  rdfs:domain owl:Thing ;
  rdfs:domain skos:Concept ;
  rdfs:domain vcard:Address ;
  rdfs:domain _:b49042 ;
  rdfs:domain _:b83024 ;
  rdfs:domain _:b157701 ;
  rdfs:domain _:b168676 ;
  rdfs:domain _:b229905 ;
  rdfs:domain _:b302287 ;
  rdfs:domain _:b327858 ;
  rdfs:domain _:b396249 ;
  rdfs:domain _:b401324 ;
  rdfs:domain _:b499218 ;
  rdfs:domain _:b541374 ;
  rdfs:domain _:b583853 ;
  rdfs:domain _:b652026 ;
  rdfs:domain _:b726818 ;
  rdfs:domain _:b763315 ;
  rdfs:domain _:b787338 ;
  rdfs:domain _:b918886 ;
  rdfs:domain _:b926654 ;
  rdfs:domain _:b955705 ;
  rdfs:label "land"@nl ;
  rdfs:range xsd:string ;
  rdfs:subPropertyOf toop:countryName ;
  rdfs:subPropertyOf vcard:country-name ;
  skos:prefLabel "land"@nl ;
.
nhr:naamDomeinnaam
  rdf:type owl:DatatypeProperty ;
  rdfs:comment "Het internetadres (URL)."@nl ;
  rdfs:domain nhr:Domeinnaam ;
  rdfs:domain owl:Thing ;
  rdfs:domain skos:Concept ;
  rdfs:domain _:b327858 ;
  rdfs:domain _:b627138 ;
  rdfs:label "naam domeinnaam"@nl ;
  rdfs:range xsd:string ;
  skos:prefLabel "naam domeinnaam"@nl ;
.
nhr:naamMaatschappelijkeActiviteit
  rdf:type owl:DatatypeProperty ;
  rdfs:comment "Eerste (handels)naam van inschrijving."@nl ;
  rdfs:comment "The official current company name as stored in the business register."@en ;
  rdfs:domain elobr:Company ;
  rdfs:domain freebr:Company ;
  rdfs:domain nhr:MaatschappelijkeActiviteit ;
  rdfs:domain dcterms:Agent ;
  rdfs:domain owl:Thing ;
  rdfs:domain skos:Concept ;
  rdfs:domain org:FormalOrganization ;
  rdfs:domain org:Organization ;
  rdfs:domain foaf:Agent ;
  rdfs:domain foaf:Organization ;
  rdfs:domain _:b156576 ;
  rdfs:domain _:b213787 ;
  rdfs:domain _:b327858 ;
  rdfs:domain _:b407513 ;
  rdfs:domain _:b420951 ;
  rdfs:domain _:b421075 ;
  rdfs:domain _:b421664 ;
  rdfs:domain _:b421928 ;
  rdfs:domain _:b772676 ;
  rdfs:domain _:b809403 ;
  rdfs:domain _:b883411 ;
  rdfs:domain _:b937877 ;
  rdfs:domain _:b938265 ;
  rdfs:label "naam maatschappelijke activiteit"@nl ;
  rdfs:range rdfs:Literal ;
  rdfs:range xsd:string ;
  rdfs:subPropertyOf elobr:EloniaCompanyName ;
  rdfs:subPropertyOf freebr:FreedoniaCompanyName ;
  rdfs:subPropertyOf toop:companyName ;
  rdfs:subPropertyOf rov:legalName ;
  skos:prefLabel "naam maatschappelijke activiteit"@nl ;
.
nhr:nummerCommunicatienummer
  rdf:type owl:DatatypeProperty ;
  rdfs:comment "communicatieNummer is het telefoon- of faxnummer zonder opmaak. Zowel het netnummer als het abonneenummer worden teruggegeven in het Communicatienummer."@nl ;
  rdfs:domain nhr:Communicatienummer ;
  rdfs:domain owl:Thing ;
  rdfs:domain skos:Concept ;
  rdfs:domain _:b18002 ;
  rdfs:domain _:b327858 ;
  rdfs:domain _:b767375 ;
  rdfs:domain _:b770826 ;
  rdfs:label "nummer communicatienummer"@nl ;
  rdfs:range xsd:string ;
  skos:prefLabel "nummer communicatienummer"@nl ;
.
nhr:plaats
  rdf:type owl:DatatypeProperty ;
  rdfs:comment "De plaatsaanduiding van het adres. Dit komt overeen met het gemeentedeel in de basisregistratie personen (BRP)."@nl ;
  rdfs:domain elobr:EloniaAddress ;
  rdfs:domain freebr:FreedoniaAddress ;
  rdfs:domain nhr:Adres ;
  rdfs:domain nhr:BinnenlandsAdres ;
  rdfs:domain toop:Address ;
  rdfs:domain owl:Thing ;
  rdfs:domain skos:Concept ;
  rdfs:domain vcard:Address ;
  rdfs:domain _:b49042 ;
  rdfs:domain _:b83024 ;
  rdfs:domain _:b157701 ;
  rdfs:domain _:b168676 ;
  rdfs:domain _:b327858 ;
  rdfs:domain _:b329657 ;
  rdfs:domain _:b396249 ;
  rdfs:domain _:b401324 ;
  rdfs:domain _:b499218 ;
  rdfs:domain _:b541374 ;
  rdfs:domain _:b583853 ;
  rdfs:domain _:b593574 ;
  rdfs:domain _:b652026 ;
  rdfs:domain _:b726818 ;
  rdfs:domain _:b763315 ;
  rdfs:domain _:b787338 ;
  rdfs:domain _:b926654 ;
  rdfs:domain _:b955705 ;
  rdfs:label "plaats"@nl ;
  rdfs:range xsd:string ;
  rdfs:subPropertyOf toop:locality ;
  rdfs:subPropertyOf vcard:locality ;
  skos:prefLabel "plaats"@nl ;
.
nhr:postbusnummer
  rdf:type owl:DatatypeProperty ;
  rdfs:comment "" ;
  rdfs:domain elobr:EloniaAddress ;
  rdfs:domain freebr:FreedoniaAddress ;
  rdfs:domain nhr:Adres ;
  rdfs:domain nhr:BinnenlandsAdres ;
  rdfs:domain toop:Address ;
  rdfs:domain owl:Thing ;
  rdfs:domain skos:Concept ;
  rdfs:domain vcard:Address ;
  rdfs:domain _:b49042 ;
  rdfs:domain _:b83024 ;
  rdfs:domain _:b157701 ;
  rdfs:domain _:b168676 ;
  rdfs:domain _:b327858 ;
  rdfs:domain _:b329657 ;
  rdfs:domain _:b396249 ;
  rdfs:domain _:b401324 ;
  rdfs:domain _:b499218 ;
  rdfs:domain _:b541374 ;
  rdfs:domain _:b583853 ;
  rdfs:domain _:b593574 ;
  rdfs:domain _:b652026 ;
  rdfs:domain _:b726818 ;
  rdfs:domain _:b763315 ;
  rdfs:domain _:b787338 ;
  rdfs:domain _:b926654 ;
  rdfs:domain _:b955705 ;
  rdfs:label "postbusnummer"@nl ;
  rdfs:range xsd:integer ;
  skos:prefLabel "postbusnummer"@nl ;
.
nhr:postcode
  rdf:type owl:DatatypeProperty ;
  rdfs:comment """De in Nederland gangbare postcode voor een Nederlands postadres, bestaande uit een numeriek deel en een alfabetisch deel. Het numerieke deel van de
postcode - bestaande uit vier cijfers - identificeert een woonplaats of een gedeelte van een woonplaats. Een postcode begint niet met een nul '0'. Het alfabetische deel van de postcode - bestaande uit twee hoofdletters - identificeert binnen een woonplaats of gedeelte van een woonplaats een groep woningen, bedrijfspanden e.d., een groep postbussen, een groep antwoordnummers of een groep PostApartnummers"""@nl ;
  rdfs:domain elobr:EloniaAddress ;
  rdfs:domain freebr:FreedoniaAddress ;
  rdfs:domain nhr:Adres ;
  rdfs:domain nhr:BinnenlandsAdres ;
  rdfs:domain toop:Address ;
  rdfs:domain owl:Thing ;
  rdfs:domain skos:Concept ;
  rdfs:domain vcard:Address ;
  rdfs:domain _:b49042 ;
  rdfs:domain _:b83024 ;
  rdfs:domain _:b157701 ;
  rdfs:domain _:b168676 ;
  rdfs:domain _:b327858 ;
  rdfs:domain _:b329657 ;
  rdfs:domain _:b396249 ;
  rdfs:domain _:b401324 ;
  rdfs:domain _:b499218 ;
  rdfs:domain _:b541374 ;
  rdfs:domain _:b583853 ;
  rdfs:domain _:b593574 ;
  rdfs:domain _:b652026 ;
  rdfs:domain _:b726818 ;
  rdfs:domain _:b763315 ;
  rdfs:domain _:b787338 ;
  rdfs:domain _:b926654 ;
  rdfs:domain _:b955705 ;
  rdfs:label "postcode"@nl ;
  rdfs:range xsd:string ;
  rdfs:subPropertyOf toop:postalCode ;
  rdfs:subPropertyOf vcard:postal-code ;
  skos:prefLabel "postcode"@nl ;
.
nhr:postcodeWoonplaats
  rdf:type owl:DatatypeProperty ;
  rdfs:comment "De postcode/woonplaats is de combinatie van een eventuele postcode en woonplaats."@nl ;
  rdfs:domain elobr:EloniaAddress ;
  rdfs:domain freebr:FreedoniaAddress ;
  rdfs:domain nhr:Adres ;
  rdfs:domain nhr:BuitenlandsAdres ;
  rdfs:domain toop:Address ;
  rdfs:domain owl:Thing ;
  rdfs:domain skos:Concept ;
  rdfs:domain vcard:Address ;
  rdfs:domain _:b49042 ;
  rdfs:domain _:b83024 ;
  rdfs:domain _:b157701 ;
  rdfs:domain _:b168676 ;
  rdfs:domain _:b229905 ;
  rdfs:domain _:b302287 ;
  rdfs:domain _:b327858 ;
  rdfs:domain _:b396249 ;
  rdfs:domain _:b401324 ;
  rdfs:domain _:b499218 ;
  rdfs:domain _:b541374 ;
  rdfs:domain _:b583853 ;
  rdfs:domain _:b652026 ;
  rdfs:domain _:b726818 ;
  rdfs:domain _:b763315 ;
  rdfs:domain _:b787338 ;
  rdfs:domain _:b918886 ;
  rdfs:domain _:b926654 ;
  rdfs:domain _:b955705 ;
  rdfs:label "postcode woonplaats"@nl ;
  rdfs:range xsd:string ;
  skos:prefLabel "postcode woonplaats"@nl ;
.
nhr:regio
  rdf:type owl:DatatypeProperty ;
  rdfs:comment "Regio is een deel van het land (streek, provincie, etc.)"@nl ;
  rdfs:domain elobr:EloniaAddress ;
  rdfs:domain freebr:FreedoniaAddress ;
  rdfs:domain nhr:Adres ;
  rdfs:domain nhr:BuitenlandsAdres ;
  rdfs:domain toop:Address ;
  rdfs:domain owl:Thing ;
  rdfs:domain skos:Concept ;
  rdfs:domain vcard:Address ;
  rdfs:domain _:b49042 ;
  rdfs:domain _:b83024 ;
  rdfs:domain _:b157701 ;
  rdfs:domain _:b168676 ;
  rdfs:domain _:b229905 ;
  rdfs:domain _:b302287 ;
  rdfs:domain _:b327858 ;
  rdfs:domain _:b396249 ;
  rdfs:domain _:b401324 ;
  rdfs:domain _:b499218 ;
  rdfs:domain _:b541374 ;
  rdfs:domain _:b583853 ;
  rdfs:domain _:b652026 ;
  rdfs:domain _:b726818 ;
  rdfs:domain _:b763315 ;
  rdfs:domain _:b787338 ;
  rdfs:domain _:b918886 ;
  rdfs:domain _:b926654 ;
  rdfs:domain _:b955705 ;
  rdfs:label "regio"@nl ;
  rdfs:range xsd:string ;
  rdfs:subPropertyOf toop:region ;
  rdfs:subPropertyOf vcard:region ;
  skos:prefLabel "regio"@nl ;
.
nhr:soortCommunicatienummer
  rdf:type owl:DatatypeProperty ;
  rdfs:comment "Bevat de waarden Telefoonnummer en Faxnummer."@nl ;
  rdfs:domain nhr:Communicatienummer ;
  rdfs:domain owl:Thing ;
  rdfs:domain skos:Concept ;
  rdfs:domain _:b18002 ;
  rdfs:domain _:b327858 ;
  rdfs:domain _:b767375 ;
  rdfs:domain _:b770826 ;
  rdfs:label "soort communicatienummer"@nl ;
  rdfs:range xsd:string ;
  skos:prefLabel "soort communicatienummer"@nl ;
.
nhr:straatHuisnummer
  rdf:type owl:DatatypeProperty ;
  rdfs:comment "Het straat/huisnummer is een combinatie van de straat en huisnummer."@nl ;
  rdfs:domain elobr:EloniaAddress ;
  rdfs:domain freebr:FreedoniaAddress ;
  rdfs:domain nhr:Adres ;
  rdfs:domain nhr:BuitenlandsAdres ;
  rdfs:domain toop:Address ;
  rdfs:domain owl:Thing ;
  rdfs:domain skos:Concept ;
  rdfs:domain vcard:Address ;
  rdfs:domain _:b49042 ;
  rdfs:domain _:b83024 ;
  rdfs:domain _:b157701 ;
  rdfs:domain _:b168676 ;
  rdfs:domain _:b229905 ;
  rdfs:domain _:b302287 ;
  rdfs:domain _:b327858 ;
  rdfs:domain _:b396249 ;
  rdfs:domain _:b401324 ;
  rdfs:domain _:b499218 ;
  rdfs:domain _:b541374 ;
  rdfs:domain _:b583853 ;
  rdfs:domain _:b652026 ;
  rdfs:domain _:b726818 ;
  rdfs:domain _:b763315 ;
  rdfs:domain _:b787338 ;
  rdfs:domain _:b918886 ;
  rdfs:domain _:b926654 ;
  rdfs:domain _:b955705 ;
  rdfs:label "straat huisnummer"@nl ;
  rdfs:range xsd:string ;
  rdfs:subPropertyOf toop:streetAddress ;
  rdfs:subPropertyOf vcard:street-address ;
  skos:prefLabel "straat huisnummer"@nl ;
.
nhr:straatnaam
  rdf:type owl:DatatypeProperty ;
  rdfs:comment "De straat van het adres."@nl ;
  rdfs:domain elobr:EloniaAddress ;
  rdfs:domain freebr:FreedoniaAddress ;
  rdfs:domain nhr:Adres ;
  rdfs:domain nhr:BinnenlandsAdres ;
  rdfs:domain toop:Address ;
  rdfs:domain owl:Thing ;
  rdfs:domain skos:Concept ;
  rdfs:domain vcard:Address ;
  rdfs:domain _:b49042 ;
  rdfs:domain _:b83024 ;
  rdfs:domain _:b157701 ;
  rdfs:domain _:b168676 ;
  rdfs:domain _:b327858 ;
  rdfs:domain _:b329657 ;
  rdfs:domain _:b396249 ;
  rdfs:domain _:b401324 ;
  rdfs:domain _:b499218 ;
  rdfs:domain _:b541374 ;
  rdfs:domain _:b583853 ;
  rdfs:domain _:b593574 ;
  rdfs:domain _:b652026 ;
  rdfs:domain _:b726818 ;
  rdfs:domain _:b763315 ;
  rdfs:domain _:b787338 ;
  rdfs:domain _:b926654 ;
  rdfs:domain _:b955705 ;
  rdfs:label "straatnaam"@nl ;
  rdfs:range xsd:string ;
  skos:prefLabel "straatnaam"@nl ;
.
nhr:toegangscodeCommunicatienummer
  rdf:type owl:DatatypeProperty ;
  rdfs:comment "De internationale toegangscode van het land waarop het nummer (telefoon of fax) betrekking heeft."@nl ;
  rdfs:domain nhr:Communicatienummer ;
  rdfs:domain owl:Thing ;
  rdfs:domain skos:Concept ;
  rdfs:domain _:b18002 ;
  rdfs:domain _:b327858 ;
  rdfs:domain _:b767375 ;
  rdfs:domain _:b770826 ;
  rdfs:label "toegangscode communicatienummer"@nl ;
  rdfs:range xsd:string ;
  skos:prefLabel "toegangscode communicatienummer"@nl ;
.
nhr:voornamen
  rdf:type owl:DatatypeProperty ;
  rdfs:comment "Voornaam of voornamen van de {NatuurlijkPersoon}."@nl ;
  rdfs:domain nhr:NatuurlijkPersoon ;
  rdfs:domain nhr:Persoon ;
  rdfs:domain dcterms:Agent ;
  rdfs:domain schema:Person ;
  rdfs:domain toop:Person ;
  rdfs:domain <http://www.w3.org/2000/10/swap/pim/contact#Person> ;
  rdfs:domain owl:Thing ;
  rdfs:domain wgs:SpatialThing ;
  rdfs:domain skos:Concept ;
  rdfs:domain foaf:Agent ;
  rdfs:domain foaf:Person ;
  rdfs:domain _:b327858 ;
  rdfs:domain _:b420951 ;
  rdfs:domain _:b421075 ;
  rdfs:domain _:b421168 ;
  rdfs:domain _:b421447 ;
  rdfs:domain _:b421664 ;
  rdfs:domain _:b421928 ;
  rdfs:domain _:b546250 ;
  rdfs:domain _:b642226 ;
  rdfs:domain _:b839515 ;
  rdfs:domain _:b937877 ;
  rdfs:domain _:b938265 ;
  rdfs:label "voornamen"@nl ;
  rdfs:range xsd:string ;
  skos:prefLabel "voornamen"@nl ;
.
nhr:wordtGeleidVanuit
  rdf:type owl:ObjectProperty ;
  rdfs:comment "Een MaatschappelijkeActiviteit wordt geleid vanuit een Vestiging."@nl ;
  rdfs:domain nhr:MaatschappelijkeActiviteit ;
  rdfs:domain dcterms:Agent ;
  rdfs:domain toop:RegisteredOrganization ;
  rdfs:domain owl:Thing ;
  rdfs:domain skos:Concept ;
  rdfs:domain org:FormalOrganization ;
  rdfs:domain org:Organization ;
  rdfs:domain rov:RegisteredOrganization ;
  rdfs:domain foaf:Agent ;
  rdfs:domain foaf:Organization ;
  rdfs:domain _:b180769 ;
  rdfs:domain _:b254570 ;
  rdfs:domain _:b327858 ;
  rdfs:domain _:b407513 ;
  rdfs:domain _:b420951 ;
  rdfs:domain _:b421075 ;
  rdfs:domain _:b421664 ;
  rdfs:domain _:b421928 ;
  rdfs:domain _:b454254 ;
  rdfs:domain _:b809403 ;
  rdfs:domain _:b826282 ;
  rdfs:domain _:b826680 ;
  rdfs:domain _:b937877 ;
  rdfs:domain _:b938265 ;
  rdfs:label "wordt geleid vanuit"@nl ;
  rdfs:range nhr:Vestiging ;
  rdfs:range toop:MainSite ;
  rdfs:range owl:Thing ;
  rdfs:range skos:Concept ;
  rdfs:range org:Site ;
  rdfs:range _:b327858 ;
  rdfs:subPropertyOf toop:hasMainSite ;
  rdfs:subPropertyOf org:hasPrimarySite ;
  rdfs:subPropertyOf org:hasSite ;
  skos:prefLabel "wordt geleid vanuit"@nl ;
.
<http://ies.jrc.ec.europa.eu/DE>
  rdf:type schema:CreativeWork ;
  rdf:type foaf:Document ;
  foaf:primaryTopic _:b421478 ;
  foaf:primaryTopic _:b937645 ;
  foaf:primaryTopic _:b937815 ;
  foaf:primaryTopic _:b938079 ;
  foaf:topic _:b421478 ;
  foaf:topic _:b937645 ;
  foaf:topic _:b937815 ;
  foaf:topic _:b938079 ;
.
<http://makxdekkers.com/>
  rdf:type schema:CreativeWork ;
  rdf:type foaf:Document ;
  foaf:primaryTopic _:b421602 ;
  foaf:primaryTopic _:b937939 ;
  foaf:primaryTopic _:b938203 ;
  foaf:primaryTopic _:b938246 ;
  foaf:topic _:b421602 ;
  foaf:topic _:b937939 ;
  foaf:topic _:b938203 ;
  foaf:topic _:b938246 ;
.
<http://purl.org/dc/aboutdcmi#DCMI>
  rdf:type dcterms:Agent ;
  rdf:type foaf:Agent ;
  rdf:type _:b420951 ;
  rdf:type _:b421075 ;
  rdf:type _:b421664 ;
  rdf:type _:b421928 ;
  rdf:type _:b937877 ;
  rdf:type _:b938265 ;
.
dc:contributor
  rdf:type owl:AnnotationProperty ;
.
dc:creator
  rdf:type owl:AnnotationProperty ;
.
dc:date
  rdf:type owl:AnnotationProperty ;
.
dc:description
  rdf:type owl:AnnotationProperty ;
.
dc:title
  rdf:type owl:AnnotationProperty ;
.
dcterms:
  dc:date "2012-06-14"^^xsd:date ;
  dc:publisher <http://purl.org/dc/aboutdcmi#DCMI> ;
  dc:title "DCMI Metadata Terms - other"@en ;
  dcterms:date "2012-06-14"^^xsd:date ;
  dcterms:modified "2012-06-14"^^xsd:date ;
  dcterms:publisher <http://purl.org/dc/aboutdcmi#DCMI> ;
  dcterms:title "DCMI Metadata Terms - other"@en ;
.
dcterms:Agent
  rdf:type dcterms:AgentClass ;
  rdf:type rdfs:Class ;
  dc:date "2008-01-14"^^xsd:date ;
  dc:description "Examples of Agent include person, organization, and software agent."@en ;
  dc:relation <http://dublincore.org/usage/terms/history/#Agent-001> ;
  dcterms:date "2008-01-14"^^xsd:date ;
  dcterms:description "Examples of Agent include person, organization, and software agent."@en ;
  dcterms:hasVersion <http://dublincore.org/usage/terms/history/#Agent-001> ;
  dcterms:issued "2008-01-14"^^xsd:date ;
  dcterms:relation <http://dublincore.org/usage/terms/history/#Agent-001> ;
  rdfs:comment "A resource that acts or has the power to act."@en ;
  rdfs:isDefinedBy dcterms: ;
  rdfs:label "Agent"@en ;
  rdfs:subClassOf rdfs:Resource ;
  rdfs:subClassOf foaf:Agent ;
  owl:equivalentClass foaf:Agent ;
.
dcterms:AgentClass
  rdf:type rdfs:Class ;
  dc:date "2008-01-14"^^xsd:date ;
  dc:date "2012-06-14"^^xsd:date ;
  dc:description "Examples of Agent Class include groups seen as classes, such as students, women, charities, lecturers."@en ;
  dc:relation <http://dublincore.org/usage/terms/history/#AgentClass-003> ;
  dcterms:date "2008-01-14"^^xsd:date ;
  dcterms:date "2012-06-14"^^xsd:date ;
  dcterms:description "Examples of Agent Class include groups seen as classes, such as students, women, charities, lecturers."@en ;
  dcterms:hasVersion <http://dublincore.org/usage/terms/history/#AgentClass-003> ;
  dcterms:issued "2008-01-14"^^xsd:date ;
  dcterms:modified "2012-06-14"^^xsd:date ;
  dcterms:relation <http://dublincore.org/usage/terms/history/#AgentClass-003> ;
  rdfs:comment "A group of agents."@en ;
  rdfs:isDefinedBy dcterms: ;
  rdfs:label "Agent Class"@en ;
  rdfs:subClassOf rdfs:Class ;
  rdfs:subClassOf owl:Thing ;
.
dcterms:BibliographicResource
  rdf:type rdfs:Class ;
  dc:date "2008-01-14"^^xsd:date ;
  dc:relation <http://dublincore.org/usage/terms/history/#BibliographicResource-001> ;
  dcterms:date "2008-01-14"^^xsd:date ;
  dcterms:hasVersion <http://dublincore.org/usage/terms/history/#BibliographicResource-001> ;
  dcterms:issued "2008-01-14"^^xsd:date ;
  dcterms:relation <http://dublincore.org/usage/terms/history/#BibliographicResource-001> ;
  rdfs:comment "A book, article, or other documentary resource."@en ;
  rdfs:isDefinedBy dcterms: ;
  rdfs:label "Bibliographic Resource"@en ;
  rdfs:subClassOf rdfs:Resource ;
.
dcterms:Box
  rdf:type rdfs:Datatype ;
  dc:date "2000-07-11"^^xsd:date ;
  dc:date "2008-01-14"^^xsd:date ;
  dc:relation <http://dublincore.org/usage/terms/history/#Box-003> ;
  dcterms:date "2000-07-11"^^xsd:date ;
  dcterms:date "2008-01-14"^^xsd:date ;
  dcterms:hasVersion <http://dublincore.org/usage/terms/history/#Box-003> ;
  dcterms:issued "2000-07-11"^^xsd:date ;
  dcterms:modified "2008-01-14"^^xsd:date ;
  dcterms:relation <http://dublincore.org/usage/terms/history/#Box-003> ;
  rdfs:comment "The set of regions in space defined by their geographic coordinates according to the DCMI Box Encoding Scheme."@en ;
  rdfs:isDefinedBy dcterms: ;
  rdfs:label "DCMI Box"@en ;
  rdfs:seeAlso <http://dublincore.org/documents/dcmi-box/> ;
  rdfs:subClassOf rdfs:Resource ;
.
dcterms:DCMIType
  rdf:type dcam:VocabularyEncodingScheme ;
  dc:date "2000-07-11"^^xsd:date ;
  dc:date "2012-06-14"^^xsd:date ;
  dc:relation <http://dublincore.org/usage/terms/history/#DCMIType-005> ;
  dcterms:date "2000-07-11"^^xsd:date ;
  dcterms:date "2012-06-14"^^xsd:date ;
  dcterms:hasVersion <http://dublincore.org/usage/terms/history/#DCMIType-005> ;
  dcterms:issued "2000-07-11"^^xsd:date ;
  dcterms:modified "2012-06-14"^^xsd:date ;
  dcterms:relation <http://dublincore.org/usage/terms/history/#DCMIType-005> ;
  rdfs:comment "The set of classes specified by the DCMI Type Vocabulary, used to categorize the nature or genre of the resource."@en ;
  rdfs:isDefinedBy dcterms: ;
  rdfs:label "DCMI Type Vocabulary"@en ;
  rdfs:seeAlso <http://purl.org/dc/dcmitype/> ;
.
dcterms:DDC
  rdf:type dcam:VocabularyEncodingScheme ;
  dc:date "2000-07-11"^^xsd:date ;
  dc:date "2008-01-14"^^xsd:date ;
  dc:relation <http://dublincore.org/usage/terms/history/#DDC-003> ;
  dcterms:date "2000-07-11"^^xsd:date ;
  dcterms:date "2008-01-14"^^xsd:date ;
  dcterms:hasVersion <http://dublincore.org/usage/terms/history/#DDC-003> ;
  dcterms:issued "2000-07-11"^^xsd:date ;
  dcterms:modified "2008-01-14"^^xsd:date ;
  dcterms:relation <http://dublincore.org/usage/terms/history/#DDC-003> ;
  rdfs:comment "The set of conceptual resources specified by the Dewey Decimal Classification."@en ;
  rdfs:isDefinedBy dcterms: ;
  rdfs:label "DDC"@en ;
  rdfs:seeAlso <http://www.oclc.org/dewey/> ;
.
dcterms:FileFormat
  rdf:type rdfs:Class ;
  dc:date "2008-01-14"^^xsd:date ;
  dc:description "Examples include the formats defined by the list of Internet Media Types."@en ;
  dc:relation <http://dublincore.org/usage/terms/history/#FileFormat-001> ;
  dcterms:date "2008-01-14"^^xsd:date ;
  dcterms:description "Examples include the formats defined by the list of Internet Media Types."@en ;
  dcterms:hasVersion <http://dublincore.org/usage/terms/history/#FileFormat-001> ;
  dcterms:issued "2008-01-14"^^xsd:date ;
  dcterms:relation <http://dublincore.org/usage/terms/history/#FileFormat-001> ;
  rdfs:comment "A digital resource format."@en ;
  rdfs:isDefinedBy dcterms: ;
  rdfs:label "File Format"@en ;
  rdfs:subClassOf dcterms:MediaType ;
  rdfs:subClassOf dcterms:MediaTypeOrExtent ;
.
dcterms:Frequency
  rdf:type rdfs:Class ;
  dc:date "2008-01-14"^^xsd:date ;
  dc:relation <http://dublincore.org/usage/terms/history/#Frequency-001> ;
  dcterms:date "2008-01-14"^^xsd:date ;
  dcterms:hasVersion <http://dublincore.org/usage/terms/history/#Frequency-001> ;
  dcterms:issued "2008-01-14"^^xsd:date ;
  dcterms:relation <http://dublincore.org/usage/terms/history/#Frequency-001> ;
  rdfs:comment "A rate at which something recurs."@en ;
  rdfs:isDefinedBy dcterms: ;
  rdfs:label "Frequency"@en ;
  rdfs:subClassOf rdfs:Resource ;
.
dcterms:IMT
  rdf:type dcam:VocabularyEncodingScheme ;
  dc:date "2000-07-11"^^xsd:date ;
  dc:date "2008-01-14"^^xsd:date ;
  dc:relation <http://dublincore.org/usage/terms/history/#IMT-004> ;
  dcterms:date "2000-07-11"^^xsd:date ;
  dcterms:date "2008-01-14"^^xsd:date ;
  dcterms:hasVersion <http://dublincore.org/usage/terms/history/#IMT-004> ;
  dcterms:issued "2000-07-11"^^xsd:date ;
  dcterms:modified "2008-01-14"^^xsd:date ;
  dcterms:relation <http://dublincore.org/usage/terms/history/#IMT-004> ;
  rdfs:comment "The set of media types specified by the Internet Assigned Numbers Authority."@en ;
  rdfs:isDefinedBy dcterms: ;
  rdfs:label "IMT"@en ;
  rdfs:seeAlso <http://www.iana.org/assignments/media-types/> ;
.
dcterms:ISO3166
  rdf:type rdfs:Datatype ;
  dc:date "2000-07-11"^^xsd:date ;
  dc:date "2008-01-14"^^xsd:date ;
  dc:relation <http://dublincore.org/usage/terms/history/#ISO3166-004> ;
  dcterms:date "2000-07-11"^^xsd:date ;
  dcterms:date "2008-01-14"^^xsd:date ;
  dcterms:hasVersion <http://dublincore.org/usage/terms/history/#ISO3166-004> ;
  dcterms:issued "2000-07-11"^^xsd:date ;
  dcterms:modified "2008-01-14"^^xsd:date ;
  dcterms:relation <http://dublincore.org/usage/terms/history/#ISO3166-004> ;
  rdfs:comment "The set of codes listed in ISO 3166-1 for the representation of names of countries."@en ;
  rdfs:isDefinedBy dcterms: ;
  rdfs:label "ISO 3166"@en ;
  rdfs:seeAlso <http://www.iso.org/iso/en/prods-services/iso3166ma/02iso-3166-code-lists/list-en1.html> ;
  rdfs:subClassOf rdfs:Resource ;
.
dcterms:ISO639-2
  rdf:type rdfs:Datatype ;
  dc:date "2000-07-11"^^xsd:date ;
  dc:date "2008-01-14"^^xsd:date ;
  dc:relation <http://dublincore.org/usage/terms/history/#ISO639-2-003> ;
  dcterms:date "2000-07-11"^^xsd:date ;
  dcterms:date "2008-01-14"^^xsd:date ;
  dcterms:hasVersion <http://dublincore.org/usage/terms/history/#ISO639-2-003> ;
  dcterms:issued "2000-07-11"^^xsd:date ;
  dcterms:modified "2008-01-14"^^xsd:date ;
  dcterms:relation <http://dublincore.org/usage/terms/history/#ISO639-2-003> ;
  rdfs:comment "The three-letter alphabetic codes listed in ISO639-2 for the representation of names of languages."@en ;
  rdfs:isDefinedBy dcterms: ;
  rdfs:label "ISO 639-2"@en ;
  rdfs:seeAlso <http://lcweb.loc.gov/standards/iso639-2/langhome.html> ;
  rdfs:subClassOf rdfs:Resource ;
.
dcterms:ISO639-3
  rdf:type rdfs:Datatype ;
  dc:date "2008-01-14"^^xsd:date ;
  dc:relation <http://dublincore.org/usage/terms/history/#ISO639-3-001> ;
  dcterms:date "2008-01-14"^^xsd:date ;
  dcterms:hasVersion <http://dublincore.org/usage/terms/history/#ISO639-3-001> ;
  dcterms:issued "2008-01-14"^^xsd:date ;
  dcterms:relation <http://dublincore.org/usage/terms/history/#ISO639-3-001> ;
  rdfs:comment "The set of three-letter codes listed in ISO 639-3 for the representation of names of languages."@en ;
  rdfs:isDefinedBy dcterms: ;
  rdfs:label "ISO 639-3"@en ;
  rdfs:seeAlso <http://www.sil.org/iso639-3/> ;
  rdfs:subClassOf rdfs:Resource ;
.
dcterms:Jurisdiction
  rdf:type rdfs:Class ;
  dc:date "2008-01-14"^^xsd:date ;
  dc:relation <http://dublincore.org/usage/terms/history/#Jurisdiction-001> ;
  dcterms:date "2008-01-14"^^xsd:date ;
  dcterms:hasVersion <http://dublincore.org/usage/terms/history/#Jurisdiction-001> ;
  dcterms:issued "2008-01-14"^^xsd:date ;
  dcterms:relation <http://dublincore.org/usage/terms/history/#Jurisdiction-001> ;
  rdfs:comment "The extent or range of judicial, law enforcement, or other authority."@en ;
  rdfs:isDefinedBy dcterms: ;
  rdfs:label "Jurisdiction"@en ;
  rdfs:subClassOf dcterms:LocationPeriodOrJurisdiction ;
.
dcterms:LCC
  rdf:type dcam:VocabularyEncodingScheme ;
  dc:date "2000-07-11"^^xsd:date ;
  dc:date "2008-01-14"^^xsd:date ;
  dc:relation <http://dublincore.org/usage/terms/history/#LCC-003> ;
  dcterms:date "2000-07-11"^^xsd:date ;
  dcterms:date "2008-01-14"^^xsd:date ;
  dcterms:hasVersion <http://dublincore.org/usage/terms/history/#LCC-003> ;
  dcterms:issued "2000-07-11"^^xsd:date ;
  dcterms:modified "2008-01-14"^^xsd:date ;
  dcterms:relation <http://dublincore.org/usage/terms/history/#LCC-003> ;
  rdfs:comment "The set of conceptual resources specified by the Library of Congress Classification."@en ;
  rdfs:isDefinedBy dcterms: ;
  rdfs:label "LCC"@en ;
  rdfs:seeAlso <http://lcweb.loc.gov/catdir/cpso/lcco/lcco.html> ;
.
dcterms:LCSH
  rdf:type dcam:VocabularyEncodingScheme ;
  dc:date "2000-07-11"^^xsd:date ;
  dc:date "2008-01-14"^^xsd:date ;
  dc:relation <http://dublincore.org/usage/terms/history/#LCSH-003> ;
  dcterms:date "2000-07-11"^^xsd:date ;
  dcterms:date "2008-01-14"^^xsd:date ;
  dcterms:hasVersion <http://dublincore.org/usage/terms/history/#LCSH-003> ;
  dcterms:issued "2000-07-11"^^xsd:date ;
  dcterms:modified "2008-01-14"^^xsd:date ;
  dcterms:relation <http://dublincore.org/usage/terms/history/#LCSH-003> ;
  rdfs:comment "The set of labeled concepts specified by the Library of Congress Subject Headings."@en ;
  rdfs:isDefinedBy dcterms: ;
  rdfs:label "LCSH"@en ;
.
dcterms:LicenseDocument
  rdf:type rdfs:Class ;
  dc:date "2008-01-14"^^xsd:date ;
  dc:relation <http://dublincore.org/usage/terms/history/#LicenseDocument-001> ;
  dcterms:date "2008-01-14"^^xsd:date ;
  dcterms:hasVersion <http://dublincore.org/usage/terms/history/#LicenseDocument-001> ;
  dcterms:issued "2008-01-14"^^xsd:date ;
  dcterms:relation <http://dublincore.org/usage/terms/history/#LicenseDocument-001> ;
  rdfs:comment "A legal document giving official permission to do something with a Resource."@en ;
  rdfs:isDefinedBy dcterms: ;
  rdfs:label "License Document"@en ;
  rdfs:subClassOf dcterms:RightsStatement ;
.
dcterms:LinguisticSystem
  rdf:type rdfs:Class ;
  dc:date "2008-01-14"^^xsd:date ;
  dc:description "Examples include written, spoken, sign, and computer languages."@en ;
  dc:relation <http://dublincore.org/usage/terms/history/#LinguisticSystem-001> ;
  dcterms:date "2008-01-14"^^xsd:date ;
  dcterms:description "Examples include written, spoken, sign, and computer languages."@en ;
  dcterms:hasVersion <http://dublincore.org/usage/terms/history/#LinguisticSystem-001> ;
  dcterms:issued "2008-01-14"^^xsd:date ;
  dcterms:relation <http://dublincore.org/usage/terms/history/#LinguisticSystem-001> ;
  rdfs:comment "A system of signs, symbols, sounds, gestures, or rules used in communication."@en ;
  rdfs:isDefinedBy dcterms: ;
  rdfs:label "Linguistic System"@en ;
  rdfs:subClassOf rdfs:Resource ;
.
dcterms:Location
  rdf:type rdfs:Class ;
  dc:date "2008-01-14"^^xsd:date ;
  dc:relation <http://dublincore.org/usage/terms/history/#Location-001> ;
  dcterms:date "2008-01-14"^^xsd:date ;
  dcterms:hasVersion <http://dublincore.org/usage/terms/history/#Location-001> ;
  dcterms:issued "2008-01-14"^^xsd:date ;
  dcterms:relation <http://dublincore.org/usage/terms/history/#Location-001> ;
  rdfs:comment "A spatial region or named place."@en ;
  rdfs:isDefinedBy dcterms: ;
  rdfs:label "Location"@en ;
  rdfs:subClassOf dcterms:LocationPeriodOrJurisdiction ;
.
dcterms:LocationPeriodOrJurisdiction
  rdf:type rdfs:Class ;
  dc:date "2008-01-14"^^xsd:date ;
  dc:relation <http://dublincore.org/usage/terms/history/#LocationPeriodOrJurisdiction-001> ;
  dcterms:date "2008-01-14"^^xsd:date ;
  dcterms:hasVersion <http://dublincore.org/usage/terms/history/#LocationPeriodOrJurisdiction-001> ;
  dcterms:issued "2008-01-14"^^xsd:date ;
  dcterms:relation <http://dublincore.org/usage/terms/history/#LocationPeriodOrJurisdiction-001> ;
  rdfs:comment "A location, period of time, or jurisdiction."@en ;
  rdfs:isDefinedBy dcterms: ;
  rdfs:label "Location, Period, or Jurisdiction"@en ;
  rdfs:subClassOf rdfs:Resource ;
.
dcterms:MESH
  rdf:type dcam:VocabularyEncodingScheme ;
  dc:date "2000-07-11"^^xsd:date ;
  dc:date "2008-01-14"^^xsd:date ;
  dc:relation <http://dublincore.org/usage/terms/history/#MESH-003> ;
  dcterms:date "2000-07-11"^^xsd:date ;
  dcterms:date "2008-01-14"^^xsd:date ;
  dcterms:hasVersion <http://dublincore.org/usage/terms/history/#MESH-003> ;
  dcterms:issued "2000-07-11"^^xsd:date ;
  dcterms:modified "2008-01-14"^^xsd:date ;
  dcterms:relation <http://dublincore.org/usage/terms/history/#MESH-003> ;
  rdfs:comment "The set of labeled concepts specified by the Medical Subject Headings."@en ;
  rdfs:isDefinedBy dcterms: ;
  rdfs:label "MeSH"@en ;
  rdfs:seeAlso <http://www.nlm.nih.gov/mesh/meshhome.html> ;
.
dcterms:MediaType
  rdf:type rdfs:Class ;
  dc:date "2008-01-14"^^xsd:date ;
  dc:relation <http://dublincore.org/usage/terms/history/#MediaType-001> ;
  dcterms:date "2008-01-14"^^xsd:date ;
  dcterms:hasVersion <http://dublincore.org/usage/terms/history/#MediaType-001> ;
  dcterms:issued "2008-01-14"^^xsd:date ;
  dcterms:relation <http://dublincore.org/usage/terms/history/#MediaType-001> ;
  rdfs:comment "A file format or physical medium."@en ;
  rdfs:isDefinedBy dcterms: ;
  rdfs:label "Media Type"@en ;
  rdfs:subClassOf dcterms:MediaTypeOrExtent ;
.
dcterms:MediaTypeOrExtent
  rdf:type rdfs:Class ;
  dc:date "2008-01-14"^^xsd:date ;
  dc:relation <http://dublincore.org/usage/terms/history/#MediaTypeOrExtent-001> ;
  dcterms:date "2008-01-14"^^xsd:date ;
  dcterms:hasVersion <http://dublincore.org/usage/terms/history/#MediaTypeOrExtent-001> ;
  dcterms:issued "2008-01-14"^^xsd:date ;
  dcterms:relation <http://dublincore.org/usage/terms/history/#MediaTypeOrExtent-001> ;
  rdfs:comment "A media type or extent."@en ;
  rdfs:isDefinedBy dcterms: ;
  rdfs:label "Media Type or Extent"@en ;
  rdfs:subClassOf rdfs:Resource ;
.
dcterms:MethodOfAccrual
  rdf:type rdfs:Class ;
  dc:date "2008-01-14"^^xsd:date ;
  dc:relation <http://dublincore.org/usage/terms/history/#MethodOfAccrual-001> ;
  dcterms:date "2008-01-14"^^xsd:date ;
  dcterms:hasVersion <http://dublincore.org/usage/terms/history/#MethodOfAccrual-001> ;
  dcterms:issued "2008-01-14"^^xsd:date ;
  dcterms:relation <http://dublincore.org/usage/terms/history/#MethodOfAccrual-001> ;
  rdfs:comment "A method by which resources are added to a collection."@en ;
  rdfs:isDefinedBy dcterms: ;
  rdfs:label "Method of Accrual"@en ;
  rdfs:subClassOf rdfs:Resource ;
.
dcterms:MethodOfInstruction
  rdf:type rdfs:Class ;
  dc:date "2008-01-14"^^xsd:date ;
  dc:relation <http://dublincore.org/usage/terms/history/#MethodOfInstruction-001> ;
  dcterms:date "2008-01-14"^^xsd:date ;
  dcterms:hasVersion <http://dublincore.org/usage/terms/history/#MethodOfInstruction-001> ;
  dcterms:issued "2008-01-14"^^xsd:date ;
  dcterms:relation <http://dublincore.org/usage/terms/history/#MethodOfInstruction-001> ;
  rdfs:comment "A process that is used to engender knowledge, attitudes, and skills."@en ;
  rdfs:isDefinedBy dcterms: ;
  rdfs:label "Method of Instruction"@en ;
  rdfs:subClassOf rdfs:Resource ;
.
dcterms:NLM
  rdf:type dcam:VocabularyEncodingScheme ;
  dc:date "2005-06-13"^^xsd:date ;
  dc:date "2008-01-14"^^xsd:date ;
  dc:relation <http://dublincore.org/usage/terms/history/#NLM-002> ;
  dcterms:date "2005-06-13"^^xsd:date ;
  dcterms:date "2008-01-14"^^xsd:date ;
  dcterms:hasVersion <http://dublincore.org/usage/terms/history/#NLM-002> ;
  dcterms:issued "2005-06-13"^^xsd:date ;
  dcterms:modified "2008-01-14"^^xsd:date ;
  dcterms:relation <http://dublincore.org/usage/terms/history/#NLM-002> ;
  rdfs:comment "The set of conceptual resources specified by the National Library of Medicine Classification."@en ;
  rdfs:isDefinedBy dcterms: ;
  rdfs:label "NLM"@en ;
  rdfs:seeAlso <http://wwwcf.nlm.nih.gov/class/> ;
.
dcterms:Period
  rdf:type rdfs:Datatype ;
  dc:date "2000-07-11"^^xsd:date ;
  dc:date "2008-01-14"^^xsd:date ;
  dc:relation <http://dublincore.org/usage/terms/history/#Period-003> ;
  dcterms:date "2000-07-11"^^xsd:date ;
  dcterms:date "2008-01-14"^^xsd:date ;
  dcterms:hasVersion <http://dublincore.org/usage/terms/history/#Period-003> ;
  dcterms:issued "2000-07-11"^^xsd:date ;
  dcterms:modified "2008-01-14"^^xsd:date ;
  dcterms:relation <http://dublincore.org/usage/terms/history/#Period-003> ;
  rdfs:comment "The set of time intervals defined by their limits according to the DCMI Period Encoding Scheme."@en ;
  rdfs:isDefinedBy dcterms: ;
  rdfs:label "DCMI Period"@en ;
  rdfs:seeAlso <http://dublincore.org/documents/dcmi-period/> ;
  rdfs:subClassOf rdfs:Resource ;
.
dcterms:PeriodOfTime
  rdf:type rdfs:Class ;
  dc:date "2008-01-14"^^xsd:date ;
  dc:relation <http://dublincore.org/usage/terms/history/#PeriodOfTime-001> ;
  dcterms:date "2008-01-14"^^xsd:date ;
  dcterms:hasVersion <http://dublincore.org/usage/terms/history/#PeriodOfTime-001> ;
  dcterms:issued "2008-01-14"^^xsd:date ;
  dcterms:relation <http://dublincore.org/usage/terms/history/#PeriodOfTime-001> ;
  rdfs:comment "An interval of time that is named or defined by its start and end dates."@en ;
  rdfs:isDefinedBy dcterms: ;
  rdfs:label "Period of Time"@en ;
  rdfs:subClassOf dcterms:LocationPeriodOrJurisdiction ;
.
dcterms:PhysicalMedium
  rdf:type rdfs:Class ;
  dc:date "2008-01-14"^^xsd:date ;
  dc:description "Examples include paper, canvas, or DVD."@en ;
  dc:relation <http://dublincore.org/usage/terms/history/#PhysicalMedium-001> ;
  dcterms:date "2008-01-14"^^xsd:date ;
  dcterms:description "Examples include paper, canvas, or DVD."@en ;
  dcterms:hasVersion <http://dublincore.org/usage/terms/history/#PhysicalMedium-001> ;
  dcterms:issued "2008-01-14"^^xsd:date ;
  dcterms:relation <http://dublincore.org/usage/terms/history/#PhysicalMedium-001> ;
  rdfs:comment "A physical material or carrier."@en ;
  rdfs:isDefinedBy dcterms: ;
  rdfs:label "Physical Medium"@en ;
  rdfs:subClassOf dcterms:MediaType ;
  rdfs:subClassOf dcterms:MediaTypeOrExtent ;
.
dcterms:PhysicalResource
  rdf:type rdfs:Class ;
  dc:date "2008-01-14"^^xsd:date ;
  dc:relation <http://dublincore.org/usage/terms/history/#PhysicalResource-001> ;
  dcterms:date "2008-01-14"^^xsd:date ;
  dcterms:hasVersion <http://dublincore.org/usage/terms/history/#PhysicalResource-001> ;
  dcterms:issued "2008-01-14"^^xsd:date ;
  dcterms:relation <http://dublincore.org/usage/terms/history/#PhysicalResource-001> ;
  rdfs:comment "A material thing."@en ;
  rdfs:isDefinedBy dcterms: ;
  rdfs:label "Physical Resource"@en ;
  rdfs:subClassOf rdfs:Resource ;
.
dcterms:Point
  rdf:type rdfs:Datatype ;
  dc:date "2000-07-11"^^xsd:date ;
  dc:date "2008-01-14"^^xsd:date ;
  dc:relation <http://dublincore.org/usage/terms/history/#Point-003> ;
  dcterms:date "2000-07-11"^^xsd:date ;
  dcterms:date "2008-01-14"^^xsd:date ;
  dcterms:hasVersion <http://dublincore.org/usage/terms/history/#Point-003> ;
  dcterms:issued "2000-07-11"^^xsd:date ;
  dcterms:modified "2008-01-14"^^xsd:date ;
  dcterms:relation <http://dublincore.org/usage/terms/history/#Point-003> ;
  rdfs:comment "The set of points in space defined by their geographic coordinates according to the DCMI Point Encoding Scheme."@en ;
  rdfs:isDefinedBy dcterms: ;
  rdfs:label "DCMI Point"@en ;
  rdfs:seeAlso <http://dublincore.org/documents/dcmi-point/> ;
  rdfs:subClassOf rdfs:Resource ;
.
dcterms:Policy
  rdf:type rdfs:Class ;
  dc:date "2008-01-14"^^xsd:date ;
  dc:relation <http://dublincore.org/usage/terms/history/#Policy-001> ;
  dcterms:date "2008-01-14"^^xsd:date ;
  dcterms:hasVersion <http://dublincore.org/usage/terms/history/#Policy-001> ;
  dcterms:issued "2008-01-14"^^xsd:date ;
  dcterms:relation <http://dublincore.org/usage/terms/history/#Policy-001> ;
  rdfs:comment "A plan or course of action by an authority, intended to influence and determine decisions, actions, and other matters."@en ;
  rdfs:isDefinedBy dcterms: ;
  rdfs:label "Policy"@en ;
  rdfs:subClassOf rdfs:Resource ;
.
dcterms:ProvenanceStatement
  rdf:type rdfs:Class ;
  dc:date "2008-01-14"^^xsd:date ;
  dc:relation <http://dublincore.org/usage/terms/history/#ProvenanceStatement-001> ;
  dcterms:date "2008-01-14"^^xsd:date ;
  dcterms:hasVersion <http://dublincore.org/usage/terms/history/#ProvenanceStatement-001> ;
  dcterms:issued "2008-01-14"^^xsd:date ;
  dcterms:relation <http://dublincore.org/usage/terms/history/#ProvenanceStatement-001> ;
  rdfs:comment "A statement of any changes in ownership and custody of a resource since its creation that are significant for its authenticity, integrity, and interpretation."@en ;
  rdfs:isDefinedBy dcterms: ;
  rdfs:label "Provenance Statement"@en ;
  rdfs:subClassOf rdfs:Resource ;
.
dcterms:RFC1766
  rdf:type rdfs:Datatype ;
  dc:date "2000-07-11"^^xsd:date ;
  dc:date "2008-01-14"^^xsd:date ;
  dc:relation <http://dublincore.org/usage/terms/history/#RFC1766-003> ;
  dcterms:date "2000-07-11"^^xsd:date ;
  dcterms:date "2008-01-14"^^xsd:date ;
  dcterms:hasVersion <http://dublincore.org/usage/terms/history/#RFC1766-003> ;
  dcterms:issued "2000-07-11"^^xsd:date ;
  dcterms:modified "2008-01-14"^^xsd:date ;
  dcterms:relation <http://dublincore.org/usage/terms/history/#RFC1766-003> ;
  rdfs:comment "The set of tags, constructed according to RFC 1766, for the identification of languages."@en ;
  rdfs:isDefinedBy dcterms: ;
  rdfs:label "RFC 1766"@en ;
  rdfs:seeAlso <http://www.ietf.org/rfc/rfc1766.txt> ;
  rdfs:subClassOf rdfs:Resource ;
.
dcterms:RFC3066
  rdf:type rdfs:Datatype ;
  dc:date "2002-07-13"^^xsd:date ;
  dc:date "2008-01-14"^^xsd:date ;
  dc:description "RFC 3066 has been obsoleted by RFC 4646."@en ;
  dc:relation <http://dublincore.org/usage/terms/history/#RFC3066-002> ;
  dcterms:date "2002-07-13"^^xsd:date ;
  dcterms:date "2008-01-14"^^xsd:date ;
  dcterms:description "RFC 3066 has been obsoleted by RFC 4646."@en ;
  dcterms:hasVersion <http://dublincore.org/usage/terms/history/#RFC3066-002> ;
  dcterms:issued "2002-07-13"^^xsd:date ;
  dcterms:modified "2008-01-14"^^xsd:date ;
  dcterms:relation <http://dublincore.org/usage/terms/history/#RFC3066-002> ;
  rdfs:comment "The set of tags constructed according to RFC 3066 for the identification of languages."@en ;
  rdfs:isDefinedBy dcterms: ;
  rdfs:label "RFC 3066"@en ;
  rdfs:seeAlso <http://www.ietf.org/rfc/rfc3066.txt> ;
  rdfs:subClassOf rdfs:Resource ;
.
dcterms:RFC4646
  rdf:type rdfs:Datatype ;
  dc:date "2008-01-14"^^xsd:date ;
  dc:description "RFC 4646 obsoletes RFC 3066."@en ;
  dc:relation <http://dublincore.org/usage/terms/history/#RFC4646-001> ;
  dcterms:date "2008-01-14"^^xsd:date ;
  dcterms:description "RFC 4646 obsoletes RFC 3066."@en ;
  dcterms:hasVersion <http://dublincore.org/usage/terms/history/#RFC4646-001> ;
  dcterms:issued "2008-01-14"^^xsd:date ;
  dcterms:relation <http://dublincore.org/usage/terms/history/#RFC4646-001> ;
  rdfs:comment "The set of tags constructed according to RFC 4646 for the identification of languages."@en ;
  rdfs:isDefinedBy dcterms: ;
  rdfs:label "RFC 4646"@en ;
  rdfs:seeAlso <http://www.ietf.org/rfc/rfc4646.txt> ;
  rdfs:subClassOf rdfs:Resource ;
.
dcterms:RFC5646
  rdf:type rdfs:Datatype ;
  dc:date "2010-10-11"^^xsd:date ;
  dc:description "RFC 5646 obsoletes RFC 4646."@en ;
  dc:relation <http://dublincore.org/usage/terms/history/#RFC5646-001> ;
  dcterms:date "2010-10-11"^^xsd:date ;
  dcterms:description "RFC 5646 obsoletes RFC 4646."@en ;
  dcterms:hasVersion <http://dublincore.org/usage/terms/history/#RFC5646-001> ;
  dcterms:issued "2010-10-11"^^xsd:date ;
  dcterms:relation <http://dublincore.org/usage/terms/history/#RFC5646-001> ;
  rdfs:comment "The set of tags constructed according to RFC 5646 for the identification of languages."@en ;
  rdfs:isDefinedBy dcterms: ;
  rdfs:label "RFC 5646"@en ;
  rdfs:seeAlso <http://www.ietf.org/rfc/rfc5646.txt> ;
  rdfs:subClassOf rdfs:Resource ;
.
dcterms:RightsStatement
  rdf:type rdfs:Class ;
  dc:date "2008-01-14"^^xsd:date ;
  dc:relation <http://dublincore.org/usage/terms/history/#RightsStatement-001> ;
  dcterms:date "2008-01-14"^^xsd:date ;
  dcterms:hasVersion <http://dublincore.org/usage/terms/history/#RightsStatement-001> ;
  dcterms:issued "2008-01-14"^^xsd:date ;
  dcterms:relation <http://dublincore.org/usage/terms/history/#RightsStatement-001> ;
  rdfs:comment "A statement about the intellectual property rights (IPR) held in or over a Resource, a legal document giving official permission to do something with a resource, or a statement about access rights."@en ;
  rdfs:isDefinedBy dcterms: ;
  rdfs:label "Rights Statement"@en ;
  rdfs:subClassOf rdfs:Resource ;
.
dcterms:SizeOrDuration
  rdf:type rdfs:Class ;
  dc:date "2008-01-14"^^xsd:date ;
  dc:description "Examples include a number of pages, a specification of length, width, and breadth, or a period in hours, minutes, and seconds."@en ;
  dc:relation <http://dublincore.org/usage/terms/history/#SizeOrDuration-001> ;
  dcterms:date "2008-01-14"^^xsd:date ;
  dcterms:description "Examples include a number of pages, a specification of length, width, and breadth, or a period in hours, minutes, and seconds."@en ;
  dcterms:hasVersion <http://dublincore.org/usage/terms/history/#SizeOrDuration-001> ;
  dcterms:issued "2008-01-14"^^xsd:date ;
  dcterms:relation <http://dublincore.org/usage/terms/history/#SizeOrDuration-001> ;
  rdfs:comment "A dimension or extent, or a time taken to play or execute."@en ;
  rdfs:isDefinedBy dcterms: ;
  rdfs:label "Size or Duration"@en ;
  rdfs:subClassOf dcterms:MediaTypeOrExtent ;
.
dcterms:Standard
  rdf:type rdfs:Class ;
  dc:date "2008-01-14"^^xsd:date ;
  dc:relation <http://dublincore.org/usage/terms/history/#Standard-001> ;
  dcterms:date "2008-01-14"^^xsd:date ;
  dcterms:hasVersion <http://dublincore.org/usage/terms/history/#Standard-001> ;
  dcterms:issued "2008-01-14"^^xsd:date ;
  dcterms:relation <http://dublincore.org/usage/terms/history/#Standard-001> ;
  rdfs:comment "A basis for comparison; a reference point against which other things can be evaluated."@en ;
  rdfs:isDefinedBy dcterms: ;
  rdfs:label "Standard"@en ;
  rdfs:subClassOf rdfs:Resource ;
.
dcterms:TGN
  rdf:type dcam:VocabularyEncodingScheme ;
  dc:date "2000-07-11"^^xsd:date ;
  dc:date "2008-01-14"^^xsd:date ;
  dc:relation <http://dublincore.org/usage/terms/history/#TGN-003> ;
  dcterms:date "2000-07-11"^^xsd:date ;
  dcterms:date "2008-01-14"^^xsd:date ;
  dcterms:hasVersion <http://dublincore.org/usage/terms/history/#TGN-003> ;
  dcterms:issued "2000-07-11"^^xsd:date ;
  dcterms:modified "2008-01-14"^^xsd:date ;
  dcterms:relation <http://dublincore.org/usage/terms/history/#TGN-003> ;
  rdfs:comment "The set of places specified by the Getty Thesaurus of Geographic Names."@en ;
  rdfs:isDefinedBy dcterms: ;
  rdfs:label "TGN"@en ;
  rdfs:seeAlso <http://www.getty.edu/research/tools/vocabulary/tgn/index.html> ;
.
dcterms:UDC
  rdf:type dcam:VocabularyEncodingScheme ;
  dc:date "2000-07-11"^^xsd:date ;
  dc:date "2008-01-14"^^xsd:date ;
  dc:relation <http://dublincore.org/usage/terms/history/#UDC-003> ;
  dcterms:date "2000-07-11"^^xsd:date ;
  dcterms:date "2008-01-14"^^xsd:date ;
  dcterms:hasVersion <http://dublincore.org/usage/terms/history/#UDC-003> ;
  dcterms:issued "2000-07-11"^^xsd:date ;
  dcterms:modified "2008-01-14"^^xsd:date ;
  dcterms:relation <http://dublincore.org/usage/terms/history/#UDC-003> ;
  rdfs:comment "The set of conceptual resources specified by the Universal Decimal Classification."@en ;
  rdfs:isDefinedBy dcterms: ;
  rdfs:label "UDC"@en ;
  rdfs:seeAlso <http://www.udcc.org/> ;
.
dcterms:URI
  rdf:type rdfs:Datatype ;
  dc:date "2000-07-11"^^xsd:date ;
  dc:date "2008-01-14"^^xsd:date ;
  dc:relation <http://dublincore.org/usage/terms/history/#URI-003> ;
  dcterms:date "2000-07-11"^^xsd:date ;
  dcterms:date "2008-01-14"^^xsd:date ;
  dcterms:hasVersion <http://dublincore.org/usage/terms/history/#URI-003> ;
  dcterms:issued "2000-07-11"^^xsd:date ;
  dcterms:modified "2008-01-14"^^xsd:date ;
  dcterms:relation <http://dublincore.org/usage/terms/history/#URI-003> ;
  rdfs:comment "The set of identifiers constructed according to the generic syntax for Uniform Resource Identifiers as specified by the Internet Engineering Task Force."@en ;
  rdfs:isDefinedBy dcterms: ;
  rdfs:label "URI"@en ;
  rdfs:seeAlso <http://www.ietf.org/rfc/rfc3986.txt> ;
  rdfs:subClassOf rdfs:Resource ;
.
dcterms:W3CDTF
  rdf:type rdfs:Datatype ;
  dc:date "2000-07-11"^^xsd:date ;
  dc:date "2008-01-14"^^xsd:date ;
  dc:relation <http://dublincore.org/usage/terms/history/#W3CDTF-003> ;
  dcterms:date "2000-07-11"^^xsd:date ;
  dcterms:date "2008-01-14"^^xsd:date ;
  dcterms:hasVersion <http://dublincore.org/usage/terms/history/#W3CDTF-003> ;
  dcterms:issued "2000-07-11"^^xsd:date ;
  dcterms:modified "2008-01-14"^^xsd:date ;
  dcterms:relation <http://dublincore.org/usage/terms/history/#W3CDTF-003> ;
  rdfs:comment "The set of dates and times constructed according to the W3C Date and Time Formats Specification."@en ;
  rdfs:isDefinedBy dcterms: ;
  rdfs:label "W3C-DTF"@en ;
  rdfs:seeAlso <http://www.w3.org/TR/NOTE-datetime> ;
  rdfs:subClassOf rdfs:Resource ;
.
dcterms:abstract
  rdf:type rdf:Property ;
  dc:date "2000-07-11"^^xsd:date ;
  dc:date "2008-01-14"^^xsd:date ;
  dc:relation <http://dublincore.org/usage/terms/history/#abstract-003> ;
  dcterms:date "2000-07-11"^^xsd:date ;
  dcterms:date "2008-01-14"^^xsd:date ;
  dcterms:hasVersion <http://dublincore.org/usage/terms/history/#abstract-003> ;
  dcterms:issued "2000-07-11"^^xsd:date ;
  dcterms:modified "2008-01-14"^^xsd:date ;
  dcterms:relation <http://dublincore.org/usage/terms/history/#abstract-003> ;
  rdfs:comment "A summary of the resource."@en ;
  rdfs:isDefinedBy dcterms: ;
  rdfs:label "Abstract"@en ;
  rdfs:subPropertyOf dc:description ;
  rdfs:subPropertyOf dcterms:description ;
.
dcterms:accessRights
  rdf:type rdf:Property ;
  dc:date "2003-02-15"^^xsd:date ;
  dc:date "2008-01-14"^^xsd:date ;
  dc:description "Access Rights may include information regarding access or restrictions based on privacy, security, or other policies."@en ;
  dc:relation <http://dublincore.org/usage/terms/history/#accessRights-002> ;
  dcterms:date "2003-02-15"^^xsd:date ;
  dcterms:date "2008-01-14"^^xsd:date ;
  dcterms:description "Access Rights may include information regarding access or restrictions based on privacy, security, or other policies."@en ;
  dcterms:hasVersion <http://dublincore.org/usage/terms/history/#accessRights-002> ;
  dcterms:issued "2003-02-15"^^xsd:date ;
  dcterms:modified "2008-01-14"^^xsd:date ;
  dcterms:relation <http://dublincore.org/usage/terms/history/#accessRights-002> ;
  rdfs:comment "Information about who can access the resource or an indication of its security status."@en ;
  rdfs:isDefinedBy dcterms: ;
  rdfs:label "Access Rights"@en ;
  rdfs:range dcterms:RightsStatement ;
  rdfs:subPropertyOf dc:rights ;
  rdfs:subPropertyOf dcterms:rights ;
.
dcterms:accrualMethod
  rdf:type rdf:Property ;
  dc:date "2005-06-13"^^xsd:date ;
  dc:date "2010-10-11"^^xsd:date ;
  dc:relation <http://dublincore.org/usage/terms/history/#accrualMethod-003> ;
  dcterms:date "2005-06-13"^^xsd:date ;
  dcterms:date "2010-10-11"^^xsd:date ;
  dcterms:hasVersion <http://dublincore.org/usage/terms/history/#accrualMethod-003> ;
  dcterms:issued "2005-06-13"^^xsd:date ;
  dcterms:modified "2010-10-11"^^xsd:date ;
  dcterms:relation <http://dublincore.org/usage/terms/history/#accrualMethod-003> ;
  rdfs:comment "The method by which items are added to a collection."@en ;
  rdfs:domain <http://purl.org/dc/dcmitype/Collection> ;
  rdfs:isDefinedBy dcterms: ;
  rdfs:label "Accrual Method"@en ;
  rdfs:range dcterms:MethodOfAccrual ;
.
dcterms:accrualPeriodicity
  rdf:type rdf:Property ;
  dc:date "2005-06-13"^^xsd:date ;
  dc:date "2010-10-11"^^xsd:date ;
  dc:relation <http://dublincore.org/usage/terms/history/#accrualPeriodicity-003> ;
  dcterms:date "2005-06-13"^^xsd:date ;
  dcterms:date "2010-10-11"^^xsd:date ;
  dcterms:hasVersion <http://dublincore.org/usage/terms/history/#accrualPeriodicity-003> ;
  dcterms:issued "2005-06-13"^^xsd:date ;
  dcterms:modified "2010-10-11"^^xsd:date ;
  dcterms:relation <http://dublincore.org/usage/terms/history/#accrualPeriodicity-003> ;
  rdfs:comment "The frequency with which items are added to a collection."@en ;
  rdfs:domain <http://purl.org/dc/dcmitype/Collection> ;
  rdfs:isDefinedBy dcterms: ;
  rdfs:label "Accrual Periodicity"@en ;
  rdfs:range dcterms:Frequency ;
.
dcterms:accrualPolicy
  rdf:type rdf:Property ;
  dc:date "2005-06-13"^^xsd:date ;
  dc:date "2010-10-11"^^xsd:date ;
  dc:relation <http://dublincore.org/usage/terms/history/#accrualPolicy-003> ;
  dcterms:date "2005-06-13"^^xsd:date ;
  dcterms:date "2010-10-11"^^xsd:date ;
  dcterms:hasVersion <http://dublincore.org/usage/terms/history/#accrualPolicy-003> ;
  dcterms:issued "2005-06-13"^^xsd:date ;
  dcterms:modified "2010-10-11"^^xsd:date ;
  dcterms:relation <http://dublincore.org/usage/terms/history/#accrualPolicy-003> ;
  rdfs:comment "The policy governing the addition of items to a collection."@en ;
  rdfs:domain <http://purl.org/dc/dcmitype/Collection> ;
  rdfs:isDefinedBy dcterms: ;
  rdfs:label "Accrual Policy"@en ;
  rdfs:range dcterms:Policy ;
.
dcterms:alternative
  rdf:type rdf:Property ;
  dc:date "2000-07-11"^^xsd:date ;
  dc:date "2010-10-11"^^xsd:date ;
  dc:description "The distinction between titles and alternative titles is application-specific."@en ;
  dc:relation <http://dublincore.org/usage/terms/history/#alternative-003> ;
  dcterms:date "2000-07-11"^^xsd:date ;
  dcterms:date "2010-10-11"^^xsd:date ;
  dcterms:description "The distinction between titles and alternative titles is application-specific."@en ;
  dcterms:hasVersion <http://dublincore.org/usage/terms/history/#alternative-003> ;
  dcterms:issued "2000-07-11"^^xsd:date ;
  dcterms:modified "2010-10-11"^^xsd:date ;
  dcterms:relation <http://dublincore.org/usage/terms/history/#alternative-003> ;
  rdfs:comment "An alternative name for the resource."@en ;
  rdfs:isDefinedBy dcterms: ;
  rdfs:label "Alternative Title"@en ;
  rdfs:range rdfs:Literal ;
  rdfs:subPropertyOf dc:title ;
  rdfs:subPropertyOf dcterms:title ;
.
dcterms:audience
  rdf:type rdf:Property ;
  dc:date "2001-05-21"^^xsd:date ;
  dc:date "2008-01-14"^^xsd:date ;
  dc:relation <http://dublincore.org/usage/terms/history/#audience-003> ;
  dcterms:date "2001-05-21"^^xsd:date ;
  dcterms:date "2008-01-14"^^xsd:date ;
  dcterms:hasVersion <http://dublincore.org/usage/terms/history/#audience-003> ;
  dcterms:issued "2001-05-21"^^xsd:date ;
  dcterms:modified "2008-01-14"^^xsd:date ;
  dcterms:relation <http://dublincore.org/usage/terms/history/#audience-003> ;
  rdfs:comment "A class of entity for whom the resource is intended or useful."@en ;
  rdfs:isDefinedBy dcterms: ;
  rdfs:label "Audience"@en ;
  rdfs:range dcterms:AgentClass ;
  rdfs:range rdfs:Class ;
  rdfs:range owl:Thing ;
.
dcterms:available
  rdf:type rdf:Property ;
  dc:date "2000-07-11"^^xsd:date ;
  dc:date "2008-01-14"^^xsd:date ;
  dc:relation <http://dublincore.org/usage/terms/history/#available-003> ;
  dcterms:date "2000-07-11"^^xsd:date ;
  dcterms:date "2008-01-14"^^xsd:date ;
  dcterms:hasVersion <http://dublincore.org/usage/terms/history/#available-003> ;
  dcterms:issued "2000-07-11"^^xsd:date ;
  dcterms:modified "2008-01-14"^^xsd:date ;
  dcterms:relation <http://dublincore.org/usage/terms/history/#available-003> ;
  rdfs:comment "Date (often a range) that the resource became or will become available."@en ;
  rdfs:isDefinedBy dcterms: ;
  rdfs:label "Date Available"@en ;
  rdfs:range rdfs:Literal ;
  rdfs:subPropertyOf dc:date ;
  rdfs:subPropertyOf dcterms:date ;
.
dcterms:bibliographicCitation
  rdf:type rdf:Property ;
  dc:date "2003-02-15"^^xsd:date ;
  dc:date "2008-01-14"^^xsd:date ;
  dc:description "Recommended practice is to include sufficient bibliographic detail to identify the resource as unambiguously as possible."@en ;
  dc:relation <http://dublincore.org/usage/terms/history/#bibliographicCitation-002> ;
  dcterms:date "2003-02-15"^^xsd:date ;
  dcterms:date "2008-01-14"^^xsd:date ;
  dcterms:description "Recommended practice is to include sufficient bibliographic detail to identify the resource as unambiguously as possible."@en ;
  dcterms:hasVersion <http://dublincore.org/usage/terms/history/#bibliographicCitation-002> ;
  dcterms:issued "2003-02-15"^^xsd:date ;
  dcterms:modified "2008-01-14"^^xsd:date ;
  dcterms:relation <http://dublincore.org/usage/terms/history/#bibliographicCitation-002> ;
  rdfs:comment "A bibliographic reference for the resource."@en ;
  rdfs:domain dcterms:BibliographicResource ;
  rdfs:isDefinedBy dcterms: ;
  rdfs:label "Bibliographic Citation"@en ;
  rdfs:range rdfs:Literal ;
  rdfs:subPropertyOf dc:identifier ;
  rdfs:subPropertyOf dcterms:identifier ;
.
dcterms:conformsTo
  rdf:type rdf:Property ;
  dc:date "2001-05-21"^^xsd:date ;
  dc:date "2008-01-14"^^xsd:date ;
  dc:relation <http://dublincore.org/usage/terms/history/#conformsTo-003> ;
  dcterms:date "2001-05-21"^^xsd:date ;
  dcterms:date "2008-01-14"^^xsd:date ;
  dcterms:hasVersion <http://dublincore.org/usage/terms/history/#conformsTo-003> ;
  dcterms:issued "2001-05-21"^^xsd:date ;
  dcterms:modified "2008-01-14"^^xsd:date ;
  dcterms:relation <http://dublincore.org/usage/terms/history/#conformsTo-003> ;
  rdfs:comment "An established standard to which the described resource conforms."@en ;
  rdfs:isDefinedBy dcterms: ;
  rdfs:label "Conforms To"@en ;
  rdfs:range dcterms:Standard ;
  rdfs:subPropertyOf dc:relation ;
  rdfs:subPropertyOf dcterms:relation ;
.
dcterms:contributor
  rdf:type rdf:Property ;
  dc:date "2008-01-14"^^xsd:date ;
  dc:date "2010-10-11"^^xsd:date ;
  dc:description "Examples of a Contributor include a person, an organization, or a service."@en ;
  dc:relation <http://dublincore.org/usage/terms/history/#contributorT-001> ;
  dcterms:date "2008-01-14"^^xsd:date ;
  dcterms:date "2010-10-11"^^xsd:date ;
  dcterms:description "Examples of a Contributor include a person, an organization, or a service."@en ;
  dcterms:hasVersion <http://dublincore.org/usage/terms/history/#contributorT-001> ;
  dcterms:issued "2008-01-14"^^xsd:date ;
  dcterms:modified "2010-10-11"^^xsd:date ;
  dcterms:relation <http://dublincore.org/usage/terms/history/#contributorT-001> ;
  rdfs:comment "An entity responsible for making contributions to the resource."@en ;
  rdfs:isDefinedBy dcterms: ;
  rdfs:label "Contributor"@en ;
  rdfs:range dcterms:Agent ;
  rdfs:range owl:Thing ;
  rdfs:range foaf:Agent ;
  rdfs:range _:b420951 ;
  rdfs:range _:b421075 ;
  rdfs:range _:b421664 ;
  rdfs:range _:b421928 ;
  rdfs:range _:b937877 ;
  rdfs:range _:b938265 ;
  rdfs:subPropertyOf dc:contributor ;
.
dcterms:coverage
  rdf:type rdf:Property ;
  dc:date "2008-01-14"^^xsd:date ;
  dc:description "Spatial topic and spatial applicability may be a named place or a location specified by its geographic coordinates. Temporal topic may be a named period, date, or date range. A jurisdiction may be a named administrative entity or a geographic place to which the resource applies. Recommended best practice is to use a controlled vocabulary such as the Thesaurus of Geographic Names [TGN]. Where appropriate, named places or time periods can be used in preference to numeric identifiers such as sets of coordinates or date ranges."@en ;
  dc:relation <http://dublincore.org/usage/terms/history/#coverageT-001> ;
  dcterms:date "2008-01-14"^^xsd:date ;
  dcterms:description "Spatial topic and spatial applicability may be a named place or a location specified by its geographic coordinates. Temporal topic may be a named period, date, or date range. A jurisdiction may be a named administrative entity or a geographic place to which the resource applies. Recommended best practice is to use a controlled vocabulary such as the Thesaurus of Geographic Names [TGN]. Where appropriate, named places or time periods can be used in preference to numeric identifiers such as sets of coordinates or date ranges."@en ;
  dcterms:hasVersion <http://dublincore.org/usage/terms/history/#coverageT-001> ;
  dcterms:issued "2008-01-14"^^xsd:date ;
  dcterms:modified "2008-01-14"^^xsd:date ;
  dcterms:relation <http://dublincore.org/usage/terms/history/#coverageT-001> ;
  rdfs:comment "The spatial or temporal topic of the resource, the spatial applicability of the resource, or the jurisdiction under which the resource is relevant."@en ;
  rdfs:isDefinedBy dcterms: ;
  rdfs:label "Coverage"@en ;
  rdfs:range dcterms:LocationPeriodOrJurisdiction ;
  rdfs:subPropertyOf dc:coverage ;
.
dcterms:created
  rdf:type rdf:Property ;
  dc:date "2000-07-11"^^xsd:date ;
  dc:date "2008-01-14"^^xsd:date ;
  dc:relation <http://dublincore.org/usage/terms/history/#created-003> ;
  dcterms:date "2000-07-11"^^xsd:date ;
  dcterms:date "2008-01-14"^^xsd:date ;
  dcterms:hasVersion <http://dublincore.org/usage/terms/history/#created-003> ;
  dcterms:issued "2000-07-11"^^xsd:date ;
  dcterms:modified "2008-01-14"^^xsd:date ;
  dcterms:relation <http://dublincore.org/usage/terms/history/#created-003> ;
  rdfs:comment "Date of creation of the resource."@en ;
  rdfs:isDefinedBy dcterms: ;
  rdfs:label "Date Created"@en ;
  rdfs:range rdfs:Literal ;
  rdfs:subPropertyOf dc:date ;
  rdfs:subPropertyOf dcterms:date ;
.
dcterms:creator
  rdf:type rdf:Property ;
  dc:date "2008-01-14"^^xsd:date ;
  dc:date "2010-10-11"^^xsd:date ;
  dc:description "Examples of a Creator include a person, an organization, or a service."@en ;
  dc:relation <http://dublincore.org/usage/terms/history/#creatorT-002> ;
  dcterms:date "2008-01-14"^^xsd:date ;
  dcterms:date "2010-10-11"^^xsd:date ;
  dcterms:description "Examples of a Creator include a person, an organization, or a service."@en ;
  dcterms:hasVersion <http://dublincore.org/usage/terms/history/#creatorT-002> ;
  dcterms:issued "2008-01-14"^^xsd:date ;
  dcterms:modified "2010-10-11"^^xsd:date ;
  dcterms:relation <http://dublincore.org/usage/terms/history/#creatorT-002> ;
  rdfs:comment "An entity primarily responsible for making the resource."@en ;
  rdfs:domain elobr:EloniaBusinessCode ;
  rdfs:domain freebr:FreedoniaBusinessCode ;
  rdfs:domain toop:CompanyCode ;
  rdfs:domain owl:Thing ;
  rdfs:domain adms:Identifier ;
  rdfs:isDefinedBy dcterms: ;
  rdfs:label "Creator"@en ;
  rdfs:range dcterms:Agent ;
  rdfs:range owl:Thing ;
  rdfs:range foaf:Agent ;
  rdfs:range _:b420951 ;
  rdfs:range _:b421075 ;
  rdfs:range _:b421664 ;
  rdfs:range _:b421928 ;
  rdfs:range _:b937877 ;
  rdfs:range _:b938265 ;
  rdfs:subPropertyOf dc:contributor ;
  rdfs:subPropertyOf dc:creator ;
  rdfs:subPropertyOf dcterms:contributor ;
  rdfs:subPropertyOf foaf:maker ;
  owl:equivalentProperty elobr:EloniaRegistrationAuthority ;
  owl:equivalentProperty freebr:FreedoniaRegistrationAuthority ;
  owl:equivalentProperty toop:registrationAuthority ;
  owl:equivalentProperty foaf:maker ;
.
dcterms:date
  rdf:type rdf:Property ;
  dc:date "2008-01-14"^^xsd:date ;
  dc:description "Date may be used to express temporal information at any level of granularity.  Recommended best practice is to use an encoding scheme, such as the W3CDTF profile of ISO 8601 [W3CDTF]."@en ;
  dc:relation <http://dublincore.org/usage/terms/history/#dateT-001> ;
  dcterms:date "2008-01-14"^^xsd:date ;
  dcterms:description "Date may be used to express temporal information at any level of granularity.  Recommended best practice is to use an encoding scheme, such as the W3CDTF profile of ISO 8601 [W3CDTF]."@en ;
  dcterms:hasVersion <http://dublincore.org/usage/terms/history/#dateT-001> ;
  dcterms:issued "2008-01-14"^^xsd:date ;
  dcterms:modified "2008-01-14"^^xsd:date ;
  dcterms:relation <http://dublincore.org/usage/terms/history/#dateT-001> ;
  rdfs:comment "A point or period of time associated with an event in the lifecycle of the resource."@en ;
  rdfs:isDefinedBy dcterms: ;
  rdfs:label "Date"@en ;
  rdfs:range rdfs:Literal ;
  rdfs:subPropertyOf dc:date ;
.
dcterms:dateAccepted
  rdf:type rdf:Property ;
  dc:date "2002-07-13"^^xsd:date ;
  dc:date "2008-01-14"^^xsd:date ;
  dc:description "Examples of resources to which a Date Accepted may be relevant are a thesis (accepted by a university department) or an article (accepted by a journal)."@en ;
  dc:relation <http://dublincore.org/usage/terms/history/#dateAccepted-002> ;
  dcterms:date "2002-07-13"^^xsd:date ;
  dcterms:date "2008-01-14"^^xsd:date ;
  dcterms:description "Examples of resources to which a Date Accepted may be relevant are a thesis (accepted by a university department) or an article (accepted by a journal)."@en ;
  dcterms:hasVersion <http://dublincore.org/usage/terms/history/#dateAccepted-002> ;
  dcterms:issued "2002-07-13"^^xsd:date ;
  dcterms:modified "2008-01-14"^^xsd:date ;
  dcterms:relation <http://dublincore.org/usage/terms/history/#dateAccepted-002> ;
  rdfs:comment "Date of acceptance of the resource."@en ;
  rdfs:isDefinedBy dcterms: ;
  rdfs:label "Date Accepted"@en ;
  rdfs:range rdfs:Literal ;
  rdfs:subPropertyOf dc:date ;
  rdfs:subPropertyOf dcterms:date ;
.
dcterms:dateCopyrighted
  rdf:type rdf:Property ;
  dc:date "2002-07-13"^^xsd:date ;
  dc:date "2008-01-14"^^xsd:date ;
  dc:relation <http://dublincore.org/usage/terms/history/#dateCopyrighted-002> ;
  dcterms:date "2002-07-13"^^xsd:date ;
  dcterms:date "2008-01-14"^^xsd:date ;
  dcterms:hasVersion <http://dublincore.org/usage/terms/history/#dateCopyrighted-002> ;
  dcterms:issued "2002-07-13"^^xsd:date ;
  dcterms:modified "2008-01-14"^^xsd:date ;
  dcterms:relation <http://dublincore.org/usage/terms/history/#dateCopyrighted-002> ;
  rdfs:comment "Date of copyright."@en ;
  rdfs:isDefinedBy dcterms: ;
  rdfs:label "Date Copyrighted"@en ;
  rdfs:range rdfs:Literal ;
  rdfs:subPropertyOf dc:date ;
  rdfs:subPropertyOf dcterms:date ;
.
dcterms:dateSubmitted
  rdf:type rdf:Property ;
  dc:date "2002-07-13"^^xsd:date ;
  dc:date "2008-01-14"^^xsd:date ;
  dc:description "Examples of resources to which a Date Submitted may be relevant are a thesis (submitted to a university department) or an article (submitted to a journal)."@en ;
  dc:relation <http://dublincore.org/usage/terms/history/#dateSubmitted-002> ;
  dcterms:date "2002-07-13"^^xsd:date ;
  dcterms:date "2008-01-14"^^xsd:date ;
  dcterms:description "Examples of resources to which a Date Submitted may be relevant are a thesis (submitted to a university department) or an article (submitted to a journal)."@en ;
  dcterms:hasVersion <http://dublincore.org/usage/terms/history/#dateSubmitted-002> ;
  dcterms:issued "2002-07-13"^^xsd:date ;
  dcterms:modified "2008-01-14"^^xsd:date ;
  dcterms:relation <http://dublincore.org/usage/terms/history/#dateSubmitted-002> ;
  rdfs:comment "Date of submission of the resource."@en ;
  rdfs:isDefinedBy dcterms: ;
  rdfs:label "Date Submitted"@en ;
  rdfs:range rdfs:Literal ;
  rdfs:subPropertyOf dc:date ;
  rdfs:subPropertyOf dcterms:date ;
.
dcterms:description
  rdf:type rdf:Property ;
  dc:date "2008-01-14"^^xsd:date ;
  dc:description "Description may include but is not limited to: an abstract, a table of contents, a graphical representation, or a free-text account of the resource."@en ;
  dc:relation <http://dublincore.org/usage/terms/history/#descriptionT-001> ;
  dcterms:date "2008-01-14"^^xsd:date ;
  dcterms:description "Description may include but is not limited to: an abstract, a table of contents, a graphical representation, or a free-text account of the resource."@en ;
  dcterms:hasVersion <http://dublincore.org/usage/terms/history/#descriptionT-001> ;
  dcterms:issued "2008-01-14"^^xsd:date ;
  dcterms:modified "2008-01-14"^^xsd:date ;
  dcterms:relation <http://dublincore.org/usage/terms/history/#descriptionT-001> ;
  rdfs:comment "An account of the resource."@en ;
  rdfs:isDefinedBy dcterms: ;
  rdfs:label "Description"@en ;
  rdfs:subPropertyOf dc:description ;
.
dcterms:educationLevel
  rdf:type rdf:Property ;
  dc:date "2002-07-13"^^xsd:date ;
  dc:date "2008-01-14"^^xsd:date ;
  dc:relation <http://dublincore.org/usage/terms/history/#educationLevel-002> ;
  dcterms:date "2002-07-13"^^xsd:date ;
  dcterms:date "2008-01-14"^^xsd:date ;
  dcterms:hasVersion <http://dublincore.org/usage/terms/history/#educationLevel-002> ;
  dcterms:issued "2002-07-13"^^xsd:date ;
  dcterms:modified "2008-01-14"^^xsd:date ;
  dcterms:relation <http://dublincore.org/usage/terms/history/#educationLevel-002> ;
  rdfs:comment "A class of entity, defined in terms of progression through an educational or training context, for which the described resource is intended."@en ;
  rdfs:isDefinedBy dcterms: ;
  rdfs:label "Audience Education Level"@en ;
  rdfs:range dcterms:AgentClass ;
  rdfs:range rdfs:Class ;
  rdfs:range owl:Thing ;
  rdfs:subPropertyOf dcterms:audience ;
.
dcterms:extent
  rdf:type rdf:Property ;
  dc:date "2000-07-11"^^xsd:date ;
  dc:date "2008-01-14"^^xsd:date ;
  dc:relation <http://dublincore.org/usage/terms/history/#extent-003> ;
  dcterms:date "2000-07-11"^^xsd:date ;
  dcterms:date "2008-01-14"^^xsd:date ;
  dcterms:hasVersion <http://dublincore.org/usage/terms/history/#extent-003> ;
  dcterms:issued "2000-07-11"^^xsd:date ;
  dcterms:modified "2008-01-14"^^xsd:date ;
  dcterms:relation <http://dublincore.org/usage/terms/history/#extent-003> ;
  rdfs:comment "The size or duration of the resource."@en ;
  rdfs:isDefinedBy dcterms: ;
  rdfs:label "Extent"@en ;
  rdfs:range dcterms:MediaTypeOrExtent ;
  rdfs:range dcterms:SizeOrDuration ;
  rdfs:subPropertyOf dc:format ;
  rdfs:subPropertyOf dcterms:format ;
.
dcterms:format
  rdf:type rdf:Property ;
  dc:date "2008-01-14"^^xsd:date ;
  dc:description "Examples of dimensions include size and duration. Recommended best practice is to use a controlled vocabulary such as the list of Internet Media Types [MIME]."@en ;
  dc:relation <http://dublincore.org/usage/terms/history/#formatT-001> ;
  dcterms:date "2008-01-14"^^xsd:date ;
  dcterms:description "Examples of dimensions include size and duration. Recommended best practice is to use a controlled vocabulary such as the list of Internet Media Types [MIME]."@en ;
  dcterms:hasVersion <http://dublincore.org/usage/terms/history/#formatT-001> ;
  dcterms:issued "2008-01-14"^^xsd:date ;
  dcterms:modified "2008-01-14"^^xsd:date ;
  dcterms:relation <http://dublincore.org/usage/terms/history/#formatT-001> ;
  rdfs:comment "The file format, physical medium, or dimensions of the resource."@en ;
  rdfs:isDefinedBy dcterms: ;
  rdfs:label "Format"@en ;
  rdfs:range dcterms:MediaTypeOrExtent ;
  rdfs:subPropertyOf dc:format ;
.
dcterms:hasFormat
  rdf:type rdf:Property ;
  dc:date "2000-07-11"^^xsd:date ;
  dc:date "2008-01-14"^^xsd:date ;
  dc:relation <http://dublincore.org/usage/terms/history/#hasFormat-003> ;
  dcterms:date "2000-07-11"^^xsd:date ;
  dcterms:date "2008-01-14"^^xsd:date ;
  dcterms:hasVersion <http://dublincore.org/usage/terms/history/#hasFormat-003> ;
  dcterms:issued "2000-07-11"^^xsd:date ;
  dcterms:modified "2008-01-14"^^xsd:date ;
  dcterms:relation <http://dublincore.org/usage/terms/history/#hasFormat-003> ;
  rdfs:comment "A related resource that is substantially the same as the pre-existing described resource, but in another format."@en ;
  rdfs:isDefinedBy dcterms: ;
  rdfs:label "Has Format"@en ;
  rdfs:subPropertyOf dc:relation ;
  rdfs:subPropertyOf dcterms:relation ;
  skos:note "This term is intended to be used with non-literal values as defined in the DCMI Abstract Model (http://dublincore.org/documents/abstract-model/).  As of December 2007, the DCMI Usage Board is seeking a way to express this intention with a formal range declaration."@en ;
.
dcterms:hasPart
  rdf:type rdf:Property ;
  dc:date "2000-07-11"^^xsd:date ;
  dc:date "2008-01-14"^^xsd:date ;
  dc:relation <http://dublincore.org/usage/terms/history/#hasPart-003> ;
  dcterms:date "2000-07-11"^^xsd:date ;
  dcterms:date "2008-01-14"^^xsd:date ;
  dcterms:hasVersion <http://dublincore.org/usage/terms/history/#hasPart-003> ;
  dcterms:issued "2000-07-11"^^xsd:date ;
  dcterms:modified "2008-01-14"^^xsd:date ;
  dcterms:relation <http://dublincore.org/usage/terms/history/#hasPart-003> ;
  rdfs:comment "A related resource that is included either physically or logically in the described resource."@en ;
  rdfs:isDefinedBy dcterms: ;
  rdfs:label "Has Part"@en ;
  rdfs:subPropertyOf dc:relation ;
  rdfs:subPropertyOf dcterms:relation ;
  skos:note "This term is intended to be used with non-literal values as defined in the DCMI Abstract Model (http://dublincore.org/documents/abstract-model/).  As of December 2007, the DCMI Usage Board is seeking a way to express this intention with a formal range declaration."@en ;
.
dcterms:hasVersion
  rdf:type rdf:Property ;
  dc:date "2000-07-11"^^xsd:date ;
  dc:date "2008-01-14"^^xsd:date ;
  dc:relation <http://dublincore.org/usage/terms/history/#hasVersion-003> ;
  dcterms:date "2000-07-11"^^xsd:date ;
  dcterms:date "2008-01-14"^^xsd:date ;
  dcterms:hasVersion <http://dublincore.org/usage/terms/history/#hasVersion-003> ;
  dcterms:issued "2000-07-11"^^xsd:date ;
  dcterms:modified "2008-01-14"^^xsd:date ;
  dcterms:relation <http://dublincore.org/usage/terms/history/#hasVersion-003> ;
  rdfs:comment "A related resource that is a version, edition, or adaptation of the described resource."@en ;
  rdfs:isDefinedBy dcterms: ;
  rdfs:label "Has Version"@en ;
  rdfs:subPropertyOf dc:relation ;
  rdfs:subPropertyOf dcterms:relation ;
  skos:note "This term is intended to be used with non-literal values as defined in the DCMI Abstract Model (http://dublincore.org/documents/abstract-model/).  As of December 2007, the DCMI Usage Board is seeking a way to express this intention with a formal range declaration."@en ;
.
dcterms:identifier
  rdf:type rdf:Property ;
  dc:date "2008-01-14"^^xsd:date ;
  dc:description "Recommended best practice is to identify the resource by means of a string conforming to a formal identification system. "@en ;
  dc:relation <http://dublincore.org/usage/terms/history/#identifierT-001> ;
  dcterms:date "2008-01-14"^^xsd:date ;
  dcterms:description "Recommended best practice is to identify the resource by means of a string conforming to a formal identification system. "@en ;
  dcterms:hasVersion <http://dublincore.org/usage/terms/history/#identifierT-001> ;
  dcterms:issued "2008-01-14"^^xsd:date ;
  dcterms:modified "2008-01-14"^^xsd:date ;
  dcterms:relation <http://dublincore.org/usage/terms/history/#identifierT-001> ;
  rdfs:comment "An unambiguous reference to the resource within a given context."@en ;
  rdfs:isDefinedBy dcterms: ;
  rdfs:label "Identifier"@en ;
  rdfs:range rdfs:Literal ;
  rdfs:subPropertyOf dc:identifier ;
.
dcterms:instructionalMethod
  rdf:type rdf:Property ;
  dc:date "2005-06-13"^^xsd:date ;
  dc:date "2008-01-14"^^xsd:date ;
  dc:description "Instructional Method will typically include ways of presenting instructional materials or conducting instructional activities, patterns of learner-to-learner and learner-to-instructor interactions, and mechanisms by which group and individual levels of learning are measured.  Instructional methods include all aspects of the instruction and learning processes from planning and implementation through evaluation and feedback."@en ;
  dc:relation <http://dublincore.org/usage/terms/history/#instructionalMethod-002> ;
  dcterms:date "2005-06-13"^^xsd:date ;
  dcterms:date "2008-01-14"^^xsd:date ;
  dcterms:description "Instructional Method will typically include ways of presenting instructional materials or conducting instructional activities, patterns of learner-to-learner and learner-to-instructor interactions, and mechanisms by which group and individual levels of learning are measured.  Instructional methods include all aspects of the instruction and learning processes from planning and implementation through evaluation and feedback."@en ;
  dcterms:hasVersion <http://dublincore.org/usage/terms/history/#instructionalMethod-002> ;
  dcterms:issued "2005-06-13"^^xsd:date ;
  dcterms:modified "2008-01-14"^^xsd:date ;
  dcterms:relation <http://dublincore.org/usage/terms/history/#instructionalMethod-002> ;
  rdfs:comment "A process, used to engender knowledge, attitudes and skills, that the described resource is designed to support."@en ;
  rdfs:isDefinedBy dcterms: ;
  rdfs:label "Instructional Method"@en ;
  rdfs:range dcterms:MethodOfInstruction ;
.
dcterms:isFormatOf
  rdf:type rdf:Property ;
  dc:date "2000-07-11"^^xsd:date ;
  dc:date "2008-01-14"^^xsd:date ;
  dc:relation <http://dublincore.org/usage/terms/history/#isFormatOf-003> ;
  dcterms:date "2000-07-11"^^xsd:date ;
  dcterms:date "2008-01-14"^^xsd:date ;
  dcterms:hasVersion <http://dublincore.org/usage/terms/history/#isFormatOf-003> ;
  dcterms:issued "2000-07-11"^^xsd:date ;
  dcterms:modified "2008-01-14"^^xsd:date ;
  dcterms:relation <http://dublincore.org/usage/terms/history/#isFormatOf-003> ;
  rdfs:comment "A related resource that is substantially the same as the described resource, but in another format."@en ;
  rdfs:isDefinedBy dcterms: ;
  rdfs:label "Is Format Of"@en ;
  rdfs:subPropertyOf dc:relation ;
  rdfs:subPropertyOf dcterms:relation ;
  skos:note "This term is intended to be used with non-literal values as defined in the DCMI Abstract Model (http://dublincore.org/documents/abstract-model/).  As of December 2007, the DCMI Usage Board is seeking a way to express this intention with a formal range declaration."@en ;
.
dcterms:isPartOf
  rdf:type rdf:Property ;
  dc:date "2000-07-11"^^xsd:date ;
  dc:date "2008-01-14"^^xsd:date ;
  dc:relation <http://dublincore.org/usage/terms/history/#isPartOf-003> ;
  dcterms:date "2000-07-11"^^xsd:date ;
  dcterms:date "2008-01-14"^^xsd:date ;
  dcterms:hasVersion <http://dublincore.org/usage/terms/history/#isPartOf-003> ;
  dcterms:issued "2000-07-11"^^xsd:date ;
  dcterms:modified "2008-01-14"^^xsd:date ;
  dcterms:relation <http://dublincore.org/usage/terms/history/#isPartOf-003> ;
  rdfs:comment "A related resource in which the described resource is physically or logically included."@en ;
  rdfs:isDefinedBy dcterms: ;
  rdfs:label "Is Part Of"@en ;
  rdfs:subPropertyOf dc:relation ;
  rdfs:subPropertyOf dcterms:relation ;
  skos:note "This term is intended to be used with non-literal values as defined in the DCMI Abstract Model (http://dublincore.org/documents/abstract-model/).  As of December 2007, the DCMI Usage Board is seeking a way to express this intention with a formal range declaration."@en ;
.
dcterms:isReferencedBy
  rdf:type rdf:Property ;
  dc:date "2000-07-11"^^xsd:date ;
  dc:date "2008-01-14"^^xsd:date ;
  dc:relation <http://dublincore.org/usage/terms/history/#isReferencedBy-003> ;
  dcterms:date "2000-07-11"^^xsd:date ;
  dcterms:date "2008-01-14"^^xsd:date ;
  dcterms:hasVersion <http://dublincore.org/usage/terms/history/#isReferencedBy-003> ;
  dcterms:issued "2000-07-11"^^xsd:date ;
  dcterms:modified "2008-01-14"^^xsd:date ;
  dcterms:relation <http://dublincore.org/usage/terms/history/#isReferencedBy-003> ;
  rdfs:comment "A related resource that references, cites, or otherwise points to the described resource."@en ;
  rdfs:isDefinedBy dcterms: ;
  rdfs:label "Is Referenced By"@en ;
  rdfs:subPropertyOf dc:relation ;
  rdfs:subPropertyOf dcterms:relation ;
  skos:note "This term is intended to be used with non-literal values as defined in the DCMI Abstract Model (http://dublincore.org/documents/abstract-model/).  As of December 2007, the DCMI Usage Board is seeking a way to express this intention with a formal range declaration."@en ;
.
dcterms:isReplacedBy
  rdf:type rdf:Property ;
  dc:date "2000-07-11"^^xsd:date ;
  dc:date "2008-01-14"^^xsd:date ;
  dc:relation <http://dublincore.org/usage/terms/history/#isReplacedBy-003> ;
  dcterms:date "2000-07-11"^^xsd:date ;
  dcterms:date "2008-01-14"^^xsd:date ;
  dcterms:hasVersion <http://dublincore.org/usage/terms/history/#isReplacedBy-003> ;
  dcterms:issued "2000-07-11"^^xsd:date ;
  dcterms:modified "2008-01-14"^^xsd:date ;
  dcterms:relation <http://dublincore.org/usage/terms/history/#isReplacedBy-003> ;
  rdfs:comment "A related resource that supplants, displaces, or supersedes the described resource."@en ;
  rdfs:isDefinedBy dcterms: ;
  rdfs:label "Is Replaced By"@en ;
  rdfs:subPropertyOf dc:relation ;
  rdfs:subPropertyOf dcterms:relation ;
  skos:note "This term is intended to be used with non-literal values as defined in the DCMI Abstract Model (http://dublincore.org/documents/abstract-model/).  As of December 2007, the DCMI Usage Board is seeking a way to express this intention with a formal range declaration."@en ;
.
dcterms:isRequiredBy
  rdf:type rdf:Property ;
  dc:date "2000-07-11"^^xsd:date ;
  dc:date "2008-01-14"^^xsd:date ;
  dc:relation <http://dublincore.org/usage/terms/history/#isRequiredBy-003> ;
  dcterms:date "2000-07-11"^^xsd:date ;
  dcterms:date "2008-01-14"^^xsd:date ;
  dcterms:hasVersion <http://dublincore.org/usage/terms/history/#isRequiredBy-003> ;
  dcterms:issued "2000-07-11"^^xsd:date ;
  dcterms:modified "2008-01-14"^^xsd:date ;
  dcterms:relation <http://dublincore.org/usage/terms/history/#isRequiredBy-003> ;
  rdfs:comment "A related resource that requires the described resource to support its function, delivery, or coherence."@en ;
  rdfs:isDefinedBy dcterms: ;
  rdfs:label "Is Required By"@en ;
  rdfs:subPropertyOf dc:relation ;
  rdfs:subPropertyOf dcterms:relation ;
  skos:note "This term is intended to be used with non-literal values as defined in the DCMI Abstract Model (http://dublincore.org/documents/abstract-model/).  As of December 2007, the DCMI Usage Board is seeking a way to express this intention with a formal range declaration."@en ;
.
dcterms:isVersionOf
  rdf:type rdf:Property ;
  dc:date "2000-07-11"^^xsd:date ;
  dc:date "2008-01-14"^^xsd:date ;
  dc:description "Changes in version imply substantive changes in content rather than differences in format."@en ;
  dc:relation <http://dublincore.org/usage/terms/history/#isVersionOf-003> ;
  dcterms:date "2000-07-11"^^xsd:date ;
  dcterms:date "2008-01-14"^^xsd:date ;
  dcterms:description "Changes in version imply substantive changes in content rather than differences in format."@en ;
  dcterms:hasVersion <http://dublincore.org/usage/terms/history/#isVersionOf-003> ;
  dcterms:issued "2000-07-11"^^xsd:date ;
  dcterms:modified "2008-01-14"^^xsd:date ;
  dcterms:relation <http://dublincore.org/usage/terms/history/#isVersionOf-003> ;
  rdfs:comment "A related resource of which the described resource is a version, edition, or adaptation."@en ;
  rdfs:isDefinedBy dcterms: ;
  rdfs:label "Is Version Of"@en ;
  rdfs:subPropertyOf dc:relation ;
  rdfs:subPropertyOf dcterms:relation ;
  skos:note "This term is intended to be used with non-literal values as defined in the DCMI Abstract Model (http://dublincore.org/documents/abstract-model/).  As of December 2007, the DCMI Usage Board is seeking a way to express this intention with a formal range declaration."@en ;
.
dcterms:issued
  rdf:type rdf:Property ;
  dc:date "2000-07-11"^^xsd:date ;
  dc:date "2008-01-14"^^xsd:date ;
  dc:relation <http://dublincore.org/usage/terms/history/#issued-003> ;
  dcterms:date "2000-07-11"^^xsd:date ;
  dcterms:date "2008-01-14"^^xsd:date ;
  dcterms:hasVersion <http://dublincore.org/usage/terms/history/#issued-003> ;
  dcterms:issued "2000-07-11"^^xsd:date ;
  dcterms:modified "2008-01-14"^^xsd:date ;
  dcterms:relation <http://dublincore.org/usage/terms/history/#issued-003> ;
  rdfs:comment "Date of formal issuance (e.g., publication) of the resource."@en ;
  rdfs:isDefinedBy dcterms: ;
  rdfs:label "Date Issued"@en ;
  rdfs:range rdfs:Literal ;
  rdfs:subPropertyOf dc:date ;
  rdfs:subPropertyOf dcterms:date ;
.
dcterms:language
  rdf:type rdf:Property ;
  dc:date "2008-01-14"^^xsd:date ;
  dc:description "Recommended best practice is to use a controlled vocabulary such as RFC 4646 [RFC4646]."@en ;
  dc:relation <http://dublincore.org/usage/terms/history/#languageT-001> ;
  dcterms:date "2008-01-14"^^xsd:date ;
  dcterms:description "Recommended best practice is to use a controlled vocabulary such as RFC 4646 [RFC4646]."@en ;
  dcterms:hasVersion <http://dublincore.org/usage/terms/history/#languageT-001> ;
  dcterms:issued "2008-01-14"^^xsd:date ;
  dcterms:modified "2008-01-14"^^xsd:date ;
  dcterms:relation <http://dublincore.org/usage/terms/history/#languageT-001> ;
  rdfs:comment "A language of the resource."@en ;
  rdfs:isDefinedBy dcterms: ;
  rdfs:label "Language"@en ;
  rdfs:range dcterms:LinguisticSystem ;
  rdfs:subPropertyOf dc:language ;
.
dcterms:license
  rdf:type rdf:Property ;
  dc:date "2004-06-14"^^xsd:date ;
  dc:date "2008-01-14"^^xsd:date ;
  dc:relation <http://dublincore.org/usage/terms/history/#license-002> ;
  dcterms:date "2004-06-14"^^xsd:date ;
  dcterms:date "2008-01-14"^^xsd:date ;
  dcterms:hasVersion <http://dublincore.org/usage/terms/history/#license-002> ;
  dcterms:issued "2004-06-14"^^xsd:date ;
  dcterms:modified "2008-01-14"^^xsd:date ;
  dcterms:relation <http://dublincore.org/usage/terms/history/#license-002> ;
  rdfs:comment "A legal document giving official permission to do something with the resource."@en ;
  rdfs:isDefinedBy dcterms: ;
  rdfs:label "License"@en ;
  rdfs:range dcterms:LicenseDocument ;
  rdfs:range dcterms:RightsStatement ;
  rdfs:subPropertyOf dc:rights ;
  rdfs:subPropertyOf dcterms:rights ;
.
dcterms:mediator
  rdf:type rdf:Property ;
  dc:date "2001-05-21"^^xsd:date ;
  dc:date "2008-01-14"^^xsd:date ;
  dc:description "In an educational context, a mediator might be a parent, teacher, teaching assistant, or care-giver."@en ;
  dc:relation <http://dublincore.org/usage/terms/history/#mediator-003> ;
  dcterms:date "2001-05-21"^^xsd:date ;
  dcterms:date "2008-01-14"^^xsd:date ;
  dcterms:description "In an educational context, a mediator might be a parent, teacher, teaching assistant, or care-giver."@en ;
  dcterms:hasVersion <http://dublincore.org/usage/terms/history/#mediator-003> ;
  dcterms:issued "2001-05-21"^^xsd:date ;
  dcterms:modified "2008-01-14"^^xsd:date ;
  dcterms:relation <http://dublincore.org/usage/terms/history/#mediator-003> ;
  rdfs:comment "An entity that mediates access to the resource and for whom the resource is intended or useful."@en ;
  rdfs:isDefinedBy dcterms: ;
  rdfs:label "Mediator"@en ;
  rdfs:range dcterms:AgentClass ;
  rdfs:range rdfs:Class ;
  rdfs:range owl:Thing ;
  rdfs:subPropertyOf dcterms:audience ;
.
dcterms:medium
  rdf:type rdf:Property ;
  dc:date "2000-07-11"^^xsd:date ;
  dc:date "2008-01-14"^^xsd:date ;
  dc:relation <http://dublincore.org/usage/terms/history/#medium-003> ;
  dcterms:date "2000-07-11"^^xsd:date ;
  dcterms:date "2008-01-14"^^xsd:date ;
  dcterms:hasVersion <http://dublincore.org/usage/terms/history/#medium-003> ;
  dcterms:issued "2000-07-11"^^xsd:date ;
  dcterms:modified "2008-01-14"^^xsd:date ;
  dcterms:relation <http://dublincore.org/usage/terms/history/#medium-003> ;
  rdfs:comment "The material or physical carrier of the resource."@en ;
  rdfs:domain dcterms:PhysicalResource ;
  rdfs:isDefinedBy dcterms: ;
  rdfs:label "Medium"@en ;
  rdfs:range dcterms:MediaType ;
  rdfs:range dcterms:MediaTypeOrExtent ;
  rdfs:range dcterms:PhysicalMedium ;
  rdfs:subPropertyOf dc:format ;
  rdfs:subPropertyOf dcterms:format ;
.
dcterms:modified
  rdf:type rdf:Property ;
  dc:date "2000-07-11"^^xsd:date ;
  dc:date "2008-01-14"^^xsd:date ;
  dc:relation <http://dublincore.org/usage/terms/history/#modified-003> ;
  dcterms:date "2000-07-11"^^xsd:date ;
  dcterms:date "2008-01-14"^^xsd:date ;
  dcterms:hasVersion <http://dublincore.org/usage/terms/history/#modified-003> ;
  dcterms:issued "2000-07-11"^^xsd:date ;
  dcterms:modified "2008-01-14"^^xsd:date ;
  dcterms:relation <http://dublincore.org/usage/terms/history/#modified-003> ;
  rdfs:comment "Date on which the resource was changed."@en ;
  rdfs:isDefinedBy dcterms: ;
  rdfs:label "Date Modified"@en ;
  rdfs:range rdfs:Literal ;
  rdfs:subPropertyOf dc:date ;
  rdfs:subPropertyOf dcterms:date ;
.
dcterms:provenance
  rdf:type rdf:Property ;
  dc:date "2004-09-20"^^xsd:date ;
  dc:date "2008-01-14"^^xsd:date ;
  dc:description "The statement may include a description of any changes successive custodians made to the resource."@en ;
  dc:relation <http://dublincore.org/usage/terms/history/#provenance-002> ;
  dcterms:date "2004-09-20"^^xsd:date ;
  dcterms:date "2008-01-14"^^xsd:date ;
  dcterms:description "The statement may include a description of any changes successive custodians made to the resource."@en ;
  dcterms:hasVersion <http://dublincore.org/usage/terms/history/#provenance-002> ;
  dcterms:issued "2004-09-20"^^xsd:date ;
  dcterms:modified "2008-01-14"^^xsd:date ;
  dcterms:relation <http://dublincore.org/usage/terms/history/#provenance-002> ;
  rdfs:comment "A statement of any changes in ownership and custody of the resource since its creation that are significant for its authenticity, integrity, and interpretation."@en ;
  rdfs:isDefinedBy dcterms: ;
  rdfs:label "Provenance"@en ;
  rdfs:range dcterms:ProvenanceStatement ;
.
dcterms:publisher
  rdf:type rdf:Property ;
  dc:date "2008-01-14"^^xsd:date ;
  dc:date "2010-10-11"^^xsd:date ;
  dc:description "Examples of a Publisher include a person, an organization, or a service."@en ;
  dc:relation <http://dublincore.org/usage/terms/history/#publisherT-001> ;
  dcterms:date "2008-01-14"^^xsd:date ;
  dcterms:date "2010-10-11"^^xsd:date ;
  dcterms:description "Examples of a Publisher include a person, an organization, or a service."@en ;
  dcterms:hasVersion <http://dublincore.org/usage/terms/history/#publisherT-001> ;
  dcterms:issued "2008-01-14"^^xsd:date ;
  dcterms:modified "2010-10-11"^^xsd:date ;
  dcterms:relation <http://dublincore.org/usage/terms/history/#publisherT-001> ;
  rdfs:comment "An entity responsible for making the resource available."@en ;
  rdfs:isDefinedBy dcterms: ;
  rdfs:label "Publisher"@en ;
  rdfs:range dcterms:Agent ;
  rdfs:range owl:Thing ;
  rdfs:range foaf:Agent ;
  rdfs:range _:b420951 ;
  rdfs:range _:b421075 ;
  rdfs:range _:b421664 ;
  rdfs:range _:b421928 ;
  rdfs:range _:b937877 ;
  rdfs:range _:b938265 ;
  rdfs:subPropertyOf dc:publisher ;
.
dcterms:references
  rdf:type rdf:Property ;
  dc:date "2000-07-11"^^xsd:date ;
  dc:date "2008-01-14"^^xsd:date ;
  dc:relation <http://dublincore.org/usage/terms/history/#references-003> ;
  dcterms:date "2000-07-11"^^xsd:date ;
  dcterms:date "2008-01-14"^^xsd:date ;
  dcterms:hasVersion <http://dublincore.org/usage/terms/history/#references-003> ;
  dcterms:issued "2000-07-11"^^xsd:date ;
  dcterms:modified "2008-01-14"^^xsd:date ;
  dcterms:relation <http://dublincore.org/usage/terms/history/#references-003> ;
  rdfs:comment "A related resource that is referenced, cited, or otherwise pointed to by the described resource."@en ;
  rdfs:isDefinedBy dcterms: ;
  rdfs:label "References"@en ;
  rdfs:subPropertyOf dc:relation ;
  rdfs:subPropertyOf dcterms:relation ;
  skos:note "This term is intended to be used with non-literal values as defined in the DCMI Abstract Model (http://dublincore.org/documents/abstract-model/).  As of December 2007, the DCMI Usage Board is seeking a way to express this intention with a formal range declaration."@en ;
.
dcterms:relation
  rdf:type rdf:Property ;
  dc:date "2008-01-14"^^xsd:date ;
  dc:description "Recommended best practice is to identify the related resource by means of a string conforming to a formal identification system. "@en ;
  dc:relation <http://dublincore.org/usage/terms/history/#relationT-001> ;
  dcterms:date "2008-01-14"^^xsd:date ;
  dcterms:description "Recommended best practice is to identify the related resource by means of a string conforming to a formal identification system. "@en ;
  dcterms:hasVersion <http://dublincore.org/usage/terms/history/#relationT-001> ;
  dcterms:issued "2008-01-14"^^xsd:date ;
  dcterms:modified "2008-01-14"^^xsd:date ;
  dcterms:relation <http://dublincore.org/usage/terms/history/#relationT-001> ;
  rdfs:comment "A related resource."@en ;
  rdfs:isDefinedBy dcterms: ;
  rdfs:label "Relation"@en ;
  rdfs:subPropertyOf dc:relation ;
  skos:note "This term is intended to be used with non-literal values as defined in the DCMI Abstract Model (http://dublincore.org/documents/abstract-model/).  As of December 2007, the DCMI Usage Board is seeking a way to express this intention with a formal range declaration."@en ;
.
dcterms:replaces
  rdf:type rdf:Property ;
  dc:date "2000-07-11"^^xsd:date ;
  dc:date "2008-01-14"^^xsd:date ;
  dc:relation <http://dublincore.org/usage/terms/history/#replaces-003> ;
  dcterms:date "2000-07-11"^^xsd:date ;
  dcterms:date "2008-01-14"^^xsd:date ;
  dcterms:hasVersion <http://dublincore.org/usage/terms/history/#replaces-003> ;
  dcterms:issued "2000-07-11"^^xsd:date ;
  dcterms:modified "2008-01-14"^^xsd:date ;
  dcterms:relation <http://dublincore.org/usage/terms/history/#replaces-003> ;
  rdfs:comment "A related resource that is supplanted, displaced, or superseded by the described resource."@en ;
  rdfs:isDefinedBy dcterms: ;
  rdfs:label "Replaces"@en ;
  rdfs:subPropertyOf dc:relation ;
  rdfs:subPropertyOf dcterms:relation ;
  skos:note "This term is intended to be used with non-literal values as defined in the DCMI Abstract Model (http://dublincore.org/documents/abstract-model/).  As of December 2007, the DCMI Usage Board is seeking a way to express this intention with a formal range declaration."@en ;
.
dcterms:requires
  rdf:type rdf:Property ;
  dc:date "2000-07-11"^^xsd:date ;
  dc:date "2008-01-14"^^xsd:date ;
  dc:relation <http://dublincore.org/usage/terms/history/#requires-003> ;
  dcterms:date "2000-07-11"^^xsd:date ;
  dcterms:date "2008-01-14"^^xsd:date ;
  dcterms:hasVersion <http://dublincore.org/usage/terms/history/#requires-003> ;
  dcterms:issued "2000-07-11"^^xsd:date ;
  dcterms:modified "2008-01-14"^^xsd:date ;
  dcterms:relation <http://dublincore.org/usage/terms/history/#requires-003> ;
  rdfs:comment "A related resource that is required by the described resource to support its function, delivery, or coherence."@en ;
  rdfs:isDefinedBy dcterms: ;
  rdfs:label "Requires"@en ;
  rdfs:subPropertyOf dc:relation ;
  rdfs:subPropertyOf dcterms:relation ;
  skos:note "This term is intended to be used with non-literal values as defined in the DCMI Abstract Model (http://dublincore.org/documents/abstract-model/).  As of December 2007, the DCMI Usage Board is seeking a way to express this intention with a formal range declaration."@en ;
.
dcterms:rights
  rdf:type rdf:Property ;
  dc:date "2008-01-14"^^xsd:date ;
  dc:description "Typically, rights information includes a statement about various property rights associated with the resource, including intellectual property rights."@en ;
  dc:relation <http://dublincore.org/usage/terms/history/#rightsT-001> ;
  dcterms:date "2008-01-14"^^xsd:date ;
  dcterms:description "Typically, rights information includes a statement about various property rights associated with the resource, including intellectual property rights."@en ;
  dcterms:hasVersion <http://dublincore.org/usage/terms/history/#rightsT-001> ;
  dcterms:issued "2008-01-14"^^xsd:date ;
  dcterms:modified "2008-01-14"^^xsd:date ;
  dcterms:relation <http://dublincore.org/usage/terms/history/#rightsT-001> ;
  rdfs:comment "Information about rights held in and over the resource."@en ;
  rdfs:isDefinedBy dcterms: ;
  rdfs:label "Rights"@en ;
  rdfs:range dcterms:RightsStatement ;
  rdfs:subPropertyOf dc:rights ;
.
dcterms:rightsHolder
  rdf:type rdf:Property ;
  dc:date "2004-06-14"^^xsd:date ;
  dc:date "2008-01-14"^^xsd:date ;
  dc:relation <http://dublincore.org/usage/terms/history/#rightsHolder-002> ;
  dcterms:date "2004-06-14"^^xsd:date ;
  dcterms:date "2008-01-14"^^xsd:date ;
  dcterms:hasVersion <http://dublincore.org/usage/terms/history/#rightsHolder-002> ;
  dcterms:issued "2004-06-14"^^xsd:date ;
  dcterms:modified "2008-01-14"^^xsd:date ;
  dcterms:relation <http://dublincore.org/usage/terms/history/#rightsHolder-002> ;
  rdfs:comment "A person or organization owning or managing rights over the resource."@en ;
  rdfs:isDefinedBy dcterms: ;
  rdfs:label "Rights Holder"@en ;
  rdfs:range dcterms:Agent ;
  rdfs:range owl:Thing ;
  rdfs:range foaf:Agent ;
  rdfs:range _:b420951 ;
  rdfs:range _:b421075 ;
  rdfs:range _:b421664 ;
  rdfs:range _:b421928 ;
  rdfs:range _:b937877 ;
  rdfs:range _:b938265 ;
.
dcterms:source
  rdf:type rdf:Property ;
  dc:date "2008-01-14"^^xsd:date ;
  dc:description "The described resource may be derived from the related resource in whole or in part. Recommended best practice is to identify the related resource by means of a string conforming to a formal identification system."@en ;
  dc:relation <http://dublincore.org/usage/terms/history/#sourceT-001> ;
  dcterms:date "2008-01-14"^^xsd:date ;
  dcterms:description "The described resource may be derived from the related resource in whole or in part. Recommended best practice is to identify the related resource by means of a string conforming to a formal identification system."@en ;
  dcterms:hasVersion <http://dublincore.org/usage/terms/history/#sourceT-001> ;
  dcterms:issued "2008-01-14"^^xsd:date ;
  dcterms:modified "2008-01-14"^^xsd:date ;
  dcterms:relation <http://dublincore.org/usage/terms/history/#sourceT-001> ;
  rdfs:comment "A related resource from which the described resource is derived."@en ;
  rdfs:isDefinedBy dcterms: ;
  rdfs:label "Source"@en ;
  rdfs:subPropertyOf dc:relation ;
  rdfs:subPropertyOf dc:source ;
  rdfs:subPropertyOf dcterms:relation ;
  skos:note "This term is intended to be used with non-literal values as defined in the DCMI Abstract Model (http://dublincore.org/documents/abstract-model/).  As of December 2007, the DCMI Usage Board is seeking a way to express this intention with a formal range declaration."@en ;
.
dcterms:spatial
  rdf:type rdf:Property ;
  dc:date "2000-07-11"^^xsd:date ;
  dc:date "2008-01-14"^^xsd:date ;
  dc:relation <http://dublincore.org/usage/terms/history/#spatial-003> ;
  dcterms:date "2000-07-11"^^xsd:date ;
  dcterms:date "2008-01-14"^^xsd:date ;
  dcterms:hasVersion <http://dublincore.org/usage/terms/history/#spatial-003> ;
  dcterms:issued "2000-07-11"^^xsd:date ;
  dcterms:modified "2008-01-14"^^xsd:date ;
  dcterms:relation <http://dublincore.org/usage/terms/history/#spatial-003> ;
  rdfs:comment "Spatial characteristics of the resource."@en ;
  rdfs:isDefinedBy dcterms: ;
  rdfs:label "Spatial Coverage"@en ;
  rdfs:range dcterms:Location ;
  rdfs:range dcterms:LocationPeriodOrJurisdiction ;
  rdfs:subPropertyOf dc:coverage ;
  rdfs:subPropertyOf dcterms:coverage ;
.
dcterms:subject
  rdf:type rdf:Property ;
  dc:date "2008-01-14"^^xsd:date ;
  dc:date "2012-06-14"^^xsd:date ;
  dc:description "Typically, the subject will be represented using keywords, key phrases, or classification codes. Recommended best practice is to use a controlled vocabulary."@en ;
  dc:relation <http://dublincore.org/usage/terms/history/#subjectT-002> ;
  dcterms:date "2008-01-14"^^xsd:date ;
  dcterms:date "2012-06-14"^^xsd:date ;
  dcterms:description "Typically, the subject will be represented using keywords, key phrases, or classification codes. Recommended best practice is to use a controlled vocabulary."@en ;
  dcterms:hasVersion <http://dublincore.org/usage/terms/history/#subjectT-002> ;
  dcterms:issued "2008-01-14"^^xsd:date ;
  dcterms:modified "2012-06-14"^^xsd:date ;
  dcterms:relation <http://dublincore.org/usage/terms/history/#subjectT-002> ;
  rdfs:comment "The topic of the resource."@en ;
  rdfs:isDefinedBy dcterms: ;
  rdfs:label "Subject"@en ;
  rdfs:subPropertyOf dc:subject ;
  skos:note "This term is intended to be used with non-literal values as defined in the DCMI Abstract Model (http://dublincore.org/documents/abstract-model/).  As of December 2007, the DCMI Usage Board is seeking a way to express this intention with a formal range declaration."@en ;
.
dcterms:tableOfContents
  rdf:type rdf:Property ;
  dc:date "2000-07-11"^^xsd:date ;
  dc:date "2008-01-14"^^xsd:date ;
  dc:relation <http://dublincore.org/usage/terms/history/#tableOfContents-003> ;
  dcterms:date "2000-07-11"^^xsd:date ;
  dcterms:date "2008-01-14"^^xsd:date ;
  dcterms:hasVersion <http://dublincore.org/usage/terms/history/#tableOfContents-003> ;
  dcterms:issued "2000-07-11"^^xsd:date ;
  dcterms:modified "2008-01-14"^^xsd:date ;
  dcterms:relation <http://dublincore.org/usage/terms/history/#tableOfContents-003> ;
  rdfs:comment "A list of subunits of the resource."@en ;
  rdfs:isDefinedBy dcterms: ;
  rdfs:label "Table Of Contents"@en ;
  rdfs:subPropertyOf dc:description ;
  rdfs:subPropertyOf dcterms:description ;
.
dcterms:temporal
  rdf:type rdf:Property ;
  dc:date "2000-07-11"^^xsd:date ;
  dc:date "2008-01-14"^^xsd:date ;
  dc:relation <http://dublincore.org/usage/terms/history/#temporal-003> ;
  dcterms:date "2000-07-11"^^xsd:date ;
  dcterms:date "2008-01-14"^^xsd:date ;
  dcterms:hasVersion <http://dublincore.org/usage/terms/history/#temporal-003> ;
  dcterms:issued "2000-07-11"^^xsd:date ;
  dcterms:modified "2008-01-14"^^xsd:date ;
  dcterms:relation <http://dublincore.org/usage/terms/history/#temporal-003> ;
  rdfs:comment "Temporal characteristics of the resource."@en ;
  rdfs:isDefinedBy dcterms: ;
  rdfs:label "Temporal Coverage"@en ;
  rdfs:range dcterms:LocationPeriodOrJurisdiction ;
  rdfs:range dcterms:PeriodOfTime ;
  rdfs:subPropertyOf dc:coverage ;
  rdfs:subPropertyOf dcterms:coverage ;
.
dcterms:title
  rdf:type rdf:Property ;
  dc:date "2008-01-14"^^xsd:date ;
  dc:date "2010-10-11"^^xsd:date ;
  dc:relation <http://dublincore.org/usage/terms/history/#titleT-002> ;
  dcterms:date "2008-01-14"^^xsd:date ;
  dcterms:date "2010-10-11"^^xsd:date ;
  dcterms:hasVersion <http://dublincore.org/usage/terms/history/#titleT-002> ;
  dcterms:issued "2008-01-14"^^xsd:date ;
  dcterms:modified "2010-10-11"^^xsd:date ;
  dcterms:relation <http://dublincore.org/usage/terms/history/#titleT-002> ;
  rdfs:comment "A name given to the resource."@en ;
  rdfs:isDefinedBy dcterms: ;
  rdfs:label "Title"@en ;
  rdfs:range rdfs:Literal ;
  rdfs:subPropertyOf dc:title ;
.
dcterms:type
  rdf:type rdf:Property ;
  dc:date "2008-01-14"^^xsd:date ;
  dc:description "Recommended best practice is to use a controlled vocabulary such as the DCMI Type Vocabulary [DCMITYPE]. To describe the file format, physical medium, or dimensions of the resource, use the Format element."@en ;
  dc:relation <http://dublincore.org/usage/terms/history/#typeT-001> ;
  dcterms:date "2008-01-14"^^xsd:date ;
  dcterms:description "Recommended best practice is to use a controlled vocabulary such as the DCMI Type Vocabulary [DCMITYPE]. To describe the file format, physical medium, or dimensions of the resource, use the Format element."@en ;
  dcterms:hasVersion <http://dublincore.org/usage/terms/history/#typeT-001> ;
  dcterms:issued "2008-01-14"^^xsd:date ;
  dcterms:modified "2008-01-14"^^xsd:date ;
  dcterms:relation <http://dublincore.org/usage/terms/history/#typeT-001> ;
  rdfs:comment "The nature or genre of the resource."@en ;
  rdfs:isDefinedBy dcterms: ;
  rdfs:label "Type"@en ;
  rdfs:range rdfs:Class ;
  rdfs:range owl:Thing ;
  rdfs:subPropertyOf dc:type ;
.
dcterms:valid
  rdf:type rdf:Property ;
  dc:date "2000-07-11"^^xsd:date ;
  dc:date "2008-01-14"^^xsd:date ;
  dc:relation <http://dublincore.org/usage/terms/history/#valid-003> ;
  dcterms:date "2000-07-11"^^xsd:date ;
  dcterms:date "2008-01-14"^^xsd:date ;
  dcterms:hasVersion <http://dublincore.org/usage/terms/history/#valid-003> ;
  dcterms:issued "2000-07-11"^^xsd:date ;
  dcterms:modified "2008-01-14"^^xsd:date ;
  dcterms:relation <http://dublincore.org/usage/terms/history/#valid-003> ;
  rdfs:comment "Date (often a range) of validity of a resource."@en ;
  rdfs:isDefinedBy dcterms: ;
  rdfs:label "Date Valid"@en ;
  rdfs:range rdfs:Literal ;
  rdfs:subPropertyOf dc:date ;
  rdfs:subPropertyOf dcterms:date ;
.
gr:BusinessEntity
  rdfs:subClassOf org:FormalOrganization ;
.
schema:CreativeWork
  rdfs:subClassOf foaf:Document ;
  owl:equivalentClass foaf:Document ;
.
schema:ImageObject
  rdfs:subClassOf foaf:Image ;
  owl:equivalentClass foaf:Image ;
.
schema:Person
  owl:equivalentClass toop:Person ;
  owl:equivalentClass <http://www.w3.org/2000/10/swap/pim/contact#Person> ;
  owl:equivalentClass foaf:Person ;
.
<http://toop.eu/organization>
  rdf:type owl:Ontology ;
  spin:imports <http://topbraid.org/spin/owlrl-all> ;
  spin:imports <http://topbraid.org/spin/rdfsplus> ;
  spin:imports <http://topbraid.org/spin/skosspin> ;
  spin:imports <http://topbraid.org/spin/spinowl> ;
  owl:imports <file:///C:/Users/veerrjjd/TBCMEWorkspace/TopBraid/SKOS/skos-core.ttl.tbc> ;
  owl:imports <http://spinrdf.org/spin> ;
  owl:imports <https://www.w3.org/2009/08/skos-reference/skos.rdf> ;
  owl:versionIRI <http://ec.toop.org/ns/2017/12/organization> ;
  owl:versionInfo "$Date: 2017/12/27 16:31:41$" ;
.
toop:Address
  rdf:type owl:Class ;
  rdfs:comment "The postal address and/or the visiting address of a physical site of the company"@en ;
  rdfs:label "Physical address_"@en ;
  rdfs:subClassOf owl:Thing ;
  owl:equivalentClass elobr:EloniaAddress ;
  owl:equivalentClass freebr:FreedoniaAddress ;
  owl:equivalentClass vcard:Address ;
  owl:equivalentClass _:b49042 ;
.
toop:Address_1
  rdf:type elobr:EloniaAddress ;
  rdf:type freebr:FreedoniaAddress ;
  rdf:type toop:Address ;
  rdf:type vcard:Address ;
  rdf:type _:b49042 ;
  rdf:type _:b83024 ;
  rdf:type _:b401324 ;
  rdf:type _:b541374 ;
  rdf:type _:b583853 ;
  rdf:type _:b652026 ;
  rdf:type _:b763315 ;
  rdf:type _:b955705 ;
  toop:countryName "Nederland" ;
  vcard:country-name "Nederland" ;
.
toop:Address_card1
  rdf:type elobr:EloniaAddress ;
  rdf:type freebr:FreedoniaAddress ;
  rdf:type toop:Address ;
  rdf:type vcard:Address ;
  rdf:type _:b49042 ;
  rdf:type _:b83024 ;
  rdf:type _:b401324 ;
  rdf:type _:b541374 ;
  rdf:type _:b583853 ;
  rdf:type _:b652026 ;
  rdf:type _:b763315 ;
  rdf:type _:b955705 ;
  rdfs:comment "" ;
  rdfs:label "Address card1" ;
  rdfs:label "Address card1_"@nl ;
  skos:prefLabel "Address card1" ;
.
toop:CompanyCode
  rdf:type owl:Class ;
  rdfs:comment "The unique official company identifier_ "@en ;
  rdfs:label "Company code" ;
  rdfs:label "Company code_"@en ;
  rdfs:subClassOf adms:Identifier ;
  owl:equivalentClass elobr:EloniaBusinessCode ;
  owl:equivalentClass freebr:FreedoniaBusinessCode ;
  skos:prefLabel "Company code" ;
.
toop:CompanyCode_1
  rdf:type elobr:EloniaBusinessCode ;
  rdf:type freebr:FreedoniaBusinessCode ;
  rdf:type toop:CompanyCode ;
.
toop:CompanyContactNumber
  rdf:type owl:Class ;
  rdfs:subClassOf owl:Thing ;
.
toop:CompanyEmailAddress
  rdf:type owl:Class ;
  rdfs:subClassOf owl:Thing ;
.
toop:CompanyTypeScheme
  rdf:type rdfs:Class ;
  rdf:type owl:Class ;
  rdfs:comment "Represents the member states' recognized company types, expressed in a consistent manner in a SKOS Concept Scheme"@en ;
  rdfs:label "CompanyTypeScheme" ;
  rdfs:label "CompanyTypeScheme"@en ;
  rdfs:subClassOf skos:ConceptScheme ;
  owl:equivalentClass skos:ConceptScheme ;
  skos:prefLabel "CompanyTypeScheme" ;
.
toop:DocumentType
  rdf:type owl:Class ;
  rdfs:comment "The document type represents a grouping of concepts into a single document, e.g. company registration document, birth certificate document, mandate evidence document etc." ;
  rdfs:label "Document type" ;
  rdfs:subClassOf owl:Thing ;
.
toop:Foundation
  rdf:type rdfs:Class ;
  rdf:type owl:Class ;
  rdfs:comment "Represents the event that resulted in the foundation of the organization "@en ;
  rdfs:label "Foundation" ;
  rdfs:label "Foundation"@en ;
  rdfs:subClassOf org:ChangeEvent ;
  skos:prefLabel "Foundation" ;
.
toop:MainSite
  rdf:type rdfs:Class ;
  rdf:type owl:Class ;
  rdfs:comment "Represents the main office and/or premise at which the organization is located. Many organizations are spread across multiple sites and many sites will host multiple locations."@en ;
  rdfs:label "Site" ;
  rdfs:label "Site"@en ;
  rdfs:subClassOf org:Site ;
  skos:prefLabel "Site" ;
.
toop:MyCompCode-Id123456
  rdf:type elobr:Company ;
  rdf:type elobr:EloniaBusinessCode ;
  rdf:type freebr:Company ;
  rdf:type freebr:FreedoniaBusinessCode ;
  rdf:type adms:Identifier ;
  rdf:type _:b327858 ;
  elobr:EloniaLegalStatusEffectiveDate "2017-10-23"^^xsd:date ;
  elobr:EloniaRegistrationAuthority toop:NL-KvK ;
  freebr:FreedoniaLegalStatusEffectiveDate "2017-10-23"^^xsd:date ;
  freebr:FreedoniaRegistrationAuthority toop:NL-KvK ;
  dc:contributor toop:NL-KvK ;
  dc:creator toop:NL-KvK ;
  dc:date "2017-10-23"^^xsd:date ;
  dcterms:contributor toop:NL-KvK ;
  dcterms:creator toop:NL-KvK ;
  dcterms:date "2017-10-23"^^xsd:date ;
  dcterms:issued "2017-10-23"^^xsd:date ;
  toop:legalStatusEffectiveDate "2017-10-23"^^xsd:date ;
  toop:registrationAuthority toop:NL-KvK ;
  rdfs:comment "My company code, as instance of toop:CompanyCode class, representing the unique official company identifier as laid down by the registration authority_"@en ;
  rdfs:label "MyCompCode-Id123456_"@en ;
  adms:schemeAgency "NL-KvK Kamer van Koophandel"@nl ;
  foaf:maker toop:NL-KvK ;
.
toop:MyHasMainSite
  rdf:type toop:MainSite ;
  toop:siteOf toop:MyRegOrg_1 ;
  rdfs:comment "" ;
  rdfs:label "MyHasMainSite" ;
  rdfs:label "MyHasMainSite"@nl ;
  skos:prefLabel "MyHasMainSite" ;
  org:siteOf toop:MyRegOrg_1 ;
.
toop:MyOrganization_0
  rdf:type vcard:Organization ;
  rdf:type vcard:VCard ;
  rdf:type _:b57053 ;
  rdfs:comment "The vCard describing the main site of the company or legal person."@en ;
  rdfs:label "Mijn Organization_0"@nl ;
  rdfs:label "MyOrganization_0" ;
  skos:prefLabel "MyOrganization_0" ;
.
toop:MyOrganization_1
  rdf:type vcard:Organization ;
  rdf:type vcard:VCard ;
  rdf:type _:b57053 ;
  rdfs:comment "" ;
  rdfs:label "MijnOrganization 1_"@nl ;
  rdfs:label "My Organization 1" ;
  skos:prefLabel "My Organization 1" ;
.
toop:MyOrganization_2
  rdf:type vcard:Organization ;
  rdf:type vcard:VCard ;
  rdf:type _:b57053 ;
  rdfs:comment "" ;
  rdfs:label "Mijn Organization 2_"@nl ;
  rdfs:label "My Organization 2" ;
  skos:prefLabel "My Organization 2" ;
.
toop:MyRegOrg_1
  rdf:type elobr:Company ;
  rdf:type freebr:Company ;
  rdf:type dcterms:Agent ;
  rdf:type toop:RegisteredOrganization ;
  rdf:type _:b327858 ;
  rdf:type _:b420951 ;
  rdf:type _:b421075 ;
  rdf:type _:b421664 ;
  rdf:type _:b421928 ;
  rdf:type _:b937877 ;
  rdf:type _:b938265 ;
  elobr:EloniaCompanyName "My Own Company (legal name)" ;
  freebr:FreedoniaCompanyName "My Own Company (legal name)" ;
  toop:companyName "My Own Company (legal name)" ;
  toop:hasMainSite toop:MyHasMainSite ;
  rdfs:comment "My organization as instance from the toop:RegisteredOrganization Class" ;
  rdfs:label "Mijn reg org klas 1_"@nl ;
  rdfs:label "My organization as instance from the toop:RegisteredOrganization Class" ;
  skos:prefLabel "My organization as instance from the toop:RegisteredOrganization Class" ;
  org:hasPrimarySite toop:MyHasMainSite ;
  org:hasSite toop:MyHasMainSite ;
  rov:legalName "My Own Company (legal name)" ;
.
toop:NL-KvK
  rdf:type dcterms:Agent ;
  rdf:type foaf:Agent ;
  rdf:type _:b420951 ;
  rdf:type _:b421075 ;
  rdf:type _:b421664 ;
  rdf:type _:b421928 ;
  rdf:type _:b937877 ;
  rdf:type _:b938265 ;
  rdfs:comment "De Kamer van Koophandel is de autoriteit voor Nederland voor het registreren van ondermeer bedrijven"@nl ;
  rdfs:comment "The Dutch Chamber of Commerce, acting as registration authority for The Netherlands"@en ;
  rdfs:label "NL-Kv k_"@en ;
  foaf:made toop:MyCompCode-Id123456 ;
.
toop:Person
  rdf:type rdfs:Class ;
  rdf:type owl:Class ;
  rdfs:comment "This is the person" ;
  rdfs:subClassOf owl:Thing ;
  owl:equivalentClass schema:Person ;
  owl:equivalentClass <http://www.w3.org/2000/10/swap/pim/contact#Person> ;
  owl:equivalentClass foaf:Person ;
.
toop:RegisteredOrganization
  rdf:type rdfs:Class ;
  rdf:type owl:Class ;
  spin:query [
      rdf:type sp:Select ;
      sp:resultVariables (
          [
            sp:varName "s" ;
          ]
          [
            sp:varName "o" ;
          ]
        ) ;
      sp:where (
          [
            sp:object [
                sp:varName "o" ;
              ] ;
            sp:predicate [
                sp:varName "p" ;
              ] ;
            sp:subject [
                sp:varName "s" ;
              ] ;
          ]
          [
            rdf:type sp:Filter ;
            sp:expression [
                rdf:type sp:or ;
                sp:arg1 [
                    rdf:type sp:eq ;
                    sp:arg1 [
                        sp:varName "p" ;
                      ] ;
                    sp:arg2 owl:equivalentClass ;
                  ] ;
                sp:arg2 [
                    rdf:type sp:eq ;
                    sp:arg1 [
                        sp:varName "p" ;
                      ] ;
                    sp:arg2 owl:equivalentProperty ;
                  ] ;
              ] ;
          ]
          [
            rdf:type sp:Filter ;
            sp:expression [
                rdf:type sp:strstarts ;
                sp:arg1 [
                    rdf:type sp:str ;
                    sp:arg1 [
                        sp:varName "s" ;
                      ] ;
                  ] ;
                sp:arg2 "http://toop.eu/organization#" ;
              ] ;
          ]
          [
            rdf:type sp:Filter ;
            sp:expression [
                rdf:type sp:strstarts ;
                sp:arg1 [
                    rdf:type sp:str ;
                    sp:arg1 [
                        sp:varName "o" ;
                      ] ;
                  ] ;
                sp:arg2 "http://example.register.elo/elonia-business-register#" ;
              ] ;
          ]
        ) ;
    ] ;
  spin:query [
      rdf:type sp:Select ;
      sp:resultVariables (
          [
            sp:varName "s" ;
          ]
          [
            sp:varName "p" ;
          ]
          [
            sp:varName "v" ;
          ]
        ) ;
      sp:where (
          [
            rdf:type sp:Union ;
            sp:elements (
                (
                  [
                    sp:object [
                        sp:varName "o" ;
                      ] ;
                    sp:predicate rdfs:subClassOf ;
                    sp:subject [
                        sp:varName "s" ;
                      ] ;
                  ]
                  [
                    rdf:type sp:Filter ;
                    sp:expression [
                        rdf:type sp:eq ;
                        sp:arg1 [
                            sp:varName "s" ;
                          ] ;
                        sp:arg2 toop:RegisteredOrganization ;
                      ] ;
                  ]
                  [
                    sp:object [
                        sp:varName "p" ;
                      ] ;
                    sp:predicate owl:onProperty ;
                    sp:subject [
                        sp:varName "o" ;
                      ] ;
                  ]
                  [
                    sp:object [
                        sp:varName "v" ;
                      ] ;
                    sp:predicate owl:someValuesFrom ;
                    sp:subject [
                        sp:varName "o" ;
                      ] ;
                  ]
                )
                (
                  [
                    sp:object [
                        sp:varName "o" ;
                      ] ;
                    sp:predicate rdfs:subClassOf ;
                    sp:subject [
                        sp:varName "s" ;
                      ] ;
                  ]
                  [
                    rdf:type sp:Filter ;
                    sp:expression [
                        rdf:type sp:eq ;
                        sp:arg1 [
                            sp:varName "s" ;
                          ] ;
                        sp:arg2 toop:RegisteredOrganization ;
                      ] ;
                  ]
                  [
                    sp:object [
                        sp:varName "p" ;
                      ] ;
                    sp:predicate owl:onProperty ;
                    sp:subject [
                        sp:varName "o" ;
                      ] ;
                  ]
                  [
                    sp:object [
                        sp:varName "v" ;
                      ] ;
                    sp:predicate owl:cardinality ;
                    sp:subject [
                        sp:varName "o" ;
                      ] ;
                  ]
                )
              ) ;
          ]
        ) ;
    ] ;
  rdfs:comment "The TOOP Registered Orginization class represents an organization that has gained legal status by one of the European member states. It is a direct subclass of the rov:RegisteredOrganization class."@en ;
  rdfs:label "Registered organization"@en ;
  rdfs:subClassOf rov:RegisteredOrganization ;
  rdfs:subClassOf _:b180769 ;
  rdfs:subClassOf _:b254570 ;
  rdfs:subClassOf _:b454254 ;
  rdfs:subClassOf _:b826282 ;
  rdfs:subClassOf _:b826680 ;
.
toop:Registration
  rdf:type rdfs:Class ;
  rdf:type owl:Class ;
  rdfs:comment "Represents the event that resulted in the registration of the organization."@en ;
  rdfs:label "Registration" ;
  rdfs:label "Registration"@en ;
  rdfs:subClassOf org:ChangeEvent ;
  skos:prefLabel "Registration" ;
.
toop:SSNumber
  rdf:type rdfs:Class ;
  rdfs:comment "The social security number of the company_"@en ;
  rdfs:label "SSNumber" ;
  rdfs:label "SSNumber"@en ;
  rdfs:subClassOf adms:Identifier ;
  owl:equivalentClass elobr:EloniaSSNumber ;
  owl:equivalentClass freebr:FreedoniaSSNumber ;
  skos:prefLabel "SSNumber" ;
.
toop:VATNumber
  rdf:type rdfs:Class ;
  rdfs:comment "The value added tax number of the company"@en ;
  rdfs:label "VATNumber" ;
  rdfs:label "VATNumber"@en ;
  rdfs:subClassOf adms:Identifier ;
  owl:equivalentClass elobr:EloniaVATNumber ;
  owl:equivalentClass freebr:FreedoniaVATNumber ;
  skos:prefLabel "VATNumber" ;
.
toop:activityDeclaration
  rdf:type rdf:Property ;
  rdfs:comment "The description of the main activity of the company as free text description recorded on the registry. This tag should be used to give a description of the company activity in the local language. This should be used in conjunction with the CompanyNaceCode."@en ;
  rdfs:label "activity declaration" ;
  rdfs:label "activity declaration"@en ;
  rdfs:subPropertyOf dc:description ;
  rdfs:subPropertyOf dcterms:description ;
  owl:equivalentProperty elobr:EloniaActivityDeclaration ;
  owl:equivalentProperty freebr:FreedoniaActivityDeclaration ;
  skos:prefLabel "activity declaration" ;
.
toop:addressCompanyEmailAddress
  rdf:type owl:DatatypeProperty ;
  rdfs:domain toop:CompanyEmailAddress ;
  rdfs:domain owl:Thing ;
.
toop:age
  rdf:type owl:DatatypeProperty ;
  rdfs:domain dcterms:Agent ;
  rdfs:domain schema:Person ;
  rdfs:domain toop:Person ;
  rdfs:domain <http://www.w3.org/2000/10/swap/pim/contact#Person> ;
  rdfs:domain owl:Thing ;
  rdfs:domain wgs:SpatialThing ;
  rdfs:domain foaf:Agent ;
  rdfs:domain foaf:Person ;
  rdfs:domain _:b420951 ;
  rdfs:domain _:b421075 ;
  rdfs:domain _:b421664 ;
  rdfs:domain _:b421928 ;
  rdfs:domain _:b937877 ;
  rdfs:domain _:b938265 ;
  rdfs:range rdfs:Literal ;
  owl:equivalentProperty foaf:age ;
.
toop:birthday
  rdf:type owl:DatatypeProperty ;
  rdfs:domain dcterms:Agent ;
  rdfs:domain schema:Person ;
  rdfs:domain toop:Person ;
  rdfs:domain <http://www.w3.org/2000/10/swap/pim/contact#Person> ;
  rdfs:domain owl:Thing ;
  rdfs:domain wgs:SpatialThing ;
  rdfs:domain foaf:Agent ;
  rdfs:domain foaf:Person ;
  rdfs:domain _:b420951 ;
  rdfs:domain _:b421075 ;
  rdfs:domain _:b421664 ;
  rdfs:domain _:b421928 ;
  rdfs:domain _:b937877 ;
  rdfs:domain _:b938265 ;
  rdfs:range rdfs:Literal ;
  owl:equivalentProperty foaf:birthday ;
.
toop:companyContactNumber
  rdf:type owl:ObjectProperty ;
  rdfs:domain dcterms:Agent ;
  rdfs:domain toop:RegisteredOrganization ;
  rdfs:domain owl:Thing ;
  rdfs:domain vcard:Kind ;
  rdfs:domain vcard:VCard ;
  rdfs:domain org:FormalOrganization ;
  rdfs:domain org:Organization ;
  rdfs:domain rov:RegisteredOrganization ;
  rdfs:domain foaf:Agent ;
  rdfs:domain foaf:Organization ;
  rdfs:domain _:b57053 ;
  rdfs:domain _:b180769 ;
  rdfs:domain _:b254570 ;
  rdfs:domain _:b420951 ;
  rdfs:domain _:b421075 ;
  rdfs:domain _:b421664 ;
  rdfs:domain _:b421928 ;
  rdfs:domain _:b454254 ;
  rdfs:domain _:b826282 ;
  rdfs:domain _:b826680 ;
  rdfs:domain _:b937877 ;
  rdfs:domain _:b938265 ;
  rdfs:range toop:CompanyContactNumber ;
  rdfs:range owl:Thing ;
  owl:equivalentProperty vcard:hasTelephone ;
  owl:equivalentProperty vcard:tel ;
.
toop:companyEmailAddress
  rdf:type owl:ObjectProperty ;
  rdfs:domain dcterms:Agent ;
  rdfs:domain toop:RegisteredOrganization ;
  rdfs:domain owl:Thing ;
  rdfs:domain vcard:Kind ;
  rdfs:domain vcard:VCard ;
  rdfs:domain org:FormalOrganization ;
  rdfs:domain org:Organization ;
  rdfs:domain rov:RegisteredOrganization ;
  rdfs:domain foaf:Agent ;
  rdfs:domain foaf:Organization ;
  rdfs:domain _:b57053 ;
  rdfs:domain _:b180769 ;
  rdfs:domain _:b254570 ;
  rdfs:domain _:b420951 ;
  rdfs:domain _:b421075 ;
  rdfs:domain _:b421664 ;
  rdfs:domain _:b421928 ;
  rdfs:domain _:b454254 ;
  rdfs:domain _:b826282 ;
  rdfs:domain _:b826680 ;
  rdfs:domain _:b937877 ;
  rdfs:domain _:b938265 ;
  rdfs:range toop:CompanyEmailAddress ;
  rdfs:range owl:Thing ;
  rdfs:range vcard:Email ;
  rdfs:range _:b583853 ;
  rdfs:range _:b652026 ;
  owl:equivalentProperty vcard:email ;
  owl:equivalentProperty vcard:hasEmail ;
.
toop:companyNaceCode
  rdf:type owl:ObjectProperty ;
  rdfs:comment "The description of the main activity of the company as free text description recorded on the registry. This tag should be used to give a description of the company activity in the local language. This should be used in conjunction with the CompanyNaceCode"@en ;
  rdfs:domain dcterms:Agent ;
  rdfs:domain owl:Thing ;
  rdfs:domain org:Organization ;
  rdfs:domain foaf:Agent ;
  rdfs:domain foaf:Organization ;
  rdfs:domain _:b420951 ;
  rdfs:domain _:b421075 ;
  rdfs:domain _:b421664 ;
  rdfs:domain _:b421928 ;
  rdfs:domain _:b937877 ;
  rdfs:domain _:b938265 ;
  rdfs:label "company NACE code" ;
  rdfs:label "company NACE code"@en ;
  rdfs:range owl:Thing ;
  rdfs:range skos:Concept ;
  rdfs:range _:b327858 ;
  rdfs:subPropertyOf org:classification ;
  rdfs:subPropertyOf rov:orgActivity ;
  owl:equivalentProperty elobr:EloniaCompanyNaceCode ;
  owl:equivalentProperty freebr:FreedoniaCompanyNaceCode ;
  skos:prefLabel "company NACE code" ;
.
toop:companyName
  rdf:type owl:DatatypeProperty ;
  rdfs:comment "The official current company name as stored in the business register_"@en ;
  rdfs:domain elobr:Company ;
  rdfs:domain freebr:Company ;
  rdfs:domain dcterms:Agent ;
  rdfs:domain owl:Thing ;
  rdfs:domain skos:Concept ;
  rdfs:domain org:FormalOrganization ;
  rdfs:domain org:Organization ;
  rdfs:domain foaf:Agent ;
  rdfs:domain foaf:Organization ;
  rdfs:domain _:b156576 ;
  rdfs:domain _:b213787 ;
  rdfs:domain _:b327858 ;
  rdfs:domain _:b420951 ;
  rdfs:domain _:b421075 ;
  rdfs:domain _:b421664 ;
  rdfs:domain _:b421928 ;
  rdfs:domain _:b772676 ;
  rdfs:domain _:b883411 ;
  rdfs:domain _:b937877 ;
  rdfs:domain _:b938265 ;
  rdfs:label "company name" ;
  rdfs:range rdfs:Literal ;
  rdfs:range xsd:string ;
  rdfs:subPropertyOf rov:legalName ;
  owl:equivalentProperty elobr:EloniaCompanyName ;
  owl:equivalentProperty freebr:FreedoniaCompanyName ;
.
toop:companyType
  rdf:type rdf:Property ;
  rdf:type owl:ObjectProperty ;
  rdfs:comment "The legal type of the company_"@en ;
  rdfs:domain elobr:Company ;
  rdfs:domain freebr:Company ;
  rdfs:domain dcterms:Agent ;
  rdfs:domain toop:RegisteredOrganization ;
  rdfs:domain owl:Thing ;
  rdfs:domain skos:Concept ;
  rdfs:domain org:FormalOrganization ;
  rdfs:domain org:Organization ;
  rdfs:domain rov:RegisteredOrganization ;
  rdfs:domain foaf:Agent ;
  rdfs:domain foaf:Organization ;
  rdfs:domain _:b156576 ;
  rdfs:domain _:b180769 ;
  rdfs:domain _:b213787 ;
  rdfs:domain _:b254570 ;
  rdfs:domain _:b327858 ;
  rdfs:domain _:b420951 ;
  rdfs:domain _:b421075 ;
  rdfs:domain _:b421664 ;
  rdfs:domain _:b421928 ;
  rdfs:domain _:b454254 ;
  rdfs:domain _:b772676 ;
  rdfs:domain _:b826282 ;
  rdfs:domain _:b826680 ;
  rdfs:domain _:b883411 ;
  rdfs:domain _:b937877 ;
  rdfs:domain _:b938265 ;
  rdfs:label "company type" ;
  rdfs:label "company type"@en ;
  rdfs:range owl:Thing ;
  rdfs:range skos:Concept ;
  rdfs:range _:b327858 ;
  rdfs:range _:b875853 ;
  rdfs:subPropertyOf org:classification ;
  owl:equivalentProperty elobr:EloniaCompanyType ;
  owl:equivalentProperty freebr:FreedoniaCompanyType ;
  owl:equivalentProperty rov:orgType ;
  skos:prefLabel "company type" ;
.
toop:contactType
  rdf:type owl:ObjectProperty ;
  rdfs:domain toop:CompanyContactNumber ;
  rdfs:domain owl:Thing ;
  rdfs:range owl:Thing ;
  rdfs:range vcard:TelephoneType ;
.
toop:countryName
  rdf:type owl:DatatypeProperty ;
  rdfs:comment "The country name associated with the address of the organization."@en ;
  rdfs:domain elobr:EloniaAddress ;
  rdfs:domain freebr:FreedoniaAddress ;
  rdfs:domain toop:Address ;
  rdfs:domain owl:Thing ;
  rdfs:domain vcard:Address ;
  rdfs:domain _:b49042 ;
  rdfs:domain _:b83024 ;
  rdfs:domain _:b157701 ;
  rdfs:domain _:b168676 ;
  rdfs:domain _:b396249 ;
  rdfs:domain _:b401324 ;
  rdfs:domain _:b499218 ;
  rdfs:domain _:b541374 ;
  rdfs:domain _:b583853 ;
  rdfs:domain _:b652026 ;
  rdfs:domain _:b726818 ;
  rdfs:domain _:b763315 ;
  rdfs:domain _:b787338 ;
  rdfs:domain _:b926654 ;
  rdfs:domain _:b955705 ;
  rdfs:label "country name" ;
  rdfs:range xsd:string ;
  owl:equivalentProperty vcard:country-name ;
.
toop:familyName
  rdf:type owl:DatatypeProperty ;
  rdfs:domain dcterms:Agent ;
  rdfs:domain schema:Person ;
  rdfs:domain toop:Person ;
  rdfs:domain <http://www.w3.org/2000/10/swap/pim/contact#Person> ;
  rdfs:domain owl:Thing ;
  rdfs:domain wgs:SpatialThing ;
  rdfs:domain foaf:Agent ;
  rdfs:domain foaf:Person ;
  rdfs:domain _:b420951 ;
  rdfs:domain _:b421075 ;
  rdfs:domain _:b421664 ;
  rdfs:domain _:b421928 ;
  rdfs:domain _:b937877 ;
  rdfs:domain _:b938265 ;
  rdfs:range rdfs:Literal ;
  owl:equivalentProperty foaf:familyName ;
.
toop:foundationDate
  rdf:type owl:DatatypeProperty ;
  rdfs:comment "Represents the date at which the company started. "@en ;
  rdfs:domain toop:Foundation ;
  rdfs:domain owl:Thing ;
  rdfs:domain org:ChangeEvent ;
  rdfs:domain prov:Activity ;
  rdfs:domain _:b53184 ;
  rdfs:domain _:b170340 ;
  rdfs:domain _:b399839 ;
  rdfs:domain _:b715640 ;
  rdfs:domain _:b895567 ;
  rdfs:domain _:b897711 ;
  rdfs:label "foundation date" ;
  rdfs:label "foundation date"@en ;
  rdfs:range xsd:dateTime ;
  rdfs:range _:b115973 ;
  rdfs:range _:b148299 ;
  rdfs:range _:b671381 ;
  rdfs:range _:b719479 ;
  rdfs:subPropertyOf prov:startedAtTime ;
  skos:prefLabel "foundation date" ;
.
toop:givenName
  rdf:type owl:DatatypeProperty ;
  rdfs:domain dcterms:Agent ;
  rdfs:domain schema:Person ;
  rdfs:domain toop:Person ;
  rdfs:domain <http://www.w3.org/2000/10/swap/pim/contact#Person> ;
  rdfs:domain owl:Thing ;
  rdfs:domain wgs:SpatialThing ;
  rdfs:domain foaf:Agent ;
  rdfs:domain foaf:Person ;
  rdfs:domain _:b420951 ;
  rdfs:domain _:b421075 ;
  rdfs:domain _:b421664 ;
  rdfs:domain _:b421928 ;
  rdfs:domain _:b937877 ;
  rdfs:domain _:b938265 ;
  owl:equivalentProperty foaf:givenName ;
.
toop:hasAddress
  rdf:type owl:ObjectProperty ;
  rdfs:comment "Represents a pointer to physical or virtual address of the company."@en ;
  rdfs:domain owl:Thing ;
  rdfs:domain org:Site ;
  rdfs:label "has address" ;
  rdfs:label "has address_"@en ;
  rdfs:range elobr:EloniaAddress ;
  rdfs:range freebr:FreedoniaAddress ;
  rdfs:range toop:Address ;
  rdfs:range owl:Thing ;
  rdfs:range vcard:Address ;
  rdfs:range _:b49042 ;
  rdfs:range _:b83024 ;
  rdfs:range _:b157701 ;
  rdfs:range _:b168676 ;
  rdfs:range _:b396249 ;
  rdfs:range _:b401324 ;
  rdfs:range _:b499218 ;
  rdfs:range _:b541374 ;
  rdfs:range _:b583853 ;
  rdfs:range _:b652026 ;
  rdfs:range _:b726818 ;
  rdfs:range _:b763315 ;
  rdfs:range _:b787338 ;
  rdfs:range _:b926654 ;
  rdfs:range _:b955705 ;
  rdfs:subPropertyOf org:siteAddress ;
  skos:prefLabel "has address" ;
.
toop:hasCompanyCode
  rdf:type owl:ObjectProperty ;
  rdfs:comment "The property of a registered organization of having a main code that is the unique identifier recorded in the registry. This tag should be used to give an identifier of the company in the local language. It should be used in conjunction with the CompanyNaceCode."@en ;
  rdfs:domain dcterms:Agent ;
  rdfs:domain owl:Thing ;
  rdfs:domain org:FormalOrganization ;
  rdfs:domain org:Organization ;
  rdfs:domain rov:RegisteredOrganization ;
  rdfs:domain foaf:Agent ;
  rdfs:domain foaf:Organization ;
  rdfs:domain _:b420951 ;
  rdfs:domain _:b421075 ;
  rdfs:domain _:b421664 ;
  rdfs:domain _:b421928 ;
  rdfs:domain _:b937877 ;
  rdfs:domain _:b938265 ;
  rdfs:label "company code" ;
  rdfs:label "company code"@en ;
  rdfs:range adms:Identifier ;
  rdfs:subPropertyOf adms:identifier ;
  rdfs:subPropertyOf rov:registration ;
  skos:prefLabel "company code" ;
.
toop:hasMainSite
  rdf:type owl:ObjectProperty ;
  rdfs:comment "The main site of the company."@en ;
  rdfs:domain dcterms:Agent ;
  rdfs:domain toop:RegisteredOrganization ;
  rdfs:domain owl:Thing ;
  rdfs:domain org:FormalOrganization ;
  rdfs:domain org:Organization ;
  rdfs:domain rov:RegisteredOrganization ;
  rdfs:domain foaf:Agent ;
  rdfs:domain foaf:Organization ;
  rdfs:domain _:b180769 ;
  rdfs:domain _:b254570 ;
  rdfs:domain _:b420951 ;
  rdfs:domain _:b421075 ;
  rdfs:domain _:b421664 ;
  rdfs:domain _:b421928 ;
  rdfs:domain _:b454254 ;
  rdfs:domain _:b826282 ;
  rdfs:domain _:b826680 ;
  rdfs:domain _:b937877 ;
  rdfs:domain _:b938265 ;
  rdfs:label "has main site" ;
  rdfs:label "has main site"@nl ;
  rdfs:range toop:MainSite ;
  rdfs:range owl:Thing ;
  rdfs:range org:Site ;
  rdfs:subPropertyOf org:hasSite ;
  owl:equivalentProperty org:hasPrimarySite ;
  owl:inverseOf toop:siteOf ;
  skos:prefLabel "has main site" ;
.
toop:hasRegistration
  rdf:type rdf:Property ;
  rdfs:comment "This is the property that makes the link between a registered organization and the registration event." ;
  rdfs:domain dcterms:Agent ;
  rdfs:domain toop:RegisteredOrganization ;
  rdfs:domain owl:Thing ;
  rdfs:domain org:FormalOrganization ;
  rdfs:domain org:Organization ;
  rdfs:domain rov:RegisteredOrganization ;
  rdfs:domain foaf:Agent ;
  rdfs:domain foaf:Organization ;
  rdfs:domain _:b180769 ;
  rdfs:domain _:b254570 ;
  rdfs:domain _:b420951 ;
  rdfs:domain _:b421075 ;
  rdfs:domain _:b421664 ;
  rdfs:domain _:b421928 ;
  rdfs:domain _:b454254 ;
  rdfs:domain _:b826282 ;
  rdfs:domain _:b826680 ;
  rdfs:domain _:b937877 ;
  rdfs:domain _:b938265 ;
  rdfs:label "has registration"@en ;
  rdfs:range toop:Registration ;
  rdfs:range owl:Thing ;
  rdfs:range org:ChangeEvent ;
  rdfs:range prov:Activity ;
  rdfs:range _:b53184 ;
  rdfs:range _:b170340 ;
  rdfs:range _:b399839 ;
  rdfs:range _:b715640 ;
  rdfs:range _:b895567 ;
  rdfs:range _:b897711 ;
  skos:prefLabel "has registration"@en ;
.
toop:legalRepresentativeOf
  rdf:type owl:ObjectProperty ;
  rdfs:domain dcterms:Agent ;
  rdfs:domain schema:Person ;
  rdfs:domain toop:Person ;
  rdfs:domain <http://www.w3.org/2000/10/swap/pim/contact#Person> ;
  rdfs:domain owl:Thing ;
  rdfs:domain wgs:SpatialThing ;
  rdfs:domain foaf:Agent ;
  rdfs:domain foaf:Person ;
  rdfs:domain _:b420951 ;
  rdfs:domain _:b421075 ;
  rdfs:domain _:b421664 ;
  rdfs:domain _:b421928 ;
  rdfs:domain _:b937877 ;
  rdfs:domain _:b938265 ;
  rdfs:range dcterms:Agent ;
  rdfs:range toop:RegisteredOrganization ;
  rdfs:range owl:Thing ;
  rdfs:range org:FormalOrganization ;
  rdfs:range org:Organization ;
  rdfs:range rov:RegisteredOrganization ;
  rdfs:range foaf:Agent ;
  rdfs:range foaf:Organization ;
  rdfs:range _:b180769 ;
  rdfs:range _:b254570 ;
  rdfs:range _:b420951 ;
  rdfs:range _:b421075 ;
  rdfs:range _:b421664 ;
  rdfs:range _:b421928 ;
  rdfs:range _:b454254 ;
  rdfs:range _:b826282 ;
  rdfs:range _:b826680 ;
  rdfs:range _:b937877 ;
  rdfs:range _:b938265 ;
  rdfs:subPropertyOf org:memberOf ;
.
toop:legalStatus
  rdf:type rdf:Property ;
  rdfs:comment "The current legal status of a company (active, ended, ...)"@en ;
  rdfs:domain elobr:Company ;
  rdfs:domain elobr:EloniaBusinessCode ;
  rdfs:domain freebr:Company ;
  rdfs:domain freebr:FreedoniaBusinessCode ;
  rdfs:domain dcterms:Agent ;
  rdfs:domain toop:CompanyCode ;
  rdfs:domain owl:Thing ;
  rdfs:domain skos:Concept ;
  rdfs:domain adms:Identifier ;
  rdfs:domain org:Organization ;
  rdfs:domain foaf:Agent ;
  rdfs:domain foaf:Organization ;
  rdfs:domain _:b156576 ;
  rdfs:domain _:b213787 ;
  rdfs:domain _:b327858 ;
  rdfs:domain _:b420951 ;
  rdfs:domain _:b421075 ;
  rdfs:domain _:b421664 ;
  rdfs:domain _:b421928 ;
  rdfs:domain _:b772676 ;
  rdfs:domain _:b883411 ;
  rdfs:domain _:b937877 ;
  rdfs:domain _:b938265 ;
  rdfs:label "legal status" ;
  rdfs:label "legal status"@en ;
  rdfs:range owl:Thing ;
  rdfs:range skos:Concept ;
  rdfs:range _:b327858 ;
  rdfs:subPropertyOf org:classification ;
  owl:equivalentProperty elobr:EloniaLegalStatus ;
  owl:equivalentProperty freebr:FreedoniaLegalStatus ;
  owl:equivalentProperty rov:orgStatus ;
  skos:prefLabel "legal status" ;
.
toop:legalStatusEffectiveDate
  rdf:type rdf:Property ;
  rdfs:comment "The date at which the current legal status became effective_"@en ;
  rdfs:domain elobr:Company ;
  rdfs:domain elobr:EloniaBusinessCode ;
  rdfs:domain freebr:Company ;
  rdfs:domain freebr:FreedoniaBusinessCode ;
  rdfs:domain toop:CompanyCode ;
  rdfs:domain owl:Thing ;
  rdfs:domain skos:Concept ;
  rdfs:domain adms:Identifier ;
  rdfs:domain _:b156576 ;
  rdfs:domain _:b213787 ;
  rdfs:domain _:b327858 ;
  rdfs:domain _:b772676 ;
  rdfs:domain _:b883411 ;
  rdfs:label "legal status effective date" ;
  rdfs:label "legal status effective date"@en ;
  rdfs:range rdfs:Literal ;
  rdfs:subPropertyOf dc:date ;
  rdfs:subPropertyOf dcterms:date ;
  rdfs:subPropertyOf dcterms:issued ;
  owl:equivalentProperty elobr:EloniaLegalStatusEffectiveDate ;
  owl:equivalentProperty freebr:FreedoniaLegalStatusEffectiveDate ;
  skos:prefLabel "legal status effective date" ;
.
toop:locality
  rdf:type owl:DatatypeProperty ;
  rdfs:comment "The locality (e.g. city or town) associated with the address of the organization."@en ;
  rdfs:domain elobr:EloniaAddress ;
  rdfs:domain freebr:FreedoniaAddress ;
  rdfs:domain toop:Address ;
  rdfs:domain owl:Thing ;
  rdfs:domain vcard:Address ;
  rdfs:domain _:b49042 ;
  rdfs:domain _:b83024 ;
  rdfs:domain _:b157701 ;
  rdfs:domain _:b168676 ;
  rdfs:domain _:b396249 ;
  rdfs:domain _:b401324 ;
  rdfs:domain _:b499218 ;
  rdfs:domain _:b541374 ;
  rdfs:domain _:b583853 ;
  rdfs:domain _:b652026 ;
  rdfs:domain _:b726818 ;
  rdfs:domain _:b763315 ;
  rdfs:domain _:b787338 ;
  rdfs:domain _:b926654 ;
  rdfs:domain _:b955705 ;
  rdfs:label "locality" ;
  rdfs:range xsd:string ;
  owl:equivalentProperty vcard:locality ;
.
toop:numberCompanyContactNumber
  rdf:type owl:DatatypeProperty ;
  rdfs:domain toop:CompanyContactNumber ;
  rdfs:domain owl:Thing ;
.
toop:postalCode
  rdf:type owl:DatatypeProperty ;
  rdfs:comment "The postal code associated with the address of the organization."@en ;
  rdfs:domain elobr:EloniaAddress ;
  rdfs:domain freebr:FreedoniaAddress ;
  rdfs:domain toop:Address ;
  rdfs:domain owl:Thing ;
  rdfs:domain vcard:Address ;
  rdfs:domain _:b49042 ;
  rdfs:domain _:b83024 ;
  rdfs:domain _:b157701 ;
  rdfs:domain _:b168676 ;
  rdfs:domain _:b396249 ;
  rdfs:domain _:b401324 ;
  rdfs:domain _:b499218 ;
  rdfs:domain _:b541374 ;
  rdfs:domain _:b583853 ;
  rdfs:domain _:b652026 ;
  rdfs:domain _:b726818 ;
  rdfs:domain _:b763315 ;
  rdfs:domain _:b787338 ;
  rdfs:domain _:b926654 ;
  rdfs:domain _:b955705 ;
  rdfs:label "postal code" ;
  rdfs:range xsd:string ;
  owl:equivalentProperty vcard:postal-code ;
.
toop:region
  rdf:type owl:DatatypeProperty ;
  rdfs:comment "The region (e.g. state or province) associated with the address of the organization."@en ;
  rdfs:domain elobr:EloniaAddress ;
  rdfs:domain freebr:FreedoniaAddress ;
  rdfs:domain toop:Address ;
  rdfs:domain owl:Thing ;
  rdfs:domain vcard:Address ;
  rdfs:domain _:b49042 ;
  rdfs:domain _:b83024 ;
  rdfs:domain _:b157701 ;
  rdfs:domain _:b168676 ;
  rdfs:domain _:b396249 ;
  rdfs:domain _:b401324 ;
  rdfs:domain _:b499218 ;
  rdfs:domain _:b541374 ;
  rdfs:domain _:b583853 ;
  rdfs:domain _:b652026 ;
  rdfs:domain _:b726818 ;
  rdfs:domain _:b763315 ;
  rdfs:domain _:b787338 ;
  rdfs:domain _:b926654 ;
  rdfs:domain _:b955705 ;
  rdfs:label "region" ;
  rdfs:range xsd:string ;
  owl:equivalentProperty vcard:region ;
.
toop:registrationAuthority
  rdf:type owl:ObjectProperty ;
  rdfs:comment "The reference to the official register that has registered the company"@en ;
  rdfs:domain elobr:EloniaBusinessCode ;
  rdfs:domain freebr:FreedoniaBusinessCode ;
  rdfs:domain toop:CompanyCode ;
  rdfs:domain owl:Thing ;
  rdfs:domain adms:Identifier ;
  rdfs:label "registration authority" ;
  rdfs:label "registration authority"@en ;
  rdfs:range dcterms:Agent ;
  rdfs:range owl:Thing ;
  rdfs:range foaf:Agent ;
  rdfs:range _:b420951 ;
  rdfs:range _:b421075 ;
  rdfs:range _:b421664 ;
  rdfs:range _:b421928 ;
  rdfs:range _:b937877 ;
  rdfs:range _:b938265 ;
  rdfs:subPropertyOf dc:contributor ;
  rdfs:subPropertyOf dc:creator ;
  rdfs:subPropertyOf dcterms:contributor ;
  owl:equivalentProperty elobr:EloniaRegistrationAuthority ;
  owl:equivalentProperty freebr:FreedoniaRegistrationAuthority ;
  owl:equivalentProperty dcterms:creator ;
  owl:equivalentProperty foaf:maker ;
  skos:prefLabel "registration authority" ;
.
toop:registrationDate
  rdf:type owl:DatatypeProperty ;
  rdfs:comment "Represents the date at which the company started. "@en ;
  rdfs:domain toop:Registration ;
  rdfs:domain owl:Thing ;
  rdfs:domain org:ChangeEvent ;
  rdfs:domain prov:Activity ;
  rdfs:domain _:b53184 ;
  rdfs:domain _:b170340 ;
  rdfs:domain _:b399839 ;
  rdfs:domain _:b715640 ;
  rdfs:domain _:b895567 ;
  rdfs:domain _:b897711 ;
  rdfs:label "registration date" ;
  rdfs:label "registration date"@en ;
  rdfs:range xsd:date ;
  rdfs:range xsd:dateTime ;
  rdfs:range _:b115973 ;
  rdfs:range _:b148299 ;
  rdfs:range _:b671381 ;
  rdfs:range _:b719479 ;
  rdfs:subPropertyOf prov:startedAtTime ;
  owl:equivalentProperty elobr:EloniaRegistrationDate ;
  owl:equivalentProperty freebr:FreedoniaRegistrationDate ;
  skos:prefLabel "registration date" ;
.
toop:registrationNumber
  rdf:type owl:DatatypeProperty ;
  rdfs:comment "The number of the company as recorded on the register. In some jurisdictions, the number on the register may be different from the official company number. This field must be populated in all service requests even when the RegistrationNumber is the same as the CompanyCode "@en ;
  rdfs:domain dcterms:Agent ;
  rdfs:domain owl:Thing ;
  rdfs:domain org:Organization ;
  rdfs:domain foaf:Agent ;
  rdfs:domain foaf:Organization ;
  rdfs:domain _:b420951 ;
  rdfs:domain _:b421075 ;
  rdfs:domain _:b421664 ;
  rdfs:domain _:b421928 ;
  rdfs:domain _:b937877 ;
  rdfs:domain _:b938265 ;
  rdfs:label "registration number" ;
  rdfs:label "registration number"@en ;
  rdfs:subPropertyOf skos:notation ;
  owl:equivalentProperty elobr:EloniaRegistrationNumber ;
  owl:equivalentProperty freebr:FreedoniaRegistrationNumber ;
  owl:equivalentProperty org:identifier ;
  skos:prefLabel "registration number" ;
.
toop:siteOf
  rdf:type owl:ObjectProperty ;
  rdfs:comment "A virtual or physical site is the site of a registered organization"@en ;
  rdfs:domain owl:Thing ;
  rdfs:domain org:Site ;
  rdfs:label "site of_"@en ;
  rdfs:range dcterms:Agent ;
  rdfs:range owl:Thing ;
  rdfs:range org:Organization ;
  rdfs:range foaf:Agent ;
  rdfs:range foaf:Organization ;
  rdfs:range _:b420951 ;
  rdfs:range _:b421075 ;
  rdfs:range _:b421664 ;
  rdfs:range _:b421928 ;
  rdfs:range _:b937877 ;
  rdfs:range _:b938265 ;
  owl:equivalentProperty org:siteOf ;
.
toop:streetAddress
  rdf:type owl:DatatypeProperty ;
  rdfs:comment "The street address associated with the address of the organization."@en ;
  rdfs:domain elobr:EloniaAddress ;
  rdfs:domain freebr:FreedoniaAddress ;
  rdfs:domain toop:Address ;
  rdfs:domain owl:Thing ;
  rdfs:domain vcard:Address ;
  rdfs:domain _:b49042 ;
  rdfs:domain _:b83024 ;
  rdfs:domain _:b157701 ;
  rdfs:domain _:b168676 ;
  rdfs:domain _:b396249 ;
  rdfs:domain _:b401324 ;
  rdfs:domain _:b499218 ;
  rdfs:domain _:b541374 ;
  rdfs:domain _:b583853 ;
  rdfs:domain _:b652026 ;
  rdfs:domain _:b726818 ;
  rdfs:domain _:b763315 ;
  rdfs:domain _:b787338 ;
  rdfs:domain _:b926654 ;
  rdfs:domain _:b955705 ;
  rdfs:label "street address" ;
  rdfs:range xsd:string ;
  owl:equivalentProperty vcard:street-address ;
.
toop:websiteURL
  rdf:type owl:ObjectProperty ;
  rdfs:comment "ISSUE: currently, TBC's local import for vcard seems incomplete - vcard:has* are missing"@en ;
  rdfs:comment "Represents the website URL of the company."@en ;
  rdfs:comment "Represents the website address of the company."@en ;
  rdfs:domain toop:MainSite ;
  rdfs:domain owl:Thing ;
  rdfs:domain org:Site ;
  rdfs:label "websiteAddress" ;
  rdfs:label "websiteAddress"@en ;
  rdfs:label "websiteURL" ;
  rdfs:label "websiteURL"@en ;
  rdfs:range dcterms:URI ;
  rdfs:subPropertyOf org:siteAddress ;
  skos:prefLabel "websiteAddress" ;
  skos:prefLabel "websiteURL" ;
.
<http://www.asahi-net.or.jp/~ax2s-kmtn/>
  rdf:type schema:CreativeWork ;
  rdf:type foaf:Document ;
  foaf:primaryTopic _:b421215 ;
  foaf:primaryTopic _:b937583 ;
  foaf:primaryTopic _:b938110 ;
  foaf:topic _:b421215 ;
  foaf:topic _:b937583 ;
  foaf:topic _:b938110 ;
.
<http://www.opendatacommons.org/licenses/pddl/1.0/>
  rdf:type dcterms:LicenseDocument ;
.
<http://www.w3.org/>
  rdf:type schema:CreativeWork ;
  rdf:type foaf:Document ;
  foaf:primaryTopic _:b421137 ;
  foaf:primaryTopic _:b421711 ;
  foaf:primaryTopic _:b421804 ;
  foaf:topic _:b421137 ;
  foaf:topic _:b421711 ;
  foaf:topic _:b421804 ;
.
rdfs:Class
  rdf:type owl:Class ;
.
rdfs:comment
  rdf:type owl:AnnotationProperty ;
  rdfs:comment ""@en ;
  rdfs:isDefinedBy <http://www.w3.org/ns/prov-o#> ;
.
rdfs:isDefinedBy
  rdf:type owl:AnnotationProperty ;
.
rdfs:label
  rdf:type owl:AnnotationProperty ;
  rdfs:comment ""@en ;
  rdfs:isDefinedBy <http://www.w3.org/ns/prov-o#> ;
.
rdfs:seeAlso
  rdf:type owl:AnnotationProperty ;
  rdfs:comment ""@en ;
.
<http://www.w3.org/2000/10/swap/pim/contact#Person>
  owl:equivalentClass schema:Person ;
  owl:equivalentClass toop:Person ;
  owl:equivalentClass foaf:Person ;
.
owl:Thing
  rdf:type owl:Class ;
  rdfs:label "Thing" ;
.
owl:versionInfo
  rdf:type owl:AnnotationProperty ;
.
wgs:SpatialThing
  rdf:type owl:Class ;
  rdfs:label "Spatial Thing" ;
  rdfs:subClassOf owl:Thing ;
.
vs:term_status
  rdf:type owl:AnnotationProperty ;
.
<http://www.w3.org/2004/02/skos/core>
  rdf:type elobr:EloniaBusinessCode ;
  rdf:type freebr:FreedoniaBusinessCode ;
  elobr:EloniaRegistrationAuthority "Alistair Miles" ;
  elobr:EloniaRegistrationAuthority "Sean Bechhofer" ;
  freebr:FreedoniaRegistrationAuthority "Alistair Miles" ;
  freebr:FreedoniaRegistrationAuthority "Sean Bechhofer" ;
  dc:contributor "Alistair Miles" ;
  dc:contributor "Dave Beckett" ;
  dc:contributor "Nikki Rogers" ;
  dc:contributor "Participants in W3C's Semantic Web Deployment Working Group." ;
  dc:contributor "Sean Bechhofer" ;
  dc:creator "Alistair Miles" ;
  dc:creator "Sean Bechhofer" ;
  dc:description "An RDF vocabulary for describing the basic structure and content of concept schemes such as thesauri, classification schemes, subject heading lists, taxonomies, 'folksonomies', other types of controlled vocabulary, and also concept schemes embedded in glossaries and terminologies."@en ;
  dc:title "SKOS Vocabulary"@en ;
  dcterms:contributor "Alistair Miles" ;
  dcterms:contributor "Dave Beckett" ;
  dcterms:contributor "Nikki Rogers" ;
  dcterms:contributor "Participants in W3C's Semantic Web Deployment Working Group." ;
  dcterms:contributor "Sean Bechhofer" ;
  dcterms:creator "Alistair Miles" ;
  dcterms:creator "Sean Bechhofer" ;
  dcterms:description "An RDF vocabulary for describing the basic structure and content of concept schemes such as thesauri, classification schemes, subject heading lists, taxonomies, 'folksonomies', other types of controlled vocabulary, and also concept schemes embedded in glossaries and terminologies."@en ;
  dcterms:title "SKOS Vocabulary"@en ;
  toop:registrationAuthority "Alistair Miles" ;
  toop:registrationAuthority "Sean Bechhofer" ;
  rdfs:label "SKOS Core RDF vocabulary" ;
  rdfs:seeAlso <http://www.w3.org/TR/skos-reference/> ;
  owl:versionInfo "Modified by TopQuadrant to assert three rdfs:subClassOf owl:Thing triples." ;
  foaf:maker "Alistair Miles" ;
  foaf:maker "Sean Bechhofer" ;
.
skos:Collection
  rdf:type owl:Class ;
  rdfs:isDefinedBy <http://www.w3.org/2004/02/skos/core> ;
  rdfs:label "Collection"@en ;
  rdfs:subClassOf owl:Thing ;
  owl:disjointWith skos:Concept ;
  owl:disjointWith skos:ConceptScheme ;
  skos:definition "A meaningful collection of concepts."@en ;
  skos:note "A meaningful collection of concepts."@en ;
  skos:note "Labelled collections can be used where you would like a set of concepts to be displayed under a 'node label' in the hierarchy."@en ;
  skos:scopeNote "Labelled collections can be used where you would like a set of concepts to be displayed under a 'node label' in the hierarchy."@en ;
.
skos:Concept
  rdf:type owl:Class ;
  rdfs:isDefinedBy <http://www.w3.org/2004/02/skos/core> ;
  rdfs:label "Concept" ;
  rdfs:label "Concept"@en ;
  rdfs:subClassOf owl:Thing ;
  skos:definition "An idea or notion; a unit of thought."@en ;
  skos:note "An idea or notion; a unit of thought."@en ;
.
skos:ConceptScheme
  rdf:type owl:Class ;
  rdfs:isDefinedBy <http://www.w3.org/2004/02/skos/core> ;
  rdfs:label "Concept Scheme"@en ;
  rdfs:subClassOf toop:CompanyTypeScheme ;
  rdfs:subClassOf owl:Thing ;
  owl:disjointWith skos:Concept ;
  owl:equivalentClass toop:CompanyTypeScheme ;
  skos:definition "A set of concepts, optionally including statements about semantic relationships between those concepts."@en ;
  skos:example "Thesauri, classification schemes, subject heading lists, taxonomies, 'folksonomies', and other types of controlled vocabulary are all examples of concept schemes. Concept schemes are also embedded in glossaries and terminologies."@en ;
  skos:note "A concept scheme may be defined to include concepts from different sources."@en ;
  skos:note "A set of concepts, optionally including statements about semantic relationships between those concepts."@en ;
  skos:note "Thesauri, classification schemes, subject heading lists, taxonomies, 'folksonomies', and other types of controlled vocabulary are all examples of concept schemes. Concept schemes are also embedded in glossaries and terminologies."@en ;
  skos:scopeNote "A concept scheme may be defined to include concepts from different sources."@en ;
.
skos:OrderedCollection
  rdf:type owl:Class ;
  rdfs:isDefinedBy <http://www.w3.org/2004/02/skos/core> ;
  rdfs:label "Ordered Collection"@en ;
  rdfs:subClassOf skos:Collection ;
  skos:definition "An ordered collection of concepts, where both the grouping and the ordering are meaningful."@en ;
  skos:note "An ordered collection of concepts, where both the grouping and the ordering are meaningful."@en ;
  skos:note "Ordered collections can be used where you would like a set of concepts to be displayed in a specific order, and optionally under a 'node label'."@en ;
  skos:scopeNote "Ordered collections can be used where you would like a set of concepts to be displayed in a specific order, and optionally under a 'node label'."@en ;
.
skos:altLabel
  rdf:type rdf:Property ;
  rdf:type owl:AnnotationProperty ;
  rdfs:comment "The range of skos:altLabel is the class of RDF plain literals."@en ;
  rdfs:comment "skos:prefLabel, skos:altLabel and skos:hiddenLabel are pairwise disjoint properties."@en ;
  rdfs:isDefinedBy <http://www.w3.org/2004/02/skos/core> ;
  rdfs:label "alternative label"@en ;
  rdfs:subPropertyOf rdfs:label ;
  skos:definition "An alternative lexical label for a resource."@en ;
  skos:example "Acronyms, abbreviations, spelling variants, and irregular plural/singular forms may be included among the alternative labels for a concept. Mis-spelled terms are normally included as hidden labels (see skos:hiddenLabel)."@en ;
  skos:note "Acronyms, abbreviations, spelling variants, and irregular plural/singular forms may be included among the alternative labels for a concept. Mis-spelled terms are normally included as hidden labels (see skos:hiddenLabel)."@en ;
  skos:note "An alternative lexical label for a resource."@en ;
.
skos:broadMatch
  rdf:type rdf:Property ;
  rdf:type owl:ObjectProperty ;
  rdfs:domain owl:Thing ;
  rdfs:domain skos:Concept ;
  rdfs:domain _:b327858 ;
  rdfs:isDefinedBy <http://www.w3.org/2004/02/skos/core> ;
  rdfs:label "has broader match"@en ;
  rdfs:range owl:Thing ;
  rdfs:range skos:Concept ;
  rdfs:range _:b327858 ;
  rdfs:subPropertyOf skos:broader ;
  rdfs:subPropertyOf skos:broaderTransitive ;
  rdfs:subPropertyOf skos:mappingRelation ;
  rdfs:subPropertyOf skos:semanticRelation ;
  owl:inverseOf skos:narrowMatch ;
  skos:definition "skos:broadMatch is used to state a hierarchical mapping link between two conceptual resources in different concept schemes."@en ;
  skos:note "skos:broadMatch is used to state a hierarchical mapping link between two conceptual resources in different concept schemes."@en ;
.
skos:broader
  rdf:type rdf:Property ;
  rdf:type owl:ObjectProperty ;
  rdfs:comment "Broader concepts are typically rendered as parents in a concept hierarchy (tree)."@en ;
  rdfs:domain owl:Thing ;
  rdfs:domain skos:Concept ;
  rdfs:domain _:b327858 ;
  rdfs:isDefinedBy <http://www.w3.org/2004/02/skos/core> ;
  rdfs:label "has broader"@en ;
  rdfs:range owl:Thing ;
  rdfs:range skos:Concept ;
  rdfs:range _:b327858 ;
  rdfs:subPropertyOf skos:broaderTransitive ;
  rdfs:subPropertyOf skos:semanticRelation ;
  owl:inverseOf skos:narrower ;
  skos:definition "Relates a concept to a concept that is more general in meaning."@en ;
  skos:note "By convention, skos:broader is only used to assert an immediate (i.e. direct) hierarchical link between two conceptual resources."@en ;
  skos:note "Relates a concept to a concept that is more general in meaning."@en ;
  skos:scopeNote "By convention, skos:broader is only used to assert an immediate (i.e. direct) hierarchical link between two conceptual resources."@en ;
.
skos:broaderTransitive
  rdf:type rdf:Property ;
  rdf:type owl:ObjectProperty ;
  rdf:type owl:TransitiveProperty ;
  rdfs:domain owl:Thing ;
  rdfs:domain skos:Concept ;
  rdfs:domain _:b327858 ;
  rdfs:isDefinedBy <http://www.w3.org/2004/02/skos/core> ;
  rdfs:label "has broader transitive"@en ;
  rdfs:range owl:Thing ;
  rdfs:range skos:Concept ;
  rdfs:range _:b327858 ;
  rdfs:subPropertyOf skos:semanticRelation ;
  owl:inverseOf skos:narrowerTransitive ;
  skos:definition "skos:broaderTransitive is a transitive superproperty of skos:broader." ;
  skos:note "By convention, skos:broaderTransitive is not used to make assertions. Rather, the properties can be used to draw inferences about the transitive closure of the hierarchical relation, which is useful e.g. when implementing a simple query expansion algorithm in a search application."@en ;
  skos:note "skos:broaderTransitive is a transitive superproperty of skos:broader." ;
  skos:scopeNote "By convention, skos:broaderTransitive is not used to make assertions. Rather, the properties can be used to draw inferences about the transitive closure of the hierarchical relation, which is useful e.g. when implementing a simple query expansion algorithm in a search application."@en ;
.
skos:changeNote
  rdf:type rdf:Property ;
  rdf:type owl:AnnotationProperty ;
  rdfs:isDefinedBy <http://www.w3.org/2004/02/skos/core> ;
  rdfs:label "change note"@en ;
  rdfs:subPropertyOf skos:note ;
  skos:definition "A note about a modification to a concept."@en ;
  skos:note "A note about a modification to a concept."@en ;
.
skos:closeMatch
  rdf:type rdf:Property ;
  rdf:type owl:ObjectProperty ;
  rdf:type owl:SymmetricProperty ;
  rdfs:domain owl:Thing ;
  rdfs:domain skos:Concept ;
  rdfs:domain _:b327858 ;
  rdfs:isDefinedBy <http://www.w3.org/2004/02/skos/core> ;
  rdfs:label "has close match"@en ;
  rdfs:range owl:Thing ;
  rdfs:range skos:Concept ;
  rdfs:range _:b327858 ;
  rdfs:subPropertyOf skos:mappingRelation ;
  rdfs:subPropertyOf skos:semanticRelation ;
  skos:definition "skos:closeMatch is used to link two concepts that are sufficiently similar that they can be used interchangeably in some information retrieval applications. In order to avoid the possibility of \"compound errors\" when combining mappings across more than two concept schemes, skos:closeMatch is not declared to be a transitive property."@en ;
  skos:note "skos:closeMatch is used to link two concepts that are sufficiently similar that they can be used interchangeably in some information retrieval applications. In order to avoid the possibility of \"compound errors\" when combining mappings across more than two concept schemes, skos:closeMatch is not declared to be a transitive property."@en ;
.
skos:definition
  rdf:type rdf:Property ;
  rdf:type owl:AnnotationProperty ;
  rdfs:isDefinedBy <http://www.w3.org/2004/02/skos/core> ;
  rdfs:label "definition"@en ;
  rdfs:subPropertyOf skos:note ;
  skos:definition "A statement or formal explanation of the meaning of a concept."@en ;
  skos:note "A statement or formal explanation of the meaning of a concept."@en ;
.
skos:editorialNote
  rdf:type rdf:Property ;
  rdf:type owl:AnnotationProperty ;
  rdfs:isDefinedBy <http://www.w3.org/2004/02/skos/core> ;
  rdfs:label "editorial note"@en ;
  rdfs:subPropertyOf skos:note ;
  skos:definition "A note for an editor, translator or maintainer of the vocabulary."@en ;
  skos:note "A note for an editor, translator or maintainer of the vocabulary."@en ;
.
skos:exactMatch
  rdf:type rdf:Property ;
  rdf:type owl:ObjectProperty ;
  rdf:type owl:SymmetricProperty ;
  rdf:type owl:TransitiveProperty ;
  rdfs:comment "skos:exactMatch is disjoint with each of the properties skos:broadMatch and skos:relatedMatch."@en ;
  rdfs:domain owl:Thing ;
  rdfs:domain skos:Concept ;
  rdfs:domain _:b327858 ;
  rdfs:isDefinedBy <http://www.w3.org/2004/02/skos/core> ;
  rdfs:label "has exact match"@en ;
  rdfs:range owl:Thing ;
  rdfs:range skos:Concept ;
  rdfs:range _:b327858 ;
  rdfs:subPropertyOf skos:closeMatch ;
  rdfs:subPropertyOf skos:mappingRelation ;
  rdfs:subPropertyOf skos:semanticRelation ;
  skos:definition "skos:exactMatch is used to link two concepts, indicating a high degree of confidence that the concepts can be used interchangeably across a wide range of information retrieval applications. skos:exactMatch is a transitive property, and is a sub-property of skos:closeMatch."@en ;
  skos:note "skos:exactMatch is used to link two concepts, indicating a high degree of confidence that the concepts can be used interchangeably across a wide range of information retrieval applications. skos:exactMatch is a transitive property, and is a sub-property of skos:closeMatch."@en ;
.
skos:example
  rdf:type rdf:Property ;
  rdf:type owl:AnnotationProperty ;
  rdfs:isDefinedBy <http://www.w3.org/2004/02/skos/core> ;
  rdfs:label "example"@en ;
  rdfs:subPropertyOf skos:note ;
  skos:definition "An example of the use of a concept."@en ;
  skos:note "An example of the use of a concept."@en ;
.
skos:hasTopConcept
  rdf:type rdf:Property ;
  rdf:type owl:ObjectProperty ;
  rdfs:domain toop:CompanyTypeScheme ;
  rdfs:domain owl:Thing ;
  rdfs:domain skos:ConceptScheme ;
  rdfs:isDefinedBy <http://www.w3.org/2004/02/skos/core> ;
  rdfs:label "has top concept"@en ;
  rdfs:range owl:Thing ;
  rdfs:range skos:Concept ;
  rdfs:range _:b327858 ;
  owl:inverseOf skos:topConceptOf ;
  skos:definition "Relates, by convention, a concept scheme to a concept which is topmost in the broader/narrower concept hierarchies for that scheme, providing an entry point to these hierarchies."@en ;
  skos:note "Relates, by convention, a concept scheme to a concept which is topmost in the broader/narrower concept hierarchies for that scheme, providing an entry point to these hierarchies."@en ;
.
skos:hiddenLabel
  rdf:type rdf:Property ;
  rdf:type owl:AnnotationProperty ;
  rdfs:comment "The range of skos:hiddenLabel is the class of RDF plain literals."@en ;
  rdfs:comment "skos:prefLabel, skos:altLabel and skos:hiddenLabel are pairwise disjoint properties."@en ;
  rdfs:isDefinedBy <http://www.w3.org/2004/02/skos/core> ;
  rdfs:label "hidden label"@en ;
  rdfs:subPropertyOf rdfs:label ;
  skos:definition "A lexical label for a resource that should be hidden when generating visual displays of the resource, but should still be accessible to free text search operations."@en ;
  skos:note "A lexical label for a resource that should be hidden when generating visual displays of the resource, but should still be accessible to free text search operations."@en ;
.
skos:historyNote
  rdf:type rdf:Property ;
  rdf:type owl:AnnotationProperty ;
  rdfs:isDefinedBy <http://www.w3.org/2004/02/skos/core> ;
  rdfs:label "history note"@en ;
  rdfs:subPropertyOf skos:note ;
  skos:definition "A note about the past state/use/meaning of a concept."@en ;
  skos:note "A note about the past state/use/meaning of a concept."@en ;
.
skos:inScheme
  rdf:type rdf:Property ;
  rdf:type owl:ObjectProperty ;
  rdfs:isDefinedBy <http://www.w3.org/2004/02/skos/core> ;
  rdfs:label "is in scheme"@en ;
  rdfs:range toop:CompanyTypeScheme ;
  rdfs:range owl:Thing ;
  rdfs:range skos:ConceptScheme ;
  skos:definition "Relates a resource (for example a concept) to a concept scheme in which it is included."@en ;
  skos:note "A concept may be a member of more than one concept scheme."@en ;
  skos:note "Relates a resource (for example a concept) to a concept scheme in which it is included."@en ;
  skos:scopeNote "A concept may be a member of more than one concept scheme."@en ;
.
skos:mappingRelation
  rdf:type rdf:Property ;
  rdf:type owl:ObjectProperty ;
  rdfs:comment "These concept mapping relations mirror semantic relations, and the data model defined below is similar (with the exception of skos:exactMatch) to the data model defined for semantic relations. A distinct vocabulary is provided for concept mapping relations, to provide a convenient way to differentiate links within a concept scheme from links between concept schemes. However, this pattern of usage is not a formal requirement of the SKOS data model, and relies on informal definitions of best practice."@en ;
  rdfs:domain owl:Thing ;
  rdfs:domain skos:Concept ;
  rdfs:domain _:b327858 ;
  rdfs:isDefinedBy <http://www.w3.org/2004/02/skos/core> ;
  rdfs:label "is in mapping relation with"@en ;
  rdfs:range owl:Thing ;
  rdfs:range skos:Concept ;
  rdfs:range _:b327858 ;
  rdfs:subPropertyOf skos:semanticRelation ;
  skos:definition "Relates two concepts coming, by convention, from different schemes, and that have comparable meanings"@en ;
  skos:note "Relates two concepts coming, by convention, from different schemes, and that have comparable meanings"@en ;
.
skos:member
  rdf:type rdf:Property ;
  rdf:type owl:ObjectProperty ;
  rdfs:domain owl:Thing ;
  rdfs:domain skos:Collection ;
  rdfs:domain _:b327858 ;
  rdfs:isDefinedBy <http://www.w3.org/2004/02/skos/core> ;
  rdfs:label "has member"@en ;
  rdfs:range owl:Thing ;
  rdfs:range _:b327858 ;
  skos:definition "Relates a collection to one of its members."@en ;
  skos:note "Relates a collection to one of its members."@en ;
.
skos:memberList
  rdf:type rdf:Property ;
  rdf:type owl:FunctionalProperty ;
  rdf:type owl:ObjectProperty ;
  rdfs:comment """For any resource, every item in the list given as the value of the
      skos:memberList property is also a value of the skos:member property."""@en ;
  rdfs:domain owl:Thing ;
  rdfs:domain skos:Collection ;
  rdfs:domain skos:OrderedCollection ;
  rdfs:domain _:b327858 ;
  rdfs:isDefinedBy <http://www.w3.org/2004/02/skos/core> ;
  rdfs:label "has member list"@en ;
  rdfs:range rdf:List ;
  skos:definition "Relates an ordered collection to the RDF list containing its members."@en ;
  skos:note "Relates an ordered collection to the RDF list containing its members."@en ;
.
skos:narrowMatch
  rdf:type rdf:Property ;
  rdf:type owl:ObjectProperty ;
  rdfs:domain owl:Thing ;
  rdfs:domain skos:Concept ;
  rdfs:domain _:b327858 ;
  rdfs:isDefinedBy <http://www.w3.org/2004/02/skos/core> ;
  rdfs:label "has narrower match"@en ;
  rdfs:range owl:Thing ;
  rdfs:range skos:Concept ;
  rdfs:range _:b327858 ;
  rdfs:subPropertyOf skos:mappingRelation ;
  rdfs:subPropertyOf skos:narrower ;
  rdfs:subPropertyOf skos:narrowerTransitive ;
  rdfs:subPropertyOf skos:semanticRelation ;
  owl:inverseOf skos:broadMatch ;
  skos:definition "skos:narrowMatch is used to state a hierarchical mapping link between two conceptual resources in different concept schemes."@en ;
  skos:note "skos:narrowMatch is used to state a hierarchical mapping link between two conceptual resources in different concept schemes."@en ;
.
skos:narrower
  rdf:type rdf:Property ;
  rdf:type owl:ObjectProperty ;
  rdfs:comment "Narrower concepts are typically rendered as children in a concept hierarchy (tree)."@en ;
  rdfs:domain owl:Thing ;
  rdfs:domain skos:Concept ;
  rdfs:domain _:b327858 ;
  rdfs:isDefinedBy <http://www.w3.org/2004/02/skos/core> ;
  rdfs:label "has narrower"@en ;
  rdfs:range owl:Thing ;
  rdfs:range skos:Concept ;
  rdfs:range _:b327858 ;
  rdfs:subPropertyOf skos:narrowerTransitive ;
  rdfs:subPropertyOf skos:semanticRelation ;
  owl:inverseOf skos:broader ;
  skos:definition "Relates a concept to a concept that is more specific in meaning."@en ;
  skos:note "By convention, skos:broader is only used to assert an immediate (i.e. direct) hierarchical link between two conceptual resources."@en ;
  skos:note "Relates a concept to a concept that is more specific in meaning."@en ;
  skos:scopeNote "By convention, skos:broader is only used to assert an immediate (i.e. direct) hierarchical link between two conceptual resources."@en ;
.
skos:narrowerTransitive
  rdf:type rdf:Property ;
  rdf:type owl:ObjectProperty ;
  rdf:type owl:TransitiveProperty ;
  rdfs:domain owl:Thing ;
  rdfs:domain skos:Concept ;
  rdfs:domain _:b327858 ;
  rdfs:isDefinedBy <http://www.w3.org/2004/02/skos/core> ;
  rdfs:label "has narrower transitive"@en ;
  rdfs:range owl:Thing ;
  rdfs:range skos:Concept ;
  rdfs:range _:b327858 ;
  rdfs:subPropertyOf skos:semanticRelation ;
  owl:inverseOf skos:broaderTransitive ;
  skos:definition "skos:narrowerTransitive is a transitive superproperty of skos:narrower." ;
  skos:note "By convention, skos:narrowerTransitive is not used to make assertions. Rather, the properties can be used to draw inferences about the transitive closure of the hierarchical relation, which is useful e.g. when implementing a simple query expansion algorithm in a search application."@en ;
  skos:note "skos:narrowerTransitive is a transitive superproperty of skos:narrower." ;
  skos:scopeNote "By convention, skos:narrowerTransitive is not used to make assertions. Rather, the properties can be used to draw inferences about the transitive closure of the hierarchical relation, which is useful e.g. when implementing a simple query expansion algorithm in a search application."@en ;
.
skos:notation
  rdf:type rdf:Property ;
  rdf:type owl:DatatypeProperty ;
  rdfs:isDefinedBy <http://www.w3.org/2004/02/skos/core> ;
  rdfs:label "notation"@en ;
  skos:definition "A notation, also known as classification code, is a string of characters such as \"T58.5\" or \"303.4833\" used to uniquely identify a concept within the scope of a given concept scheme."@en ;
  skos:note "A notation, also known as classification code, is a string of characters such as \"T58.5\" or \"303.4833\" used to uniquely identify a concept within the scope of a given concept scheme."@en ;
  skos:note "By convention, skos:notation is used with a typed literal in the object position of the triple."@en ;
  skos:scopeNote "By convention, skos:notation is used with a typed literal in the object position of the triple."@en ;
.
skos:note
  rdf:type rdf:Property ;
  rdf:type owl:AnnotationProperty ;
  rdfs:isDefinedBy <http://www.w3.org/2004/02/skos/core> ;
  rdfs:label "note"@en ;
  skos:definition "A general note, for any purpose."@en ;
  skos:note "A general note, for any purpose."@en ;
  skos:note "This property may be used directly, or as a super-property for more specific note types."@en ;
  skos:scopeNote "This property may be used directly, or as a super-property for more specific note types."@en ;
.
skos:prefLabel
  rdf:type rdf:Property ;
  rdf:type owl:AnnotationProperty ;
  rdfs:comment "A resource has no more than one value of skos:prefLabel per language tag."@en ;
  rdfs:comment "The range of skos:prefLabel is the class of RDF plain literals."@en ;
  rdfs:comment """skos:prefLabel, skos:altLabel and skos:hiddenLabel are pairwise
      disjoint properties."""@en ;
  rdfs:isDefinedBy <http://www.w3.org/2004/02/skos/core> ;
  rdfs:label "preferred label"@en ;
  rdfs:subPropertyOf rdfs:label ;
  skos:definition "The preferred lexical label for a resource, in a given language."@en ;
  skos:note "The preferred lexical label for a resource, in a given language."@en ;
.
skos:related
  rdf:type rdf:Property ;
  rdf:type owl:ObjectProperty ;
  rdf:type owl:SymmetricProperty ;
  rdfs:comment "skos:related is disjoint with skos:broaderTransitive"@en ;
  rdfs:domain owl:Thing ;
  rdfs:domain skos:Concept ;
  rdfs:domain _:b327858 ;
  rdfs:isDefinedBy <http://www.w3.org/2004/02/skos/core> ;
  rdfs:label "has related"@en ;
  rdfs:range owl:Thing ;
  rdfs:range skos:Concept ;
  rdfs:range _:b327858 ;
  rdfs:subPropertyOf skos:semanticRelation ;
  skos:definition "Relates a concept to a concept with which there is an associative semantic relationship."@en ;
  skos:note "Relates a concept to a concept with which there is an associative semantic relationship."@en ;
.
skos:relatedMatch
  rdf:type rdf:Property ;
  rdf:type owl:ObjectProperty ;
  rdf:type owl:SymmetricProperty ;
  rdfs:domain owl:Thing ;
  rdfs:domain skos:Concept ;
  rdfs:domain _:b327858 ;
  rdfs:isDefinedBy <http://www.w3.org/2004/02/skos/core> ;
  rdfs:label "has related match"@en ;
  rdfs:range owl:Thing ;
  rdfs:range skos:Concept ;
  rdfs:range _:b327858 ;
  rdfs:subPropertyOf skos:mappingRelation ;
  rdfs:subPropertyOf skos:related ;
  rdfs:subPropertyOf skos:semanticRelation ;
  skos:definition "skos:relatedMatch is used to state an associative mapping link between two conceptual resources in different concept schemes."@en ;
  skos:note "skos:relatedMatch is used to state an associative mapping link between two conceptual resources in different concept schemes."@en ;
.
skos:scopeNote
  rdf:type rdf:Property ;
  rdf:type owl:AnnotationProperty ;
  rdfs:isDefinedBy <http://www.w3.org/2004/02/skos/core> ;
  rdfs:label "scope note"@en ;
  rdfs:subPropertyOf skos:note ;
  skos:definition "A note that helps to clarify the meaning and/or the use of a concept."@en ;
  skos:note "A note that helps to clarify the meaning and/or the use of a concept."@en ;
.
skos:semanticRelation
  rdf:type rdf:Property ;
  rdf:type owl:ObjectProperty ;
  rdfs:domain owl:Thing ;
  rdfs:domain skos:Concept ;
  rdfs:domain _:b327858 ;
  rdfs:isDefinedBy <http://www.w3.org/2004/02/skos/core> ;
  rdfs:label "is in semantic relation with"@en ;
  rdfs:range owl:Thing ;
  rdfs:range skos:Concept ;
  rdfs:range _:b327858 ;
  skos:definition "Links a concept to a concept related by meaning."@en ;
  skos:note "Links a concept to a concept related by meaning."@en ;
  skos:note "This property should not be used directly, but as a super-property for all properties denoting a relationship of meaning between concepts."@en ;
  skos:scopeNote "This property should not be used directly, but as a super-property for all properties denoting a relationship of meaning between concepts."@en ;
.
skos:topConceptOf
  rdf:type rdf:Property ;
  rdf:type owl:ObjectProperty ;
  rdfs:domain owl:Thing ;
  rdfs:domain skos:Concept ;
  rdfs:domain _:b327858 ;
  rdfs:isDefinedBy <http://www.w3.org/2004/02/skos/core> ;
  rdfs:label "is top concept in scheme"@en ;
  rdfs:range toop:CompanyTypeScheme ;
  rdfs:range owl:Thing ;
  rdfs:range skos:ConceptScheme ;
  rdfs:subPropertyOf skos:inScheme ;
  owl:inverseOf skos:hasTopConcept ;
  skos:definition "Relates a concept to the concept scheme that it is a top level concept of."@en ;
  skos:note "Relates a concept to the concept scheme that it is a top level concept of."@en ;
.
<http://www.w3.org/2006/vcard/ns>
  dc:creator "Brian Suda" ;
  dc:creator "Harry Halpin" ;
  dc:creator "Norman Walsh" ;
  dc:creator "Renato Iannella" ;
  dc:date "2010-01-20" ;
  dc:description "This ontology models and represents vCards in RDF using current best practices." ;
  dc:title "An Ontology for vCards" ;
  rdfs:comment "Ontology for vCard based on RFC6350"@en ;
  rdfs:label "Ontology for vCard"@en ;
  rdfs:seeAlso "http://tools.ietf.org/html/rfc2426" ;
  rdfs:seeAlso "http://www.w3.org/Submission/vcard-rdf/" ;
  owl:versionInfo "Final"@en ;
.
vcard:Acquaintance
  rdf:type owl:Class ;
  rdfs:isDefinedBy <http://www.w3.org/2006/vcard/ns> ;
  rdfs:label "Acquaintance"@en ;
  rdfs:subClassOf vcard:RelatedType ;
.
vcard:Address
  rdf:type owl:Class ;
  rdfs:comment "Resources that are vCard Addresses" ;
  rdfs:comment "To specify the components of the delivery address for the  object"@en ;
  rdfs:isDefinedBy <http://www.w3.org/2006/vcard/ns> ;
  rdfs:label "Address"@en ;
  rdfs:label "vCard Address Class" ;
  rdfs:subClassOf owl:Thing ;
  rdfs:subClassOf _:b157701 ;
  rdfs:subClassOf _:b168676 ;
  rdfs:subClassOf _:b396249 ;
  rdfs:subClassOf _:b499218 ;
  rdfs:subClassOf _:b726818 ;
  rdfs:subClassOf _:b787338 ;
  rdfs:subClassOf _:b926654 ;
  owl:disjointWith vcard:Email ;
  owl:disjointWith vcard:Label ;
  owl:disjointWith vcard:Tel ;
  owl:equivalentClass elobr:EloniaAddress ;
  owl:equivalentClass freebr:FreedoniaAddress ;
  owl:equivalentClass toop:Address ;
  owl:equivalentClass _:b49042 ;
.
vcard:Agent
  rdf:type owl:Class ;
  rdfs:isDefinedBy <http://www.w3.org/2006/vcard/ns> ;
  rdfs:label "Agent"@en ;
  rdfs:subClassOf vcard:RelatedType ;
.
vcard:BBS
  rdf:type owl:Class ;
  rdfs:comment "Bulletin Board System Communications" ;
  rdfs:comment "This class is deprecated"@en ;
  rdfs:isDefinedBy <http://www.w3.org/2006/vcard/ns> ;
  rdfs:label "BBS"@en ;
  rdfs:label "Bulletin Board System" ;
  rdfs:subClassOf vcard:Tel ;
  rdfs:subClassOf vcard:TelephoneType ;
  owl:deprecated "true"^^xsd:boolean ;
.
vcard:Car
  rdf:type owl:Class ;
  rdfs:comment "Car Telephone" ;
  rdfs:comment "This class is deprecated"@en ;
  rdfs:isDefinedBy <http://www.w3.org/2006/vcard/ns> ;
  rdfs:label "Car Phone" ;
  rdfs:label "Car"@en ;
  rdfs:subClassOf vcard:Tel ;
  rdfs:subClassOf vcard:TelephoneType ;
  owl:deprecated "true"^^xsd:boolean ;
.
vcard:Cell
  rdf:type owl:Class ;
  rdfs:comment "Also called mobile telephone"@en ;
  rdfs:comment "Cellular or Mobile Telephone" ;
  rdfs:isDefinedBy <http://www.w3.org/2006/vcard/ns> ;
  rdfs:label "Cell"@en ;
  rdfs:label "Cellular Telephone" ;
  rdfs:subClassOf vcard:Tel ;
  rdfs:subClassOf vcard:TelephoneType ;
.
vcard:Child
  rdf:type owl:Class ;
  rdfs:isDefinedBy <http://www.w3.org/2006/vcard/ns> ;
  rdfs:label "Child"@en ;
  rdfs:subClassOf vcard:RelatedType ;
.
vcard:Colleague
  rdf:type owl:Class ;
  rdfs:isDefinedBy <http://www.w3.org/2006/vcard/ns> ;
  rdfs:label "Colleague"@en ;
  rdfs:subClassOf vcard:RelatedType ;
.
vcard:Contact
  rdf:type owl:Class ;
  rdfs:isDefinedBy <http://www.w3.org/2006/vcard/ns> ;
  rdfs:label "Contact"@en ;
  rdfs:subClassOf vcard:RelatedType ;
.
vcard:Coresident
  rdf:type owl:Class ;
  rdfs:isDefinedBy <http://www.w3.org/2006/vcard/ns> ;
  rdfs:label "Coresident"@en ;
  rdfs:subClassOf vcard:RelatedType ;
.
vcard:Coworker
  rdf:type owl:Class ;
  rdfs:isDefinedBy <http://www.w3.org/2006/vcard/ns> ;
  rdfs:label "Coworker"@en ;
  rdfs:subClassOf vcard:RelatedType ;
.
vcard:Crush
  rdf:type owl:Class ;
  rdfs:isDefinedBy <http://www.w3.org/2006/vcard/ns> ;
  rdfs:label "Crush"@en ;
  rdfs:subClassOf vcard:RelatedType ;
.
vcard:Date
  rdf:type owl:Class ;
  rdfs:isDefinedBy <http://www.w3.org/2006/vcard/ns> ;
  rdfs:label "Date"@en ;
  rdfs:subClassOf vcard:RelatedType ;
.
vcard:Dom
  rdf:type owl:Class ;
  rdfs:comment "Information related to a Domestic Address or Label" ;
  rdfs:comment "This class is deprecated"@en ;
  rdfs:isDefinedBy <http://www.w3.org/2006/vcard/ns> ;
  rdfs:label "Dom"@en ;
  rdfs:label "Domestic" ;
  rdfs:subClassOf vcard:Type ;
  rdfs:subClassOf _:b401324 ;
  owl:deprecated "true"^^xsd:boolean ;
.
vcard:Email
  rdf:type owl:Class ;
  rdfs:comment "Resources that are vCard Email Addresses" ;
  rdfs:comment "To specify the electronic mail address for communication with the object the vCard represents. Use the hasEmail object property."@en ;
  rdfs:isDefinedBy <http://www.w3.org/2006/vcard/ns> ;
  rdfs:label "Email" ;
  rdfs:label "Email"@en ;
  rdfs:subClassOf owl:Thing ;
  owl:deprecated "true"^^xsd:boolean ;
  owl:disjointWith vcard:Label ;
  owl:disjointWith vcard:Tel ;
.
vcard:Emergency
  rdf:type owl:Class ;
  rdfs:isDefinedBy <http://www.w3.org/2006/vcard/ns> ;
  rdfs:label "Emergency"@en ;
  rdfs:subClassOf vcard:RelatedType ;
.
vcard:Fax
  rdf:type owl:Class ;
  rdfs:comment "Fax Communications" ;
  rdfs:isDefinedBy <http://www.w3.org/2006/vcard/ns> ;
  rdfs:label "Fax" ;
  rdfs:label "Fax"@en ;
  rdfs:subClassOf vcard:Tel ;
  rdfs:subClassOf vcard:TelephoneType ;
.
vcard:Female
  rdf:type owl:Class ;
  rdfs:isDefinedBy <http://www.w3.org/2006/vcard/ns> ;
  rdfs:label "Female"@en ;
  rdfs:subClassOf vcard:Gender ;
.
vcard:Friend
  rdf:type owl:Class ;
  rdfs:isDefinedBy <http://www.w3.org/2006/vcard/ns> ;
  rdfs:label "Friend"@en ;
  rdfs:subClassOf vcard:RelatedType ;
.
vcard:Gender
  rdf:type owl:Class ;
  rdfs:comment "Used for gender codes. The URI of the gender code must be used as the value for Gender."@en ;
  rdfs:isDefinedBy <http://www.w3.org/2006/vcard/ns> ;
  rdfs:label "Gender"@en ;
  rdfs:subClassOf owl:Thing ;
.
vcard:Group
  rdf:type owl:Class ;
  rdfs:comment "Object representing a group of persons or entities.  A group object will usually contain hasMember properties to specify the members of the group."@en ;
  rdfs:isDefinedBy <http://www.w3.org/2006/vcard/ns> ;
  rdfs:label "Group"@en ;
  rdfs:subClassOf vcard:Kind ;
  owl:disjointWith vcard:Individual ;
  owl:disjointWith vcard:Location ;
  owl:disjointWith vcard:Organization ;
  owl:equivalentClass _:b789349 ;
.
vcard:Home
  rdf:type owl:Class ;
  rdfs:comment "Information related to a Home Address, Label, or Telephone" ;
  rdfs:comment "This implies that the property is related to an individual's personal life"@en ;
  rdfs:isDefinedBy <http://www.w3.org/2006/vcard/ns> ;
  rdfs:label "Home" ;
  rdfs:label "Home"@en ;
  rdfs:subClassOf vcard:Type ;
  rdfs:subClassOf _:b763315 ;
.
vcard:ISDN
  rdf:type owl:Class ;
  rdfs:comment "ISDN Communications" ;
  rdfs:comment "This class is deprecated"@en ;
  rdfs:isDefinedBy <http://www.w3.org/2006/vcard/ns> ;
  rdfs:label "ISDN" ;
  rdfs:label "ISDN"@en ;
  rdfs:subClassOf vcard:Tel ;
  rdfs:subClassOf vcard:Type ;
  owl:deprecated "true"^^xsd:boolean ;
.
vcard:Individual
  rdf:type owl:Class ;
  rdfs:comment "An object representing a single person or entity"@en ;
  rdfs:isDefinedBy <http://www.w3.org/2006/vcard/ns> ;
  rdfs:label "Individual"@en ;
  rdfs:subClassOf vcard:Kind ;
  owl:disjointWith vcard:Location ;
  owl:disjointWith vcard:Organization ;
.
vcard:Internet
  rdf:type owl:Class ;
  rdfs:comment "Internet Email" ;
  rdfs:comment "This class is deprecated"@en ;
  rdfs:isDefinedBy <http://www.w3.org/2006/vcard/ns> ;
  rdfs:label "Internet" ;
  rdfs:label "Internet"@en ;
  rdfs:subClassOf vcard:Email ;
  rdfs:subClassOf vcard:Type ;
  owl:deprecated "true"^^xsd:boolean ;
.
vcard:Intl
  rdf:type owl:Class ;
  rdfs:comment "Information related to an International Address or Label" ;
  rdfs:comment "This class is deprecated"@en ;
  rdfs:isDefinedBy <http://www.w3.org/2006/vcard/ns> ;
  rdfs:label "International" ;
  rdfs:label "Intl"@en ;
  rdfs:subClassOf vcard:Type ;
  rdfs:subClassOf _:b83024 ;
  owl:deprecated "true"^^xsd:boolean ;
.
vcard:Kin
  rdf:type owl:Class ;
  rdfs:isDefinedBy <http://www.w3.org/2006/vcard/ns> ;
  rdfs:label "Kin"@en ;
  rdfs:subClassOf vcard:RelatedType ;
.
vcard:Kind
  rdf:type owl:Class ;
  rdfs:comment "The parent class for all objects"@en ;
  rdfs:isDefinedBy <http://www.w3.org/2006/vcard/ns> ;
  rdfs:label "Kind"@en ;
  rdfs:subClassOf owl:Thing ;
  rdfs:subClassOf vcard:VCard ;
  owl:equivalentClass vcard:VCard ;
  owl:equivalentClass _:b57053 ;
.
vcard:Label
  rdf:type owl:Class ;
  rdfs:comment "Resources that are vCard Labels" ;
  rdfs:comment "This class is deprecated"@en ;
  rdfs:isDefinedBy <http://www.w3.org/2006/vcard/ns> ;
  rdfs:label "Label" ;
  rdfs:label "Label"@en ;
  rdfs:subClassOf vcard:Type ;
  owl:deprecated "true"^^xsd:boolean ;
  owl:disjointWith vcard:Tel ;
.
vcard:Location
  rdf:type owl:Class ;
  rdfs:comment "An object representing a named geographical place"@en ;
  rdfs:comment "Resources that are vCard geographic locations" ;
  rdfs:isDefinedBy <http://www.w3.org/2006/vcard/ns> ;
  rdfs:label "Location"@en ;
  rdfs:label "vCard Geographic Location Class" ;
  rdfs:subClassOf vcard:Kind ;
  rdfs:subClassOf _:b313826 ;
  rdfs:subClassOf _:b405470 ;
  owl:disjointWith vcard:Organization ;
.
vcard:Male
  rdf:type owl:Class ;
  rdfs:isDefinedBy <http://www.w3.org/2006/vcard/ns> ;
  rdfs:label "Male"@en ;
  rdfs:subClassOf vcard:Gender ;
.
vcard:Me
  rdf:type owl:Class ;
  rdfs:isDefinedBy <http://www.w3.org/2006/vcard/ns> ;
  rdfs:label "Me"@en ;
  rdfs:subClassOf vcard:RelatedType ;
.
vcard:Met
  rdf:type owl:Class ;
  rdfs:isDefinedBy <http://www.w3.org/2006/vcard/ns> ;
  rdfs:label "Met"@en ;
  rdfs:subClassOf vcard:RelatedType ;
.
vcard:Modem
  rdf:type owl:Class ;
  rdfs:comment "Modem Communications" ;
  rdfs:comment "This class is deprecated"@en ;
  rdfs:isDefinedBy <http://www.w3.org/2006/vcard/ns> ;
  rdfs:label "Modem" ;
  rdfs:label "Modem"@en ;
  rdfs:subClassOf vcard:Tel ;
  rdfs:subClassOf vcard:TelephoneType ;
  owl:deprecated "true"^^xsd:boolean ;
.
vcard:Msg
  rdf:type owl:Class ;
  rdfs:comment "This class is deprecated"@en ;
  rdfs:comment "Voice Message Communications" ;
  rdfs:isDefinedBy <http://www.w3.org/2006/vcard/ns> ;
  rdfs:label "Msg"@en ;
  rdfs:label "Voice Messenger" ;
  rdfs:subClassOf vcard:Tel ;
  rdfs:subClassOf vcard:TelephoneType ;
  owl:deprecated "true"^^xsd:boolean ;
.
vcard:Muse
  rdf:type owl:Class ;
  rdfs:isDefinedBy <http://www.w3.org/2006/vcard/ns> ;
  rdfs:label "Muse"@en ;
  rdfs:subClassOf vcard:RelatedType ;
.
vcard:Name
  rdf:type owl:Class ;
  rdfs:comment "Resources that are vCard personal names" ;
  rdfs:comment "To specify the components of the name of the object"@en ;
  rdfs:isDefinedBy <http://www.w3.org/2006/vcard/ns> ;
  rdfs:label "Name"@en ;
  rdfs:label "vCard Name Class" ;
  rdfs:subClassOf owl:Thing ;
  rdfs:subClassOf _:b218915 ;
  rdfs:subClassOf _:b269191 ;
  rdfs:subClassOf _:b623638 ;
  rdfs:subClassOf _:b671776 ;
  rdfs:subClassOf _:b794039 ;
  owl:equivalentClass _:b568769 ;
.
vcard:Neighbor
  rdf:type owl:Class ;
  rdfs:isDefinedBy <http://www.w3.org/2006/vcard/ns> ;
  rdfs:label "Neighbor"@en ;
  rdfs:subClassOf vcard:RelatedType ;
.
vcard:None
  rdf:type owl:Class ;
  rdfs:isDefinedBy <http://www.w3.org/2006/vcard/ns> ;
  rdfs:label "None"@en ;
  rdfs:subClassOf vcard:Gender ;
.
vcard:Organization
  rdf:type owl:Class ;
  rdfs:comment """An object representing an organization.  An organization is a single entity, and might represent a business or government, a department or division within a business or government, a club, an association, or the like.
"""@en ;
  rdfs:comment "Resources that are vCard organizations" ;
  rdfs:isDefinedBy <http://www.w3.org/2006/vcard/ns> ;
  rdfs:label "Organization"@en ;
  rdfs:label "vCard Organization Class" ;
  rdfs:subClassOf vcard:Kind ;
  rdfs:subClassOf _:b757317 ;
  rdfs:subClassOf _:b938985 ;
.
vcard:Other
  rdf:type owl:Class ;
  rdfs:isDefinedBy <http://www.w3.org/2006/vcard/ns> ;
  rdfs:label "Other"@en ;
  rdfs:subClassOf vcard:Gender ;
.
vcard:PCS
  rdf:type owl:Class ;
  rdfs:comment "Personal Communications Service" ;
  rdfs:comment "This class is deprecated"@en ;
  rdfs:isDefinedBy <http://www.w3.org/2006/vcard/ns> ;
  rdfs:label "PCS"@en ;
  rdfs:label "Personal Communications Service" ;
  rdfs:subClassOf vcard:Tel ;
  rdfs:subClassOf vcard:TelephoneType ;
  owl:deprecated "true"^^xsd:boolean ;
.
vcard:Pager
  rdf:type owl:Class ;
  rdfs:comment "Pager Communications" ;
  rdfs:isDefinedBy <http://www.w3.org/2006/vcard/ns> ;
  rdfs:label "Pager Device" ;
  rdfs:label "Pager"@en ;
  rdfs:subClassOf vcard:Tel ;
  rdfs:subClassOf vcard:TelephoneType ;
.
vcard:Parcel
  rdf:type owl:Class ;
  rdfs:comment "Information related to a Parcel Address or Label" ;
  rdfs:comment "This class is deprecated"@en ;
  rdfs:isDefinedBy <http://www.w3.org/2006/vcard/ns> ;
  rdfs:label "Parcel" ;
  rdfs:label "Parcel"@en ;
  rdfs:subClassOf vcard:Type ;
  rdfs:subClassOf _:b541374 ;
  owl:deprecated "true"^^xsd:boolean ;
.
vcard:Parent
  rdf:type owl:Class ;
  rdfs:isDefinedBy <http://www.w3.org/2006/vcard/ns> ;
  rdfs:label "Parent"@en ;
  rdfs:subClassOf vcard:RelatedType ;
.
vcard:Postal
  rdf:type owl:Class ;
  rdfs:comment "Information related to a Postal Address or Label" ;
  rdfs:comment "This class is deprecated"@en ;
  rdfs:isDefinedBy <http://www.w3.org/2006/vcard/ns> ;
  rdfs:label "Postal" ;
  rdfs:label "Postal"@en ;
  rdfs:subClassOf vcard:Type ;
  rdfs:subClassOf _:b955705 ;
  owl:deprecated "true"^^xsd:boolean ;
.
vcard:Pref
  rdf:type owl:Class ;
  rdfs:comment "Information related to a Preferred Address, Email, Label, or Telephone" ;
  rdfs:comment "This class is deprecated"@en ;
  rdfs:isDefinedBy <http://www.w3.org/2006/vcard/ns> ;
  rdfs:label "Pref"@en ;
  rdfs:label "Preferred" ;
  rdfs:subClassOf vcard:Type ;
  rdfs:subClassOf _:b583853 ;
  owl:deprecated "true"^^xsd:boolean ;
.
vcard:RelatedType
  rdf:type owl:Class ;
  rdfs:comment "Used for relation type codes. The URI of the relation type code must be used as the value for the Relation Type."@en ;
  rdfs:isDefinedBy <http://www.w3.org/2006/vcard/ns> ;
  rdfs:label "Relation Type"@en ;
  rdfs:subClassOf owl:Thing ;
.
vcard:Sibling
  rdf:type owl:Class ;
  rdfs:isDefinedBy <http://www.w3.org/2006/vcard/ns> ;
  rdfs:label "Sibling"@en ;
  rdfs:subClassOf vcard:RelatedType ;
.
vcard:Spouse
  rdf:type owl:Class ;
  rdfs:isDefinedBy <http://www.w3.org/2006/vcard/ns> ;
  rdfs:label "Spouse"@en ;
  rdfs:subClassOf vcard:RelatedType ;
.
vcard:Sweetheart
  rdf:type owl:Class ;
  rdfs:isDefinedBy <http://www.w3.org/2006/vcard/ns> ;
  rdfs:label "Sweetheart"@en ;
  rdfs:subClassOf vcard:RelatedType ;
.
vcard:Tel
  rdf:type owl:Class ;
  rdfs:comment "Resources that are vCard Telephony communication mechanisms" ;
  rdfs:comment "Telephone" ;
  rdfs:comment "This class is deprecated. Use the hasTelephone object property."@en ;
  rdfs:isDefinedBy <http://www.w3.org/2006/vcard/ns> ;
  rdfs:label "Tel"@en ;
  rdfs:subClassOf owl:Thing ;
  owl:deprecated "true"^^xsd:boolean ;
.
vcard:TelephoneType
  rdf:type owl:Class ;
  rdfs:comment "Used for telephone type codes. The URI of the telephone type code must be used as the value for the Telephone Type."@en ;
  rdfs:isDefinedBy <http://www.w3.org/2006/vcard/ns> ;
  rdfs:label "Phone"@en ;
  rdfs:subClassOf owl:Thing ;
.
vcard:Text
  rdf:type owl:Class ;
  rdfs:comment "Also called sms telephone"@en ;
  rdfs:isDefinedBy <http://www.w3.org/2006/vcard/ns> ;
  rdfs:label "Text"@en ;
  rdfs:subClassOf vcard:TelephoneType ;
.
vcard:TextPhone
  rdf:type owl:Class ;
  rdfs:isDefinedBy <http://www.w3.org/2006/vcard/ns> ;
  rdfs:label "Text phone"@en ;
  rdfs:subClassOf vcard:TelephoneType ;
.
vcard:Type
  rdf:type owl:Class ;
  rdfs:comment "Used for type codes. The URI of the type code must be used as the value for Type."@en ;
  rdfs:isDefinedBy <http://www.w3.org/2006/vcard/ns> ;
  rdfs:label "Type"@en ;
  rdfs:subClassOf owl:Thing ;
.
vcard:Unknown
  rdf:type owl:Class ;
  rdfs:isDefinedBy <http://www.w3.org/2006/vcard/ns> ;
  rdfs:label "Unknown"@en ;
  rdfs:subClassOf vcard:Gender ;
.
vcard:VCard
  rdf:type owl:Class ;
  rdfs:comment "Resources that are vCards and the URIs that denote these vCards can also be the same URIs that denote people/orgs" ;
  rdfs:comment "The vCard class is  equivalent to the new Kind class, which is the parent for the four explicit types of vCards (Individual, Organization, Location, Group)"@en ;
  rdfs:isDefinedBy <http://www.w3.org/2006/vcard/ns> ;
  rdfs:label "VCard"@en ;
  rdfs:label "vCard Class" ;
  rdfs:subClassOf vcard:Kind ;
  owl:equivalentClass vcard:Kind ;
  owl:equivalentClass _:b57053 ;
.
vcard:Video
  rdf:type owl:Class ;
  rdfs:comment "Video Communications" ;
  rdfs:isDefinedBy <http://www.w3.org/2006/vcard/ns> ;
  rdfs:label "Video" ;
  rdfs:label "Video"@en ;
  rdfs:subClassOf vcard:Tel ;
  rdfs:subClassOf vcard:TelephoneType ;
.
vcard:Voice
  rdf:type owl:Class ;
  rdfs:comment "Voice Communications" ;
  rdfs:isDefinedBy <http://www.w3.org/2006/vcard/ns> ;
  rdfs:label "Voice" ;
  rdfs:label "Voice"@en ;
  rdfs:subClassOf vcard:Tel ;
  rdfs:subClassOf vcard:TelephoneType ;
.
vcard:Work
  rdf:type owl:Class ;
  rdfs:comment "Information related to a Work Address, Label, or Telephone" ;
  rdfs:comment "This implies that the property is related to an individual's work place"@en ;
  rdfs:isDefinedBy <http://www.w3.org/2006/vcard/ns> ;
  rdfs:label "Work" ;
  rdfs:label "Work"@en ;
  rdfs:subClassOf vcard:Type ;
  rdfs:subClassOf _:b652026 ;
.
vcard:X400
  rdf:type owl:Class ;
  rdfs:comment "This class is deprecated"@en ;
  rdfs:comment "X.400 Email" ;
  rdfs:isDefinedBy <http://www.w3.org/2006/vcard/ns> ;
  rdfs:label "X.400" ;
  rdfs:label "X400"@en ;
  rdfs:subClassOf vcard:Email ;
  rdfs:subClassOf vcard:Type ;
  owl:deprecated "true"^^xsd:boolean ;
.
vcard:additional-name
  rdf:type owl:DatatypeProperty ;
  rdfs:comment "An additional part of a person's name" ;
  rdfs:comment "The additional name associated with the object"@en ;
  rdfs:domain owl:Thing ;
  rdfs:domain vcard:Name ;
  rdfs:domain _:b218915 ;
  rdfs:domain _:b269191 ;
  rdfs:domain _:b568769 ;
  rdfs:domain _:b623638 ;
  rdfs:domain _:b671776 ;
  rdfs:domain _:b794039 ;
  rdfs:isDefinedBy <http://www.w3.org/2006/vcard/ns> ;
  rdfs:label "additional name" ;
  rdfs:label "additional name"@en ;
  rdfs:range xsd:string ;
.
vcard:adr
  rdf:type owl:ObjectProperty ;
  rdfs:comment "A postal or street address of a person" ;
  rdfs:comment "This object property has been mapped"@en ;
  rdfs:domain owl:Thing ;
  rdfs:domain vcard:Kind ;
  rdfs:domain vcard:VCard ;
  rdfs:domain _:b57053 ;
  rdfs:isDefinedBy <http://www.w3.org/2006/vcard/ns> ;
  rdfs:label "address" ;
  rdfs:label "address"@en ;
  rdfs:range elobr:EloniaAddress ;
  rdfs:range freebr:FreedoniaAddress ;
  rdfs:range toop:Address ;
  rdfs:range owl:Thing ;
  rdfs:range vcard:Address ;
  rdfs:range _:b49042 ;
  rdfs:range _:b83024 ;
  rdfs:range _:b157701 ;
  rdfs:range _:b168676 ;
  rdfs:range _:b396249 ;
  rdfs:range _:b401324 ;
  rdfs:range _:b499218 ;
  rdfs:range _:b541374 ;
  rdfs:range _:b583853 ;
  rdfs:range _:b652026 ;
  rdfs:range _:b726818 ;
  rdfs:range _:b763315 ;
  rdfs:range _:b787338 ;
  rdfs:range _:b926654 ;
  rdfs:range _:b955705 ;
  owl:equivalentProperty vcard:hasAddress ;
.
vcard:agent
  rdf:type owl:ObjectProperty ;
  rdfs:comment "A person that acts as one's agent" ;
  rdfs:comment "This object property has been deprecated"@en ;
  rdfs:domain owl:Thing ;
  rdfs:domain vcard:Kind ;
  rdfs:domain vcard:VCard ;
  rdfs:domain _:b57053 ;
  rdfs:isDefinedBy <http://www.w3.org/2006/vcard/ns> ;
  rdfs:label "agent" ;
  rdfs:label "agent"@en ;
  rdfs:range owl:Thing ;
  rdfs:range vcard:Kind ;
  rdfs:range vcard:VCard ;
  rdfs:range _:b57053 ;
  owl:deprecated "true"^^xsd:boolean ;
.
vcard:anniversary
  rdf:type owl:DatatypeProperty ;
  rdfs:comment "The date of marriage, or equivalent, of the object"@en ;
  rdfs:isDefinedBy <http://www.w3.org/2006/vcard/ns> ;
  rdfs:label "anniversary"@en ;
  rdfs:range _:b671381 ;
.
vcard:bday
  rdf:type owl:DatatypeProperty ;
  rdfs:comment "The birthday of a person" ;
  rdfs:comment "To specify the birth date of the object"@en ;
  rdfs:domain owl:Thing ;
  rdfs:domain vcard:Kind ;
  rdfs:domain vcard:VCard ;
  rdfs:domain _:b57053 ;
  rdfs:isDefinedBy <http://www.w3.org/2006/vcard/ns> ;
  rdfs:label "birth date"@en ;
  rdfs:label "birthday" ;
  rdfs:range _:b148299 ;
  rdfs:range _:b719479 ;
.
vcard:category
  rdf:type owl:DatatypeProperty ;
  rdfs:comment "A category of a vCard" ;
  rdfs:comment "The category information about the object, also known as tags"@en ;
  rdfs:domain owl:Thing ;
  rdfs:domain vcard:Kind ;
  rdfs:domain vcard:VCard ;
  rdfs:domain _:b57053 ;
  rdfs:isDefinedBy <http://www.w3.org/2006/vcard/ns> ;
  rdfs:label "category" ;
  rdfs:label "category"@en ;
  rdfs:range xsd:string ;
.
vcard:class
  rdf:type owl:DatatypeProperty ;
  rdfs:comment "A class (e.g., public, private, etc.) of a vCard" ;
  rdfs:comment "This data property has been deprecated"@en ;
  rdfs:domain owl:Thing ;
  rdfs:domain vcard:Kind ;
  rdfs:domain vcard:VCard ;
  rdfs:domain _:b57053 ;
  rdfs:isDefinedBy <http://www.w3.org/2006/vcard/ns> ;
  rdfs:label "class" ;
  rdfs:label "class"@en ;
  owl:deprecated "true"^^xsd:boolean ;
.
vcard:country-name
  rdf:type owl:DatatypeProperty ;
  rdfs:comment "The country name associated with the address of the object"@en ;
  rdfs:comment "The country of a postal address" ;
  rdfs:domain elobr:EloniaAddress ;
  rdfs:domain freebr:FreedoniaAddress ;
  rdfs:domain toop:Address ;
  rdfs:domain owl:Thing ;
  rdfs:domain vcard:Address ;
  rdfs:domain _:b49042 ;
  rdfs:domain _:b83024 ;
  rdfs:domain _:b157701 ;
  rdfs:domain _:b168676 ;
  rdfs:domain _:b396249 ;
  rdfs:domain _:b401324 ;
  rdfs:domain _:b499218 ;
  rdfs:domain _:b541374 ;
  rdfs:domain _:b583853 ;
  rdfs:domain _:b652026 ;
  rdfs:domain _:b726818 ;
  rdfs:domain _:b763315 ;
  rdfs:domain _:b787338 ;
  rdfs:domain _:b926654 ;
  rdfs:domain _:b955705 ;
  rdfs:isDefinedBy <http://www.w3.org/2006/vcard/ns> ;
  rdfs:label "country name"@en ;
  rdfs:label "country" ;
  rdfs:range xsd:string ;
  owl:equivalentProperty toop:countryName ;
.
vcard:email
  rdf:type owl:ObjectProperty ;
  rdfs:comment "An email address" ;
  rdfs:comment "This object property has been mapped"@en ;
  rdfs:domain dcterms:Agent ;
  rdfs:domain toop:RegisteredOrganization ;
  rdfs:domain owl:Thing ;
  rdfs:domain vcard:Kind ;
  rdfs:domain vcard:VCard ;
  rdfs:domain org:FormalOrganization ;
  rdfs:domain org:Organization ;
  rdfs:domain rov:RegisteredOrganization ;
  rdfs:domain foaf:Agent ;
  rdfs:domain foaf:Organization ;
  rdfs:domain _:b57053 ;
  rdfs:domain _:b180769 ;
  rdfs:domain _:b254570 ;
  rdfs:domain _:b420951 ;
  rdfs:domain _:b421075 ;
  rdfs:domain _:b421664 ;
  rdfs:domain _:b421928 ;
  rdfs:domain _:b454254 ;
  rdfs:domain _:b826282 ;
  rdfs:domain _:b826680 ;
  rdfs:domain _:b937877 ;
  rdfs:domain _:b938265 ;
  rdfs:isDefinedBy <http://www.w3.org/2006/vcard/ns> ;
  rdfs:label "email" ;
  rdfs:label "email"@en ;
  rdfs:range toop:CompanyEmailAddress ;
  rdfs:range owl:Thing ;
  rdfs:range vcard:Email ;
  rdfs:range _:b583853 ;
  rdfs:range _:b652026 ;
  owl:equivalentProperty toop:companyEmailAddress ;
  owl:equivalentProperty vcard:hasEmail ;
.
vcard:extended-address
  rdf:type owl:DatatypeProperty ;
  rdfs:comment "The extended address of a postal address" ;
  rdfs:comment "This data property has been deprecated"@en ;
  rdfs:domain elobr:EloniaAddress ;
  rdfs:domain freebr:FreedoniaAddress ;
  rdfs:domain toop:Address ;
  rdfs:domain owl:Thing ;
  rdfs:domain vcard:Address ;
  rdfs:domain _:b49042 ;
  rdfs:domain _:b83024 ;
  rdfs:domain _:b157701 ;
  rdfs:domain _:b168676 ;
  rdfs:domain _:b396249 ;
  rdfs:domain _:b401324 ;
  rdfs:domain _:b499218 ;
  rdfs:domain _:b541374 ;
  rdfs:domain _:b583853 ;
  rdfs:domain _:b652026 ;
  rdfs:domain _:b726818 ;
  rdfs:domain _:b763315 ;
  rdfs:domain _:b787338 ;
  rdfs:domain _:b926654 ;
  rdfs:domain _:b955705 ;
  rdfs:isDefinedBy <http://www.w3.org/2006/vcard/ns> ;
  rdfs:label "extended address"@en ;
  rdfs:label "extended" ;
  owl:deprecated "true"^^xsd:boolean ;
.
vcard:family-name
  rdf:type owl:DatatypeProperty ;
  rdfs:comment "A family name part of a person's name" ;
  rdfs:comment "The family name associated with the object"@en ;
  rdfs:domain owl:Thing ;
  rdfs:domain vcard:Name ;
  rdfs:domain _:b218915 ;
  rdfs:domain _:b269191 ;
  rdfs:domain _:b568769 ;
  rdfs:domain _:b623638 ;
  rdfs:domain _:b671776 ;
  rdfs:domain _:b794039 ;
  rdfs:isDefinedBy <http://www.w3.org/2006/vcard/ns> ;
  rdfs:label "family name" ;
  rdfs:label "family name"@en ;
  rdfs:range xsd:string ;
.
vcard:fn
  rdf:type owl:DatatypeProperty ;
  rdfs:comment "A formatted name of a person" ;
  rdfs:comment "The formatted text corresponding to the name of the object"@en ;
  rdfs:domain owl:Thing ;
  rdfs:domain vcard:Kind ;
  rdfs:domain vcard:VCard ;
  rdfs:domain _:b57053 ;
  rdfs:isDefinedBy <http://www.w3.org/2006/vcard/ns> ;
  rdfs:label "formatted name" ;
  rdfs:label "formatted name"@en ;
  rdfs:range xsd:string ;
.
vcard:geo
  rdf:type owl:ObjectProperty ;
  rdfs:comment "A geographic location associated with a person" ;
  rdfs:comment "This object property has been mapped"@en ;
  rdfs:domain owl:Thing ;
  rdfs:domain vcard:Kind ;
  rdfs:domain vcard:VCard ;
  rdfs:domain _:b57053 ;
  rdfs:isDefinedBy <http://www.w3.org/2006/vcard/ns> ;
  rdfs:label "geo"@en ;
  rdfs:label "geographic location" ;
  rdfs:range owl:Thing ;
  rdfs:range vcard:Kind ;
  rdfs:range vcard:Location ;
  rdfs:range vcard:VCard ;
  rdfs:range _:b57053 ;
  rdfs:range _:b313826 ;
  rdfs:range _:b405470 ;
  owl:equivalentProperty vcard:hasGeo ;
.
vcard:given-name
  rdf:type owl:DatatypeProperty ;
  rdfs:comment "A given name part of a person's name" ;
  rdfs:comment "The given name associated with the object"@en ;
  rdfs:domain owl:Thing ;
  rdfs:domain vcard:Name ;
  rdfs:domain _:b218915 ;
  rdfs:domain _:b269191 ;
  rdfs:domain _:b568769 ;
  rdfs:domain _:b623638 ;
  rdfs:domain _:b671776 ;
  rdfs:domain _:b794039 ;
  rdfs:isDefinedBy <http://www.w3.org/2006/vcard/ns> ;
  rdfs:label "given name" ;
  rdfs:label "given name"@en ;
  rdfs:range xsd:string ;
.
vcard:hasAdditionalName
  rdf:type owl:ObjectProperty ;
  rdfs:comment "Used to support property parameters for the additional name data property"@en ;
  rdfs:isDefinedBy <http://www.w3.org/2006/vcard/ns> ;
  rdfs:label "has additional name"@en ;
.
vcard:hasAddress
  rdf:type owl:ObjectProperty ;
  rdfs:comment "To specify the components of the delivery address for the object"@en ;
  rdfs:domain owl:Thing ;
  rdfs:domain vcard:Kind ;
  rdfs:domain vcard:VCard ;
  rdfs:domain _:b57053 ;
  rdfs:isDefinedBy <http://www.w3.org/2006/vcard/ns> ;
  rdfs:label "has address"@en ;
  rdfs:range elobr:EloniaAddress ;
  rdfs:range freebr:FreedoniaAddress ;
  rdfs:range toop:Address ;
  rdfs:range owl:Thing ;
  rdfs:range vcard:Address ;
  rdfs:range _:b49042 ;
  rdfs:range _:b83024 ;
  rdfs:range _:b157701 ;
  rdfs:range _:b168676 ;
  rdfs:range _:b396249 ;
  rdfs:range _:b401324 ;
  rdfs:range _:b499218 ;
  rdfs:range _:b541374 ;
  rdfs:range _:b583853 ;
  rdfs:range _:b652026 ;
  rdfs:range _:b726818 ;
  rdfs:range _:b763315 ;
  rdfs:range _:b787338 ;
  rdfs:range _:b926654 ;
  rdfs:range _:b955705 ;
  owl:equivalentProperty vcard:adr ;
.
vcard:hasCalendarBusy
  rdf:type owl:ObjectProperty ;
  rdfs:comment "To specify the busy time associated with the object. (Was called FBURL in RFC6350)"@en ;
  rdfs:isDefinedBy <http://www.w3.org/2006/vcard/ns> ;
  rdfs:label "has calendar busy"@en ;
.
vcard:hasCalendarLink
  rdf:type owl:ObjectProperty ;
  rdfs:comment "To specify the calendar associated with the object. (Was called CALURI in RFC6350)"@en ;
  rdfs:isDefinedBy <http://www.w3.org/2006/vcard/ns> ;
  rdfs:label "has calendar link"@en ;
.
vcard:hasCalendarRequest
  rdf:type owl:ObjectProperty ;
  rdfs:comment "To specify the calendar user address to which a scheduling request be sent for the object. (Was called CALADRURI in RFC6350)"@en ;
  rdfs:isDefinedBy <http://www.w3.org/2006/vcard/ns> ;
  rdfs:label "has calendar request"@en ;
.
vcard:hasCategory
  rdf:type owl:ObjectProperty ;
  rdfs:comment "Used to support property parameters for the category data property"@en ;
  rdfs:isDefinedBy <http://www.w3.org/2006/vcard/ns> ;
  rdfs:label "has category"@en ;
.
vcard:hasCountryName
  rdf:type owl:ObjectProperty ;
  rdfs:comment "Used to support property parameters for the country name data property"@en ;
  rdfs:isDefinedBy <http://www.w3.org/2006/vcard/ns> ;
  rdfs:label "has country name"@en ;
.
vcard:hasEmail
  rdf:type owl:ObjectProperty ;
  rdfs:comment "To specify the electronic mail address for communication with the object"@en ;
  rdfs:domain dcterms:Agent ;
  rdfs:domain toop:RegisteredOrganization ;
  rdfs:domain owl:Thing ;
  rdfs:domain vcard:Kind ;
  rdfs:domain vcard:VCard ;
  rdfs:domain org:FormalOrganization ;
  rdfs:domain org:Organization ;
  rdfs:domain rov:RegisteredOrganization ;
  rdfs:domain foaf:Agent ;
  rdfs:domain foaf:Organization ;
  rdfs:domain _:b57053 ;
  rdfs:domain _:b180769 ;
  rdfs:domain _:b254570 ;
  rdfs:domain _:b420951 ;
  rdfs:domain _:b421075 ;
  rdfs:domain _:b421664 ;
  rdfs:domain _:b421928 ;
  rdfs:domain _:b454254 ;
  rdfs:domain _:b826282 ;
  rdfs:domain _:b826680 ;
  rdfs:domain _:b937877 ;
  rdfs:domain _:b938265 ;
  rdfs:isDefinedBy <http://www.w3.org/2006/vcard/ns> ;
  rdfs:label "has email"@en ;
  rdfs:range toop:CompanyEmailAddress ;
  rdfs:range owl:Thing ;
  rdfs:range vcard:Email ;
  rdfs:range _:b583853 ;
  rdfs:range _:b652026 ;
  owl:equivalentProperty toop:companyEmailAddress ;
  owl:equivalentProperty vcard:email ;
.
vcard:hasFN
  rdf:type owl:ObjectProperty ;
  rdfs:comment "Used to support property parameters for the formatted name data property"@en ;
  rdfs:isDefinedBy <http://www.w3.org/2006/vcard/ns> ;
  rdfs:label "has formatted name"@en ;
.
vcard:hasFamilyName
  rdf:type owl:ObjectProperty ;
  rdfs:comment "Used to support property parameters for the family name data property"@en ;
  rdfs:isDefinedBy <http://www.w3.org/2006/vcard/ns> ;
  rdfs:label "has family name"@en ;
.
vcard:hasGender
  rdf:type owl:ObjectProperty ;
  rdfs:comment "To specify  the sex or gender identity of the object. URIs are recommended to enable interoperable sex and gender codes to be used."@en ;
  rdfs:isDefinedBy <http://www.w3.org/2006/vcard/ns> ;
  rdfs:label "has gender"@en ;
.
vcard:hasGeo
  rdf:type owl:ObjectProperty ;
  rdfs:comment "To specify information related to the global positioning of the object. May also be used as a property parameter."@en ;
  rdfs:domain owl:Thing ;
  rdfs:domain vcard:Kind ;
  rdfs:domain vcard:VCard ;
  rdfs:domain _:b57053 ;
  rdfs:isDefinedBy <http://www.w3.org/2006/vcard/ns> ;
  rdfs:label "has geo"@en ;
  rdfs:range owl:Thing ;
  rdfs:range vcard:Kind ;
  rdfs:range vcard:Location ;
  rdfs:range vcard:VCard ;
  rdfs:range _:b57053 ;
  rdfs:range _:b313826 ;
  rdfs:range _:b405470 ;
  owl:equivalentProperty vcard:geo ;
.
vcard:hasGivenName
  rdf:type owl:ObjectProperty ;
  rdfs:comment "Used to support property parameters for the given name data property"@en ;
  rdfs:isDefinedBy <http://www.w3.org/2006/vcard/ns> ;
  rdfs:label "has given name"@en ;
.
vcard:hasHonorificPrefix
  rdf:type owl:ObjectProperty ;
  rdfs:comment "Used to support property parameters for the honorific prefix data property"@en ;
  rdfs:isDefinedBy <http://www.w3.org/2006/vcard/ns> ;
  rdfs:label "has honorific prefix"@en ;
.
vcard:hasHonorificSuffix
  rdf:type owl:ObjectProperty ;
  rdfs:comment "Used to support property parameters for the honorific suffix data property"@en ;
  rdfs:isDefinedBy <http://www.w3.org/2006/vcard/ns> ;
  rdfs:label "has honorific suffix"@en ;
.
vcard:hasInstantMessage
  rdf:type owl:ObjectProperty ;
  rdfs:comment "To specify the instant messaging and presence protocol communications with the object. (Was called IMPP in RFC6350)"@en ;
  rdfs:isDefinedBy <http://www.w3.org/2006/vcard/ns> ;
  rdfs:label "has messaging"@en ;
.
vcard:hasKey
  rdf:type owl:ObjectProperty ;
  rdfs:comment "To specify a public key or authentication certificate associated with the object"@en ;
  rdfs:domain owl:Thing ;
  rdfs:domain vcard:Kind ;
  rdfs:domain vcard:VCard ;
  rdfs:domain _:b57053 ;
  rdfs:isDefinedBy <http://www.w3.org/2006/vcard/ns> ;
  rdfs:label "has key"@en ;
  rdfs:subPropertyOf vcard:key ;
  owl:equivalentProperty vcard:key ;
.
vcard:hasLanguage
  rdf:type owl:ObjectProperty ;
  rdfs:comment "Used to support property parameters for the language data property"@en ;
  rdfs:isDefinedBy <http://www.w3.org/2006/vcard/ns> ;
  rdfs:label "has language"@en ;
.
vcard:hasLocality
  rdf:type owl:ObjectProperty ;
  rdfs:comment "Used to support property parameters for the locality data property"@en ;
  rdfs:isDefinedBy <http://www.w3.org/2006/vcard/ns> ;
  rdfs:label "has locality"@en ;
.
vcard:hasLogo
  rdf:type owl:ObjectProperty ;
  rdfs:comment "To specify a graphic image of a logo associated with the object "@en ;
  rdfs:domain owl:Thing ;
  rdfs:domain vcard:Kind ;
  rdfs:domain vcard:VCard ;
  rdfs:domain _:b57053 ;
  rdfs:isDefinedBy <http://www.w3.org/2006/vcard/ns> ;
  rdfs:label "has logo"@en ;
  rdfs:subPropertyOf vcard:logo ;
  owl:equivalentProperty vcard:logo ;
.
vcard:hasMember
  rdf:type owl:ObjectProperty ;
  rdfs:comment "To include a member in the group this object represents. (This property can only be used by Group individuals)"@en ;
  rdfs:domain owl:Thing ;
  rdfs:domain vcard:Group ;
  rdfs:domain vcard:Kind ;
  rdfs:domain vcard:VCard ;
  rdfs:domain _:b29166 ;
  rdfs:domain _:b57053 ;
  rdfs:domain _:b780263 ;
  rdfs:domain _:b789349 ;
  rdfs:isDefinedBy <http://www.w3.org/2006/vcard/ns> ;
  rdfs:label "has member"@en ;
  rdfs:range owl:Thing ;
  rdfs:range vcard:Kind ;
  rdfs:range vcard:VCard ;
  rdfs:range _:b57053 ;
.
vcard:hasName
  rdf:type owl:ObjectProperty ;
  rdfs:comment "To specify the components of the name of the object"@en ;
  rdfs:domain owl:Thing ;
  rdfs:domain vcard:Kind ;
  rdfs:domain vcard:VCard ;
  rdfs:domain _:b57053 ;
  rdfs:isDefinedBy <http://www.w3.org/2006/vcard/ns> ;
  rdfs:label "has name"@en ;
  rdfs:range owl:Thing ;
  rdfs:range vcard:Name ;
  rdfs:range _:b218915 ;
  rdfs:range _:b269191 ;
  rdfs:range _:b568769 ;
  rdfs:range _:b623638 ;
  rdfs:range _:b671776 ;
  rdfs:range _:b794039 ;
  rdfs:subPropertyOf vcard:n ;
  owl:equivalentProperty vcard:n ;
.
vcard:hasNickname
  rdf:type owl:ObjectProperty ;
  rdfs:comment "Used to support property parameters for the nickname data property"@en ;
  rdfs:isDefinedBy <http://www.w3.org/2006/vcard/ns> ;
  rdfs:label "has nickname"@en ;
  rdfs:seeAlso vcard:nickname ;
.
vcard:hasNote
  rdf:type owl:ObjectProperty ;
  rdfs:comment "Used to support property parameters for the note data property"@en ;
  rdfs:isDefinedBy <http://www.w3.org/2006/vcard/ns> ;
  rdfs:label "has note"@en ;
.
vcard:hasOrganizationName
  rdf:type owl:ObjectProperty ;
  rdfs:comment "Used to support property parameters for the organization name data property"@en ;
  rdfs:isDefinedBy <http://www.w3.org/2006/vcard/ns> ;
  rdfs:label "has organization name"@en ;
.
vcard:hasOrganizationUnit
  rdf:type owl:ObjectProperty ;
  rdfs:comment "Used to support property parameters for the organization unit name data property"@en ;
  rdfs:isDefinedBy <http://www.w3.org/2006/vcard/ns> ;
  rdfs:label "has organization unit name"@en ;
.
vcard:hasPhoto
  rdf:type owl:ObjectProperty ;
  rdfs:comment "To specify an image or photograph information that annotates some aspect of the object"@en ;
  rdfs:domain owl:Thing ;
  rdfs:domain vcard:Kind ;
  rdfs:domain vcard:VCard ;
  rdfs:domain _:b57053 ;
  rdfs:isDefinedBy <http://www.w3.org/2006/vcard/ns> ;
  rdfs:label "has photo"@en ;
  rdfs:subPropertyOf vcard:photo ;
  owl:equivalentProperty vcard:photo ;
.
vcard:hasPostalCode
  rdf:type owl:ObjectProperty ;
  rdfs:comment "Used to support property parameters for the postal code data property"@en ;
  rdfs:isDefinedBy <http://www.w3.org/2006/vcard/ns> ;
  rdfs:label "has postal code"@en ;
.
vcard:hasRegion
  rdf:type owl:ObjectProperty ;
  rdfs:comment "Used to support property parameters for the region data property"@en ;
  rdfs:isDefinedBy <http://www.w3.org/2006/vcard/ns> ;
  rdfs:label "has region"@en ;
.
vcard:hasRelated
  rdf:type owl:ObjectProperty ;
  rdfs:comment "To specify a relationship between another entity and the entity represented by this object"@en ;
  rdfs:isDefinedBy <http://www.w3.org/2006/vcard/ns> ;
  rdfs:label "has related"@en ;
.
vcard:hasRole
  rdf:type owl:ObjectProperty ;
  rdfs:comment "Used to support property parameters for the role data property"@en ;
  rdfs:isDefinedBy <http://www.w3.org/2006/vcard/ns> ;
  rdfs:label "has role"@en ;
.
vcard:hasSound
  rdf:type owl:ObjectProperty ;
  rdfs:comment "To specify a digital sound content information that annotates some aspect of the object"@en ;
  rdfs:domain owl:Thing ;
  rdfs:domain vcard:Kind ;
  rdfs:domain vcard:VCard ;
  rdfs:domain _:b57053 ;
  rdfs:isDefinedBy <http://www.w3.org/2006/vcard/ns> ;
  rdfs:label "has sound"@en ;
  rdfs:subPropertyOf vcard:sound ;
  owl:equivalentProperty vcard:sound ;
.
vcard:hasSource
  rdf:type owl:ObjectProperty ;
  rdfs:comment "To identify the source of directory information of the object"@en ;
  rdfs:isDefinedBy <http://www.w3.org/2006/vcard/ns> ;
  rdfs:label "has source"@en ;
.
vcard:hasStreetAddress
  rdf:type owl:ObjectProperty ;
  rdfs:comment "Used to support property parameters for the street address data property"@en ;
  rdfs:isDefinedBy <http://www.w3.org/2006/vcard/ns> ;
  rdfs:label "has street address"@en ;
.
vcard:hasTelephone
  rdf:type owl:ObjectProperty ;
  rdfs:comment "To specify the telephone number for telephony communication with the object"@en ;
  rdfs:domain dcterms:Agent ;
  rdfs:domain toop:RegisteredOrganization ;
  rdfs:domain owl:Thing ;
  rdfs:domain vcard:Kind ;
  rdfs:domain vcard:VCard ;
  rdfs:domain org:FormalOrganization ;
  rdfs:domain org:Organization ;
  rdfs:domain rov:RegisteredOrganization ;
  rdfs:domain foaf:Agent ;
  rdfs:domain foaf:Organization ;
  rdfs:domain _:b57053 ;
  rdfs:domain _:b180769 ;
  rdfs:domain _:b254570 ;
  rdfs:domain _:b420951 ;
  rdfs:domain _:b421075 ;
  rdfs:domain _:b421664 ;
  rdfs:domain _:b421928 ;
  rdfs:domain _:b454254 ;
  rdfs:domain _:b826282 ;
  rdfs:domain _:b826680 ;
  rdfs:domain _:b937877 ;
  rdfs:domain _:b938265 ;
  rdfs:isDefinedBy <http://www.w3.org/2006/vcard/ns> ;
  rdfs:label "has telephone"@en ;
  rdfs:range toop:CompanyContactNumber ;
  rdfs:range owl:Thing ;
  rdfs:subPropertyOf vcard:tel ;
  owl:equivalentProperty toop:companyContactNumber ;
  owl:equivalentProperty vcard:tel ;
.
vcard:hasTitle
  rdf:type owl:ObjectProperty ;
  rdfs:comment "Used to support property parameters for the title data property"@en ;
  rdfs:isDefinedBy <http://www.w3.org/2006/vcard/ns> ;
  rdfs:label "has title"@en ;
.
vcard:hasUID
  rdf:type owl:ObjectProperty ;
  rdfs:comment "To specify a value that represents a globally unique identifier corresponding to the object"@en ;
  rdfs:isDefinedBy <http://www.w3.org/2006/vcard/ns> ;
  rdfs:label "has uid"@en ;
.
vcard:hasURL
  rdf:type owl:ObjectProperty ;
  rdfs:comment "To specify a uniform resource locator associated with the object"@en ;
  rdfs:domain owl:Thing ;
  rdfs:domain vcard:Kind ;
  rdfs:domain vcard:VCard ;
  rdfs:domain _:b57053 ;
  rdfs:isDefinedBy <http://www.w3.org/2006/vcard/ns> ;
  rdfs:label "has url"@en ;
  rdfs:subPropertyOf vcard:url ;
  owl:equivalentProperty vcard:url ;
.
vcard:hasValue
  rdf:type owl:ObjectProperty ;
  rdfs:comment "Used to indicate the resource value of an object property that requires property parameters"@en ;
  rdfs:isDefinedBy <http://www.w3.org/2006/vcard/ns> ;
  rdfs:label "has value"@en ;
.
vcard:honorific-prefix
  rdf:type owl:DatatypeProperty ;
  rdfs:comment "An honorific prefix part of a person's name" ;
  rdfs:comment "The honorific prefix of the name associated with the object"@en ;
  rdfs:domain owl:Thing ;
  rdfs:domain vcard:Name ;
  rdfs:domain _:b218915 ;
  rdfs:domain _:b269191 ;
  rdfs:domain _:b568769 ;
  rdfs:domain _:b623638 ;
  rdfs:domain _:b671776 ;
  rdfs:domain _:b794039 ;
  rdfs:isDefinedBy <http://www.w3.org/2006/vcard/ns> ;
  rdfs:label "honorific prefix" ;
  rdfs:label "honorific prefix"@en ;
  rdfs:range xsd:string ;
.
vcard:honorific-suffix
  rdf:type owl:DatatypeProperty ;
  rdfs:comment "An honorific suffix part of a person's name" ;
  rdfs:comment "The honorific suffix of the name associated with the object"@en ;
  rdfs:domain owl:Thing ;
  rdfs:domain vcard:Name ;
  rdfs:domain _:b218915 ;
  rdfs:domain _:b269191 ;
  rdfs:domain _:b568769 ;
  rdfs:domain _:b623638 ;
  rdfs:domain _:b671776 ;
  rdfs:domain _:b794039 ;
  rdfs:isDefinedBy <http://www.w3.org/2006/vcard/ns> ;
  rdfs:label "honorific suffix" ;
  rdfs:label "honorific suffix"@en ;
  rdfs:range xsd:string ;
.
vcard:key
  rdf:type owl:ObjectProperty ;
  rdfs:comment "A key (e.g, PKI key) of a person" ;
  rdfs:comment "This object property has been mapped"@en ;
  rdfs:domain owl:Thing ;
  rdfs:domain vcard:Kind ;
  rdfs:domain vcard:VCard ;
  rdfs:domain _:b57053 ;
  rdfs:isDefinedBy <http://www.w3.org/2006/vcard/ns> ;
  rdfs:label "key" ;
  rdfs:label "key"@en ;
  rdfs:subPropertyOf vcard:hasKey ;
  owl:equivalentProperty vcard:hasKey ;
.
vcard:label
  rdf:type owl:DatatypeProperty ;
  rdfs:comment "The formatted version of a postal address (a string with embedded line breaks, punctuation, etc.)" ;
  rdfs:comment "This data property has been deprecated"@en ;
  rdfs:domain elobr:EloniaAddress ;
  rdfs:domain freebr:FreedoniaAddress ;
  rdfs:domain toop:Address ;
  rdfs:domain owl:Thing ;
  rdfs:domain vcard:Address ;
  rdfs:domain _:b49042 ;
  rdfs:domain _:b83024 ;
  rdfs:domain _:b157701 ;
  rdfs:domain _:b168676 ;
  rdfs:domain _:b396249 ;
  rdfs:domain _:b401324 ;
  rdfs:domain _:b499218 ;
  rdfs:domain _:b541374 ;
  rdfs:domain _:b583853 ;
  rdfs:domain _:b652026 ;
  rdfs:domain _:b726818 ;
  rdfs:domain _:b763315 ;
  rdfs:domain _:b787338 ;
  rdfs:domain _:b926654 ;
  rdfs:domain _:b955705 ;
  rdfs:isDefinedBy <http://www.w3.org/2006/vcard/ns> ;
  rdfs:label "address label" ;
  rdfs:label "label"@en ;
  owl:deprecated "true"^^xsd:boolean ;
.
vcard:language
  rdf:type owl:DatatypeProperty ;
  rdfs:comment "To specify the language that may be used for contacting the object. May also be used as a property parameter."@en ;
  rdfs:isDefinedBy <http://www.w3.org/2006/vcard/ns> ;
  rdfs:label "language"@en ;
.
vcard:latitude
  rdf:type owl:DatatypeProperty ;
  rdfs:comment "The latitude of the location of the vCard object" ;
  rdfs:comment "This data property has been deprecated. See hasGeo"@en ;
  rdfs:domain owl:Thing ;
  rdfs:domain vcard:Kind ;
  rdfs:domain vcard:Location ;
  rdfs:domain vcard:VCard ;
  rdfs:domain _:b57053 ;
  rdfs:domain _:b313826 ;
  rdfs:domain _:b405470 ;
  rdfs:isDefinedBy <http://www.w3.org/2006/vcard/ns> ;
  rdfs:label "geographic latitude" ;
  rdfs:label "latitude"@en ;
  rdfs:range xsd:float ;
  owl:deprecated "true"^^xsd:boolean ;
.
vcard:locality
  rdf:type owl:DatatypeProperty ;
  rdfs:comment "The locality (e.g. city or town) associated with the address of the object"@en ;
  rdfs:comment "The locality (e.g., city) of a postal address" ;
  rdfs:domain elobr:EloniaAddress ;
  rdfs:domain freebr:FreedoniaAddress ;
  rdfs:domain toop:Address ;
  rdfs:domain owl:Thing ;
  rdfs:domain vcard:Address ;
  rdfs:domain _:b49042 ;
  rdfs:domain _:b83024 ;
  rdfs:domain _:b157701 ;
  rdfs:domain _:b168676 ;
  rdfs:domain _:b396249 ;
  rdfs:domain _:b401324 ;
  rdfs:domain _:b499218 ;
  rdfs:domain _:b541374 ;
  rdfs:domain _:b583853 ;
  rdfs:domain _:b652026 ;
  rdfs:domain _:b726818 ;
  rdfs:domain _:b763315 ;
  rdfs:domain _:b787338 ;
  rdfs:domain _:b926654 ;
  rdfs:domain _:b955705 ;
  rdfs:isDefinedBy <http://www.w3.org/2006/vcard/ns> ;
  rdfs:label "locality" ;
  rdfs:label "locality"@en ;
  rdfs:range xsd:string ;
  owl:equivalentProperty toop:locality ;
.
vcard:logo
  rdf:type owl:ObjectProperty ;
  rdfs:comment "A logo associated with a person or their organization" ;
  rdfs:comment "This object property has been mapped"@en ;
  rdfs:domain owl:Thing ;
  rdfs:domain vcard:Kind ;
  rdfs:domain vcard:VCard ;
  rdfs:domain _:b57053 ;
  rdfs:isDefinedBy <http://www.w3.org/2006/vcard/ns> ;
  rdfs:label "logo" ;
  rdfs:label "logo"@en ;
  rdfs:subPropertyOf vcard:hasLogo ;
  owl:equivalentProperty vcard:hasLogo ;
.
vcard:longitude
  rdf:type owl:DatatypeProperty ;
  rdfs:comment "The longitude of the location of the vCard object" ;
  rdfs:comment "This data property has been deprecated. See hasGeo"@en ;
  rdfs:domain owl:Thing ;
  rdfs:domain vcard:Kind ;
  rdfs:domain vcard:Location ;
  rdfs:domain vcard:VCard ;
  rdfs:domain _:b57053 ;
  rdfs:domain _:b313826 ;
  rdfs:domain _:b405470 ;
  rdfs:isDefinedBy <http://www.w3.org/2006/vcard/ns> ;
  rdfs:label "geographic longitude" ;
  rdfs:label "longitude"@en ;
  rdfs:range xsd:float ;
  owl:deprecated "true"^^xsd:boolean ;
.
vcard:mailer
  rdf:type owl:DatatypeProperty ;
  rdfs:comment "A mailer associated with a vCard" ;
  rdfs:comment "This data property has been deprecated"@en ;
  rdfs:domain owl:Thing ;
  rdfs:domain vcard:Kind ;
  rdfs:domain vcard:VCard ;
  rdfs:domain _:b57053 ;
  rdfs:isDefinedBy <http://www.w3.org/2006/vcard/ns> ;
  rdfs:label "mailer" ;
  rdfs:label "mailer"@en ;
  owl:deprecated "true"^^xsd:boolean ;
.
vcard:n
  rdf:type owl:ObjectProperty ;
  rdfs:comment "The components of the name of a person" ;
  rdfs:comment "This object property has been mapped"@en ;
  rdfs:domain owl:Thing ;
  rdfs:domain vcard:Kind ;
  rdfs:domain vcard:VCard ;
  rdfs:domain _:b57053 ;
  rdfs:isDefinedBy <http://www.w3.org/2006/vcard/ns> ;
  rdfs:label "name" ;
  rdfs:label "name"@en ;
  rdfs:range owl:Thing ;
  rdfs:range vcard:Name ;
  rdfs:range _:b218915 ;
  rdfs:range _:b269191 ;
  rdfs:range _:b568769 ;
  rdfs:range _:b623638 ;
  rdfs:range _:b671776 ;
  rdfs:range _:b794039 ;
  rdfs:subPropertyOf vcard:hasName ;
  owl:equivalentProperty vcard:hasName ;
.
vcard:nickname
  rdf:type owl:DatatypeProperty ;
  rdfs:comment "The nick name associated with the object"@en ;
  rdfs:comment "The nickname of a person" ;
  rdfs:domain owl:Thing ;
  rdfs:domain vcard:Kind ;
  rdfs:domain vcard:VCard ;
  rdfs:domain _:b57053 ;
  rdfs:isDefinedBy <http://www.w3.org/2006/vcard/ns> ;
  rdfs:label "nickname" ;
  rdfs:label "nickname"@en ;
  rdfs:range xsd:string ;
.
vcard:note
  rdf:type owl:DatatypeProperty ;
  rdfs:comment "A note associated with the object"@en ;
  rdfs:comment "Notes about a person on a vCard" ;
  rdfs:domain owl:Thing ;
  rdfs:domain vcard:Kind ;
  rdfs:domain vcard:VCard ;
  rdfs:domain _:b57053 ;
  rdfs:isDefinedBy <http://www.w3.org/2006/vcard/ns> ;
  rdfs:label "note"@en ;
  rdfs:label "notes" ;
  rdfs:range xsd:string ;
.
vcard:org
  rdf:type owl:ObjectProperty ;
  rdfs:comment "An organization associated with a person" ;
  rdfs:comment "This object property has been mapped. Use the organization-name data property."@en ;
  rdfs:domain owl:Thing ;
  rdfs:domain vcard:Kind ;
  rdfs:domain vcard:Organization ;
  rdfs:domain vcard:VCard ;
  rdfs:domain _:b57053 ;
  rdfs:domain _:b757317 ;
  rdfs:domain _:b938985 ;
  rdfs:isDefinedBy <http://www.w3.org/2006/vcard/ns> ;
  rdfs:label "organization" ;
  rdfs:label "organization"@en ;
  rdfs:range xsd:string ;
  rdfs:range owl:Thing ;
  rdfs:range vcard:Kind ;
  rdfs:range vcard:Organization ;
  rdfs:range vcard:VCard ;
  rdfs:range _:b57053 ;
  rdfs:range _:b757317 ;
  rdfs:range _:b938985 ;
  owl:equivalentProperty vcard:organization-name ;
.
vcard:organization-name
  rdf:type owl:DatatypeProperty ;
  rdfs:comment "The name of an organization" ;
  rdfs:comment "To specify the organizational name associated with the object"@en ;
  rdfs:domain owl:Thing ;
  rdfs:domain vcard:Kind ;
  rdfs:domain vcard:Organization ;
  rdfs:domain vcard:VCard ;
  rdfs:domain _:b57053 ;
  rdfs:domain _:b757317 ;
  rdfs:domain _:b938985 ;
  rdfs:isDefinedBy <http://www.w3.org/2006/vcard/ns> ;
  rdfs:label "name" ;
  rdfs:label "organization name"@en ;
  rdfs:range xsd:string ;
  rdfs:range owl:Thing ;
  rdfs:range vcard:Kind ;
  rdfs:range vcard:Organization ;
  rdfs:range vcard:VCard ;
  rdfs:range _:b57053 ;
  rdfs:range _:b757317 ;
  rdfs:range _:b938985 ;
  owl:equivalentProperty vcard:org ;
.
vcard:organization-unit
  rdf:type owl:DatatypeProperty ;
  rdfs:comment "The name of a unit within an organization" ;
  rdfs:comment "To specify the organizational unit name associated with the object"@en ;
  rdfs:domain owl:Thing ;
  rdfs:domain vcard:Kind ;
  rdfs:domain vcard:Organization ;
  rdfs:domain vcard:VCard ;
  rdfs:domain _:b57053 ;
  rdfs:domain _:b757317 ;
  rdfs:domain _:b938985 ;
  rdfs:isDefinedBy <http://www.w3.org/2006/vcard/ns> ;
  rdfs:label "organizational unit name"@en ;
  rdfs:label "unit" ;
  rdfs:range xsd:string ;
  rdfs:range owl:Thing ;
  rdfs:range vcard:Kind ;
  rdfs:range vcard:Organization ;
  rdfs:range vcard:VCard ;
  rdfs:range _:b57053 ;
  rdfs:range _:b757317 ;
  rdfs:range _:b938985 ;
  rdfs:subPropertyOf vcard:org ;
  rdfs:subPropertyOf vcard:organization-name ;
.
vcard:photo
  rdf:type owl:ObjectProperty ;
  rdfs:comment "A photograph of a person" ;
  rdfs:comment "This object property has been mapped"@en ;
  rdfs:domain owl:Thing ;
  rdfs:domain vcard:Kind ;
  rdfs:domain vcard:VCard ;
  rdfs:domain _:b57053 ;
  rdfs:isDefinedBy <http://www.w3.org/2006/vcard/ns> ;
  rdfs:label "photo" ;
  rdfs:label "photo"@en ;
  rdfs:subPropertyOf vcard:hasPhoto ;
  owl:equivalentProperty vcard:hasPhoto ;
.
vcard:post-office-box
  rdf:type owl:DatatypeProperty ;
  rdfs:comment "The post office box of a postal address" ;
  rdfs:comment "This data property has been deprecated"@en ;
  rdfs:domain elobr:EloniaAddress ;
  rdfs:domain freebr:FreedoniaAddress ;
  rdfs:domain toop:Address ;
  rdfs:domain owl:Thing ;
  rdfs:domain vcard:Address ;
  rdfs:domain _:b49042 ;
  rdfs:domain _:b83024 ;
  rdfs:domain _:b157701 ;
  rdfs:domain _:b168676 ;
  rdfs:domain _:b396249 ;
  rdfs:domain _:b401324 ;
  rdfs:domain _:b499218 ;
  rdfs:domain _:b541374 ;
  rdfs:domain _:b583853 ;
  rdfs:domain _:b652026 ;
  rdfs:domain _:b726818 ;
  rdfs:domain _:b763315 ;
  rdfs:domain _:b787338 ;
  rdfs:domain _:b926654 ;
  rdfs:domain _:b955705 ;
  rdfs:isDefinedBy <http://www.w3.org/2006/vcard/ns> ;
  rdfs:label "P.O. Box" ;
  rdfs:label "post office box"@en ;
  owl:deprecated "true"^^xsd:boolean ;
.
vcard:postal-code
  rdf:type owl:DatatypeProperty ;
  rdfs:comment "The postal code (e.g., U.S. ZIP code) of a postal address" ;
  rdfs:comment "The postal code associated with the address of the object"@en ;
  rdfs:domain elobr:EloniaAddress ;
  rdfs:domain freebr:FreedoniaAddress ;
  rdfs:domain toop:Address ;
  rdfs:domain owl:Thing ;
  rdfs:domain vcard:Address ;
  rdfs:domain _:b49042 ;
  rdfs:domain _:b83024 ;
  rdfs:domain _:b157701 ;
  rdfs:domain _:b168676 ;
  rdfs:domain _:b396249 ;
  rdfs:domain _:b401324 ;
  rdfs:domain _:b499218 ;
  rdfs:domain _:b541374 ;
  rdfs:domain _:b583853 ;
  rdfs:domain _:b652026 ;
  rdfs:domain _:b726818 ;
  rdfs:domain _:b763315 ;
  rdfs:domain _:b787338 ;
  rdfs:domain _:b926654 ;
  rdfs:domain _:b955705 ;
  rdfs:isDefinedBy <http://www.w3.org/2006/vcard/ns> ;
  rdfs:label "postal code" ;
  rdfs:label "postal code"@en ;
  rdfs:range xsd:string ;
  owl:equivalentProperty toop:postalCode ;
.
vcard:prodid
  rdf:type owl:DatatypeProperty ;
  rdfs:comment "The Identifier for the product that created the vCard object" ;
  rdfs:comment "To specify the identifier for the product that created the object"@en ;
  rdfs:domain owl:Thing ;
  rdfs:domain vcard:Kind ;
  rdfs:domain vcard:VCard ;
  rdfs:domain _:b57053 ;
  rdfs:isDefinedBy <http://www.w3.org/2006/vcard/ns> ;
  rdfs:label "prodid" ;
  rdfs:label "product id"@en ;
  rdfs:range xsd:string ;
.
vcard:region
  rdf:type owl:DatatypeProperty ;
  rdfs:comment "The region (e.g. state or province) associated with the address of the object"@en ;
  rdfs:comment "The region (e.g., state or province) of a postal address" ;
  rdfs:domain elobr:EloniaAddress ;
  rdfs:domain freebr:FreedoniaAddress ;
  rdfs:domain toop:Address ;
  rdfs:domain owl:Thing ;
  rdfs:domain vcard:Address ;
  rdfs:domain _:b49042 ;
  rdfs:domain _:b83024 ;
  rdfs:domain _:b157701 ;
  rdfs:domain _:b168676 ;
  rdfs:domain _:b396249 ;
  rdfs:domain _:b401324 ;
  rdfs:domain _:b499218 ;
  rdfs:domain _:b541374 ;
  rdfs:domain _:b583853 ;
  rdfs:domain _:b652026 ;
  rdfs:domain _:b726818 ;
  rdfs:domain _:b763315 ;
  rdfs:domain _:b787338 ;
  rdfs:domain _:b926654 ;
  rdfs:domain _:b955705 ;
  rdfs:isDefinedBy <http://www.w3.org/2006/vcard/ns> ;
  rdfs:label "region" ;
  rdfs:label "region"@en ;
  rdfs:range xsd:string ;
  owl:equivalentProperty toop:region ;
.
vcard:rev
  rdf:type owl:DatatypeProperty ;
  rdfs:comment "The timestamp of a revision of a vCard" ;
  rdfs:comment "To specify revision information about the object"@en ;
  rdfs:domain owl:Thing ;
  rdfs:domain vcard:Kind ;
  rdfs:domain vcard:VCard ;
  rdfs:domain _:b57053 ;
  rdfs:isDefinedBy <http://www.w3.org/2006/vcard/ns> ;
  rdfs:label "revision" ;
  rdfs:label "revision"@en ;
  rdfs:range xsd:dateTime ;
  rdfs:range _:b115973 ;
  rdfs:range _:b148299 ;
  rdfs:range _:b671381 ;
  rdfs:range _:b719479 ;
.
vcard:role
  rdf:type owl:DatatypeProperty ;
  rdfs:comment "A role a person plays within an organization" ;
  rdfs:comment "To specify the function or part played in a particular situation by the object"@en ;
  rdfs:domain owl:Thing ;
  rdfs:domain vcard:Kind ;
  rdfs:domain vcard:VCard ;
  rdfs:domain _:b57053 ;
  rdfs:isDefinedBy <http://www.w3.org/2006/vcard/ns> ;
  rdfs:label "role" ;
  rdfs:label "role"@en ;
  rdfs:range xsd:string ;
.
vcard:sort-string
  rdf:type owl:DatatypeProperty ;
  rdfs:comment "A version of a person's name suitable for collation" ;
  rdfs:comment "To specify the string to be used for national-language-specific sorting. Used as a property parameter only."@en ;
  rdfs:domain owl:Thing ;
  rdfs:domain vcard:Kind ;
  rdfs:domain vcard:VCard ;
  rdfs:domain _:b57053 ;
  rdfs:isDefinedBy <http://www.w3.org/2006/vcard/ns> ;
  rdfs:label "sort as"@en ;
  rdfs:label "sort" ;
  rdfs:range xsd:string ;
.
vcard:sound
  rdf:type owl:ObjectProperty ;
  rdfs:comment "A sound (e.g., a greeting or pronounciation) of a person" ;
  rdfs:comment "This object property has been mapped"@en ;
  rdfs:domain owl:Thing ;
  rdfs:domain vcard:Kind ;
  rdfs:domain vcard:VCard ;
  rdfs:domain _:b57053 ;
  rdfs:isDefinedBy <http://www.w3.org/2006/vcard/ns> ;
  rdfs:label "sound" ;
  rdfs:label "sound"@en ;
  rdfs:subPropertyOf vcard:hasSound ;
  owl:equivalentProperty vcard:hasSound ;
.
vcard:street-address
  rdf:type owl:DatatypeProperty ;
  rdfs:comment "The street address associated with the address of the object"@en ;
  rdfs:comment "The street address of a postal address" ;
  rdfs:domain elobr:EloniaAddress ;
  rdfs:domain freebr:FreedoniaAddress ;
  rdfs:domain toop:Address ;
  rdfs:domain owl:Thing ;
  rdfs:domain vcard:Address ;
  rdfs:domain _:b49042 ;
  rdfs:domain _:b83024 ;
  rdfs:domain _:b157701 ;
  rdfs:domain _:b168676 ;
  rdfs:domain _:b396249 ;
  rdfs:domain _:b401324 ;
  rdfs:domain _:b499218 ;
  rdfs:domain _:b541374 ;
  rdfs:domain _:b583853 ;
  rdfs:domain _:b652026 ;
  rdfs:domain _:b726818 ;
  rdfs:domain _:b763315 ;
  rdfs:domain _:b787338 ;
  rdfs:domain _:b926654 ;
  rdfs:domain _:b955705 ;
  rdfs:isDefinedBy <http://www.w3.org/2006/vcard/ns> ;
  rdfs:label "street address"@en ;
  rdfs:label "street" ;
  rdfs:range xsd:string ;
  owl:equivalentProperty toop:streetAddress ;
.
vcard:tel
  rdf:type owl:ObjectProperty ;
  rdfs:comment "A telephone number of a person" ;
  rdfs:comment "This object property has been mapped"@en ;
  rdfs:domain dcterms:Agent ;
  rdfs:domain toop:RegisteredOrganization ;
  rdfs:domain owl:Thing ;
  rdfs:domain vcard:Kind ;
  rdfs:domain vcard:VCard ;
  rdfs:domain org:FormalOrganization ;
  rdfs:domain org:Organization ;
  rdfs:domain rov:RegisteredOrganization ;
  rdfs:domain foaf:Agent ;
  rdfs:domain foaf:Organization ;
  rdfs:domain _:b57053 ;
  rdfs:domain _:b180769 ;
  rdfs:domain _:b254570 ;
  rdfs:domain _:b420951 ;
  rdfs:domain _:b421075 ;
  rdfs:domain _:b421664 ;
  rdfs:domain _:b421928 ;
  rdfs:domain _:b454254 ;
  rdfs:domain _:b826282 ;
  rdfs:domain _:b826680 ;
  rdfs:domain _:b937877 ;
  rdfs:domain _:b938265 ;
  rdfs:isDefinedBy <http://www.w3.org/2006/vcard/ns> ;
  rdfs:label "phone" ;
  rdfs:label "telephone"@en ;
  rdfs:range toop:CompanyContactNumber ;
  rdfs:range owl:Thing ;
  rdfs:subPropertyOf vcard:hasTelephone ;
  owl:equivalentProperty toop:companyContactNumber ;
  owl:equivalentProperty vcard:hasTelephone ;
.
vcard:title
  rdf:type owl:DatatypeProperty ;
  rdfs:comment "A person's title" ;
  rdfs:comment "To specify the position or job of the object"@en ;
  rdfs:domain owl:Thing ;
  rdfs:domain vcard:Kind ;
  rdfs:domain vcard:VCard ;
  rdfs:domain _:b57053 ;
  rdfs:isDefinedBy <http://www.w3.org/2006/vcard/ns> ;
  rdfs:label "title" ;
  rdfs:label "title"@en ;
  rdfs:range xsd:string ;
.
vcard:tz
  rdf:type owl:DatatypeProperty ;
  rdfs:comment "A timezone associated with a person" ;
  rdfs:comment "To indicate time zone information that is specific to the object. May also be used as a property parameter."@en ;
  rdfs:domain owl:Thing ;
  rdfs:domain vcard:Kind ;
  rdfs:domain vcard:VCard ;
  rdfs:domain _:b57053 ;
  rdfs:isDefinedBy <http://www.w3.org/2006/vcard/ns> ;
  rdfs:label "time zone"@en ;
  rdfs:label "timezone" ;
  rdfs:range xsd:string ;
.
vcard:uid
  rdf:type owl:DatatypeProperty ;
  rdfs:comment "A UID of a person's vCard" ;
  rdfs:domain owl:Thing ;
  rdfs:domain vcard:Kind ;
  rdfs:domain vcard:VCard ;
  rdfs:domain _:b57053 ;
  rdfs:label "uid" ;
.
vcard:url
  rdf:type owl:ObjectProperty ;
  rdfs:comment "A URL associated with a person" ;
  rdfs:comment "This object property has been mapped"@en ;
  rdfs:domain owl:Thing ;
  rdfs:domain vcard:Kind ;
  rdfs:domain vcard:VCard ;
  rdfs:domain _:b57053 ;
  rdfs:isDefinedBy <http://www.w3.org/2006/vcard/ns> ;
  rdfs:label "url" ;
  rdfs:label "url"@en ;
  rdfs:subPropertyOf vcard:hasURL ;
  owl:equivalentProperty vcard:hasURL ;
.
vcard:value
  rdf:type owl:DatatypeProperty ;
  rdfs:comment "Used to indicate the literal value of a data property that requires property parameters"@en ;
  rdfs:isDefinedBy <http://www.w3.org/2006/vcard/ns> ;
  rdfs:label "value"@en ;
.
<http://www.w3.org/2008/05/skos-xl>
  rdf:type elobr:EloniaBusinessCode ;
  rdf:type freebr:FreedoniaBusinessCode ;
  elobr:EloniaRegistrationAuthority "Alistair Miles" ;
  elobr:EloniaRegistrationAuthority "Sean Bechhofer" ;
  freebr:FreedoniaRegistrationAuthority "Alistair Miles" ;
  freebr:FreedoniaRegistrationAuthority "Sean Bechhofer" ;
  dc:contributor "Alistair Miles" ;
  dc:contributor "Participants in W3C's Semantic Web Deployment Working Group." ;
  dc:contributor "Scott Henninger and Holger Knublauch (for this modified version)" ;
  dc:contributor "Sean Bechhofer" ;
  dc:creator "Alistair Miles" ;
  dc:creator "Sean Bechhofer" ;
  dc:description "An RDF vocabulary extending SKOS and allowing the description and linking of lexical entities."@en ;
  dc:title "SKOS XL Vocabulary"@en ;
  dcterms:contributor "Alistair Miles" ;
  dcterms:contributor "Participants in W3C's Semantic Web Deployment Working Group." ;
  dcterms:contributor "Scott Henninger and Holger Knublauch (for this modified version)" ;
  dcterms:contributor "Sean Bechhofer" ;
  dcterms:creator "Alistair Miles" ;
  dcterms:creator "Sean Bechhofer" ;
  dcterms:description "An RDF vocabulary extending SKOS and allowing the description and linking of lexical entities."@en ;
  dcterms:title "SKOS XL Vocabulary"@en ;
  toop:registrationAuthority "Alistair Miles" ;
  toop:registrationAuthority "Sean Bechhofer" ;
  rdfs:comment """This is a modified version of SKOS-XL that is optimized for use within TopBraid. The changes compared to the official version are:

- introduced a prefix \"skosxl\"
- the domain of skosxl:altLabel and skosxl:hiddenLabel is skos:Concept
- skosxl:literalForm has been made an rdfs:subPropertyOf rdfs:label
- skosxl:Label has been asserted to be a subclass of owl:Thing
- the restriction that each skosxl:Label must have exactly one value has been changed to min 1 to allow values in multiple languages.
- the rdfs:labels of the skosxl:xyLabel properties have been changed to include \"(object)\" to distinguish them from the namesake skos properties.""" ;
  rdfs:label "SKOS XL Vocabulary" ;
  rdfs:seeAlso <http://www.w3.org/2008/05/skos> ;
  foaf:maker "Alistair Miles" ;
  foaf:maker "Sean Bechhofer" ;
.
skosxl:Label
  rdf:type owl:Class ;
  rdfs:isDefinedBy <http://www.w3.org/2008/05/skos-xl> ;
  rdfs:label "Label"@en ;
  rdfs:subClassOf owl:Thing ;
  rdfs:subClassOf _:b481819 ;
  owl:disjointWith skos:Collection ;
  owl:disjointWith skos:Concept ;
  owl:disjointWith skos:ConceptScheme ;
  skos:definition "A special class of lexical entities."@en ;
  skos:note "A special class of lexical entities."@en ;
.
skosxl:altLabel
  rdf:type rdf:Property ;
  rdf:type owl:ObjectProperty ;
  rdfs:comment "If C skosxl:altLabel L and L skosxl:literalForm V, then X skos:altLabel V."@en ;
  rdfs:domain owl:Thing ;
  rdfs:domain skos:Concept ;
  rdfs:domain _:b327858 ;
  rdfs:isDefinedBy <http://www.w3.org/2008/05/skos-xl> ;
  rdfs:label "alternative label (object)"@en ;
  rdfs:range owl:Thing ;
  rdfs:range skosxl:Label ;
  rdfs:range _:b481819 ;
  rdfs:seeAlso skos:altLabel ;
  skos:definition "The property skosxl:altLabel is used to associate an skosxl:Label with a skos:Concept. The property is analogous to skos:altLabel."@en ;
  skos:note "The property skosxl:altLabel is used to associate an skosxl:Label with a skos:Concept. The property is analogous to skos:altLabel."@en ;
.
skosxl:hiddenLabel
  rdf:type rdf:Property ;
  rdf:type owl:ObjectProperty ;
  rdfs:comment "If C skosxl:hiddenLabel L and L skosxl:literalForm V, then C skos:hiddenLabel V."@en ;
  rdfs:domain owl:Thing ;
  rdfs:domain skos:Concept ;
  rdfs:domain _:b327858 ;
  rdfs:isDefinedBy <http://www.w3.org/2008/05/skos-xl> ;
  rdfs:label "hidden label (object)"@en ;
  rdfs:range owl:Thing ;
  rdfs:range skosxl:Label ;
  rdfs:range _:b481819 ;
  rdfs:seeAlso skos:hiddenLabel ;
  skos:definition "The property skosxl:hiddenLabel is used to associate an skosxl:Label with a skos:Concept. The property is analogous to skos:hiddenLabel."@en ;
  skos:note "The property skosxl:hiddenLabel is used to associate an skosxl:Label with a skos:Concept. The property is analogous to skos:hiddenLabel."@en ;
.
skosxl:labelRelation
  rdf:type rdf:Property ;
  rdf:type owl:ObjectProperty ;
  rdf:type owl:SymmetricProperty ;
  rdfs:domain owl:Thing ;
  rdfs:domain skosxl:Label ;
  rdfs:domain _:b481819 ;
  rdfs:isDefinedBy <http://www.w3.org/2008/05/skos-xl> ;
  rdfs:label "label relation"@en ;
  rdfs:range owl:Thing ;
  rdfs:range skosxl:Label ;
  rdfs:range _:b481819 ;
  skos:definition "The property skosxl:labelRelation is used for representing binary ('direct') relations between instances of the class skosxl:Label."@en ;
  skos:note "The property skosxl:labelRelation is used for representing binary ('direct') relations between instances of the class skosxl:Label."@en ;
  skos:note "skosxl:labelRelation is not intended to be used directly, but rather as the basis for a design pattern which can be refined for more specific labeling scenarios."@en ;
  skos:scopeNote "skosxl:labelRelation is not intended to be used directly, but rather as the basis for a design pattern which can be refined for more specific labeling scenarios."@en ;
.
skosxl:literalForm
  rdf:type rdf:Property ;
  rdf:type owl:DatatypeProperty ;
  rdfs:comment "If two instances of the class skosxl:Label have the same literal form, they are not necessarily the same resource."@en ;
  rdfs:comment "The range of skosxl:literalForm is the class of RDF plain literals."@en ;
  rdfs:domain owl:Thing ;
  rdfs:domain skosxl:Label ;
  rdfs:domain _:b481819 ;
  rdfs:isDefinedBy <http://www.w3.org/2008/05/skos-xl> ;
  rdfs:label "literal form"@en ;
  rdfs:subPropertyOf rdfs:label ;
  skos:definition "The property skosxl:literalForm is used to give the literal form of an skosxl:Label."@en ;
  skos:note "The property skosxl:literalForm is used to give the literal form of an skosxl:Label."@en ;
.
skosxl:prefLabel
  rdf:type rdf:Property ;
  rdf:type owl:ObjectProperty ;
  rdfs:comment "If C skosxl:prefLabel L and L skosxl:literalForm V, then X skos:prefLabel V."@en ;
  rdfs:isDefinedBy <http://www.w3.org/2008/05/skos-xl> ;
  rdfs:label "preferred label (object)"@en ;
  rdfs:range owl:Thing ;
  rdfs:range skosxl:Label ;
  rdfs:range _:b481819 ;
  rdfs:seeAlso skos:prefLabel ;
  skos:definition "The property skosxl:prefLabel is used to associate an skosxl:Label with a skos:Concept. The property is analogous to skos:prefLabel."@en ;
  skos:note "The property skosxl:prefLabel is used to associate an skosxl:Label with a skos:Concept. The property is analogous to skos:prefLabel."@en ;
.
<http://www.w3.org/2011/gld/>
  rdf:type schema:CreativeWork ;
  rdf:type foaf:Document ;
  foaf:primaryTopic _:b11589 ;
  foaf:topic _:b11589 ;
  foaf:topic _:b251823 ;
  foaf:topic _:b421509 ;
  foaf:topic _:b421773 ;
.
<http://www.w3.org/People/all#phila>
  rdf:type schema:CreativeWork ;
  rdf:type foaf:Document ;
  foaf:primaryTopic _:b421866 ;
  foaf:primaryTopic _:b421897 ;
  foaf:primaryTopic _:b937319 ;
  foaf:primaryTopic _:b937970 ;
  foaf:topic _:b421866 ;
  foaf:topic _:b421897 ;
  foaf:topic _:b937319 ;
  foaf:topic _:b937970 ;
.
<http://www.w3.org/TR/2013/NOTE-vocab-adms-20130528/adms20130520.png>
  rdf:type schema:CreativeWork ;
  rdf:type schema:ImageObject ;
  rdf:type foaf:Image ;
  rdfs:label "Asset Description Metadata Schema (ADMS) UML Class Diagram" ;
  foaf:depicts <http://www.w3.org/ns/adms> ;
.
<http://www.w3.org/TR/2013/NOTE-vocab-regorg-20130528/>
  dc:title "Registered Organization Vocabulary" ;
  dcterms:title "Registered Organization Vocabulary" ;
.
<http://www.w3.org/TR/2013/NOTE-vocab-regorg-20130528/regorg20130508.png>
  rdf:type schema:CreativeWork ;
  rdf:type schema:ImageObject ;
  rdf:type foaf:Image ;
  rdfs:label "Registered Organization vocabulary UML Class Diagram" ;
  foaf:depicts <http://www.w3.org/ns/regorg> ;
.
<http://www.w3.org/TR/vocab-adms/>
  dc:title "Asset Description Metadata Schema (ADMS)" ;
  dcterms:title "Asset Description Metadata Schema (ADMS)" ;
.
<http://www.w3.org/ns/adms>
  rdf:type elobr:EloniaBusinessCode ;
  rdf:type freebr:FreedoniaBusinessCode ;
  rdf:type <http://labs.mondeca.com/vocab/voaf#Vocabulary> ;
  elobr:EloniaRegistrationAuthority _:b421509 ;
  elobr:EloniaRegistrationAuthority _:b421602 ;
  elobr:EloniaRegistrationAuthority _:b421773 ;
  elobr:EloniaRegistrationAuthority _:b421866 ;
  elobr:EloniaRegistrationAuthority _:b421897 ;
  elobr:EloniaRegistrationAuthority _:b937319 ;
  elobr:EloniaRegistrationAuthority _:b937381 ;
  elobr:EloniaRegistrationAuthority _:b937505 ;
  elobr:EloniaRegistrationAuthority _:b937610 ;
  elobr:EloniaRegistrationAuthority _:b937939 ;
  elobr:EloniaRegistrationAuthority _:b937970 ;
  elobr:EloniaRegistrationAuthority _:b938203 ;
  elobr:EloniaRegistrationAuthority _:b938234 ;
  elobr:EloniaRegistrationAuthority _:b938246 ;
  freebr:FreedoniaRegistrationAuthority _:b421509 ;
  freebr:FreedoniaRegistrationAuthority _:b421602 ;
  freebr:FreedoniaRegistrationAuthority _:b421773 ;
  freebr:FreedoniaRegistrationAuthority _:b421866 ;
  freebr:FreedoniaRegistrationAuthority _:b421897 ;
  freebr:FreedoniaRegistrationAuthority _:b937319 ;
  freebr:FreedoniaRegistrationAuthority _:b937381 ;
  freebr:FreedoniaRegistrationAuthority _:b937505 ;
  freebr:FreedoniaRegistrationAuthority _:b937610 ;
  freebr:FreedoniaRegistrationAuthority _:b937939 ;
  freebr:FreedoniaRegistrationAuthority _:b937970 ;
  freebr:FreedoniaRegistrationAuthority _:b938203 ;
  freebr:FreedoniaRegistrationAuthority _:b938234 ;
  freebr:FreedoniaRegistrationAuthority _:b938246 ;
  dc:contributor _:b421509 ;
  dc:contributor _:b421602 ;
  dc:contributor _:b421773 ;
  dc:contributor _:b421866 ;
  dc:contributor _:b421897 ;
  dc:contributor _:b937319 ;
  dc:contributor _:b937381 ;
  dc:contributor _:b937505 ;
  dc:contributor _:b937610 ;
  dc:contributor _:b937939 ;
  dc:contributor _:b937970 ;
  dc:contributor _:b938203 ;
  dc:contributor _:b938234 ;
  dc:contributor _:b938246 ;
  dc:creator _:b421509 ;
  dc:creator _:b421602 ;
  dc:creator _:b421773 ;
  dc:creator _:b421866 ;
  dc:creator _:b421897 ;
  dc:creator _:b937319 ;
  dc:creator _:b937381 ;
  dc:creator _:b937505 ;
  dc:creator _:b937610 ;
  dc:creator _:b937939 ;
  dc:creator _:b937970 ;
  dc:creator _:b938203 ;
  dc:creator _:b938234 ;
  dc:creator _:b938246 ;
  dc:date "2013-05-24"^^xsd:date ;
  dc:date "2013-12-21"^^xsd:date ;
  dc:date "2015-07-22"^^xsd:date ;
  dc:description "ADMS is a profile of DCAT, used to describe semantic assets (or just 'Assets'), defined as highly reusable metadata (e.g. xml schemata, generic data models) and reference data (e.g. code lists, taxonomies, dictionaries, vocabularies) that are used for eGovernment system development." ;
  dc:description """This is the RDF encoding of the 
      <a xmlns=\"http://www.w3.org/ns/adms#\" href=\"http://www.w3.org/TR/vocab-adms/\">Asset Description Metadata Schema</a>, 
      originally developed under the European Union's <a xmlns=\"http://www.w3.org/ns/adms#\" href=\"http://ec.europa.eu/isa/\">ISA Programme</a> 
      and further developed by the W3C <a xmlns=\"http://www.w3.org/ns/adms#\" href=\"http://www.w3.org/2011/gld/\">Government Linked Data Working Group</a>. It re-uses terms 
      from several other vocabularies, notably Dublin Core, with elements of SKOS, FOAF 
      and more.
    """^^rdf:XMLLiteral ;
  dcterms:abstract "ADMS is a profile of DCAT, used to describe semantic assets (or just 'Assets'), defined as highly reusable metadata (e.g. xml schemata, generic data models) and reference data (e.g. code lists, taxonomies, dictionaries, vocabularies) that are used for eGovernment system development." ;
  dcterms:contributor _:b421509 ;
  dcterms:contributor _:b421602 ;
  dcterms:contributor _:b421773 ;
  dcterms:contributor _:b421866 ;
  dcterms:contributor _:b421897 ;
  dcterms:contributor _:b937319 ;
  dcterms:contributor _:b937381 ;
  dcterms:contributor _:b937505 ;
  dcterms:contributor _:b937610 ;
  dcterms:contributor _:b937939 ;
  dcterms:contributor _:b937970 ;
  dcterms:contributor _:b938203 ;
  dcterms:contributor _:b938234 ;
  dcterms:contributor _:b938246 ;
  dcterms:creator _:b421509 ;
  dcterms:creator _:b421602 ;
  dcterms:creator _:b421773 ;
  dcterms:creator _:b421866 ;
  dcterms:creator _:b421897 ;
  dcterms:creator _:b937319 ;
  dcterms:creator _:b937381 ;
  dcterms:creator _:b937505 ;
  dcterms:creator _:b937610 ;
  dcterms:creator _:b937939 ;
  dcterms:creator _:b937970 ;
  dcterms:creator _:b938203 ;
  dcterms:creator _:b938234 ;
  dcterms:creator _:b938246 ;
  dcterms:date "2013-05-24"^^xsd:date ;
  dcterms:date "2013-12-21"^^xsd:date ;
  dcterms:date "2015-07-22"^^xsd:date ;
  dcterms:description "ADMS is a profile of DCAT, used to describe semantic assets (or just 'Assets'), defined as highly reusable metadata (e.g. xml schemata, generic data models) and reference data (e.g. code lists, taxonomies, dictionaries, vocabularies) that are used for eGovernment system development." ;
  dcterms:description """This is the RDF encoding of the 
      <a xmlns=\"http://www.w3.org/ns/adms#\" href=\"http://www.w3.org/TR/vocab-adms/\">Asset Description Metadata Schema</a>, 
      originally developed under the European Union's <a xmlns=\"http://www.w3.org/ns/adms#\" href=\"http://ec.europa.eu/isa/\">ISA Programme</a> 
      and further developed by the W3C <a xmlns=\"http://www.w3.org/ns/adms#\" href=\"http://www.w3.org/2011/gld/\">Government Linked Data Working Group</a>. It re-uses terms 
      from several other vocabularies, notably Dublin Core, with elements of SKOS, FOAF 
      and more.
    """^^rdf:XMLLiteral ;
  dcterms:modified "2013-05-24"^^xsd:date ;
  dcterms:modified "2013-12-21"^^xsd:date ;
  dcterms:modified "2015-07-22"^^xsd:date ;
  vann:preferredNamespacePrefix "adms" ;
  vann:preferredNamespaceUri "http://www.w3.org/ns/adms#" ;
  voaf:specializes <http://www.w3.org/dcat> ;
  toop:registrationAuthority _:b421509 ;
  toop:registrationAuthority _:b421602 ;
  toop:registrationAuthority _:b421773 ;
  toop:registrationAuthority _:b421866 ;
  toop:registrationAuthority _:b421897 ;
  toop:registrationAuthority _:b937319 ;
  toop:registrationAuthority _:b937381 ;
  toop:registrationAuthority _:b937505 ;
  toop:registrationAuthority _:b937610 ;
  toop:registrationAuthority _:b937939 ;
  toop:registrationAuthority _:b937970 ;
  toop:registrationAuthority _:b938203 ;
  toop:registrationAuthority _:b938234 ;
  toop:registrationAuthority _:b938246 ;
  rdfs:comment "This file specifies the set of RDF classes and properties used in ADMS"@en ;
  rdfs:label "Asset Description Metadata Schema (ADMS)"@en ;
  owl:versionInfo "21 December 2013 - with correction to URI of the schema cf. using the namespace"@en ;
  wdrs:describedby <http://www.w3.org/TR/vocab-adms/> ;
  foaf:depiction <http://www.w3.org/TR/2013/NOTE-vocab-adms-20130528/adms20130520.png> ;
  foaf:maker _:b421509 ;
  foaf:maker _:b421602 ;
  foaf:maker _:b421773 ;
  foaf:maker _:b421866 ;
  foaf:maker _:b421897 ;
  foaf:maker _:b937319 ;
  foaf:maker _:b937381 ;
  foaf:maker _:b937505 ;
  foaf:maker _:b937610 ;
  foaf:maker _:b937939 ;
  foaf:maker _:b937970 ;
  foaf:maker _:b938203 ;
  foaf:maker _:b938234 ;
  foaf:maker _:b938246 ;
.
adms:Asset
  rdf:type rdfs:Class ;
  dc:identifier "adms:Asset" ;
  dcterms:identifier "adms:Asset" ;
  rdfs:comment "An Asset is an abstract entity that reflects the intellectual content of the asset and represents those characteristics of the asset that are independent of its physical embodiment. This abstract entity combines the FRBR entities work (a distinct intellectual or artistic creation) and expression (the intellectual or artistic realization of a work). Assets can be versioned. Every time the intellectual content of an asset changes, the result is considered to be a new asset that can be linked to previous and next versions of the Asset. The physical embodiment of an Asset is called an Asset Distribution. A particular Asset may have zero or more Asset Distributions."@en ;
  rdfs:isDefinedBy <http://www.w3.org/TR/vocab-adms/> ;
  rdfs:label "Asset"@en ;
  rdfs:subClassOf rdfs:Resource ;
  rdfs:subClassOf dcat:Dataset ;
.
adms:AssetDistribution
  rdf:type rdfs:Class ;
  dc:identifier "adms:AssetDistribution" ;
  dcterms:identifier "adms:AssetDistribution" ;
  rdfs:comment "An Asset Distribution represents a particular physical embodiment of an Asset, which is an example of the FRBR entity manifestation (the physical embodiment of an expression of a work). An Asset Distribution is typically a downloadable computer file (but in principle it could also be a paper document) that implements the intellectual content of an Asset. A particular Asset Distribution is associated with one and only one Asset, while all Distributions of an Asset share the same intellectual content in different physical formats. Asset Distributions themselves are not versioned."@en ;
  rdfs:isDefinedBy <http://www.w3.org/TR/vocab-adms/> ;
  rdfs:label "Asset Distribution"@en ;
  rdfs:subClassOf rdfs:Resource ;
  rdfs:subClassOf dcat:Distribution ;
.
adms:AssetRepository
  rdf:type rdfs:Class ;
  dc:identifier "adms:AssetRepository" ;
  dcterms:identifier "adms:AssetRepository" ;
  rdfs:comment "An Asset Repository is a system or service that provides facilities for storage and maintenance of descriptions of Assets and Asset Distributions, and functionality that allows users to search and access these descriptions. An Asset Repository will typically contain descriptions of several Assets and related Asset Distributions."@en ;
  rdfs:isDefinedBy <http://www.w3.org/TR/vocab-adms/> ;
  rdfs:label "Asset Repository"@en ;
  rdfs:subClassOf rdfs:Resource ;
  rdfs:subClassOf dcat:Catalog ;
.
adms:Identifier
  rdf:type rdfs:Class ;
  dc:identifier "adms:Identifier" ;
  dcterms:identifier "adms:Identifier" ;
  rdfs:comment """This class is based on the UN/CEFACT 
    Identifier complex type defined in See Section 5.8 of Core Components Data Type Catalogue Version 3.1 (http://www.unece.org/fileadmin/DAM/cefact/codesfortrade/CCTS/CCTS-DTCatalogueVersion3p1.pdf)
    In RDF this is expressed using the following properties:
    - the content string should be provided using skos:notation, datatyped with the identifier scheme (inclduing the version number if appropriate);
    - use dcterms:creator to link to a class describing the agency that manages the identifier scheme or adms:schemaAgency to provide the name as a literal.
    Although not part of the ADMS conceptual model, it may be useful to provide further properties to the Identifier class such as
    dcterms:created to provide the date on which the identifier was issued."""^^rdf:XMLLiteral ;
  rdfs:isDefinedBy <http://www.w3.org/TR/vocab-adms/> ;
  rdfs:label "Identifier"@en ;
  rdfs:subClassOf rdfs:Resource ;
.
adms:identifier
  rdf:type rdf:Property ;
  rdf:type owl:ObjectProperty ;
  dc:identifier "adms:identifier" ;
  dcterms:identifier "adms:identifier" ;
  rdfs:comment """adms:identifier is used to link any resource to 
      an instance of adms:Identifier which is its range. N.B. it is not appropriate to use 
      dcterms:identifer to link to the Identifier class as its range is rdfs:Literal.
      ADMS uses this to provide any identifier for the Asset."""^^rdf:XMLLiteral ;
  rdfs:isDefinedBy <http://www.w3.org/TR/vocab-adms/> ;
  rdfs:label "identifier"@en ;
  rdfs:range adms:Identifier ;
.
adms:includedAsset
  rdf:type rdf:Property ;
  rdf:type owl:ObjectProperty ;
  dc:identifier "adms:includedAsset" ;
  dcterms:identifier "adms:includedAsset" ;
  rdfs:comment "Links to an Asset that is contained in the Asset being described, e.g. when there are several vocabularies defined in a single document."@en ;
  rdfs:domain adms:Asset ;
  rdfs:domain dcat:Dataset ;
  rdfs:isDefinedBy <http://www.w3.org/TR/vocab-adms/> ;
  rdfs:label "included asset"@en ;
  rdfs:range adms:Asset ;
  rdfs:range dcat:Dataset ;
.
adms:interoperabilityLevel
  rdf:type rdf:Property ;
  rdf:type owl:ObjectProperty ;
  dc:identifier "adms:interoperabilityLevel" ;
  dcterms:identifier "adms:interoperabilityLevel" ;
  rdfs:comment "Links an Asset to its adms:InteroperabilityLevel. Since this is encoded using skos:Concept, that is the defined range for this property."^^rdf:XMLLiteral ;
  rdfs:domain adms:Asset ;
  rdfs:domain dcat:Dataset ;
  rdfs:isDefinedBy <http://www.w3.org/TR/vocab-adms/> ;
  rdfs:label "interoperability level"@en ;
  rdfs:range owl:Thing ;
  rdfs:range skos:Concept ;
  rdfs:range _:b327858 ;
.
adms:last
  rdf:type rdf:Property ;
  rdf:type owl:ObjectProperty ;
  dc:identifier "adms:last" ;
  dcterms:identifier "adms:last" ;
  rdfs:comment "A link to the current or latest version of the Asset." ;
  rdfs:isDefinedBy <http://www.w3.org/TR/vocab-adms/> ;
  rdfs:label "last"@en ;
  rdfs:subPropertyOf <http://www.w3.org/1999/xhtml/vocab#last> ;
.
adms:next
  rdf:type rdf:Property ;
  rdf:type owl:ObjectProperty ;
  dc:identifier "adms:next" ;
  dcterms:identifier "adms:next" ;
  rdfs:comment "A link to the next version of the Asset." ;
  rdfs:isDefinedBy <http://www.w3.org/TR/vocab-adms/> ;
  rdfs:label "next"@en ;
  rdfs:subPropertyOf <http://www.w3.org/1999/xhtml/vocab#next> ;
.
adms:prev
  rdf:type rdf:Property ;
  rdf:type owl:ObjectProperty ;
  dc:identifier "adms:prev" ;
  dcterms:identifier "adms:prev" ;
  rdfs:comment "A link to the previous version of the Asset." ;
  rdfs:isDefinedBy <http://www.w3.org/TR/vocab-adms/> ;
  rdfs:label "prev"@en ;
  rdfs:subPropertyOf <http://www.w3.org/1999/xhtml/vocab#prev> ;
.
adms:representationTechnique
  rdf:type rdf:Property ;
  rdf:type owl:ObjectProperty ;
  dc:identifier "adms:representationTechnique" ;
  dcterms:identifier "adms:representationTechnique" ;
  rdfs:comment "Links an adms:AssetDistribution to a skos:Concept that is its adms:RepresentationTechnique."^^rdf:XMLLiteral ;
  rdfs:isDefinedBy <http://www.w3.org/TR/vocab-adms/> ;
  rdfs:label "representation technique"@en ;
  rdfs:range owl:Thing ;
  rdfs:range skos:Concept ;
  rdfs:range _:b327858 ;
.
adms:sample
  rdf:type rdf:Property ;
  rdf:type owl:ObjectProperty ;
  dc:identifier "adms:sample" ;
  dcterms:identifier "adms:sample" ;
  rdfs:comment "Links to a sample of an Asset (which is itself an Asset)."@en ;
  rdfs:domain adms:Asset ;
  rdfs:domain dcat:Dataset ;
  rdfs:isDefinedBy <http://www.w3.org/TR/vocab-adms/> ;
  rdfs:label "sample"@en ;
  rdfs:range adms:Asset ;
  rdfs:range dcat:Dataset ;
.
adms:schemeAgency
  rdf:type rdf:Property ;
  rdf:type owl:DatatypeProperty ;
  dc:identifier "adms:schemeAgency" ;
  dcterms:identifier "adms:schemeAgency" ;
  rdfs:comment "The name of the agency responsible for issuing the identifier"@en ;
  rdfs:domain adms:Identifier ;
  rdfs:isDefinedBy <http://www.w3.org/TR/vocab-adms/> ;
  rdfs:label "scheme agency"@en ;
  rdfs:range rdfs:Literal ;
.
adms:status
  rdf:type rdf:Property ;
  rdf:type owl:ObjectProperty ;
  dc:identifier "adms:status" ;
  dcterms:identifier "adms:status" ;
  rdfs:comment """Links to the status of the Asset or Asset Distribution 
      in the context of a particular workflow process. Since Status is defined using a skos:Concept, 
      that is the defined range for this property."""^^rdf:XMLLiteral ;
  rdfs:isDefinedBy <http://www.w3.org/TR/vocab-adms/> ;
  rdfs:label "status"@en ;
  rdfs:range owl:Thing ;
  rdfs:range skos:Concept ;
  rdfs:range _:b327858 ;
.
adms:supportedSchema
  rdf:type rdf:Property ;
  rdf:type owl:ObjectProperty ;
  dc:identifier "adms:supportedSchema" ;
  dcterms:identifier "adms:supportedSchema" ;
  rdfs:comment "A schema according to which the Asset Repository can provide data about its content, e.g. ADMS"@en ;
  rdfs:isDefinedBy <http://www.w3.org/TR/vocab-adms/> ;
  rdfs:label "supported schema"@en ;
  rdfs:range adms:Asset ;
  rdfs:range dcat:Dataset ;
.
adms:translation
  rdf:type rdf:Property ;
  rdf:type owl:ObjectProperty ;
  dc:identifier "adms:translation" ;
  dcterms:identifier "adms:translation" ;
  rdfs:comment "Links Assets that are translations of each other."@en ;
  rdfs:isDefinedBy <http://www.w3.org/TR/vocab-adms/> ;
  rdfs:label "translation"@en ;
.
adms:versionNotes
  rdf:type rdf:Property ;
  rdf:type owl:DatatypeProperty ;
  dc:identifier "adms:versionNotes" ;
  dcterms:identifier "adms:versionNotes" ;
  rdfs:comment "A description of changes between this version and the previous version of the Asset."@en ;
  rdfs:isDefinedBy <http://www.w3.org/TR/vocab-adms/> ;
  rdfs:label "version notes"@en ;
  rdfs:range rdfs:Literal ;
.
org:
  dc:contributor _:b421013 ;
  dc:contributor _:b421044 ;
  dc:contributor _:b421106 ;
  dc:contributor _:b421215 ;
  dc:contributor _:b421277 ;
  dc:contributor _:b421308 ;
  dc:contributor _:b421339 ;
  dc:contributor _:b421401 ;
  dc:contributor _:b421497 ;
  dc:contributor _:b421540 ;
  dc:contributor _:b421571 ;
  dc:contributor _:b421633 ;
  dc:contributor _:b421835 ;
  dc:contributor _:b937284 ;
  dc:contributor _:b937346 ;
  dc:contributor _:b937408 ;
  dc:contributor _:b937486 ;
  dc:contributor _:b937548 ;
  dc:contributor _:b937583 ;
  dc:contributor _:b937672 ;
  dc:contributor _:b937769 ;
  dc:contributor _:b937908 ;
  dc:contributor _:b938001 ;
  dc:contributor _:b938032 ;
  dc:contributor _:b938110 ;
  dc:contributor _:b938141 ;
  dc:contributor _:b938172 ;
  dc:date "2010-05-28"^^xsd:date ;
  dc:date "2010-06-09"^^xsd:date ;
  dc:date "2010-10-08"^^xsd:date ;
  dc:date "2012-09-30"^^xsd:date ;
  dc:date "2012-10-06"^^xsd:date ;
  dc:date "2013-02-15"^^xsd:date ;
  dc:date "2013-12-16"^^xsd:date ;
  dc:date "2014-01-02"^^xsd:date ;
  dc:date "2014-01-25"^^xsd:date ;
  dc:date "2014-02-05"^^xsd:date ;
  dc:date "2014-04-12"^^xsd:date ;
  dc:rights <http://www.opendatacommons.org/licenses/pddl/1.0/> ;
  dc:title "Core organization ontology"@en ;
  dc:title "Ontologia delle organizzazioni"@it ;
  dc:title "Ontologie des organisations"@fr ;
  dc:title "Ontología de organizaciones"@es ;
  dcterms:contributor _:b421013 ;
  dcterms:contributor _:b421044 ;
  dcterms:contributor _:b421106 ;
  dcterms:contributor _:b421215 ;
  dcterms:contributor _:b421277 ;
  dcterms:contributor _:b421308 ;
  dcterms:contributor _:b421339 ;
  dcterms:contributor _:b421401 ;
  dcterms:contributor _:b421497 ;
  dcterms:contributor _:b421540 ;
  dcterms:contributor _:b421571 ;
  dcterms:contributor _:b421633 ;
  dcterms:contributor _:b421835 ;
  dcterms:contributor _:b937284 ;
  dcterms:contributor _:b937346 ;
  dcterms:contributor _:b937408 ;
  dcterms:contributor _:b937486 ;
  dcterms:contributor _:b937548 ;
  dcterms:contributor _:b937583 ;
  dcterms:contributor _:b937672 ;
  dcterms:contributor _:b937769 ;
  dcterms:contributor _:b937908 ;
  dcterms:contributor _:b938001 ;
  dcterms:contributor _:b938032 ;
  dcterms:contributor _:b938110 ;
  dcterms:contributor _:b938141 ;
  dcterms:contributor _:b938172 ;
  dcterms:created "2010-05-28"^^xsd:date ;
  dcterms:date "2010-05-28"^^xsd:date ;
  dcterms:date "2010-06-09"^^xsd:date ;
  dcterms:date "2010-10-08"^^xsd:date ;
  dcterms:date "2012-09-30"^^xsd:date ;
  dcterms:date "2012-10-06"^^xsd:date ;
  dcterms:date "2013-02-15"^^xsd:date ;
  dcterms:date "2013-12-16"^^xsd:date ;
  dcterms:date "2014-01-02"^^xsd:date ;
  dcterms:date "2014-01-25"^^xsd:date ;
  dcterms:date "2014-02-05"^^xsd:date ;
  dcterms:date "2014-04-12"^^xsd:date ;
  dcterms:license <http://www.opendatacommons.org/licenses/pddl/1.0/> ;
  dcterms:modified "2010-06-09"^^xsd:date ;
  dcterms:modified "2010-10-08"^^xsd:date ;
  dcterms:modified "2012-09-30"^^xsd:date ;
  dcterms:modified "2012-10-06"^^xsd:date ;
  dcterms:modified "2013-02-15"^^xsd:date ;
  dcterms:modified "2013-12-16"^^xsd:date ;
  dcterms:modified "2014-01-02"^^xsd:date ;
  dcterms:modified "2014-01-25"^^xsd:date ;
  dcterms:modified "2014-02-05"^^xsd:date ;
  dcterms:modified "2014-04-12"^^xsd:date ;
  dcterms:rights <http://www.opendatacommons.org/licenses/pddl/1.0/> ;
  dcterms:title "Core organization ontology"@en ;
  dcterms:title "Ontologia delle organizzazioni"@it ;
  dcterms:title "Ontologie des organisations"@fr ;
  dcterms:title "Ontología de organizaciones"@es ;
  rdfs:comment "Vocabolario per descrivere strutture organizzative, le quali possono essere specializzate in una vasta varietà di tipi di organizzazione"@it ;
  rdfs:comment "Vocabulario para describir organizaciones, adaptable a una amplia variedad de ellas."@es ;
  rdfs:comment "Vocabulary for describing organizational structures, specializable to a broad variety of types of organization."@en ;
  rdfs:label "Core organization ontology"@en ;
  rdfs:label "Ontologia delle organizzazioni"@it ;
  rdfs:label "Ontologie des organisations"@fr ;
  rdfs:label "Ontología de organizaciones"@es ;
  rdfs:seeAlso <http://www.w3.org/TR/vocab-org/> ;
  owl:versionInfo "0.8" ;
.
org:ChangeEvent
  rdf:type rdfs:Class ;
  rdf:type owl:Class ;
  rdfs:comment "Evento que da como resultado un cambio sustancial en la organización, por ejemplo, una fusión o una reestructuración total. Está pensado para situaciones en las que la organización resultante es lo suficientemente distinta de las organizaciones originales, tiene una identidad distinta y una URI también distinta. Se deberían definir subtipos de eventos mediante vocabularios específicos (Extension vocabularies) para referirse a categorías de eventos específicos. El momento o periodo en el que el evento ocurre se debería expresar mediante las propiedades `prov:startAtTime` y `prov:endedAtTime`, y una descripción del mismo se debería incluir mediante el uso de la propiedad `dct:description`."@es ;
  rdfs:comment "Rappresenta un evento risultato essere un importante cambiamento per un'organizzazione come ad esempio una fusione o una riorganizzazione. È pensato per quelle situazioni in cui l'organizzazione risultante si distingue da quella originale sufficientemente da essere rappresentata con una URI differente. Le estensioni del vocabolario dovrebbero definire le sotto-classi per esprimere particolari categorie di eventi. L'istante o l'intervallo in cui l'evento accade dovrebbe essere espresso tramite `prov:startAtTime` e`prov:endedAtTime`. Una descrizione dovrebbe essere fornita attraverso `dct:description`."@it ;
  rdfs:comment "Represents an event which resulted in a major change to an organization such as a merger or complete restructuring. It is intended for situations where the resulting organization is sufficient distinct from the original organizations that it has a distinct identity and distinct URI. Extension vocabularies should define sub-classes of this to denote particular categories of event. The instant or interval at which the event occurred should be given by `prov:startAtTime` and `prov:endedAtTime`, a description should be given by `dct:description`. "@en ;
  rdfs:comment "Représente un Évènement impliquant un changement majeur dans l'Organisation, comme une fusion ou une restructuration. Prévu pour des situations ou l'organisation finale est suffisamment différente des Organisations originales pour qu'elle ait une identité et une URI distinctes. Des vocabulaires d'extension devraient définir des sous-classes de celle-ci pour annoter les différentes catégories d'Évènemenents. Le moment ou l'intervalle de l'Évènement devrait être indiqué avec `prov:startAtTime` et `prov:endedAtTime`, et une description avec la classe `dct:description`. "@fr ;
  rdfs:comment "合併や完全な再編などの組織に大きな変化をもたらした出来事を表わします。これは、結果として作成される組織と元の組織とが、別のアイデンティティーと別のURIを持つに足るほど異なる状況を対象としています。"@ja ;
  rdfs:isDefinedBy <http://www.w3.org/ns/org> ;
  rdfs:label "Change Event"@en ;
  rdfs:label "Evento di cambiamento"@it ;
  rdfs:label "evento de cambio"@es ;
  rdfs:label "Évènement"@fr ;
  rdfs:subClassOf prov:Activity ;
.
org:FormalOrganization
  rdf:type rdfs:Class ;
  rdf:type owl:Class ;
  rdfs:comment "An Organization which is recognized in the world at large, in particular in legal jurisdictions, with associated rights and responsibilities. Examples include a Corporation, Charity, Government or Church. Note that this is a super class of `gr:BusinessEntity` and it is recommended to use the GoodRelations vocabulary to denote Business classifications such as DUNS or NAICS."@en ;
  rdfs:comment "Organización reconocida a nivel mundial, en particular en jurisdicciones legales, con derechos y responsabilidades asociadas. Algunos ejemplos son: organización corporativa, organización benéfica, organización gubernamental, organización religiosa. Se debe tener en cuenta que ésta es una superclase de `gr:BusinessEntity` y que se recomienda el uso del vocabulario GoodRelations para referirse a clasificaciones de negocios tales como DUNS o NAICS."@es ;
  rdfs:comment "Un'organizzazione che è riconosciuta a livello mondiale o, in generale, all'interno di una qualche giurisdizione, e che quindi possiede diritti e responsabilità. Ad esempio aziende, enti governativi, associazioni di volontariato. Si noti che questa è una superclasse di `gr:BusinessEntity` e che quindi è raccomandabile usare il vocabolario GoodRelations per esprimere classificazioni di tipo industriale e commerciale come DUNS e NAICS."@it ;
  rdfs:comment "Une Organisation reconnue, en particulier par les juridictions locales, ayant des droits et des responsabilités. Exemples : entreprises, association à but non-lucratif, collectivité, église. Notez que c'est une super-classe de `gr:BusinessEntity` et qu'il est recommandé d'utiliser le vocabulaire GoodRelations pour indiquer les classifications économiques comme le code NACE."@fr ;
  rdfs:comment "関連する権利と責任を有する（特に法的管轄区域において）世界中に広く認識されている組織。例には、企業、慈善団体、政府や教会が含まれます。"@ja ;
  rdfs:isDefinedBy <http://www.w3.org/ns/org> ;
  rdfs:label "Formal Organization"@en ;
  rdfs:label "Organisation Formelle"@fr ;
  rdfs:label "Organizzazione formale"@it ;
  rdfs:label "organización formal"@es ;
  rdfs:subClassOf org:Organization ;
  rdfs:subClassOf foaf:Organization ;
.
org:Head
  rdf:type org:Role ;
  rdf:type _:b327858 ;
  rdfs:comment "A role corresponding to the `org:headOf` property"@en ;
  rdfs:comment "Actividad correspondiente a la propiedad `org:headOf`."@es ;
  rdfs:comment "Un ruolo corrispondente alla proprietà `org:headOf`."@it ;
  rdfs:comment "Un rôle correspondant à la propriété `org:headOf`"@fr ;
  rdfs:isDefinedBy <http://www.w3.org/ns/org> ;
  rdfs:label "director ejecutivo"@es ;
  rdfs:label "directora ejecutiva"@es ;
  rdfs:label "head"@en ;
  rdfs:label "responsabile"@it ;
  rdfs:label "responsable"@fr ;
  skos:prefLabel "head"@en ;
  skos:prefLabel "responsabile"@it ;
  skos:prefLabel "responsable"@fr ;
  org:roleProperty org:headOf ;
.
org:Membership
  rdf:type rdfs:Class ;
  rdf:type owl:Class ;
  rdfs:comment "Indica la natura della relazione di appartenenza di un Agent in un'organizzazione. Rappresenta una relazione n-aria tra un'Agent, un Organization e un Role. È possibile indicare direttamente la membership, indipendentemente dallo specifico Role, attraverso l'uso della proprietà `org:memberOf`"@it ;
  rdfs:comment "Indicates the nature of an Agent's membership of an organization. Represents an n-ary relation between an Agent, an Organization and a Role. It is possible to directly indicate membership, independent of the specific Role, through use of the `org:memberOf` property."@en ;
  rdfs:comment "Indique la nature de l'engagement d'un Agent dans une Organisation. Représente une relation n-aire entre un Agent, une Organisation et un Role. Il est possible d'indiquer directement l'appartenance à une organisation, independemment d'un rôle spécifique, à travers l'usage de la propriété `org:memberOf`."@fr ;
  rdfs:comment "Pertenencia o afiliación de un agente a una organización. Es una relación n-aria entre un agente, una organización y una actividad. Es posible indicar pertenencia mediante el uso de la propiedad `org:memberOf`, independientemente de la actividad específica que se desempeñe."@es ;
  rdfs:comment "組織のエージェントの構成員の本質を示します。"@ja ;
  rdfs:isDefinedBy <http://www.w3.org/ns/org> ;
  rdfs:label "Appartenenza"@it ;
  rdfs:label "Engagement"@fr ;
  rdfs:label "Membership"@en ;
  rdfs:label "membresía"@es ;
  rdfs:subClassOf owl:Thing ;
  owl:disjointWith org:ChangeEvent ;
  owl:disjointWith org:Site ;
.
org:Organization
  rdf:type rdfs:Class ;
  rdf:type owl:Class ;
  rdfs:comment "Grupo de personas que se organiza en una comunidad u otro tipo de estructura social, comercial o política. Dicho grupo tiene un objetivo o motivo común para su existencia que va más allá del conjunto de personas que lo forman y que puede actuar como “agente”. A menudo las organizaciones se pueden agrupar en estructuras jerárquicas. Se recomienda el uso de etiquetas de SKOS para denominar a cada “organización”. En concreto, `skos:prefLabel` para la denominación principal o recomendada (aquella reconocida legalmente, siempre que sea posible), `skos:altLabel` para denominaciones alternativas (nombre comercial, sigla, denominación por la que se conoce a la organización coloquialmente) y `skos:notation` para referirse al código que identifique a la organización en una lista de códigos. Denominaciones alternativas: _colectivo_ _corporación_ _grupo_"@es ;
  rdfs:comment "Rappresenta una collezione di persone organizzate all'interno di una communità o di una qualche struttura sociale, commerciale o politica. Il gruppo condivide un obiettivo o una ragione d'essere che va oltre gli stessi membri appartenenti al gruppo e  può agire come un Agent. Le organizzazioni si possono spesso suddividere in strutture gerarchiche. Si raccomanda di usare le label per l'Organization mediante le proprietà di SKOS. In particolare, `skos:prefLabel` per il nome principale (possibilmente un nome legalmente riconosciuto)”, `skos:altLabel` come nome alternativo (denominazione commerciale, denominazione colloquiale) e `skos:notation` per indicare un codice di una lista di codici."@it ;
  rdfs:comment "Represents a collection of people organized together into a community or other social, commercial or political structure. The group has some common purpose or reason for existence which goes beyond the set of people belonging to it and can act as an Agent. Organizations are often decomposable into hierarchical structures.  It is recommended that SKOS lexical labels should be used to label the Organization. In particular `skos:prefLabel` for the primary (possibly legally recognized name), `skos:altLabel` for alternative names (trading names, colloquial names) and `skos:notation` to denote a code from a code list. Alternative names: _Collective_ _Body_ _Org_ _Group_"@en ;
  rdfs:comment "Représente un groupe de personnes organisées en communauté où tout autre forme de structure sociale, commerciale ou politique. Le groupe a un but commun ou une raison d'être qui va au-delà de la somme des personnes qui en font partie et peut agir en tant que \"Agent\". Les organisations sont souvent décomposables en structures hiérarchisées. Il est recommandé que des labels lexicaux SKOS soient utilisés pour nommer l'Organisation. En particulier `skos:prefLabel` pour le nom principal (en général le nom légal), `skos:altLabel` pour les noms alternatifs (marques, sigles, appellations familières) et `skos:notation` pour indiquer un code provenant d'une liste de code."@fr ;
  rdfs:comment "コミュニティー、その他の社会、商業、政治的な構造に共に編入された人々の集合を表わします。グループには、そこに属する人々を超えた、存在に対するある共通の目的や理由があり、エージェント（代理）を務めることができます。組織は、多くの場合、階層構造に分割できます。"@ja ;
  rdfs:isDefinedBy <http://www.w3.org/ns/org> ;
  rdfs:label "Organisation"@fr ;
  rdfs:label "Organization"@en ;
  rdfs:label "Organizzazione"@it ;
  rdfs:label "organización"@es ;
  rdfs:subClassOf foaf:Agent ;
  rdfs:subClassOf foaf:Organization ;
  owl:disjointWith org:ChangeEvent ;
  owl:disjointWith org:Membership ;
  owl:disjointWith org:Role ;
  owl:disjointWith org:Site ;
  owl:equivalentClass foaf:Organization ;
  owl:hasKey (
      org:identifier
    ) ;
  owl:hasKey (
      org:identifier
    ) ;
  owl:hasKey (
      org:identifier
    ) ;
.
org:OrganizationalCollaboration
  rdf:type rdfs:Class ;
  rdf:type owl:Class ;
  rdfs:comment "A collaboration between two or more Organizations such as a project. It meets the criteria for being an Organization in that it has an identity and defining purpose independent of its particular members but is neither a formally recognized legal entity nor a sub-unit within some larger organization. Might typically have a shorter lifetime than the Organizations within it, but not necessarily. All members are `org:Organization`s rather than individuals and those Organizations can play particular roles within the venture. Alternative names: _Project_ _Venture_  _Endeavour_ _Consortium_ _Endeavour_"@en ;
  rdfs:comment "Colaboración determinada entre dos o más organizaciones, como en el caso de un proyecto común. Cumple con los criterios de ser una organización en sí misma, en la medida en que tiene una identidad y un propósito definido independiente de sus miembros en particular, pero no es una entidad legal formalmente reconocida ni una sub-unidad dentro de una organización más grande. La duración suele ser más corta que la de las organizaciones que lo componen, pero no necesariamente. Todos sus miembros son de tipo `org:Organization` en vez de individuos, y desempeñan una actividad concreta en el marco del proyecto de cooperación."@es ;
  rdfs:comment "Une collaboration entre deux ou plusieurs Organisations, telle qu'un projet commun. Un partenariat peut être considéré comme Organisation dans le sens ou il possède une identité et un But propre indépendant de ceux de ses membres, mais ce n'est ni une entité légale ni une sous-unité d'une Organisation plus grande. Typiquement, elle peut avoir une durée de vie plus courte que les Organisations qui la composent, mais pas nécessairement. Tous les membres sont des `org:Organization`s plutôt que des individus et ces Organisations peuvent jouer des Rôles particuliers au sein du Partenariat. "@fr ;
  rdfs:comment "È una collaborazione tra due o più Organization come ad esempio un progetto. Consente di rappresentare alcune identità dell'Organization che sono fuori dallo scopo principale e non sono formalmente riconosciute. Potrebbe anche avere un ciclo di vita limitato."@it ;
  rdfs:comment "プロジェクトなどの2つ以上の組織間のコラボレーション。それは、アイデンティティを有し、その特定のメンバーとは無関係に目的を定めているという点で、組織としての基準を満たしますが、正式に認識された法的実体でも、あるより大きな組織内のサブユニットでもありません。一般的には、その内部の組織よりも存続期間が短いかもしれませんが、必ずしもそうとは限りません。"@ja ;
  rdfs:isDefinedBy <http://www.w3.org/ns/org> ;
  rdfs:label "Collaborazione"@it ;
  rdfs:label "Endeavour"@en ;
  rdfs:label "Partenariat"@fr ;
  rdfs:label "proyecto de cooperación empresarial"@es ;
  rdfs:subClassOf org:Organization ;
  owl:equivalentClass _:b421246 ;
  owl:equivalentClass _:b937707 ;
  owl:equivalentClass _:b938296 ;
.
org:OrganizationalUnit
  rdf:type rdfs:Class ;
  rdf:type owl:Class ;
  rdfs:comment "An Organization such as a University Support Unit which is part of some larger FormalOrganization and only has full recognition within the context of that FormalOrganization, it is not a Legal Entity in its own right. Units can be large and complex containing other Units and even FormalOrganizations. Alternative names: _OU_ _Unit_ _Department_"@en ;
  rdfs:comment "Organización que forma parte de una organización formal más amplia, como el servicio de informática o centro de cálculo de una universidad, y que sólo tiene reconocimiento pleno en el contexto de dicha organización formal, pero que no es una entidad legal propiamente dicha. Estas unidades pueden ser amplias y complejas, e incluir a otras unidades o incluso a otras organizaciones formales. Denominaciones alternativas: departamento."@es ;
  rdfs:comment "Un'organizzazione come ad esempio l'unità dei sistemi informativi che è parte di una più grande FormalOrganization e che, pur essendo riconosciuta nel contesto della propria organizzazione di riferimento, non è legalmente riconosciuta come entità a sé stante. Le unità possono essere ampie e complesse e contenere al loro interno sia altre unità che addirittura FormalOrganization."@it ;
  rdfs:comment "Une organisation telle que le support informatique d'une université, qui fait partie d'une Organisation Formelle plus importante et qui ne peut être reconnue qu'en tant que membre de cette organisation supérieure, ce n'est pas une entité légale en elle-même. Les unités opérationnelles peuvent être étendues, complexes et inclure elles-mêmes d'autres branches ou Unités Opérationnelles, voire des Organisations Formelles."@fr ;
  rdfs:comment "あるより大きな組織の一部であり、その組織の中においてのみ完全に認識される部局や支援部署などの組織です。特に、その単位はそれ自体では法的実体と見なされません。"@ja ;
  rdfs:isDefinedBy <http://www.w3.org/ns/org> ;
  rdfs:label "OrganizationalUnit"@en ;
  rdfs:label "Unità Organizzativa"@it ;
  rdfs:label "Unité opérationnelle"@fr ;
  rdfs:label "unidad organizativa"@es ;
  rdfs:subClassOf org:Organization ;
.
org:Post
  rdf:type rdfs:Class ;
  rdf:type owl:Class ;
  rdfs:comment "A Post represents some position within an organization that exists independently of the person or persons filling it. Posts may be used to represent situations where a person is a member of an organization ex officio (for example the Secretary of State for Scotland is part of UK Cabinet by virtue of being Secretary of State for Scotland, not as an individual person). A post can be held by multiple people and hence can be treated as a organization in its own right."@en ;
  rdfs:comment "Puesto o posición que representa algún tipo de empleo dentro de una organización, que existe independientemente de la persona o personas que lo desempeñan. Esta clase puede utilizarse para representar situaciones en las que una persona es miembro de una organización ex oficio (por ejemplo, el Secretario de Estado escocés es parte del Gabinete del gobierno británico por virtud de ser Secretario de Estado en Escocia, y no como individuo). Un puesto puede ser desempeñado por múltiples individuos y de aquí que sea tratado como una organización en sí misma."@es ;
  rdfs:comment "Un Impiego rappresenta una posizione all'interno dell'organizzazione che esiste indipendentemente dalla persona che la ricopre. Gli impieghi possono essere utilizzati per le situazioni in cui una persona è membro di un'organizzazione o di un ufficio (ad esempio un segretario di stato). Un Impiego può essere ricoperto da più persone."@it ;
  rdfs:comment "Un Poste représente une position au sein d'une Organisation qui existe indépendamment de la personne ou des personnes qui le remplissent. Les postes peuvent être utilisés pour représenter des situations où une personne est membre d'une Organisation d'office (par exemple, le Secrétaire d'Etat pour l'Ecosse fait partie du Cabinet du Royaume-Uni du fait d'être Secrétaire d'Etat pour l'Ecosse, non pas comme une personne physique). Un poste après peut être occupé par plusieurs personnes et peut donc être considéré comme une Organisation à part entière."@fr ;
  rdfs:comment "ポストは、それを埋める人（人々）とは無関係に存在する組織内のある位置を表わします。ポストは、人が職権上、組織のメンバーである状況を表わすために使用できます（例えば、スコットランド大臣は、個人としてではなく、スコットランド大臣であることにより、英国内閣の一部です）。ポストは、複数の人々によって保持されることが可能だあるため、それ自体を組織として扱うことができます。"@ja ;
  rdfs:isDefinedBy <http://www.w3.org/ns/org> ;
  rdfs:label "Impiego"@it ;
  rdfs:label "Post"@en ;
  rdfs:label "Poste"@fr ;
  rdfs:label "puesto"@es ;
  rdfs:subClassOf owl:Thing ;
.
org:Role
  rdf:type rdfs:Class ;
  rdf:type owl:Class ;
  rdfs:comment "Denotes a role that a Person or other Agent can take in an organization. Instances of this class describe the abstract role; to denote a specific instance of a person playing that role in a specific organization use an instance of `org:Membership`. It is common for roles to be arranged in some taxonomic structure and we use SKOS to represent that. The normal SKOS lexical properties should be used when labelling the Role. Additional descriptive properties for the Role, such as a Salary band, may be added by extension vocabularies."@en ;
  rdfs:comment "Función que una persona o agente desempeña en el seno de una organización. Las instancias de esta clase describen la actividad en abstracto; si lo que se pretende es incluir una instancia que refleje la función o actividad que desempeña una persona en concreto en una organización específica, se indica el uso de instancias de la clase `org:Membership`. Es común que dichas actividades se representen en una estructura taxonómica mediante SKOS. Las propiedades léxicas de SKOS deberían utilizarse a la hora de denominar o etiquetar la actividad desempeñada. Para añadir propiedades descriptivas adicionales, como rango salarial, se tendrá que recurrir a vocabularios externos."@es ;
  rdfs:comment "Indica il ruolo che una Person o un altro Agent può assumere in un'organizzazione. Le istanze di questa classe descrivono un ruolo astratto; per esprimere il ruolo che una precisa persona ricopre in un'organizzazione si usi un'istanza di `org:Membership`. È comune organizzare i ruoli in una qualche struttura tassonomica e quindi si raccomanda SKOS per questo. Altre proprietà descrittive per il Role, come salario, possono essere aggiunte mediante l'uso di altri vocabolari."@it ;
  rdfs:comment "Indique le rôle qu'une Personne ou un autre Agent peut avoir dans une Organisation. Les instances de cette classe décrivent le rôle dans l'absolu; pour indiquer une personne ayant ce rôle spécifique dans une Organisation, utilisez une instance de `org:Membership`. Il est courant que les rôles soient organisés dans une sorte de taxonomie, ce qui peut être représenté avec SKOS. Les propriétés de libellés standards de SKOS devraient être utilisées pour libeller le Rôle. D'autres propriétés additionnelles pour ce rôle, comme une fourchette de Salaire peuvent être ajoutées par une extension de ce vocabulaire."@fr ;
  rdfs:comment "人またはその他のエージェントが組織で担うことができる役割を表わします。この種のインスタンスは、抽象的な役割を記述します。特定の組織でその役割を担っている人の特定のインスタンスを示すためには、org:Membershipのインスタンスを使用します。"@ja ;
  rdfs:isDefinedBy <http://www.w3.org/ns/org> ;
  rdfs:label "Role"@en ;
  rdfs:label "Ruolo"@it ;
  rdfs:label "Rôle"@fr ;
  rdfs:label "actividad"@es ;
  rdfs:subClassOf skos:Concept ;
  owl:disjointWith org:ChangeEvent ;
  owl:disjointWith org:Membership ;
  owl:disjointWith org:Site ;
.
org:Site
  rdf:type rdfs:Class ;
  rdf:type owl:Class ;
  rdfs:comment "An office or other premise at which the organization is located. Many organizations are spread across multiple sites and many sites will host multiple locations. In most cases a Site will be a physical location. However, we don't exclude the possibility of non-physical sites such as a virtual office with an associated post box and phone reception service. Extensions may provide subclasses to denote particular types of site."@en ;
  rdfs:comment "Oficina, local o cualquier otro lugar en el que se encuentra una organización. Muchas organizaciones están distribuidas en varias sedes, que a su vez están repartidas en distintas ubicaciones. En muchos casos una sede será un sitio o local físico. Sin embargo, no se excluye la posibilidad de lugares no físicos como oficinas virtuales con los correspondientes apartados de correo y servicio de atención telefónica. Se pueden añadir más subtipos mediante extensiones para incluir tipos especiales de lugares."@es ;
  rdfs:comment "Un ufficio o altra sede dovei l'organizzazione è situata. Molte organizzazione sono distribuite su più sedi e molte sedi ospitano più ubicazioni. Nella maggior parte dei casi un Site è una locazione fisica. Non si esclude la possibilità di indicare sedi non fisiche come ad esempio gli uffici virtuali. Le estensioni dell'ontologia potrebbero usare delle sottoclassi per rappresentare i tipi particolari di sede."@it ;
  rdfs:comment "Un établissement ou tout autre lieu dans lequel une Organisation est localisé. Beaucoup d'organisations sont dispersées à travers plusieurs sites. Dans la plupart des cas un Site sera un lieu physique. Toutefois, nous n'excluons pas la possibilité de sites non-physiques comme un bureau virtuel avec une boîte postale et un service de secrétariat mutualisé. Des extensions pourraient fournir des sous-classes pour décrire des types de sites particuliers."@fr ;
  rdfs:comment "組織が位置するオフィスやその他の敷地。多くの組織が複数のサイトに散在しており、多くのサイトが多数の場所を持つでしょう。"@ja ;
  rdfs:isDefinedBy <http://www.w3.org/ns/org> ;
  rdfs:label "Sede"@it ;
  rdfs:label "Site"@en ;
  rdfs:label "Site"@fr ;
  rdfs:label "sede"@es ;
  rdfs:subClassOf owl:Thing ;
  owl:disjointWith org:ChangeEvent ;
.
org:basedAt
  rdf:type rdf:Property ;
  rdf:type owl:ObjectProperty ;
  rdfs:comment "Indica la sede in cui una è stabilita una persona. Non esclude la possibilità che una persona sia allocata su più sedi."@it ;
  rdfs:comment "Indicates the site at which a person is based. We do not restrict the possibility that a person is based at multiple sites."@en ;
  rdfs:comment "Indique le site sur lequel une personne est basée. Nous ne limitons pas le nombre de sites sur lesquels une personne peut être basée."@fr ;
  rdfs:comment "Lugar en el que trabaja una persona. No se restringe el hecho de que una persona pueda estar adscrita a múltiples ubicaciones."@es ;
  rdfs:comment "人が基礎としているサイトを示します。人が複数のサイトを基礎としている可能性を制限しません。"@ja ;
  rdfs:domain dcterms:Agent ;
  rdfs:domain schema:Person ;
  rdfs:domain toop:Person ;
  rdfs:domain <http://www.w3.org/2000/10/swap/pim/contact#Person> ;
  rdfs:domain owl:Thing ;
  rdfs:domain wgs:SpatialThing ;
  rdfs:domain foaf:Agent ;
  rdfs:domain foaf:Person ;
  rdfs:domain _:b420951 ;
  rdfs:domain _:b421075 ;
  rdfs:domain _:b421664 ;
  rdfs:domain _:b421928 ;
  rdfs:domain _:b937877 ;
  rdfs:domain _:b938265 ;
  rdfs:isDefinedBy <http://www.w3.org/ns/org> ;
  rdfs:label "basata a"@it ;
  rdfs:label "based At"@en ;
  rdfs:label "basé à"@fr ;
  rdfs:label "trabaja en la sede"@es ;
  rdfs:range owl:Thing ;
  rdfs:range org:Site ;
.
org:changedBy
  rdf:type rdf:Property ;
  rdf:type owl:ObjectProperty ;
  rdfs:comment "Evento de cambio que resulta en una modificación en la organización. Dependiendo del evento, la organización puede dejar de existir tras el cambio. Es la relación inversa de `org:originalOrganization`."@es ;
  rdfs:comment "Indica un evento che ha contribuito al cambiamento di questa organizzazione. A seconda dell'evento, l'organizzazione potrebbe essere esistente dopo l'evento o aver cessato la propria esistenza. È l'inverso di `org:originalOrganization`."@it ;
  rdfs:comment "Indicates a change event which resulted in a change to this organization. Depending on the event the organization may or may not have continued to exist after the event. Inverse of `org:originalOrganization`."@en ;
  rdfs:comment "Indique un évènement qui a impliqué un changement dans l'Organisation. Selon l'évènement, l'Organisation a continué à exister après l'évènement, ou pas. Inverse de `org:originalOrganization`."@fr ;
  rdfs:comment "この組織の変更のきっかけとなった出来事を示します。"@ja ;
  rdfs:domain dcterms:Agent ;
  rdfs:domain owl:Thing ;
  rdfs:domain org:Organization ;
  rdfs:domain foaf:Agent ;
  rdfs:domain foaf:Organization ;
  rdfs:domain _:b420951 ;
  rdfs:domain _:b421075 ;
  rdfs:domain _:b421664 ;
  rdfs:domain _:b421928 ;
  rdfs:domain _:b937877 ;
  rdfs:domain _:b938265 ;
  rdfs:isDefinedBy <http://www.w3.org/ns/org> ;
  rdfs:label "cambiata da"@it ;
  rdfs:label "changed by"@en ;
  rdfs:label "es modificada por"@es ;
  rdfs:label "es modificado por"@es ;
  rdfs:label "modifiée par"@fr ;
  rdfs:range owl:Thing ;
  rdfs:range org:ChangeEvent ;
  rdfs:range prov:Activity ;
  rdfs:range _:b53184 ;
  rdfs:range _:b170340 ;
  rdfs:range _:b399839 ;
  rdfs:range _:b715640 ;
  rdfs:range _:b895567 ;
  rdfs:range _:b897711 ;
  owl:inverseOf org:originalOrganization ;
.
org:classification
  rdf:type rdf:Property ;
  rdf:type owl:ObjectProperty ;
  rdfs:comment "Indica una classificazione per questa Organization all'interno di un qualche schema di classificazione. Alcuni vocabolari potrebbero voler specializzare questa proprietà per avere un codominio corrispondente a uno specifico `skos:ConceptScheme`. Si noti che la presenza di questa proprietà è ancora in fase di discussione e potrebbe  essere revisionata o rimossa."@it ;
  rdfs:comment "Indicates a classification for this Organization within some classification scheme. Extension vocabularies may wish to specialize this property to have a range corresponding to a specific `skos:ConceptScheme`. This property is under discussion and may be revised or removed - in many cases organizations are best categorized by defining a sub-class hierarchy in an extension vocabulary."@en ;
  rdfs:comment "Indique une classification pour cette Organisation dans le cadre d'un schéma de classification. Il est possible de spécialiser cette propriété en utilisant un vocabulaire spécialisé pour que le champ corresponde à un concept spécifique `skos:ConceptScheme`. Cette propriété est en discussion est pourrait être révisée ou supprimée - dans de nombreux cas, les organisations sont mieux catégorisées par une hiérarchie de sous-classe dans un vocabulaire externe."@fr ;
  rdfs:comment "Ordenación jerárquica que se hace de una organización dentro de un esquema de clasificación. Es posible que algunos vocabularios especifiquen esta propiedad de forma que el rango se corresponda con un `skos:ConceptScheme` específico. La conveniencia de incluir esta propiedad se está debatiendo y puede que se revise o elimine (en muchos casos las organizaciones se clasifican mejor si se define una jerarquía de subclases en un vocabulario aparte)"@es ;
  rdfs:comment """ある分類表内のこの組織に対する分類を示します。
アプリケーションがorg:Organizationのサブクラスを組織的なカテゴリーを表わす手段として定義することも許容されることに注意してください。"""@ja ;
  rdfs:domain dcterms:Agent ;
  rdfs:domain owl:Thing ;
  rdfs:domain org:Organization ;
  rdfs:domain foaf:Agent ;
  rdfs:domain foaf:Organization ;
  rdfs:domain _:b420951 ;
  rdfs:domain _:b421075 ;
  rdfs:domain _:b421664 ;
  rdfs:domain _:b421928 ;
  rdfs:domain _:b937877 ;
  rdfs:domain _:b938265 ;
  rdfs:isDefinedBy <http://www.w3.org/ns/org> ;
  rdfs:label "classification"@en ;
  rdfs:label "classification"@fr ;
  rdfs:label "classificazione"@it ;
  rdfs:label "pertenece a la clasificación"@es ;
  rdfs:range owl:Thing ;
  rdfs:range skos:Concept ;
  rdfs:range _:b327858 ;
.
org:hasMember
  rdf:type rdf:Property ;
  rdf:type owl:ObjectProperty ;
  rdfs:comment "Indica una persona che è membro della data Organization. È l'inverso di `org:memberOf` ed è fornita per  compatibilità con `foaf:member`."@it ;
  rdfs:comment "Indicates a person who is a member of the subject Organization. Inverse of `org:memberOf`, see that property for further clarification. Provided for compatibility with `foaf:member`."@en ;
  rdfs:comment "Indique une personne membre de l'Organisation sujet. Inverse de `org:memberOf`, voyez la description de cette propriété pour plus de précisions. Fourni pour la compatibilité avec `foaf:member`."@fr ;
  rdfs:comment "Persona que es miembro de la organización en cuestión. Es la relación inversa de `org:memberOf`, véase la descripción de esa propiedad para más detalles. Se prevé compatibilidad con foaf:member`."@es ;
  rdfs:comment "対象組織のメンバーであるエージェント（人または他の組織）を示します。org:memberOfの逆。さらに明確な説明については、そのプロパティーを参照してください。"@ja ;
  rdfs:domain dcterms:Agent ;
  rdfs:domain owl:Thing ;
  rdfs:domain org:Organization ;
  rdfs:domain foaf:Agent ;
  rdfs:domain foaf:Group ;
  rdfs:domain foaf:Organization ;
  rdfs:domain _:b420951 ;
  rdfs:domain _:b421075 ;
  rdfs:domain _:b421664 ;
  rdfs:domain _:b421928 ;
  rdfs:domain _:b937877 ;
  rdfs:domain _:b938265 ;
  rdfs:isDefinedBy <http://www.w3.org/ns/org> ;
  rdfs:label "ha membro"@it ;
  rdfs:label "has member"@en ;
  rdfs:label "possède un membre"@fr ;
  rdfs:label "tiene miembro"@es ;
  rdfs:range dcterms:Agent ;
  rdfs:range owl:Thing ;
  rdfs:range foaf:Agent ;
  rdfs:range _:b420951 ;
  rdfs:range _:b421075 ;
  rdfs:range _:b421664 ;
  rdfs:range _:b421928 ;
  rdfs:range _:b937877 ;
  rdfs:range _:b938265 ;
  owl:equivalentProperty foaf:member ;
  owl:inverseOf org:memberOf ;
.
org:hasMembership
  rdf:type rdf:Property ;
  rdf:type owl:ObjectProperty ;
  rdfs:comment "Indica una relazione di appartenenza che coinvolge un Agent. È l'inverso di `org:member`."@it ;
  rdfs:comment "Indicates a membership relationship that the Agent plays. Inverse of `org:member`."@en ;
  rdfs:comment "Indique pour cet Agent un engagement dans une Organisation. Inverse de `org:member`."@fr ;
  rdfs:comment "Relación de pertenencia o afiliación a una organización en la que el agente desempeña un cargo o función. Es la relación inversa de `org:member`."@es ;
  rdfs:comment "エージェントが担う構成員関係を示します。"@ja ;
  rdfs:domain dcterms:Agent ;
  rdfs:domain owl:Thing ;
  rdfs:domain foaf:Agent ;
  rdfs:domain _:b420951 ;
  rdfs:domain _:b421075 ;
  rdfs:domain _:b421664 ;
  rdfs:domain _:b421928 ;
  rdfs:domain _:b937877 ;
  rdfs:domain _:b938265 ;
  rdfs:isDefinedBy <http://www.w3.org/ns/org> ;
  rdfs:label "appartenenza"@it ;
  rdfs:label "engagement"@fr ;
  rdfs:label "membership"@en ;
  rdfs:label "tiene membresía"@es ;
  rdfs:range owl:Thing ;
  rdfs:range org:Membership ;
  rdfs:range _:b420982 ;
  rdfs:range _:b421370 ;
  rdfs:range _:b937443 ;
  owl:inverseOf org:member ;
.
org:hasPost
  rdf:type rdf:Property ;
  rdf:type owl:ObjectProperty ;
  rdfs:comment "Indica il Post che è presente in una Organization."@it ;
  rdfs:comment "Indicate un Poste qui existe dans l'Organisation."@fr ;
  rdfs:comment "Indicates a Post which exists within the Organization."@en ;
  rdfs:comment "Posición que existe en una organización."@es ;
  rdfs:comment "組織内に存在するポストを示します。"@ja ;
  rdfs:domain dcterms:Agent ;
  rdfs:domain owl:Thing ;
  rdfs:domain org:Organization ;
  rdfs:domain foaf:Agent ;
  rdfs:domain foaf:Organization ;
  rdfs:domain _:b420951 ;
  rdfs:domain _:b421075 ;
  rdfs:domain _:b421664 ;
  rdfs:domain _:b421928 ;
  rdfs:domain _:b937877 ;
  rdfs:domain _:b938265 ;
  rdfs:isDefinedBy <http://www.w3.org/ns/org> ;
  rdfs:label "impiego"@it ;
  rdfs:label "possède un poste"@fr ;
  rdfs:label "post"@en ;
  rdfs:label "tiene puesto"@es ;
  rdfs:range owl:Thing ;
  rdfs:range org:Post ;
  rdfs:range _:b420951 ;
  rdfs:range _:b420982 ;
  rdfs:range _:b421075 ;
  rdfs:range _:b421370 ;
  rdfs:range _:b421664 ;
  rdfs:range _:b421928 ;
  rdfs:range _:b937443 ;
  rdfs:range _:b937877 ;
  rdfs:range _:b938265 ;
.
org:hasPrimarySite
  rdf:type rdf:Property ;
  rdf:type owl:ObjectProperty ;
  rdfs:comment "Indica la sede principale per l'Organization. È da considerarsi come la sede di default in cui l'Organization deve essere contattata pur non essendo necessariamente il quartier generale."@it ;
  rdfs:comment "Indicates a primary site for the Organization, this is the default means by which an Organization can be contacted and is not necessarily the formal headquarters."@en ;
  rdfs:comment "Indique le site principal d'une Organisation, le moyen par défaut par lequel l'Organisation peut être contactée et pas nécessairement le siège social légal."@fr ;
  rdfs:comment "Oficina principal de la organización, la opción por defecto para ponerse en contacto con una organización, aunque no corresponde necesariamente con las oficinas centrales de la organización."@es ;
  rdfs:comment "組織の主要サイトを示します。組織の窓口となりえるデフォルトの手段ですが、正式な本部とは限りません。"@ja ;
  rdfs:domain dcterms:Agent ;
  rdfs:domain toop:RegisteredOrganization ;
  rdfs:domain owl:Thing ;
  rdfs:domain org:FormalOrganization ;
  rdfs:domain org:Organization ;
  rdfs:domain rov:RegisteredOrganization ;
  rdfs:domain foaf:Agent ;
  rdfs:domain foaf:Organization ;
  rdfs:domain _:b180769 ;
  rdfs:domain _:b254570 ;
  rdfs:domain _:b420951 ;
  rdfs:domain _:b421075 ;
  rdfs:domain _:b421664 ;
  rdfs:domain _:b421928 ;
  rdfs:domain _:b454254 ;
  rdfs:domain _:b826282 ;
  rdfs:domain _:b826680 ;
  rdfs:domain _:b937877 ;
  rdfs:domain _:b938265 ;
  rdfs:isDefinedBy <http://www.w3.org/ns/org> ;
  rdfs:label "primary Site"@en ;
  rdfs:label "sede principale"@it ;
  rdfs:label "site principal"@fr ;
  rdfs:label "tiene sede principal en"@es ;
  rdfs:range toop:MainSite ;
  rdfs:range owl:Thing ;
  rdfs:range org:Site ;
  rdfs:subPropertyOf org:hasSite ;
  owl:equivalentProperty toop:hasMainSite ;
.
org:hasRegisteredSite
  rdf:type rdf:Property ;
  rdf:type owl:ObjectProperty ;
  rdfs:comment "Indica la sede legale per l'Organization. In molte giurisdizioni è richiesto che una FormalOrganization abbia una sede di questo tipo."@it ;
  rdfs:comment "Indicates the legally registered site for the organization, in many legal jurisdictions there is a requirement that FormalOrganizations such as Companies or Charities have such a primary designed site. "@en ;
  rdfs:comment "Indique l'établissement principal légalement enregistré pour l'Organisation. Dans de nombreuses juridictions existe l'obligation pour une Organisation Formelle d'avoir un tel site principal. "@fr ;
  rdfs:comment "Oficina o sede legalmente registrada de la organización. En muchas jurisdicciones legales existe el requisito de que organizaciones formales tales como empresas u organizaciones de beneficencia tengan una sede principal de este tipo."@es ;
  rdfs:comment "組織の法律上登録されたサイトを示し、多くの法的管轄区域では、会社や慈善団体などのFormalOrganizations（正式な組織）がそのような主要サイトを持っているという要件があります。"@ja ;
  rdfs:domain dcterms:Agent ;
  rdfs:domain toop:RegisteredOrganization ;
  rdfs:domain owl:Thing ;
  rdfs:domain org:FormalOrganization ;
  rdfs:domain org:Organization ;
  rdfs:domain rov:RegisteredOrganization ;
  rdfs:domain foaf:Agent ;
  rdfs:domain foaf:Organization ;
  rdfs:domain _:b180769 ;
  rdfs:domain _:b254570 ;
  rdfs:domain _:b420951 ;
  rdfs:domain _:b421075 ;
  rdfs:domain _:b421664 ;
  rdfs:domain _:b421928 ;
  rdfs:domain _:b454254 ;
  rdfs:domain _:b826282 ;
  rdfs:domain _:b826680 ;
  rdfs:domain _:b937877 ;
  rdfs:domain _:b938265 ;
  rdfs:isDefinedBy <http://www.w3.org/ns/org> ;
  rdfs:label "registered Site"@en ;
  rdfs:label "sede legale"@it ;
  rdfs:label "siège social"@fr ;
  rdfs:label "tiene sede registrada en"@es ;
  rdfs:range toop:MainSite ;
  rdfs:range owl:Thing ;
  rdfs:range org:Site ;
  rdfs:subPropertyOf toop:hasMainSite ;
  rdfs:subPropertyOf org:hasPrimarySite ;
  rdfs:subPropertyOf org:hasSite ;
.
org:hasSite
  rdf:type rdf:Property ;
  rdf:type owl:ObjectProperty ;
  rdfs:comment "Indica la sede in cui l'Organization ha una qualche presenza anche in modo indiretto (ad esempio un ufficio virtuale). È l'inverso di `org:siteOf`."@it ;
  rdfs:comment "Indicates a site at which the Organization has some presence even if only indirect (e.g. virtual office or a professional service which is acting as the registered address for a company). Inverse of `org:siteOf`."@en ;
  rdfs:comment "Indique un site sur lequel l'Organisation possède une présence, même indirecte (domiciliation, boite postale). Inverse de `org:siteOf`."@fr ;
  rdfs:comment "Lugar en donde la organización tiene algún tipo de presencia, incluso si es de forma indirecta (por ejemplo, una oficina virtual o servicio profesional que hagan la función de dirección registrada de la compañía). Es la relación inversa de `org:siteOf`."@es ;
  rdfs:comment "組織が、間接（例えば、会社の登録住所として機能しているバーチャル・オフィスやプロフェッショナル・サービス）のみであったとしても、ある存在感を持っているサイトを示します。"@ja ;
  rdfs:domain dcterms:Agent ;
  rdfs:domain owl:Thing ;
  rdfs:domain org:Organization ;
  rdfs:domain foaf:Agent ;
  rdfs:domain foaf:Organization ;
  rdfs:domain _:b420951 ;
  rdfs:domain _:b421075 ;
  rdfs:domain _:b421664 ;
  rdfs:domain _:b421928 ;
  rdfs:domain _:b937877 ;
  rdfs:domain _:b938265 ;
  rdfs:isDefinedBy <http://www.w3.org/ns/org> ;
  rdfs:label "a un site"@fr ;
  rdfs:label "ha sede"@it ;
  rdfs:label "has site"@en ;
  rdfs:label "tiene sede en"@es ;
  rdfs:range owl:Thing ;
  rdfs:range org:Site ;
  owl:inverseOf org:siteOf ;
.
org:hasSubOrganization
  rdf:type rdf:Property ;
  rdf:type owl:ObjectProperty ;
  rdfs:comment "Indique le statut de dépendance hiérarchique pour des Organisations ou des Unités Opérationnelles; indique une Organisation qui est une sous-partie ou une branche d'une Organisation plus large. C'est la propriété inverse de `org:subOrganizationOf`."@fr ;
  rdfs:comment "Organización jerárquica de organizaciones o unidades. Indica que una organización es parte de otra organización más amplia o pertenece a ella. Es la relación inversa de `org:subOrganizationOf`."@es ;
  rdfs:comment "Rappresenta un contenimento gerarchico di una Organization o di una OrganizationalUnit. Indica una organizzazione che è parte di una organizzazione più grande. È l'inverso di `org:subOrganizationOf`."@it ;
  rdfs:comment "Represents hierarchical containment of Organizations or Organizational Units; indicates an organization which is a sub-part or child of this organization.  Inverse of `org:subOrganizationOf`."@en ;
  rdfs:comment "組織または組織単位の階層的包含を表わします。この組織のサブパートまたは子である組織を示します。"@ja ;
  rdfs:domain dcterms:Agent ;
  rdfs:domain owl:Thing ;
  rdfs:domain org:Organization ;
  rdfs:domain foaf:Agent ;
  rdfs:domain foaf:Organization ;
  rdfs:domain _:b420951 ;
  rdfs:domain _:b421075 ;
  rdfs:domain _:b421664 ;
  rdfs:domain _:b421928 ;
  rdfs:domain _:b937877 ;
  rdfs:domain _:b938265 ;
  rdfs:isDefinedBy <http://www.w3.org/ns/org> ;
  rdfs:label "a une Sous-Organization"@fr ;
  rdfs:label "ha sotto-Organization"@it ;
  rdfs:label "has SubOrganization"@en ;
  rdfs:label "tiene suborganización"@es ;
  rdfs:range dcterms:Agent ;
  rdfs:range owl:Thing ;
  rdfs:range org:Organization ;
  rdfs:range foaf:Agent ;
  rdfs:range foaf:Organization ;
  rdfs:range _:b420951 ;
  rdfs:range _:b421075 ;
  rdfs:range _:b421664 ;
  rdfs:range _:b421928 ;
  rdfs:range _:b937877 ;
  rdfs:range _:b938265 ;
  owl:inverseOf org:subOrganizationOf ;
.
org:hasUnit
  rdf:type rdf:Property ;
  rdf:type owl:ObjectProperty ;
  rdfs:comment "Indica un'unità che è parte di questa Organization, come ad esempio un dipartimento facente parte di una più ampia FormalOrganization. È l'inverso di `org:unitOf`."@it ;
  rdfs:comment "Indicates a unit which is part of this Organization, e.g. a Department within a larger FormalOrganization. Inverse of `org:unitOf`."@en ;
  rdfs:comment "Indique une Unité qui fait partie d'une Organisation, par exemple un Départment au sein d'une Organisation Formelle plus large. Inverse de `org:unitOf`."@fr ;
  rdfs:comment "Unidad que es parte de la organización, como, por ejemplo, un departamento incluido en una organización formal más amplia."@es ;
  rdfs:comment "例えば、より大きな組織内の部局など、この組織の一部である単位を示します。"@ja ;
  rdfs:domain dcterms:Agent ;
  rdfs:domain owl:Thing ;
  rdfs:domain org:FormalOrganization ;
  rdfs:domain org:Organization ;
  rdfs:domain foaf:Agent ;
  rdfs:domain foaf:Organization ;
  rdfs:domain _:b420951 ;
  rdfs:domain _:b421075 ;
  rdfs:domain _:b421664 ;
  rdfs:domain _:b421928 ;
  rdfs:domain _:b937877 ;
  rdfs:domain _:b938265 ;
  rdfs:isDefinedBy <http://www.w3.org/ns/org> ;
  rdfs:label "contiene unidad"@es ;
  rdfs:label "ha Unit"@it ;
  rdfs:label "has Unit"@en ;
  rdfs:label "possède une Unité"@fr ;
  rdfs:range dcterms:Agent ;
  rdfs:range owl:Thing ;
  rdfs:range org:Organization ;
  rdfs:range org:OrganizationalUnit ;
  rdfs:range foaf:Agent ;
  rdfs:range foaf:Organization ;
  rdfs:range _:b420951 ;
  rdfs:range _:b421075 ;
  rdfs:range _:b421664 ;
  rdfs:range _:b421928 ;
  rdfs:range _:b937877 ;
  rdfs:range _:b938265 ;
  rdfs:subPropertyOf org:hasSubOrganization ;
  owl:inverseOf org:unitOf ;
.
org:headOf
  rdf:type rdf:Property ;
  rdf:type owl:ObjectProperty ;
  rdfs:comment "Indica che una persona è leader o responsabile formale di una Organization. Questo significa che la persona è alla radice del grafo (aciclico) creato dalle `org:reportsTo`, sebbene un'organizzazione possa avere più di un responsabile."@it ;
  rdfs:comment "Indicates that a person is the leader or formal head of the Organization. This will normally mean that they are the root of the `org:reportsTo` (acyclic) graph, though an organization may have more than one head."@en ;
  rdfs:comment "Indique qu'une personne est le directeur ou le responsable formel d'une Organisation. Ceci indique souvent qu'il est au sommet de du graphe acyclique des `org:reportsTo`, même si une organisation peut avoir plus d'un responsable."@fr ;
  rdfs:comment "Persona que es jefe o jefa, representante ,,director o directora de la organización. Esto significa que dicha persona es el rango de la relación `org:reportsTo` en el organigrama de la organización (acíclico), aunque una organización puede tener más de un jefe."@es ;
  rdfs:comment "人（または他のエージェント）が組織のリーダーや正式なトップであることを示します。"@ja ;
  rdfs:domain dcterms:Agent ;
  rdfs:domain schema:Person ;
  rdfs:domain toop:Person ;
  rdfs:domain <http://www.w3.org/2000/10/swap/pim/contact#Person> ;
  rdfs:domain owl:Thing ;
  rdfs:domain wgs:SpatialThing ;
  rdfs:domain foaf:Agent ;
  rdfs:domain foaf:Person ;
  rdfs:domain _:b420951 ;
  rdfs:domain _:b421075 ;
  rdfs:domain _:b421664 ;
  rdfs:domain _:b421928 ;
  rdfs:domain _:b937877 ;
  rdfs:domain _:b938265 ;
  rdfs:isDefinedBy <http://www.w3.org/ns/org> ;
  rdfs:label "es director ejecutivo de"@es ;
  rdfs:label "head of"@en ;
  rdfs:label "responsabile di"@it ;
  rdfs:label "responsable de"@fr ;
  rdfs:range dcterms:Agent ;
  rdfs:range owl:Thing ;
  rdfs:range org:Organization ;
  rdfs:range foaf:Agent ;
  rdfs:range foaf:Organization ;
  rdfs:range _:b420951 ;
  rdfs:range _:b421075 ;
  rdfs:range _:b421664 ;
  rdfs:range _:b421928 ;
  rdfs:range _:b937877 ;
  rdfs:range _:b938265 ;
  rdfs:subPropertyOf org:memberOf ;
.
org:heldBy
  rdf:type rdf:Property ;
  rdf:type owl:ObjectProperty ;
  rdfs:comment "Agente que ocupa un puesto."@es ;
  rdfs:comment "Indica un Agent che ricopre un Post."@it ;
  rdfs:comment "Indicate un Agent qui occupe le Poste."@fr ;
  rdfs:comment "Indicates an Agent which holds a Post."@en ;
  rdfs:comment "ポストを保持するエージェントを示します。"@ja ;
  rdfs:domain owl:Thing ;
  rdfs:domain org:Post ;
  rdfs:domain _:b420951 ;
  rdfs:domain _:b420982 ;
  rdfs:domain _:b421075 ;
  rdfs:domain _:b421370 ;
  rdfs:domain _:b421664 ;
  rdfs:domain _:b421928 ;
  rdfs:domain _:b937443 ;
  rdfs:domain _:b937877 ;
  rdfs:domain _:b938265 ;
  rdfs:isDefinedBy <http://www.w3.org/ns/org> ;
  rdfs:label "held by"@en ;
  rdfs:label "occupé par"@fr ;
  rdfs:label "ocupado por"@es ;
  rdfs:label "ricoperto da"@it ;
  rdfs:range dcterms:Agent ;
  rdfs:range owl:Thing ;
  rdfs:range foaf:Agent ;
  rdfs:range _:b420951 ;
  rdfs:range _:b421075 ;
  rdfs:range _:b421664 ;
  rdfs:range _:b421928 ;
  rdfs:range _:b937877 ;
  rdfs:range _:b938265 ;
.
org:holds
  rdf:type rdf:Property ;
  rdf:type owl:ObjectProperty ;
  rdfs:comment "Indica un Impiego ricoperto da un Agent."@it ;
  rdfs:comment "Indicate un Poste occupé par un Agent."@fr ;
  rdfs:comment "Indicates a Post held by some Agent."@en ;
  rdfs:comment "Puesto ocupado por algún agente."@es ;
  rdfs:comment "あるエージェントによって保持されているポストを示します。"@ja ;
  rdfs:domain dcterms:Agent ;
  rdfs:domain owl:Thing ;
  rdfs:domain foaf:Agent ;
  rdfs:domain _:b420951 ;
  rdfs:domain _:b421075 ;
  rdfs:domain _:b421664 ;
  rdfs:domain _:b421928 ;
  rdfs:domain _:b937877 ;
  rdfs:domain _:b938265 ;
  rdfs:isDefinedBy <http://www.w3.org/ns/org> ;
  rdfs:label "holds"@en ;
  rdfs:label "occupe"@fr ;
  rdfs:label "ocupa"@es ;
  rdfs:label "ricopre"@it ;
  rdfs:range owl:Thing ;
  rdfs:range org:Post ;
  rdfs:range _:b420951 ;
  rdfs:range _:b420982 ;
  rdfs:range _:b421075 ;
  rdfs:range _:b421370 ;
  rdfs:range _:b421664 ;
  rdfs:range _:b421928 ;
  rdfs:range _:b937443 ;
  rdfs:range _:b937877 ;
  rdfs:range _:b938265 ;
  owl:inverseOf org:heldBy ;
.
org:identifier
  rdf:type rdf:Property ;
  rdf:type owl:DatatypeProperty ;
  rdfs:comment "Código o identificador, como por ejemplo el CIF de una empresa, que permite identificar de forma inequívoca a una organización. Existen muchos códigos de identificación tanto nacionales como internacionales. Esta ontología no obliga al uso de ningún esquema en concreto. Los códigos de identificación utilizados en cada caso se deberían indicar mediante el uso de la propiedad “datatype” del valor del identificador. El uso de la propiedad “datatype” para especificar el esquema de notación utilizado está en consonancia con las buenas prácticas recomendadas para el uso de la propiedad `skos:notation`, de la que esta propiedad es una especialización."@es ;
  rdfs:comment "Donne un identifiant, comme par exemple le numéro d'enregistrement d'une entreprise, qui peut être utilisé comme identifiant unique pour l'Organisation. De nombreux schémas nationaux et internationaux sont disponibles. Cette ontologie reste neutre par rapport au schéma utilisé. Le schéma particulier utilisé devrait être indiqué par le `datatype` de la valeur de l'identifiant. Utiliser les datatypes pour distinguer les schémas de notation est cohérent avec les bonnes pratiques pour `skos:notation` dont cette propriété est une spécialisation."@fr ;
  rdfs:comment "Gives an identifier, such as a company registration number, that can be used to used to uniquely identify the organization. Many different national and international identier schemes are available. The org ontology is neutral to which schemes are used. The particular identifier scheme should be indicated by the datatype of the identifier value.  Using datatypes to distinguish the notation scheme used is consistent with recommended best practice for `skos:notation` of which this property is a specialization."@en ;
  rdfs:comment "Indica un identificatore univoco per l'organizzazione, come ad esempio la partita IVA di un'azienda. Molti schemi di identificazione a livello nazionale e internazionale sono disponibili allo scopo. L'ontologia ORG è neutrale rispetto allo schema da utilizzare. Lo schema di identificazione dovrebbe essere indicato dal datatype del valore dell'identificatore. L'uso del datatype per distinguere lo schema di identificazione è coerente con le best practice per `skos:notation`, di cui questa proprietà è una specializzazione."@it ;
  rdfs:comment "組織を一意に識別するために使用できる会社登録番号などの識別子を与えます。"@ja ;
  rdfs:domain dcterms:Agent ;
  rdfs:domain owl:Thing ;
  rdfs:domain org:Organization ;
  rdfs:domain foaf:Agent ;
  rdfs:domain foaf:Organization ;
  rdfs:domain _:b420951 ;
  rdfs:domain _:b421075 ;
  rdfs:domain _:b421664 ;
  rdfs:domain _:b421928 ;
  rdfs:domain _:b937877 ;
  rdfs:domain _:b938265 ;
  rdfs:isDefinedBy <http://www.w3.org/ns/org> ;
  rdfs:label "identifiant"@fr ;
  rdfs:label "identificatore"@it ;
  rdfs:label "identifier"@en ;
  rdfs:label "tiene identificador"@es ;
  rdfs:subPropertyOf skos:notation ;
  owl:equivalentProperty elobr:EloniaRegistrationNumber ;
  owl:equivalentProperty freebr:FreedoniaRegistrationNumber ;
  owl:equivalentProperty toop:registrationNumber ;
.
org:linkedTo
  rdf:type rdf:Property ;
  rdf:type owl:ObjectProperty ;
  rdfs:comment "2つの組織の任意の関係を示します。"@ja ;
  rdfs:comment "Indica una relazione arbitraria tra due organizzazioni. Ad esempio, specializzazioni di questa proprietà possono essere usate per denotare relazioni particolari tipo il finanziamento o la fornitura."@it ;
  rdfs:comment "Indicates an arbitrary relationship between two organizations. Specializations of this can be used to, for example, denote funding or supply chain relationships."@en ;
  rdfs:comment "Indique une relation arbitraire entre deux Organisations. Des spécialisations peuvent être utilisées pour, par exemple, qualifier une relation de fournisseur ou de financeur."@fr ;
  rdfs:comment "Relación arbitraria entre dos organizaciones. Las especializaciones de esta relación se pueden utilizar para denotar relaciones de financiación o suministro, entre otras."@es ;
  rdfs:domain dcterms:Agent ;
  rdfs:domain owl:Thing ;
  rdfs:domain org:Organization ;
  rdfs:domain foaf:Agent ;
  rdfs:domain foaf:Organization ;
  rdfs:domain _:b420951 ;
  rdfs:domain _:b421075 ;
  rdfs:domain _:b421664 ;
  rdfs:domain _:b421928 ;
  rdfs:domain _:b937877 ;
  rdfs:domain _:b938265 ;
  rdfs:isDefinedBy <http://www.w3.org/ns/org> ;
  rdfs:label "collegato a"@it ;
  rdfs:label "está relacionada con"@es ;
  rdfs:label "está relacionado con"@es ;
  rdfs:label "linked to"@en ;
  rdfs:label "relié à"@fr ;
  rdfs:range dcterms:Agent ;
  rdfs:range owl:Thing ;
  rdfs:range org:Organization ;
  rdfs:range foaf:Agent ;
  rdfs:range foaf:Organization ;
  rdfs:range _:b420951 ;
  rdfs:range _:b421075 ;
  rdfs:range _:b421664 ;
  rdfs:range _:b421928 ;
  rdfs:range _:b937877 ;
  rdfs:range _:b938265 ;
.
org:location
  rdf:type rdf:Property ;
  rdf:type owl:DatatypeProperty ;
  rdfs:comment "Gives a location description for a person within the organization, for example a _Mail Stop_ for internal posting purposes."@en ;
  rdfs:comment "Indica la descrizione del luogo presso cui è possibile reperire una persona dell'organizzazione."@it ;
  rdfs:comment "Indique la description de l'endroit ou est basé une personne de l'Organisation, par exemple pour des besoins de messagerie interne (Bureau 42)."@fr ;
  rdfs:comment "Lugar o ubicación exacta de una persona en una organización con el objetivo de facilitar, por ejemplo, la entrega de correo."@es ;
  rdfs:comment "例えば、内部配送目的のメール・ストップ（Mail Stop）などの、組織内の人の位置記述を提供します。"@ja ;
  rdfs:domain dcterms:Agent ;
  rdfs:domain schema:Person ;
  rdfs:domain toop:Person ;
  rdfs:domain <http://www.w3.org/2000/10/swap/pim/contact#Person> ;
  rdfs:domain owl:Thing ;
  rdfs:domain wgs:SpatialThing ;
  rdfs:domain foaf:Agent ;
  rdfs:domain foaf:Person ;
  rdfs:domain _:b420951 ;
  rdfs:domain _:b421075 ;
  rdfs:domain _:b421664 ;
  rdfs:domain _:b421928 ;
  rdfs:domain _:b937877 ;
  rdfs:domain _:b938265 ;
  rdfs:isDefinedBy <http://www.w3.org/ns/org> ;
  rdfs:label "está ubicada en"@es ;
  rdfs:label "está ubicado en"@es ;
  rdfs:label "localisation"@fr ;
  rdfs:label "location"@en ;
  rdfs:label "luogo"@it ;
  rdfs:range xsd:string ;
.
org:member
  rdf:type rdf:Property ;
  rdf:type owl:FunctionalProperty ;
  rdf:type owl:ObjectProperty ;
  rdfs:comment "Indica la Person (o un altro Agent) coinvolto in una relazione di Membership. È l'inverso di `org:hasMembership`."@it ;
  rdfs:comment "Indicates the Person (or other Agent including Organization) involved in the Membership relationship. Inverse of `org:hasMembership`"@en ;
  rdfs:comment "Indique une personne (ou tout autre Agent, y compris une Organisation) impliqué dans la relation d'Engagement. Inverse de `org:hasMembership`"@fr ;
  rdfs:comment "Persona (u otro agente, incluyendo una organización) que participa en la relación de membresía. Es la relación inversa de `org:hasMembership`."@es ;
  rdfs:comment "構成員関係に含まれている人（または、組織を含んでいる他のエージェント）を示します。"@ja ;
  rdfs:domain owl:Thing ;
  rdfs:domain org:Membership ;
  rdfs:domain _:b420982 ;
  rdfs:domain _:b421370 ;
  rdfs:domain _:b937443 ;
  rdfs:isDefinedBy <http://www.w3.org/ns/org> ;
  rdfs:label "es condición de miembro sobre agente"@es ;
  rdfs:label "member"@en ;
  rdfs:label "membre"@fr ;
  rdfs:label "membro"@it ;
  rdfs:range dcterms:Agent ;
  rdfs:range owl:Thing ;
  rdfs:range foaf:Agent ;
  rdfs:range _:b420951 ;
  rdfs:range _:b421075 ;
  rdfs:range _:b421664 ;
  rdfs:range _:b421928 ;
  rdfs:range _:b937877 ;
  rdfs:range _:b938265 ;
  owl:inverseOf org:hasMembership ;
.
org:memberDuring
  rdf:type rdf:Property ;
  rdf:type owl:ObjectProperty ;
  rdfs:comment "Optional property to indicate the interval for which the membership is/was valid."@en ;
  rdfs:comment "Propiedad opcional que indica el periodo durante el cual la relación de membresía o pertenencia a una organización se mantiene en vigencia."@es ;
  rdfs:comment "Proprietà opzionale per indicare l'intervallo per il quale l'appartenenza è/è stata valida."@it ;
  rdfs:comment "Propriété optionnelle pour indiquer l'intervalle durant lequel l'engagemnet est ou était valide."@fr ;
  rdfs:comment "構成員が有効である／であった期間を示すためのオプションのプロパティー。"@ja ;
  rdfs:domain owl:Thing ;
  rdfs:domain org:Membership ;
  rdfs:domain _:b420982 ;
  rdfs:domain _:b421370 ;
  rdfs:domain _:b937443 ;
  rdfs:isDefinedBy <http://www.w3.org/ns/org> ;
  rdfs:label "durée d'engagement"@fr ;
  rdfs:label "es miembro durante"@es ;
  rdfs:label "member During"@en ;
  rdfs:label "membro durante"@it ;
.
org:memberOf
  rdf:type rdf:Property ;
  rdf:type owl:ObjectProperty ;
  rdfs:comment "Indica che una persona è membro di una Organization senza una precisa indicazione sulla natura di questa appartenenza e sul suo ruolo. Si noti che la scelta del nome di questa proprietà non intende limitarla alla sola  rappresentazione formalmente di un'appartenenza. La proprietà può coprire anche altri coinvolgimenti nell'organizzazione. Questa proprietà può essere specializzata per indicare ruoli all'interno organizzazione o relazioni di diverse tipologie. Ha `org:hasmember` come proprietà inversa opzionale."@it ;
  rdfs:comment "Indicates that a person is a member of the Organization with no indication of the nature of that membership or the role played. Note that the choice of property name is not meant to limit the property to only formal membership arrangements, it is also indended to cover related concepts such as affilliation or other involvement in the organization. Extensions can specialize this relationship to indicate particular roles within the organization or more nuanced relationships to the organization. Has an optional inverse, `org:hasmember`."@en ;
  rdfs:comment "Indique qu'une personne est membre de l'Organisation sans précision sur la nature de cet engagement ou du rôle joué. Notez que le choix du nom de cette propriété ne vise pas à la limiter aux seuls engagements formels, elle peut également couvrir des concepts reliés comme l'affiliation ou le bénévolat. Des extensions peuvent spécialiser cette relation pour indiquer des rôles particuliers au sein de l'Organisation or des relations plus nuancées avec elle. Possède une propriété inverse optionnelle, `org:hasmember`."@fr ;
  rdfs:comment "Persona que pertenece a la organización o es miembro de la misma, sin que conste la naturaleza de dicha pertenencia o el papel que desempeña. Se debe tener en cuenta que la elección de una denominación para esta propiedad no significa que la propiedad esté limitada a ciertos tipos de pertenencia formales, sino que pretende cubrir conceptos relacionados como el de afiliación u otras formas de participación en la organización. Se puede hacer uso de extensiones para especializar esta relación de forma que incluya tipos específicos de pertenencia a las organizaciones o relaciones especiales con la organización."@es ;
  rdfs:comment "エージェント（人または他の組織）が組織のメンバーであることを示します。ただし、その構成員の本質や担う役割は示しません。プロパティー名の選択は、プロパティーを正式な構成員配置のみに制限することが目的ではないことに注意してください。所属や組織へのその他の関与などの関連する概念をカバーすることも意図されています。拡張により、この関係を特殊化し、組織内の特定の役割やよりニュアンスを含んだ組織との関係を示すことができます。"@ja ;
  rdfs:domain dcterms:Agent ;
  rdfs:domain owl:Thing ;
  rdfs:domain foaf:Agent ;
  rdfs:domain _:b420951 ;
  rdfs:domain _:b421075 ;
  rdfs:domain _:b421664 ;
  rdfs:domain _:b421928 ;
  rdfs:domain _:b937877 ;
  rdfs:domain _:b938265 ;
  rdfs:isDefinedBy <http://www.w3.org/ns/org> ;
  rdfs:label "es miembro de"@es ;
  rdfs:label "member of"@en ;
  rdfs:label "membre de"@fr ;
  rdfs:label "membro di"@it ;
  rdfs:range dcterms:Agent ;
  rdfs:range owl:Thing ;
  rdfs:range org:Organization ;
  rdfs:range foaf:Agent ;
  rdfs:range foaf:Organization ;
  rdfs:range _:b420951 ;
  rdfs:range _:b421075 ;
  rdfs:range _:b421664 ;
  rdfs:range _:b421928 ;
  rdfs:range _:b937877 ;
  rdfs:range _:b938265 ;
  owl:inverseOf org:hasMember ;
.
org:organization
  rdf:type rdf:Property ;
  rdf:type owl:FunctionalProperty ;
  rdf:type owl:ObjectProperty ;
  rdfs:comment "Indica l'Organization in cui l'Agent è un membro."@it ;
  rdfs:comment "Indicates Organization in which the Agent is a member."@en ;
  rdfs:comment "Indique l'Organization dont l'agent est membre."@fr ;
  rdfs:comment "Organización a la que pertenece el agente en calidad de miembro."@es ;
  rdfs:comment "エージェントがメンバーである組織を示します。"@ja ;
  rdfs:domain owl:Thing ;
  rdfs:domain org:Membership ;
  rdfs:domain _:b420982 ;
  rdfs:domain _:b421370 ;
  rdfs:domain _:b937443 ;
  rdfs:isDefinedBy <http://www.w3.org/ns/org> ;
  rdfs:label "es condición de miembro sobre organización"@es ;
  rdfs:label "organisation"@fr ;
  rdfs:label "organization"@en ;
  rdfs:label "organizzazione"@it ;
  rdfs:range dcterms:Agent ;
  rdfs:range owl:Thing ;
  rdfs:range org:Organization ;
  rdfs:range foaf:Agent ;
  rdfs:range foaf:Organization ;
  rdfs:range _:b420951 ;
  rdfs:range _:b421075 ;
  rdfs:range _:b421664 ;
  rdfs:range _:b421928 ;
  rdfs:range _:b937877 ;
  rdfs:range _:b938265 ;
.
org:originalOrganization
  rdf:type rdf:Property ;
  rdf:type owl:ObjectProperty ;
  rdfs:comment "Indica una o più organizzazioni pregresse rispetto a un evento di cambiamento. A seconda dell'evento, queste organizzazioni potrebbero essere esistenti dopo l'evento o  aver cessato la loro esistenza. È l'inverso di `org:changedBy`."@it ;
  rdfs:comment "Indicates one or more organizations that existed before the change event. Depending on the event they may or may not have continued to exist after the event. Inverse of `org:changedBy`."@en ;
  rdfs:comment "Indique une ou plusieurs organisations qui ont existé avant un évènement de changement. Selon l'évènement, ces organisations ont pu continuer à exister ou non. Inverse de `org:changedBy`. "@fr ;
  rdfs:comment "Una o más organizaciones que existían antes de que sucediera el cambio en la organización. Dependiendo del tipo de cambio, dichas organizaciones pueden haber dejado de existir o no. Es la relación inversa de `org:changedBy`."@es ;
  rdfs:comment "変更のきっかけとなった出来事以前に存在した1つ以上の組織を示します。出来事によって、出来事の後にそれらは存在し続けたかも、存在し続けなかったかもしれません。"@ja ;
  rdfs:domain owl:Thing ;
  rdfs:domain org:ChangeEvent ;
  rdfs:domain prov:Activity ;
  rdfs:domain _:b53184 ;
  rdfs:domain _:b170340 ;
  rdfs:domain _:b399839 ;
  rdfs:domain _:b715640 ;
  rdfs:domain _:b895567 ;
  rdfs:domain _:b897711 ;
  rdfs:isDefinedBy <http://www.w3.org/ns/org> ;
  rdfs:label "es organización original"@es ;
  rdfs:label "organisation originelle"@fr ;
  rdfs:label "organizzazione originale"@it ;
  rdfs:label "original organization"@en ;
  rdfs:range dcterms:Agent ;
  rdfs:range owl:Thing ;
  rdfs:range org:Organization ;
  rdfs:range prov:Entity ;
  rdfs:range foaf:Agent ;
  rdfs:range foaf:Organization ;
  rdfs:range _:b53184 ;
  rdfs:range _:b170340 ;
  rdfs:range _:b399839 ;
  rdfs:range _:b420951 ;
  rdfs:range _:b421075 ;
  rdfs:range _:b421664 ;
  rdfs:range _:b421928 ;
  rdfs:range _:b715640 ;
  rdfs:range _:b895567 ;
  rdfs:range _:b897711 ;
  rdfs:range _:b937877 ;
  rdfs:range _:b938265 ;
  rdfs:subPropertyOf prov:used ;
  rdfs:subPropertyOf prov:wasInfluencedBy ;
  owl:inverseOf org:changedBy ;
.
org:postIn
  rdf:type rdf:Property ;
  rdf:type owl:ObjectProperty ;
  rdfs:comment "Indica l'Organization in cui il Post è presente."@it ;
  rdfs:comment "Indicate l'Organisation dans laquelle le Poste existe."@fr ;
  rdfs:comment "Indicates the Organization in which the Post exists."@en ;
  rdfs:comment "Organización en la que existe el puesto."@es ;
  rdfs:comment "ポストが存在する組織を示します。"@ja ;
  rdfs:domain owl:Thing ;
  rdfs:domain org:Post ;
  rdfs:domain _:b420951 ;
  rdfs:domain _:b420982 ;
  rdfs:domain _:b421075 ;
  rdfs:domain _:b421370 ;
  rdfs:domain _:b421664 ;
  rdfs:domain _:b421928 ;
  rdfs:domain _:b937443 ;
  rdfs:domain _:b937877 ;
  rdfs:domain _:b938265 ;
  rdfs:isDefinedBy <http://www.w3.org/ns/org> ;
  rdfs:label "es un puesto en"@es ;
  rdfs:label "impiego in"@it ;
  rdfs:label "post in"@en ;
  rdfs:label "poste chez"@fr ;
  rdfs:range dcterms:Agent ;
  rdfs:range owl:Thing ;
  rdfs:range org:Organization ;
  rdfs:range foaf:Agent ;
  rdfs:range foaf:Organization ;
  rdfs:range _:b420951 ;
  rdfs:range _:b421075 ;
  rdfs:range _:b421664 ;
  rdfs:range _:b421928 ;
  rdfs:range _:b937877 ;
  rdfs:range _:b938265 ;
  owl:inverseOf org:hasPost ;
.
org:purpose
  rdf:type rdf:Property ;
  rdfs:comment "Finalidad u objetivo de la organización. La organización puede tener muchos objetivos a diferentes niveles de abstracción, pero en la naturaleza de las organizaciones está el tener una razón para existir, y la finalidad de esta propiedad es documentar dicha razón. La organización podrá tener más de un objetivo. Se recomienda el uso de vocabularios controlados o listas de códigos para indicar el objetivo, preferentemente mediante el uso de un `skos:Concept`. Sin embargo, el rango no está predeterminado, de forma que otros tipos de esquemas descriptivos tiene cabida. Se espera que ciertas especializaciones de este vocabulario o ciertos perfiles de aplicaciones restrinjan el rango del objetivo. Denominaciones alternativas: área_ _jurisdicción_ _ responsabilidad _ (especialmente cuando se aplica a unidades tales como ministerios o divisiones administrativas de los gobiernos)"@es ;
  rdfs:comment "Indica l'obiettivo di questa Organization. In generale, si possono esprimere gli obiettivi di un'organizzazione secondo diversi livelli di astrazione, ma la natura stessa dell'organizzazione ha una ragione d'essere ed è proprio questa che deve essere catturata con tale proprietà. Inoltre, un'Organization può avere obiettivi multipli. È raccomandabile che l'obiettivo faccia parte di una code list, e che sia preferibilmente un `skos:Concept`. Ad ogni modo, il codominio della proprietà è lasciato aperto per consentire altri tipi di di descrizione. Conseguentemente, eventuali specializzazioni o profili applicativi possono utilizzare quel vocabolario come codominio della proprietà."@it ;
  rdfs:comment "Indicates the purpose of this Organization. There can be many purposes at different levels of abstraction but the nature of an organization is to have a reason for existence and this property is a means to document that reason. An Organization may have multiple purposes. It is recommended that the purpose be denoted by a controlled term or code list, ideally a `skos:Concept`. However, the range is left open to allow for other types of descriptive schemes. It is expected that specializations or application profiles of this vocabulary will constrain the range of the purpose. Alternative names: _remit_ _responsibility_ (esp. if applied to OrganizationalUnits such as Government Departments)."@en ;
  rdfs:comment "Indique le but de cette Organisation. Il peut exister plusieurs buts à différents niveaux d'abstraction mais la nature d'une organisation est d'avoir une raison d'exister et cette propriété doit servir à documenter cette raison d'être. Une Organisation peut avoir plusieurs Buts. Il est recommandé que le but soit libellé à l'aide d'un vocabulaire contrôlé ou autre code établi, idéalement avec un concept `skos:Concept`. Toutefois, le champ de cette propriété est laissé ouvert et pourrait accepter d'autres schémas de description. Il est préférable que les spécialisations ou les profils d'applications de ce vocabulaire contraignent le champ de cette propriété."@fr ;
  rdfs:comment "この組織の目的を示します。異なる抽象レベルの多くの目的がありえますが、組織の本質は存在理由を持つことであり、このプロパティーはその理由をドキュメント化する手段です。組織は、複数の目的を持っている可能性があります。"@ja ;
  rdfs:domain dcterms:Agent ;
  rdfs:domain owl:Thing ;
  rdfs:domain org:Organization ;
  rdfs:domain foaf:Agent ;
  rdfs:domain foaf:Organization ;
  rdfs:domain _:b420951 ;
  rdfs:domain _:b421075 ;
  rdfs:domain _:b421664 ;
  rdfs:domain _:b421928 ;
  rdfs:domain _:b937877 ;
  rdfs:domain _:b938265 ;
  rdfs:isDefinedBy <http://www.w3.org/ns/org> ;
  rdfs:label "but"@fr ;
  rdfs:label "obiettivo"@it ;
  rdfs:label "purpose"@en ;
  rdfs:label "tiene objetivo"@es ;
.
org:remuneration
  rdf:type rdf:Property ;
  rdf:type owl:ObjectProperty ;
  rdfs:comment "Indica il salario o altra forma di remunerazione associata al ruolo. In genere, questo si denota usando uno schema di rappresentazione esistente come il `gr:PriceSpecification` ma il codominio è lasciato libero di essere specializzato a seconda delle applicazioni."@it ;
  rdfs:comment "Indicates a salary or other reward associated with the role. Typically this will be denoted using an existing representation scheme such as `gr:PriceSpecification` but the range is left open to allow applications to specialize it (e.g. to remunerationInGBP)."@en ;
  rdfs:comment "Indique un salaire ou tout autre compensation associée au Rôle. Typiquement, ceci sera annoté en utilisant un schéma existant comme  `gr:PriceSpecification` mais le champ de cette propriété est laissé ouvert afin de permettre aux applications de la spécialiser (par exemple remunerationEuro)."@fr ;
  rdfs:comment "Salario o cualquier otra remuneración asociada con la actividad. La forma usual de referirse a dicha remuneración será utilizando un esquema de representación como el propuesto en la ontología GoodRelations `gr:PriceSpecification`, pero el rango se deja abierto a que las distintas aplicaciones lo especialicen (por ejemplo, remunerationInGBP)"@es ;
  rdfs:comment "役割に関係する給料やその他の報酬を示します。"@ja ;
  rdfs:domain owl:Thing ;
  rdfs:domain skos:Concept ;
  rdfs:domain org:Role ;
  rdfs:domain _:b327858 ;
  rdfs:isDefinedBy <http://www.w3.org/ns/org> ;
  rdfs:label "recibe remuneración"@es ;
  rdfs:label "remuneration"@en ;
  rdfs:label "remunerazione"@it ;
  rdfs:label "rémuneration"@fr ;
.
org:reportsTo
  rdf:type rdf:Property ;
  rdf:type owl:ObjectProperty ;
  rdfs:comment "Indica una relazione di subordinazione all'interno dell'organigramma. La semantica precisa può variare a seconda dell'organizzazione, per esempio può essere usata per rappresentare la proprietà di supervisione oppure per le relazioni di rendicontazione."@it ;
  rdfs:comment "Indicates a reporting relationship as might be depicted on an organizational chart. The precise semantics of the reporting relationship will vary by organization but is intended to encompass both direct supervisory relationships (e.g. carrying objective and salary setting authority) and more general reporting or accountability relationships (e.g. so called _dotted line_ reporting)."@en ;
  rdfs:comment "Indique une relation de subordination comme elle pourrait figurer dans un organigramme. La sémantique précise de cette subordination pourra varier selon l'Organisation mais vise à englober aussi bien les relations hiérarchiques directes (définition d'objectifs, montant du salaire) que des relations plus générales ou organisationnelles (les liens en pointillés dans les organigrammes)."@fr ;
  rdfs:comment "Relación de subordinación que se representa en los organigramas de las organizaciones. La semántica de la relación de subordinación varía según las organizaciones, pero su intención es abarcar tanto a las relaciones de supervisión directa (por ejemplo, aquellas en las que la autoridad determina los objetivos o el salario) como a las relaciones de subordinación más generales (por ejemplo, las llamadas líneas de autoridad o de mando (y responsabilidad) (http://www.promonegocios.net/organigramas/tipos-de-organigramas.html))."@es ;
  rdfs:comment "組織図で描かれるかもしれないような上下関係を示します。エージェント間またはエージェントが就くことができるポスト間の上下関係を直接的に示すために使用できます。"@ja ;
  rdfs:domain owl:Thing ;
  rdfs:domain _:b421075 ;
  rdfs:domain _:b421928 ;
  rdfs:domain _:b938265 ;
  rdfs:isDefinedBy <http://www.w3.org/ns/org> ;
  rdfs:label "est subordonné à"@fr ;
  rdfs:label "reports to"@en ;
  rdfs:label "responde ante"@es ;
  rdfs:label "riporta a"@it ;
  rdfs:range owl:Thing ;
  rdfs:range _:b420951 ;
  rdfs:range _:b421664 ;
  rdfs:range _:b937877 ;
.
org:resultedFrom
  rdf:type rdf:Property ;
  rdf:type owl:ObjectProperty ;
  rdfs:comment "Evento que tiene como resultado la creación de una organización."@es ;
  rdfs:comment "Indica l'evento che ha permesso all'organizzazione di instaurarsi. È l'inverso di `org:resultingOrganization`."@it ;
  rdfs:comment "Indicates an event which resulted in this organization. Inverse of `org:resultingOrganization`."@en ;
  rdfs:comment "Indique un évènement dont est issue l'Organisation. Inverse de `org:resultingOrganization`."@fr ;
  rdfs:comment "この組織になった（導いた、作成された）きっかけとなった出来事を示します。"@ja ;
  rdfs:domain dcterms:Agent ;
  rdfs:domain owl:Thing ;
  rdfs:domain org:Organization ;
  rdfs:domain prov:Entity ;
  rdfs:domain foaf:Agent ;
  rdfs:domain foaf:Organization ;
  rdfs:domain _:b53184 ;
  rdfs:domain _:b170340 ;
  rdfs:domain _:b399839 ;
  rdfs:domain _:b420951 ;
  rdfs:domain _:b421075 ;
  rdfs:domain _:b421664 ;
  rdfs:domain _:b421928 ;
  rdfs:domain _:b715640 ;
  rdfs:domain _:b895567 ;
  rdfs:domain _:b897711 ;
  rdfs:domain _:b937877 ;
  rdfs:domain _:b938265 ;
  rdfs:isDefinedBy <http://www.w3.org/ns/org> ;
  rdfs:label "es el resultado de"@es ;
  rdfs:label "issue de"@fr ;
  rdfs:label "resulted from"@en ;
  rdfs:label "risultato da"@it ;
  rdfs:range owl:Thing ;
  rdfs:range org:ChangeEvent ;
  rdfs:range prov:Activity ;
  rdfs:range _:b53184 ;
  rdfs:range _:b170340 ;
  rdfs:range _:b399839 ;
  rdfs:range _:b715640 ;
  rdfs:range _:b895567 ;
  rdfs:range _:b897711 ;
  rdfs:subPropertyOf prov:wasGeneratedBy ;
  rdfs:subPropertyOf prov:wasInfluencedBy ;
  owl:inverseOf org:resultingOrganization ;
.
org:resultingOrganization
  rdf:type rdf:Property ;
  rdf:type owl:ObjectProperty ;
  rdfs:comment "Indica l'organizzazione che è stata creata o mutata a seguito dell'evento. È l'inverso di `org:resultedFrom`."@it ;
  rdfs:comment "Indicates an organization which was created or changed as a result of the event. Inverse of `org:resultedFrom`."@en ;
  rdfs:comment "Indique une organisation qui a été créée ou a été modifiée à la suite d'un Évènement de changement. Inverse de `org:resultedFrom`."@fr ;
  rdfs:comment "Organización que ha sido creada o modificada tras un evento específico.  Es la relación inversa de `org:resultedFrom`."@es ;
  rdfs:comment "出来事の結果、作成、変更された組織を示します。"@ja ;
  rdfs:domain owl:Thing ;
  rdfs:domain org:ChangeEvent ;
  rdfs:domain prov:Activity ;
  rdfs:domain _:b53184 ;
  rdfs:domain _:b170340 ;
  rdfs:domain _:b399839 ;
  rdfs:domain _:b715640 ;
  rdfs:domain _:b895567 ;
  rdfs:domain _:b897711 ;
  rdfs:isDefinedBy <http://www.w3.org/ns/org> ;
  rdfs:label "a donné naissance à"@fr ;
  rdfs:label "resulta en"@es ;
  rdfs:label "resulted in"@en ;
  rdfs:label "risultato in"@it ;
  rdfs:range dcterms:Agent ;
  rdfs:range owl:Thing ;
  rdfs:range org:Organization ;
  rdfs:range foaf:Agent ;
  rdfs:range foaf:Organization ;
  rdfs:range _:b420951 ;
  rdfs:range _:b421075 ;
  rdfs:range _:b421664 ;
  rdfs:range _:b421928 ;
  rdfs:range _:b937877 ;
  rdfs:range _:b938265 ;
  owl:inverseOf org:resultedFrom ;
.
org:role
  rdf:type rdf:Property ;
  rdf:type owl:ObjectProperty ;
  rdfs:comment "Actividad que el agente desempeña en una relación de pertenencia a una organización."@es ;
  rdfs:comment "Indica il Role che un Agent ricopre in una relazione di Membership con una Organization"@it ;
  rdfs:comment "Indicates the Role that the Agent plays in a Membership relationship with an Organization."@en ;
  rdfs:comment "Indique le Rôle de l'Agent dans son Engagement avec l'Organisation."@fr ;
  rdfs:comment "エージェントが組織との構成員関係において担う役割を示します。ポストの保持者が担う役割を示すためにorg:Postで用いることもできます。"@ja ;
  rdfs:domain owl:Thing ;
  rdfs:domain _:b420982 ;
  rdfs:domain _:b421370 ;
  rdfs:domain _:b937443 ;
  rdfs:isDefinedBy <http://www.w3.org/ns/org> ;
  rdfs:label "desempeña la actividad de"@es ;
  rdfs:label "role"@en ;
  rdfs:label "ruolo"@it ;
  rdfs:label "rôle"@fr ;
  rdfs:range owl:Thing ;
  rdfs:range skos:Concept ;
  rdfs:range org:Role ;
  rdfs:range _:b327858 ;
.
org:roleProperty
  rdf:type rdf:Property ;
  rdf:type owl:AnnotationProperty ;
  rdfs:comment "Ceci est une méta-propriété utilisée pour annoter une instance de `org:Role` ayant une sous-propriété `org:memberOf` qui peut être utilisée pour indiquer directement le rôle et pouvoir faire des requêtes plus facilement. La sémantique visée est un Engagement impliquant l'existence d'une relation de propriété directe à travers d'une règle d'inférence de la forme:  `{ [] org:member ?p; org:organization ?o; org:role [org:roleProperty ?r] } -> {?p ?r ?o}`."@fr ;
  rdfs:comment "Meta-propiedad que se utiliza para anotar una instancia de `org:Role` con una sub-propiedad de `org:memberOf`, que puede ser utilizada para indicar directamente la actividad a fin de facilitar las consultas a los datos. The intended semantics is that a Membership relation involving the Role implies the existence of a direct property relationship through an inference rule of the form: { [] org:member ?a; org:organization ?o; org:role [org:roleProperty ?r] } -> {?a ?r ?o}"@es ;
  rdfs:comment "Questa è una meta-proprietà usata per annotare un'istanza di `org:Role` con una sotto-proprietà di `org:memberOf` e può essere usata per indicare direttamente il ruolo per facilitare un'interrogazione sui dati."@it ;
  rdfs:comment "This is a metalevel property which is used to annotate an `org:Role` instance with a sub-property of `org:memberOf` that can be used to directly indicate the role for easy of query. The intended semantics is a Membership relation involving the Role implies the existence of a direct property relationship through an inference rule of the form:  `{ [] org:member ?p; org:organization ?o; org:role [org:roleProperty ?r] } -> {?p ?r ?o}`."@en ;
  rdfs:comment "これは、クエリが容易になるように役割を直接的に示すために使用できるorg:memberOfのサブプロパティーでorg:Roleインスタンスを注釈するために用いられるメタレベルのプロパティーです。"@ja ;
  rdfs:domain owl:Thing ;
  rdfs:domain skos:Concept ;
  rdfs:domain org:Role ;
  rdfs:domain _:b327858 ;
  rdfs:isDefinedBy <http://www.w3.org/ns/org> ;
  rdfs:label "desempeña la actividad de (propiedad)"@es ;
  rdfs:label "role (property)"@en ;
  rdfs:label "ruolo (proprietà)"@it ;
  rdfs:label "rôle (propriété)"@fr ;
  rdfs:range rdf:Property ;
.
org:siteAddress
  rdf:type rdf:Property ;
  rdf:type owl:ObjectProperty ;
  rdfs:comment "Dirección de la sede según una codificación adecuada. Se recomienda el uso de vCard (que utiliza el vocabulario en http://www.w3.org/TR/vcard-rdf/), pero el rango no se restringe únicamente al uso de este vocabulario sino que se permite el uso de otros códigos. La dirección puede constar de una dirección de correo electrónico, un número de teléfono o información de geo-localización, y no se limita a una dirección postal física."@es ;
  rdfs:comment "Indica un indirizzo per la sede in una codifica appropriata. Il codominio è lasciato libero ma è consigliabile l'uso del vocabolario vCard (http://www.w3.org/TR/vcard-rdf/). L'indirizzo può includere email, numero di telefono e informazioni di geolocalizzazione e non è vincolato ad essere un indirizzo fisico."@it ;
  rdfs:comment "Indicates an address for the site in a suitable encoding. Use of vCard (using the http://www.w3.org/TR/vcard-rdf/ vocabulary) is encouraged but the range is left open to allow other encodings to be used. The address may include email, telephone, and geo-location information and is not restricted to a physical address. "@en ;
  rdfs:comment "Indique une adresse pour le site dans un encodage approprié. L'usage du vocabulaire vCard ( http://www.w3.org/TR/vcard-rdf/) est encouragé, mais le range est ouvert pour permettre l'utilisation d'autres vocabulaires. L'adresse peut comporter le courriel, le téléphone, et l'information de géolocalisation; et n'est donc pas seulement limitée à une adresse physique. "@fr ;
  rdfs:comment "適切にコード化されたサイトのアドレスを示します。vCard[vcard-rdf]語彙などの有名なアドレスのコード化の使用が奨励されますが、他の符号化の使用を可能とするために値域はオープンのままにされます。アドレスには、電子メール、電話およびジオロケーション情報を含むことができ、物理的なアドレスに制限されません。"@ja ;
  rdfs:domain owl:Thing ;
  rdfs:domain org:Site ;
  rdfs:isDefinedBy <http://www.w3.org/ns/org> ;
  rdfs:label "adresse du Site"@fr ;
  rdfs:label "es la dirección de la sede"@es ;
  rdfs:label "indirizzo della sede"@it ;
  rdfs:label "site Address"@en ;
.
org:siteOf
  rdf:type rdf:Property ;
  rdf:type owl:ObjectProperty ;
  rdfs:comment "Indica un'Organization che ha una qualche presenza nella data sede. È l'inverso di `org:hasSite`."@it ;
  rdfs:comment "Indicates an Organization which has some presence at the given site. This is the inverse of `org:hasSite`."@en ;
  rdfs:comment "Indique une Organisation qui a une présence sur le site en question. Inverse de `org:hasSite`."@fr ;
  rdfs:comment "Organización que tiene ubicación en un lugar. Es la relación inversa de `org:hasSite`."@es ;
  rdfs:comment "あるサイトである存在感を持っている組織を示します。"@ja ;
  rdfs:domain owl:Thing ;
  rdfs:domain org:Site ;
  rdfs:isDefinedBy <http://www.w3.org/ns/org> ;
  rdfs:label "es sede de"@es ;
  rdfs:label "sede di"@it ;
  rdfs:label "site Of"@en ;
  rdfs:label "site de"@fr ;
  rdfs:range dcterms:Agent ;
  rdfs:range owl:Thing ;
  rdfs:range org:Organization ;
  rdfs:range foaf:Agent ;
  rdfs:range foaf:Organization ;
  rdfs:range _:b420951 ;
  rdfs:range _:b421075 ;
  rdfs:range _:b421664 ;
  rdfs:range _:b421928 ;
  rdfs:range _:b937877 ;
  rdfs:range _:b938265 ;
  owl:equivalentProperty toop:siteOf ;
  owl:inverseOf org:hasSite ;
.
org:subOrganizationOf
  rdf:type rdf:Property ;
  rdf:type owl:ObjectProperty ;
  rdfs:comment "Distribución jerárquica de organizaciones o unidades. Indica que una organización contiene a otra organización. Es la relación inversa de `org:hasSubOrganization`"@es ;
  rdfs:comment "Rappresenta un contenimento gerarchico di una Organization o di una OrganizationalUnit. È l'inverso di `org:hasSubOrganization`. Ha nome come nome alternativo hasSubOrg."@it ;
  rdfs:comment "Represents hierarchical containment of Organizations or OrganizationalUnits; indicates an Organization which contains this Organization. Inverse of `org:hasSubOrganization`."@en ;
  rdfs:comment "Représente une relation hierarchique des Organisations ou des Unités Opérationnelles; indique une Organisation sujet qui contient cette Organisation. Inverse de `org:hasSubOrganization`."@fr ;
  rdfs:comment "組織または組織単位の階層的包含を表わします。この組織を含む組織を示します。"@ja ;
  rdfs:domain dcterms:Agent ;
  rdfs:domain owl:Thing ;
  rdfs:domain org:Organization ;
  rdfs:domain foaf:Agent ;
  rdfs:domain foaf:Organization ;
  rdfs:domain _:b420951 ;
  rdfs:domain _:b421075 ;
  rdfs:domain _:b421664 ;
  rdfs:domain _:b421928 ;
  rdfs:domain _:b937877 ;
  rdfs:domain _:b938265 ;
  rdfs:isDefinedBy <http://www.w3.org/ns/org> ;
  rdfs:label "es suborganización de"@es ;
  rdfs:label "sotto-Organization di"@it ;
  rdfs:label "sous-Organization de"@fr ;
  rdfs:label "subOrganization of"@en ;
  rdfs:range dcterms:Agent ;
  rdfs:range owl:Thing ;
  rdfs:range org:Organization ;
  rdfs:range foaf:Agent ;
  rdfs:range foaf:Organization ;
  rdfs:range _:b420951 ;
  rdfs:range _:b421075 ;
  rdfs:range _:b421664 ;
  rdfs:range _:b421928 ;
  rdfs:range _:b937877 ;
  rdfs:range _:b938265 ;
  rdfs:subPropertyOf org:transitiveSubOrganizationOf ;
  owl:inverseOf org:hasSubOrganization ;
.
org:transitiveSubOrganizationOf
  rdf:type rdf:Property ;
  rdf:type owl:ObjectProperty ;
  rdf:type owl:TransitiveProperty ;
  rdfs:comment "La version transitive de la propriété subOrganizationOf, renvoie une représentation de toutes les organisations qui contiennent celle-ci. Notez que ceci est une super-propriété de la relation transitive donc elle pourrait contenir des assertions additionnelles mais cet usage n'est pas recommandé."@fr ;
  rdfs:comment "La versión transitiva de la propiedad “subOrganizationOf”, es decir, la representación de todas las organizaciones en las que esta está contenida. Téngase en cuenta que desde el punto de vista técnico esta es una propiedad que contiene a todas las propiedades transitivas, de forma que podría contener afirmaciones adicionales, aunque su uso no está aconsejado."@es ;
  rdfs:comment "The transitive closure of subOrganizationOf, giving a representation of all organizations that contain this one. Note that technically this is a super property of the transitive closure so it could contain additional assertions but such usage is discouraged."@en ;
  rdfs:comment "subOrganizationOfの推移閉包で、これを含むすべての組織の表現を与える。技術的に、これが推移閉包のスーパープロパティーであるため、追加の言明を含むことができますが、そのような使用法はお勧めできないことに注意してください。"@ja ;
  rdfs:comment "È la chiusura transitiva di subOrganizationOf, quindi rappresenta tutte le organizzazioni che la contengono. Tecnicamente, essendo una chiusura transitiva, può contenere asserzioni che non la riguardano e quindi il suo uso è sconsigliato."@it ;
  rdfs:domain dcterms:Agent ;
  rdfs:domain owl:Thing ;
  rdfs:domain org:Organization ;
  rdfs:domain foaf:Agent ;
  rdfs:domain foaf:Organization ;
  rdfs:domain _:b420951 ;
  rdfs:domain _:b421075 ;
  rdfs:domain _:b421664 ;
  rdfs:domain _:b421928 ;
  rdfs:domain _:b937877 ;
  rdfs:domain _:b938265 ;
  rdfs:isDefinedBy <http://www.w3.org/ns/org> ;
  rdfs:label "es suborganización de (transitiva)"@es ;
  rdfs:label "es suborganización de manera transitiva de"@es ;
  rdfs:label "sotto-Organization transitiva"@it ;
  rdfs:label "sous-Organization transitive de"@fr ;
  rdfs:label "transitive sub-organization"@en ;
  rdfs:range dcterms:Agent ;
  rdfs:range owl:Thing ;
  rdfs:range org:Organization ;
  rdfs:range foaf:Agent ;
  rdfs:range foaf:Organization ;
  rdfs:range _:b420951 ;
  rdfs:range _:b421075 ;
  rdfs:range _:b421664 ;
  rdfs:range _:b421928 ;
  rdfs:range _:b937877 ;
  rdfs:range _:b938265 ;
.
org:unitOf
  rdf:type rdf:Property ;
  rdf:type owl:ObjectProperty ;
  rdfs:comment "Indica un Organization di cui questa Unit fa parte, come ad esempio un dipartimento all'interno di una più vasta FormalOrganization. È l'inverso di `org:hasUnit`."@it ;
  rdfs:comment "Indicates an Organization of which this Unit is a part, e.g. a Department within a larger FormalOrganization. This is the inverse of `org:hasUnit`."@en ;
  rdfs:comment "Indique l'Organisation dont cette Organisation ou Unité fait partie, par exemple un Départment au sein d'une Organisation Formelle plus large. Inverse de `org:hasUnit`."@fr ;
  rdfs:comment "Organización de la que es parte esta unidad, por ejemplo, un departamento incluido en una organización formal más amplia."@es ;
  rdfs:comment "例えば、より大きな組織内の部局など、この単位がその一部分である組織を示します。"@ja ;
  rdfs:domain dcterms:Agent ;
  rdfs:domain owl:Thing ;
  rdfs:domain org:Organization ;
  rdfs:domain org:OrganizationalUnit ;
  rdfs:domain foaf:Agent ;
  rdfs:domain foaf:Organization ;
  rdfs:domain _:b420951 ;
  rdfs:domain _:b421075 ;
  rdfs:domain _:b421664 ;
  rdfs:domain _:b421928 ;
  rdfs:domain _:b937877 ;
  rdfs:domain _:b938265 ;
  rdfs:isDefinedBy <http://www.w3.org/ns/org> ;
  rdfs:label "es unidad de"@es ;
  rdfs:label "unit Of"@en ;
  rdfs:label "unità di"@it ;
  rdfs:label "unité de"@fr ;
  rdfs:range dcterms:Agent ;
  rdfs:range owl:Thing ;
  rdfs:range org:FormalOrganization ;
  rdfs:range org:Organization ;
  rdfs:range foaf:Agent ;
  rdfs:range foaf:Organization ;
  rdfs:range _:b420951 ;
  rdfs:range _:b421075 ;
  rdfs:range _:b421664 ;
  rdfs:range _:b421928 ;
  rdfs:range _:b937877 ;
  rdfs:range _:b938265 ;
  rdfs:subPropertyOf org:subOrganizationOf ;
  rdfs:subPropertyOf org:transitiveSubOrganizationOf ;
  owl:inverseOf org:hasUnit ;
.
prov:Activity
  rdf:type owl:Class ;
  rdfs:isDefinedBy <http://www.w3.org/ns/prov-o#> ;
  rdfs:label "Activity" ;
  rdfs:seeAlso "http://www.w3.org/TR/2013/REC-prov-constraints-20130430/#prov-dm-constraints-fig"^^xsd:anyURI ;
  rdfs:seeAlso "http://www.w3.org/TR/2013/REC-prov-dm-20130430/#term-Activity"^^xsd:anyURI ;
  rdfs:seeAlso "http://www.w3.org/TR/2013/REC-prov-n-20130430/#expression-Activity"^^xsd:anyURI ;
  rdfs:subClassOf owl:Thing ;
  owl:disjointWith prov:Entity ;
  prov:category "starting-point" ;
  prov:component "entities-activities" ;
  prov:constraints "http://www.w3.org/TR/2013/REC-prov-constraints-20130430/#prov-dm-constraints-fig"^^xsd:anyURI ;
  prov:definition "An activity is something that occurs over a period of time and acts upon or with entities; it may include consuming, processing, transforming, modifying, relocating, using, or generating entities." ;
  prov:dm "http://www.w3.org/TR/2013/REC-prov-dm-20130430/#term-Activity"^^xsd:anyURI ;
  prov:n "http://www.w3.org/TR/2013/REC-prov-n-20130430/#expression-Activity"^^xsd:anyURI ;
.
prov:ActivityInfluence
  rdf:type owl:Class ;
  rdfs:comment "ActivityInfluence provides additional descriptions of an Activity's binary influence upon any other kind of resource. Instances of ActivityInfluence use the prov:activity property to cite the influencing Activity."@en ;
  rdfs:comment "It is not recommended that the type ActivityInfluence be asserted without also asserting one of its more specific subclasses."@en ;
  rdfs:isDefinedBy <http://www.w3.org/ns/prov-o#> ;
  rdfs:label "ActivityInfluence" ;
  rdfs:seeAlso prov:activity ;
  rdfs:subClassOf prov:Influence ;
  rdfs:subClassOf _:b705303 ;
  owl:disjointWith prov:EntityInfluence ;
  prov:category "qualified" ;
  prov:definition "ActivitiyInfluence is the capacity of an activity to have an effect on the character, development, or behavior of another by means of generation, invalidation, communication, or other."@en ;
  prov:editorsDefinition "ActivitiyInfluence is the capacity of an activity to have an effect on the character, development, or behavior of another by means of generation, invalidation, communication, or other."@en ;
.
prov:Agent
  rdf:type owl:Class ;
  rdfs:isDefinedBy <http://www.w3.org/ns/prov-o#> ;
  rdfs:label "Agent" ;
  rdfs:seeAlso "http://www.w3.org/TR/2013/REC-prov-dm-20130430/#term-agent"^^xsd:anyURI ;
  rdfs:seeAlso "http://www.w3.org/TR/2013/REC-prov-n-20130430/#expression-Agent"^^xsd:anyURI ;
  rdfs:subClassOf owl:Thing ;
  owl:disjointWith prov:InstantaneousEvent ;
  prov:category "starting-point" ;
  prov:component "agents-responsibility" ;
  prov:definition "An agent is something that bears some form of responsibility for an activity taking place, for the existence of an entity, or for another agent's activity. "@en ;
  prov:dm "http://www.w3.org/TR/2013/REC-prov-dm-20130430/#term-agent"^^xsd:anyURI ;
  prov:n "http://www.w3.org/TR/2013/REC-prov-n-20130430/#expression-Agent"^^xsd:anyURI ;
.
prov:AgentInfluence
  rdf:type owl:Class ;
  rdfs:comment "AgentInfluence provides additional descriptions of an Agent's binary influence upon any other kind of resource. Instances of AgentInfluence use the prov:agent property to cite the influencing Agent."@en ;
  rdfs:comment "It is not recommended that the type AgentInfluence be asserted without also asserting one of its more specific subclasses."@en ;
  rdfs:isDefinedBy <http://www.w3.org/ns/prov-o#> ;
  rdfs:label "AgentInfluence" ;
  rdfs:seeAlso prov:agent ;
  rdfs:subClassOf prov:Influence ;
  prov:category "qualified" ;
  prov:definition "AgentInfluence is the capacity of an agent to have an effect on the character, development, or behavior of another by means of attribution, association, delegation, or other."@en ;
  prov:editorsDefinition "AgentInfluence is the capacity of an agent to have an effect on the character, development, or behavior of another by means of attribution, association, delegation, or other."@en ;
.
prov:Association
  rdf:type owl:Class ;
  rdfs:comment "An instance of prov:Association provides additional descriptions about the binary prov:wasAssociatedWith relation from an prov:Activity to some prov:Agent that had some responsiblity for it. For example, :baking prov:wasAssociatedWith :baker; prov:qualifiedAssociation [ a prov:Association; prov:agent :baker; :foo :bar ]."@en ;
  rdfs:isDefinedBy <http://www.w3.org/ns/prov-o#> ;
  rdfs:label "Association" ;
  rdfs:seeAlso prov:wasAssociatedWith ;
  rdfs:seeAlso "http://www.w3.org/TR/2013/REC-prov-dm-20130430/#term-Association"^^xsd:anyURI ;
  rdfs:seeAlso "http://www.w3.org/TR/2013/REC-prov-n-20130430/#expression-Association"^^xsd:anyURI ;
  rdfs:subClassOf prov:AgentInfluence ;
  prov:category "qualified" ;
  prov:component "agents-responsibility" ;
  prov:definition "An activity association is an assignment of responsibility to an agent for an activity, indicating that the agent had a role in the activity. It further allows for a plan to be specified, which is the plan intended by the agent to achieve some goals in the context of this activity."@en ;
  prov:dm "http://www.w3.org/TR/2013/REC-prov-dm-20130430/#term-Association"^^xsd:anyURI ;
  prov:n "http://www.w3.org/TR/2013/REC-prov-n-20130430/#expression-Association"^^xsd:anyURI ;
  prov:unqualifiedForm prov:wasAssociatedWith ;
.
prov:Attribution
  rdf:type owl:Class ;
  rdfs:comment "An instance of prov:Attribution provides additional descriptions about the binary prov:wasAttributedTo relation from an prov:Entity to some prov:Agent that had some responsible for it. For example, :cake prov:wasAttributedTo :baker; prov:qualifiedAttribution [ a prov:Attribution; prov:entity :baker; :foo :bar ]."@en ;
  rdfs:isDefinedBy <http://www.w3.org/ns/prov-o#> ;
  rdfs:label "Attribution" ;
  rdfs:seeAlso prov:wasAttributedTo ;
  rdfs:seeAlso "http://www.w3.org/TR/2013/REC-prov-constraints-20130430/#prov-dm-constraints-fig"^^xsd:anyURI ;
  rdfs:seeAlso "http://www.w3.org/TR/2013/REC-prov-dm-20130430/#term-attribution"^^xsd:anyURI ;
  rdfs:seeAlso "http://www.w3.org/TR/2013/REC-prov-n-20130430/#expression-attribution"^^xsd:anyURI ;
  rdfs:subClassOf prov:AgentInfluence ;
  prov:category "qualified" ;
  prov:component "agents-responsibility" ;
  prov:constraints "http://www.w3.org/TR/2013/REC-prov-constraints-20130430/#prov-dm-constraints-fig"^^xsd:anyURI ;
  prov:definition """Attribution is the ascribing of an entity to an agent.

When an entity e is attributed to agent ag, entity e was generated by some unspecified activity that in turn was associated to agent ag. Thus, this relation is useful when the activity is not known, or irrelevant."""@en ;
  prov:dm "http://www.w3.org/TR/2013/REC-prov-dm-20130430/#term-attribution"^^xsd:anyURI ;
  prov:n "http://www.w3.org/TR/2013/REC-prov-n-20130430/#expression-attribution"^^xsd:anyURI ;
  prov:unqualifiedForm prov:wasAttributedTo ;
.
prov:Bundle
  rdf:type owl:Class ;
  rdfs:comment "Note that there are kinds of bundles (e.g. handwritten letters, audio recordings, etc.) that are not expressed in PROV-O, but can be still be described by PROV-O."@en ;
  rdfs:isDefinedBy <http://www.w3.org/ns/prov-o#> ;
  rdfs:label "Bundle" ;
  rdfs:seeAlso "http://www.w3.org/TR/2013/REC-prov-dm-20130430/#term-bundle-entity"^^xsd:anyURI ;
  rdfs:seeAlso "http://www.w3.org/TR/2013/REC-prov-n-20130430/#expression-bundle-declaration"^^xsd:anyURI ;
  rdfs:subClassOf prov:Entity ;
  prov:category "expanded" ;
  prov:definition "A bundle is a named set of provenance descriptions, and is itself an Entity, so allowing provenance of provenance to be expressed."@en ;
  prov:dm "http://www.w3.org/TR/2013/REC-prov-dm-20130430/#term-bundle-entity"^^xsd:anyURI ;
  prov:n "http://www.w3.org/TR/2013/REC-prov-n-20130430/#expression-bundle-declaration"^^xsd:anyURI ;
.
prov:Collection
  rdf:type owl:Class ;
  rdfs:isDefinedBy <http://www.w3.org/ns/prov-o#> ;
  rdfs:label "Collection" ;
  rdfs:seeAlso "http://www.w3.org/TR/2013/REC-prov-dm-20130430/#term-collection"^^xsd:anyURI ;
  rdfs:subClassOf prov:Entity ;
  prov:category "expanded" ;
  prov:component "collections" ;
  prov:definition "A collection is an entity that provides a structure to some constituents, which are themselves entities. These constituents are said to be member of the collections."@en ;
  prov:dm "http://www.w3.org/TR/2013/REC-prov-dm-20130430/#term-collection"^^xsd:anyURI ;
.
prov:Communication
  rdf:type owl:Class ;
  rdfs:comment "An instance of prov:Communication provides additional descriptions about the binary prov:wasInformedBy relation from an informed prov:Activity to the prov:Activity that informed it. For example, :you_jumping_off_bridge prov:wasInformedBy :everyone_else_jumping_off_bridge; prov:qualifiedCommunication [ a prov:Communication; prov:activity :everyone_else_jumping_off_bridge; :foo :bar ]."@en ;
  rdfs:isDefinedBy <http://www.w3.org/ns/prov-o#> ;
  rdfs:label "Communication" ;
  rdfs:seeAlso prov:wasInformedBy ;
  rdfs:seeAlso "http://www.w3.org/TR/2013/REC-prov-constraints-20130430/#prov-dm-constraints-fig"^^xsd:anyURI ;
  rdfs:seeAlso "http://www.w3.org/TR/2013/REC-prov-dm-20130430/#term-Communication"^^xsd:anyURI ;
  rdfs:seeAlso "http://www.w3.org/TR/2013/REC-prov-n-20130430/#expression-wasInformedBy"^^xsd:anyURI ;
  rdfs:subClassOf prov:ActivityInfluence ;
  prov:category "qualified" ;
  prov:component "entities-activities" ;
  prov:constraints "http://www.w3.org/TR/2013/REC-prov-constraints-20130430/#prov-dm-constraints-fig"^^xsd:anyURI ;
  prov:definition "Communication is the exchange of an entity by two activities, one activity using the entity generated by the other." ;
  prov:dm "http://www.w3.org/TR/2013/REC-prov-dm-20130430/#term-Communication"^^xsd:anyURI ;
  prov:n "http://www.w3.org/TR/2013/REC-prov-n-20130430/#expression-wasInformedBy"^^xsd:anyURI ;
  prov:unqualifiedForm prov:wasInformedBy ;
.
prov:Delegation
  rdf:type owl:Class ;
  rdfs:comment "An instance of prov:Delegation provides additional descriptions about the binary prov:actedOnBehalfOf relation from a performing prov:Agent to some prov:Agent for whom it was performed. For example, :mixing prov:wasAssociatedWith :toddler . :toddler prov:actedOnBehalfOf :mother; prov:qualifiedDelegation [ a prov:Delegation; prov:entity :mother; :foo :bar ]."@en ;
  rdfs:isDefinedBy <http://www.w3.org/ns/prov-o#> ;
  rdfs:label "Delegation" ;
  rdfs:seeAlso prov:actedOnBehalfOf ;
  rdfs:seeAlso "http://www.w3.org/TR/2013/REC-prov-dm-20130430/#term-delegation"^^xsd:anyURI ;
  rdfs:seeAlso "http://www.w3.org/TR/2013/REC-prov-n-20130430/#expression-delegation"^^xsd:anyURI ;
  rdfs:subClassOf prov:AgentInfluence ;
  prov:category "qualified" ;
  prov:component "agents-responsibility" ;
  prov:definition """Delegation is the assignment of authority and responsibility to an agent (by itself or by another agent) to carry out a specific activity as a delegate or representative, while the agent it acts on behalf of retains some responsibility for the outcome of the delegated work.

For example, a student acted on behalf of his supervisor, who acted on behalf of the department chair, who acted on behalf of the university; all those agents are responsible in some way for the activity that took place but we do not say explicitly who bears responsibility and to what degree."""@en ;
  prov:dm "http://www.w3.org/TR/2013/REC-prov-dm-20130430/#term-delegation"^^xsd:anyURI ;
  prov:n "http://www.w3.org/TR/2013/REC-prov-n-20130430/#expression-delegation"^^xsd:anyURI ;
  prov:unqualifiedForm prov:actedOnBehalfOf ;
.
prov:Derivation
  rdf:type owl:Class ;
  rdfs:comment "An instance of prov:Derivation provides additional descriptions about the binary prov:wasDerivedFrom relation from some derived prov:Entity to another prov:Entity from which it was derived. For example, :chewed_bubble_gum prov:wasDerivedFrom :unwrapped_bubble_gum; prov:qualifiedDerivation [ a prov:Derivation; prov:entity :unwrapped_bubble_gum; :foo :bar ]."@en ;
  rdfs:comment "The more specific forms of prov:Derivation (i.e., prov:Revision, prov:Quotation, prov:PrimarySource) should be asserted if they apply."@en ;
  rdfs:isDefinedBy <http://www.w3.org/ns/prov-o#> ;
  rdfs:label "Derivation" ;
  rdfs:seeAlso prov:wasDerivedFrom ;
  rdfs:seeAlso "http://www.w3.org/TR/2013/REC-prov-constraints-20130430/#prov-dm-constraints-fig"^^xsd:anyURI ;
  rdfs:seeAlso "http://www.w3.org/TR/2013/REC-prov-dm-20130430/#term-Derivation"^^xsd:anyURI ;
  rdfs:seeAlso "http://www.w3.org/TR/2013/REC-prov-n-20130430/#Derivation-Relation"^^xsd:anyURI ;
  rdfs:subClassOf prov:EntityInfluence ;
  prov:category "qualified" ;
  prov:component "derivations" ;
  prov:constraints "http://www.w3.org/TR/2013/REC-prov-constraints-20130430/#prov-dm-constraints-fig"^^xsd:anyURI ;
  prov:definition "A derivation is a transformation of an entity into another, an update of an entity resulting in a new one, or the construction of a new entity based on a pre-existing entity."@en ;
  prov:dm "http://www.w3.org/TR/2013/REC-prov-dm-20130430/#term-Derivation"^^xsd:anyURI ;
  prov:n "http://www.w3.org/TR/2013/REC-prov-n-20130430/#Derivation-Relation"^^xsd:anyURI ;
  prov:unqualifiedForm prov:wasDerivedFrom ;
.
prov:EmptyCollection
  rdf:type owl:Class ;
  rdf:type owl:NamedIndividual ;
  rdfs:isDefinedBy <http://www.w3.org/ns/prov-o#> ;
  rdfs:label "EmptyCollection"@en ;
  rdfs:subClassOf prov:Collection ;
  prov:category "expanded" ;
  prov:component "collections" ;
  prov:definition "An empty collection is a collection without members."@en ;
.
prov:End
  rdf:type owl:Class ;
  rdfs:comment "An instance of prov:End provides additional descriptions about the binary prov:wasEndedBy relation from some ended prov:Activity to an prov:Entity that ended it. For example, :ball_game prov:wasEndedBy :buzzer; prov:qualifiedEnd [ a prov:End; prov:entity :buzzer; :foo :bar; prov:atTime '2012-03-09T08:05:08-05:00'^^xsd:dateTime ]."@en ;
  rdfs:isDefinedBy <http://www.w3.org/ns/prov-o#> ;
  rdfs:label "End" ;
  rdfs:seeAlso prov:wasEndedBy ;
  rdfs:seeAlso "http://www.w3.org/TR/2013/REC-prov-constraints-20130430/#prov-dm-constraints-fig"^^xsd:anyURI ;
  rdfs:seeAlso "http://www.w3.org/TR/2013/REC-prov-dm-20130430/#term-End"^^xsd:anyURI ;
  rdfs:seeAlso "http://www.w3.org/TR/2013/REC-prov-n-20130430/#expression-End"^^xsd:anyURI ;
  rdfs:subClassOf prov:EntityInfluence ;
  rdfs:subClassOf prov:InstantaneousEvent ;
  prov:category "qualified" ;
  prov:component "entities-activities" ;
  prov:constraints "http://www.w3.org/TR/2013/REC-prov-constraints-20130430/#prov-dm-constraints-fig"^^xsd:anyURI ;
  prov:definition "End is when an activity is deemed to have been ended by an entity, known as trigger. The activity no longer exists after its end. Any usage, generation, or invalidation involving an activity precedes the activity's end. An end may refer to a trigger entity that terminated the activity, or to an activity, known as ender that generated the trigger."@en ;
  prov:dm "http://www.w3.org/TR/2013/REC-prov-dm-20130430/#term-End"^^xsd:anyURI ;
  prov:n "http://www.w3.org/TR/2013/REC-prov-n-20130430/#expression-End"^^xsd:anyURI ;
  prov:unqualifiedForm prov:wasEndedBy ;
.
prov:Entity
  rdf:type owl:Class ;
  rdfs:isDefinedBy <http://www.w3.org/ns/prov-o#> ;
  rdfs:label "Entity" ;
  rdfs:seeAlso "http://www.w3.org/TR/2013/REC-prov-constraints-20130430/#prov-dm-constraints-fig"^^xsd:anyURI ;
  rdfs:seeAlso "http://www.w3.org/TR/2013/REC-prov-dm-20130430/#term-entity"^^xsd:anyURI ;
  rdfs:seeAlso "http://www.w3.org/TR/2013/REC-prov-n-20130430/#expression-Entity"^^xsd:anyURI ;
  rdfs:subClassOf owl:Thing ;
  owl:disjointWith prov:InstantaneousEvent ;
  prov:category "starting-point" ;
  prov:component "entities-activities" ;
  prov:constraints "http://www.w3.org/TR/2013/REC-prov-constraints-20130430/#prov-dm-constraints-fig"^^xsd:anyURI ;
  prov:definition "An entity is a physical, digital, conceptual, or other kind of thing with some fixed aspects; entities may be real or imaginary. "@en ;
  prov:dm "http://www.w3.org/TR/2013/REC-prov-dm-20130430/#term-entity"^^xsd:anyURI ;
  prov:n "http://www.w3.org/TR/2013/REC-prov-n-20130430/#expression-Entity"^^xsd:anyURI ;
.
prov:EntityInfluence
  rdf:type owl:Class ;
  rdfs:comment "EntityInfluence provides additional descriptions of an Entity's binary influence upon any other kind of resource. Instances of EntityInfluence use the prov:entity property to cite the influencing Entity."@en ;
  rdfs:comment "It is not recommended that the type EntityInfluence be asserted without also asserting one of its more specific subclasses."@en ;
  rdfs:isDefinedBy <http://www.w3.org/ns/prov-o#> ;
  rdfs:label "EntityInfluence" ;
  rdfs:seeAlso prov:entity ;
  rdfs:subClassOf prov:Influence ;
  prov:category "qualified" ;
  prov:definition "EntityInfluence is the capacity of an entity to have an effect on the character, development, or behavior of another by means of usage, start, end, derivation, or other. "@en ;
  prov:editorsDefinition "EntityInfluence is the capacity of an entity to have an effect on the character, development, or behavior of another by means of usage, start, end, derivation, or other. "@en ;
.
prov:Generation
  rdf:type owl:Class ;
  rdfs:comment "An instance of prov:Generation provides additional descriptions about the binary prov:wasGeneratedBy relation from a generated prov:Entity to the prov:Activity that generated it. For example, :cake prov:wasGeneratedBy :baking; prov:qualifiedGeneration [ a prov:Generation; prov:activity :baking; :foo :bar ]."@en ;
  rdfs:isDefinedBy <http://www.w3.org/ns/prov-o#> ;
  rdfs:label "Generation" ;
  rdfs:seeAlso prov:wasGeneratedBy ;
  rdfs:seeAlso "http://www.w3.org/TR/2013/REC-prov-constraints-20130430/#prov-dm-constraints-fig"^^xsd:anyURI ;
  rdfs:seeAlso "http://www.w3.org/TR/2013/REC-prov-dm-20130430/#term-Generation"^^xsd:anyURI ;
  rdfs:seeAlso "http://www.w3.org/TR/2013/REC-prov-n-20130430/#expression-Generation"^^xsd:anyURI ;
  rdfs:subClassOf prov:ActivityInfluence ;
  rdfs:subClassOf prov:InstantaneousEvent ;
  prov:category "qualified" ;
  prov:component "entities-activities" ;
  prov:constraints "http://www.w3.org/TR/2013/REC-prov-constraints-20130430/#prov-dm-constraints-fig"^^xsd:anyURI ;
  prov:definition "Generation is the completion of production of a new entity by an activity. This entity did not exist before generation and becomes available for usage after this generation."@en ;
  prov:dm "http://www.w3.org/TR/2013/REC-prov-dm-20130430/#term-Generation"^^xsd:anyURI ;
  prov:n "http://www.w3.org/TR/2013/REC-prov-n-20130430/#expression-Generation"^^xsd:anyURI ;
  prov:unqualifiedForm prov:wasGeneratedBy ;
.
prov:Influence
  rdf:type owl:Class ;
  rdfs:comment "An instance of prov:Influence provides additional descriptions about the binary prov:wasInfluencedBy relation from some influenced Activity, Entity, or Agent to the influencing Activity, Entity, or Agent. For example, :stomach_ache prov:wasInfluencedBy :spoon; prov:qualifiedInfluence [ a prov:Influence; prov:entity :spoon; :foo :bar ] . Because prov:Influence is a broad relation, the more specific relations (Communication, Delegation, End, etc.) should be used when applicable."@en ;
  rdfs:comment "Because prov:Influence is a broad relation, its most specific subclasses (e.g. prov:Communication, prov:Delegation, prov:End, prov:Revision, etc.) should be used when applicable."@en ;
  rdfs:isDefinedBy <http://www.w3.org/ns/prov-o#> ;
  rdfs:label "Influence" ;
  rdfs:seeAlso prov:wasInfluencedBy ;
  rdfs:seeAlso "http://www.w3.org/TR/2013/REC-prov-dm-20130430/#term-influence"^^xsd:anyURI ;
  rdfs:seeAlso "http://www.w3.org/TR/2013/REC-prov-n-20130430/#expression-influence"^^xsd:anyURI ;
  rdfs:subClassOf owl:Thing ;
  prov:category "qualified" ;
  prov:component "derivations" ;
  prov:definition "Influence is the capacity of an entity, activity, or agent to have an effect on the character, development, or behavior of another by means of usage, start, end, generation, invalidation, communication, derivation, attribution, association, or delegation."@en ;
  prov:dm "http://www.w3.org/TR/2013/REC-prov-dm-20130430/#term-influence"^^xsd:anyURI ;
  prov:n "http://www.w3.org/TR/2013/REC-prov-n-20130430/#expression-influence"^^xsd:anyURI ;
  prov:unqualifiedForm prov:wasInfluencedBy ;
.
prov:InstantaneousEvent
  rdf:type owl:Class ;
  rdfs:comment "An instantaneous event, or event for short, happens in the world and marks a change in the world, in its activities and in its entities. The term 'event' is commonly used in process algebra with a similar meaning. Events represent communications or interactions; they are assumed to be atomic and instantaneous."@en ;
  rdfs:isDefinedBy <http://www.w3.org/ns/prov-o#> ;
  rdfs:label "InstantaneousEvent" ;
  rdfs:seeAlso "http://www.w3.org/TR/2013/REC-prov-constraints-20130430/#dfn-event"^^xsd:anyURI ;
  rdfs:subClassOf owl:Thing ;
  prov:category "qualified" ;
  prov:component "entities-activities" ;
  prov:constraints "http://www.w3.org/TR/2013/REC-prov-constraints-20130430/#dfn-event"^^xsd:anyURI ;
  prov:definition "The PROV data model is implicitly based on a notion of instantaneous events (or just events), that mark transitions in the world. Events include generation, usage, or invalidation of entities, as well as starting or ending of activities. This notion of event is not first-class in the data model, but it is useful for explaining its other concepts and its semantics."@en ;
.
prov:Invalidation
  rdf:type owl:Class ;
  rdfs:comment "An instance of prov:Invalidation provides additional descriptions about the binary prov:wasInvalidatedBy relation from an invalidated prov:Entity to the prov:Activity that invalidated it. For example, :uncracked_egg prov:wasInvalidatedBy :baking; prov:qualifiedInvalidation [ a prov:Invalidation; prov:activity :baking; :foo :bar ]."@en ;
  rdfs:isDefinedBy <http://www.w3.org/ns/prov-o#> ;
  rdfs:label "Invalidation" ;
  rdfs:seeAlso prov:wasInvalidatedBy ;
  rdfs:seeAlso "http://www.w3.org/TR/2013/REC-prov-constraints-20130430/#prov-dm-constraints-fig"^^xsd:anyURI ;
  rdfs:seeAlso "http://www.w3.org/TR/2013/REC-prov-dm-20130430/#term-Invalidation"^^xsd:anyURI ;
  rdfs:seeAlso "http://www.w3.org/TR/2013/REC-prov-n-20130430/#expression-Invalidation"^^xsd:anyURI ;
  rdfs:subClassOf prov:ActivityInfluence ;
  rdfs:subClassOf prov:InstantaneousEvent ;
  prov:category "qualified" ;
  prov:component "entities-activities" ;
  prov:constraints "http://www.w3.org/TR/2013/REC-prov-constraints-20130430/#prov-dm-constraints-fig"^^xsd:anyURI ;
  prov:definition "Invalidation is the start of the destruction, cessation, or expiry of an existing entity by an activity. The entity is no longer available for use (or further invalidation) after invalidation. Any generation or usage of an entity precedes its invalidation." ;
  prov:dm "http://www.w3.org/TR/2013/REC-prov-dm-20130430/#term-Invalidation"^^xsd:anyURI ;
  prov:n "http://www.w3.org/TR/2013/REC-prov-n-20130430/#expression-Invalidation"^^xsd:anyURI ;
  prov:unqualifiedForm prov:wasInvalidatedBy ;
.
prov:Location
  rdf:type owl:Class ;
  rdfs:isDefinedBy <http://www.w3.org/ns/prov-o#> ;
  rdfs:label "Location" ;
  rdfs:seeAlso prov:atLocation ;
  rdfs:seeAlso "http://www.w3.org/TR/2013/REC-prov-dm-20130430/#term-attribute-location"^^xsd:anyURI ;
  rdfs:seeAlso "http://www.w3.org/TR/2013/REC-prov-n-20130430/#expression-attribute"^^xsd:anyURI ;
  rdfs:subClassOf owl:Thing ;
  prov:category "expanded" ;
  prov:definition "A location can be an identifiable geographic place (ISO 19112), but it can also be a non-geographic place such as a directory, row, or column. As such, there are numerous ways in which location can be expressed, such as by a coordinate, address, landmark, and so forth."@en ;
  prov:dm "http://www.w3.org/TR/2013/REC-prov-dm-20130430/#term-attribute-location"^^xsd:anyURI ;
  prov:n "http://www.w3.org/TR/2013/REC-prov-n-20130430/#expression-attribute"^^xsd:anyURI ;
.
prov:Organization
  rdf:type owl:Class ;
  rdfs:isDefinedBy <http://www.w3.org/ns/prov-o#> ;
  rdfs:label "Organization" ;
  rdfs:seeAlso "http://www.w3.org/TR/2013/REC-prov-dm-20130430/#term-agent"^^xsd:anyURI ;
  rdfs:seeAlso "http://www.w3.org/TR/2013/REC-prov-n-20130430/#expression-types"^^xsd:anyURI ;
  rdfs:subClassOf prov:Agent ;
  prov:category "expanded" ;
  prov:component "agents-responsibility" ;
  prov:definition "An organization is a social or legal institution such as a company, society, etc." ;
  prov:dm "http://www.w3.org/TR/2013/REC-prov-dm-20130430/#term-agent"^^xsd:anyURI ;
  prov:n "http://www.w3.org/TR/2013/REC-prov-n-20130430/#expression-types"^^xsd:anyURI ;
.
prov:Person
  rdf:type owl:Class ;
  rdfs:isDefinedBy <http://www.w3.org/ns/prov-o#> ;
  rdfs:label "Person" ;
  rdfs:seeAlso "http://www.w3.org/TR/2013/REC-prov-dm-20130430/#term-agent"^^xsd:anyURI ;
  rdfs:seeAlso "http://www.w3.org/TR/2013/REC-prov-n-20130430/#expression-types"^^xsd:anyURI ;
  rdfs:subClassOf prov:Agent ;
  prov:category "expanded" ;
  prov:component "agents-responsibility" ;
  prov:definition "Person agents are people."@en ;
  prov:dm "http://www.w3.org/TR/2013/REC-prov-dm-20130430/#term-agent"^^xsd:anyURI ;
  prov:n "http://www.w3.org/TR/2013/REC-prov-n-20130430/#expression-types"^^xsd:anyURI ;
.
prov:Plan
  rdf:type owl:Class ;
  rdfs:comment "There exist no prescriptive requirement on the nature of plans, their representation, the actions or steps they consist of, or their intended goals. Since plans may evolve over time, it may become necessary to track their provenance, so plans themselves are entities. Representing the plan explicitly in the provenance can be useful for various tasks: for example, to validate the execution as represented in the provenance record, to manage expectation failures, or to provide explanations."@en ;
  rdfs:isDefinedBy <http://www.w3.org/ns/prov-o#> ;
  rdfs:label "Plan" ;
  rdfs:seeAlso "http://www.w3.org/TR/2013/REC-prov-dm-20130430/#term-Association"^^xsd:anyURI ;
  rdfs:seeAlso "http://www.w3.org/TR/2013/REC-prov-n-20130430/#expression-Association"^^xsd:anyURI ;
  rdfs:subClassOf prov:Entity ;
  prov:category "expanded" ;
  prov:category "qualified" ;
  prov:component "agents-responsibility" ;
  prov:definition "A plan is an entity that represents a set of actions or steps intended by one or more agents to achieve some goals." ;
  prov:dm "http://www.w3.org/TR/2013/REC-prov-dm-20130430/#term-Association"^^xsd:anyURI ;
  prov:n "http://www.w3.org/TR/2013/REC-prov-n-20130430/#expression-Association"^^xsd:anyURI ;
.
prov:PrimarySource
  rdf:type owl:Class ;
  rdfs:comment "An instance of prov:PrimarySource provides additional descriptions about the binary prov:hadPrimarySource relation from some secondary prov:Entity to an earlier, primary prov:Entity. For example, :blog prov:hadPrimarySource :newsArticle; prov:qualifiedPrimarySource [ a prov:PrimarySource; prov:entity :newsArticle; :foo :bar ] ."@en ;
  rdfs:isDefinedBy <http://www.w3.org/ns/prov-o#> ;
  rdfs:label "PrimarySource" ;
  rdfs:seeAlso prov:hadPrimarySource ;
  rdfs:seeAlso "http://www.w3.org/TR/2013/REC-prov-dm-20130430/#term-primary-source"^^xsd:anyURI ;
  rdfs:seeAlso "http://www.w3.org/TR/2013/REC-prov-n-20130430/#expression-original-source"^^xsd:anyURI ;
  rdfs:subClassOf prov:Derivation ;
  prov:category "qualified" ;
  prov:component "derivations" ;
  prov:definition """A primary source for a topic refers to something produced by some agent with direct experience and knowledge about the topic, at the time of the topic's study, without benefit from hindsight.

Because of the directness of primary sources, they 'speak for themselves' in ways that cannot be captured through the filter of secondary sources. As such, it is important for secondary sources to reference those primary sources from which they were derived, so that their reliability can be investigated.

A primary source relation is a particular case of derivation of secondary materials from their primary sources. It is recognized that the determination of primary sources can be up to interpretation, and should be done according to conventions accepted within the application's domain."""@en ;
  prov:dm "http://www.w3.org/TR/2013/REC-prov-dm-20130430/#term-primary-source"^^xsd:anyURI ;
  prov:n "http://www.w3.org/TR/2013/REC-prov-n-20130430/#expression-original-source"^^xsd:anyURI ;
  prov:unqualifiedForm prov:hadPrimarySource ;
.
prov:Quotation
  rdf:type owl:Class ;
  rdfs:comment "An instance of prov:Quotation provides additional descriptions about the binary prov:wasQuotedFrom relation from some taken prov:Entity from an earlier, larger prov:Entity. For example, :here_is_looking_at_you_kid prov:wasQuotedFrom :casablanca_script; prov:qualifiedQuotation [ a prov:Quotation; prov:entity :casablanca_script; :foo :bar ]."@en ;
  rdfs:isDefinedBy <http://www.w3.org/ns/prov-o#> ;
  rdfs:label "Quotation" ;
  rdfs:seeAlso prov:wasQuotedFrom ;
  rdfs:seeAlso "http://www.w3.org/TR/2013/REC-prov-dm-20130430/#term-quotation"^^xsd:anyURI ;
  rdfs:seeAlso "http://www.w3.org/TR/2013/REC-prov-n-20130430/#expression-quotation"^^xsd:anyURI ;
  rdfs:subClassOf prov:Derivation ;
  prov:category "qualified" ;
  prov:component "derivations" ;
  prov:definition "A quotation is the repeat of (some or all of) an entity, such as text or image, by someone who may or may not be its original author. Quotation is a particular case of derivation."@en ;
  prov:dm "http://www.w3.org/TR/2013/REC-prov-dm-20130430/#term-quotation"^^xsd:anyURI ;
  prov:n "http://www.w3.org/TR/2013/REC-prov-n-20130430/#expression-quotation"^^xsd:anyURI ;
  prov:unqualifiedForm prov:wasQuotedFrom ;
.
prov:Revision
  rdf:type owl:Class ;
  rdfs:comment "An instance of prov:Revision provides additional descriptions about the binary prov:wasRevisionOf relation from some newer prov:Entity to an earlier prov:Entity. For example, :draft_2 prov:wasRevisionOf :draft_1; prov:qualifiedRevision [ a prov:Revision; prov:entity :draft_1; :foo :bar ]."@en ;
  rdfs:isDefinedBy <http://www.w3.org/ns/prov-o#> ;
  rdfs:label "Revision" ;
  rdfs:seeAlso prov:wasRevisionOf ;
  rdfs:seeAlso "http://www.w3.org/TR/2013/REC-prov-dm-20130430/#term-revision"^^xsd:anyURI ;
  rdfs:seeAlso "http://www.w3.org/TR/2013/REC-prov-n-20130430/#expression-Revision"^^xsd:anyURI ;
  rdfs:subClassOf prov:Derivation ;
  prov:category "qualified" ;
  prov:component "derivations" ;
  prov:definition "A revision is a derivation for which the resulting entity is a revised version of some original. The implication here is that the resulting entity contains substantial content from the original. Revision is a particular case of derivation."@en ;
  prov:dm "http://www.w3.org/TR/2013/REC-prov-dm-20130430/#term-revision"^^xsd:anyURI ;
  prov:n "http://www.w3.org/TR/2013/REC-prov-n-20130430/#expression-Revision"^^xsd:anyURI ;
  prov:unqualifiedForm prov:wasRevisionOf ;
.
prov:Role
  rdf:type owl:Class ;
  rdfs:isDefinedBy <http://www.w3.org/ns/prov-o#> ;
  rdfs:label "Role" ;
  rdfs:seeAlso prov:hadRole ;
  rdfs:seeAlso "http://www.w3.org/TR/2013/REC-prov-dm-20130430/#term-attribute-role"^^xsd:anyURI ;
  rdfs:seeAlso "http://www.w3.org/TR/2013/REC-prov-n-20130430/#expression-attribute"^^xsd:anyURI ;
  rdfs:subClassOf owl:Thing ;
  prov:category "qualified" ;
  prov:component "agents-responsibility" ;
  prov:definition "A role is the function of an entity or agent with respect to an activity, in the context of a usage, generation, invalidation, association, start, and end."@en ;
  prov:dm "http://www.w3.org/TR/2013/REC-prov-dm-20130430/#term-attribute-role"^^xsd:anyURI ;
  prov:n "http://www.w3.org/TR/2013/REC-prov-n-20130430/#expression-attribute"^^xsd:anyURI ;
.
prov:SoftwareAgent
  rdf:type owl:Class ;
  rdfs:isDefinedBy <http://www.w3.org/ns/prov-o#> ;
  rdfs:label "SoftwareAgent" ;
  rdfs:seeAlso "http://www.w3.org/TR/2013/REC-prov-dm-20130430/#term-agent"^^xsd:anyURI ;
  rdfs:seeAlso "http://www.w3.org/TR/2013/REC-prov-n-20130430/#expression-types"^^xsd:anyURI ;
  rdfs:subClassOf prov:Agent ;
  prov:category "expanded" ;
  prov:component "agents-responsibility" ;
  prov:definition "A software agent is running software."@en ;
  prov:dm "http://www.w3.org/TR/2013/REC-prov-dm-20130430/#term-agent"^^xsd:anyURI ;
  prov:n "http://www.w3.org/TR/2013/REC-prov-n-20130430/#expression-types"^^xsd:anyURI ;
.
prov:Start
  rdf:type owl:Class ;
  rdfs:comment "An instance of prov:Start provides additional descriptions about the binary prov:wasStartedBy relation from some started prov:Activity to an prov:Entity that started it. For example, :foot_race prov:wasStartedBy :bang; prov:qualifiedStart [ a prov:Start; prov:entity :bang; :foo :bar; prov:atTime '2012-03-09T08:05:08-05:00'^^xsd:dateTime ] ."@en ;
  rdfs:isDefinedBy <http://www.w3.org/ns/prov-o#> ;
  rdfs:label "Start" ;
  rdfs:seeAlso prov:wasStartedBy ;
  rdfs:seeAlso "http://www.w3.org/TR/2013/REC-prov-constraints-20130430/#prov-dm-constraints-fig"^^xsd:anyURI ;
  rdfs:seeAlso "http://www.w3.org/TR/2013/REC-prov-dm-20130430/#term-Start"^^xsd:anyURI ;
  rdfs:seeAlso "http://www.w3.org/TR/2013/REC-prov-n-20130430/#expression-Start"^^xsd:anyURI ;
  rdfs:subClassOf prov:EntityInfluence ;
  rdfs:subClassOf prov:InstantaneousEvent ;
  prov:category "qualified" ;
  prov:component "entities-activities" ;
  prov:constraints "http://www.w3.org/TR/2013/REC-prov-constraints-20130430/#prov-dm-constraints-fig"^^xsd:anyURI ;
  prov:definition "Start is when an activity is deemed to have been started by an entity, known as trigger. The activity did not exist before its start. Any usage, generation, or invalidation involving an activity follows the activity's start. A start may refer to a trigger entity that set off the activity, or to an activity, known as starter, that generated the trigger."@en ;
  prov:dm "http://www.w3.org/TR/2013/REC-prov-dm-20130430/#term-Start"^^xsd:anyURI ;
  prov:n "http://www.w3.org/TR/2013/REC-prov-n-20130430/#expression-Start"^^xsd:anyURI ;
  prov:unqualifiedForm prov:wasStartedBy ;
.
prov:Usage
  rdf:type owl:Class ;
  rdfs:comment "An instance of prov:Usage provides additional descriptions about the binary prov:used relation from some prov:Activity to an prov:Entity that it used. For example, :keynote prov:used :podium; prov:qualifiedUsage [ a prov:Usage; prov:entity :podium; :foo :bar ]."@en ;
  rdfs:isDefinedBy <http://www.w3.org/ns/prov-o#> ;
  rdfs:label "Usage" ;
  rdfs:seeAlso prov:used ;
  rdfs:seeAlso "http://www.w3.org/TR/2013/REC-prov-constraints-20130430/#prov-dm-constraints-fig"^^xsd:anyURI ;
  rdfs:seeAlso "http://www.w3.org/TR/2013/REC-prov-dm-20130430/#term-Usage"^^xsd:anyURI ;
  rdfs:seeAlso "http://www.w3.org/TR/2013/REC-prov-n-20130430/#expression-Usage"^^xsd:anyURI ;
  rdfs:subClassOf prov:EntityInfluence ;
  rdfs:subClassOf prov:InstantaneousEvent ;
  prov:category "qualified" ;
  prov:component "entities-activities" ;
  prov:constraints "http://www.w3.org/TR/2013/REC-prov-constraints-20130430/#prov-dm-constraints-fig"^^xsd:anyURI ;
  prov:definition "Usage is the beginning of utilizing an entity by an activity. Before usage, the activity had not begun to utilize this entity and could not have been affected by the entity."@en ;
  prov:dm "http://www.w3.org/TR/2013/REC-prov-dm-20130430/#term-Usage"^^xsd:anyURI ;
  prov:n "http://www.w3.org/TR/2013/REC-prov-n-20130430/#expression-Usage"^^xsd:anyURI ;
  prov:unqualifiedForm prov:used ;
.
prov:actedOnBehalfOf
  rdf:type owl:ObjectProperty ;
  rdfs:comment "An object property to express the accountability of an agent towards another agent. The subordinate agent acted on behalf of the responsible agent in an actual activity. "@en ;
  rdfs:domain owl:Thing ;
  rdfs:domain prov:Agent ;
  rdfs:domain _:b53184 ;
  rdfs:domain _:b170340 ;
  rdfs:domain _:b399839 ;
  rdfs:domain _:b715640 ;
  rdfs:domain _:b895567 ;
  rdfs:domain _:b897711 ;
  rdfs:isDefinedBy <http://www.w3.org/ns/prov-o#> ;
  rdfs:label "actedOnBehalfOf" ;
  rdfs:range owl:Thing ;
  rdfs:range prov:Agent ;
  rdfs:range _:b53184 ;
  rdfs:range _:b170340 ;
  rdfs:range _:b399839 ;
  rdfs:range _:b715640 ;
  rdfs:range _:b895567 ;
  rdfs:range _:b897711 ;
  rdfs:seeAlso prov:Delegation ;
  rdfs:seeAlso prov:qualifiedDelegation ;
  rdfs:subPropertyOf prov:wasInfluencedBy ;
  owl:propertyChainAxiom (
      prov:qualifiedDelegation
      prov:agent
    ) ;
  prov:category "starting-point" ;
  prov:component "agents-responsibility" ;
  prov:inverse "hadDelegate" ;
  prov:qualifiedForm prov:Delegation ;
  prov:qualifiedForm prov:qualifiedDelegation ;
.
prov:activity
  rdf:type owl:ObjectProperty ;
  rdfs:domain owl:Thing ;
  rdfs:domain prov:ActivityInfluence ;
  rdfs:domain prov:Influence ;
  rdfs:domain _:b705303 ;
  rdfs:isDefinedBy <http://www.w3.org/ns/prov-o#> ;
  rdfs:label "activity" ;
  rdfs:range owl:Thing ;
  rdfs:range prov:Activity ;
  rdfs:range _:b53184 ;
  rdfs:range _:b170340 ;
  rdfs:range _:b399839 ;
  rdfs:range _:b715640 ;
  rdfs:range _:b895567 ;
  rdfs:range _:b897711 ;
  rdfs:subPropertyOf prov:influencer ;
  prov:category "qualified" ;
  prov:definition "The prov:activity property references an prov:Activity which influenced a resource. This property applies to an prov:ActivityInfluence, which is given by a subproperty of prov:qualifiedInfluence from the influenced prov:Entity, prov:Activity or prov:Agent." ;
  prov:editorialNote "This property behaves in spirit like rdf:object; it references the object of a prov:wasInfluencedBy triple."@en ;
  prov:editorsDefinition "The prov:activity property references an prov:Activity which influenced a resource. This property applies to an prov:ActivityInfluence, which is given by a subproperty of prov:qualifiedInfluence from the influenced prov:Entity, prov:Activity or prov:Agent." ;
  prov:inverse "activityOfInfluence" ;
.
prov:agent
  rdf:type owl:ObjectProperty ;
  rdfs:domain owl:Thing ;
  rdfs:domain prov:AgentInfluence ;
  rdfs:domain prov:Influence ;
  rdfs:isDefinedBy <http://www.w3.org/ns/prov-o#> ;
  rdfs:label "agent" ;
  rdfs:range owl:Thing ;
  rdfs:range prov:Agent ;
  rdfs:range _:b53184 ;
  rdfs:range _:b170340 ;
  rdfs:range _:b399839 ;
  rdfs:range _:b715640 ;
  rdfs:range _:b895567 ;
  rdfs:range _:b897711 ;
  rdfs:subPropertyOf prov:influencer ;
  prov:category "qualified" ;
  prov:definition "The prov:agent property references an prov:Agent which influenced a resource. This property applies to an prov:AgentInfluence, which is given by a subproperty of prov:qualifiedInfluence from the influenced prov:Entity, prov:Activity or prov:Agent."@en ;
  prov:editorialNote "This property behaves in spirit like rdf:object; it references the object of a prov:wasInfluencedBy triple."@en ;
  prov:editorsDefinition "The prov:agent property references an prov:Agent which influenced a resource. This property applies to an prov:AgentInfluence, which is given by a subproperty of prov:qualifiedInfluence from the influenced prov:Entity, prov:Activity or prov:Agent."@en ;
  prov:inverse "agentOfInfluence" ;
.
prov:alternateOf
  rdf:type owl:ObjectProperty ;
  rdfs:domain owl:Thing ;
  rdfs:domain prov:Entity ;
  rdfs:domain _:b53184 ;
  rdfs:domain _:b170340 ;
  rdfs:domain _:b399839 ;
  rdfs:domain _:b715640 ;
  rdfs:domain _:b895567 ;
  rdfs:domain _:b897711 ;
  rdfs:isDefinedBy <http://www.w3.org/ns/prov-o#> ;
  rdfs:label "alternateOf" ;
  rdfs:range owl:Thing ;
  rdfs:range prov:Entity ;
  rdfs:range _:b53184 ;
  rdfs:range _:b170340 ;
  rdfs:range _:b399839 ;
  rdfs:range _:b715640 ;
  rdfs:range _:b895567 ;
  rdfs:range _:b897711 ;
  rdfs:seeAlso prov:specializationOf ;
  rdfs:seeAlso "http://www.w3.org/TR/2013/REC-prov-constraints-20130430/#prov-dm-constraints-fig"^^xsd:anyURI ;
  rdfs:seeAlso "http://www.w3.org/TR/2013/REC-prov-dm-20130430/#term-alternate"^^xsd:anyURI ;
  rdfs:seeAlso "http://www.w3.org/TR/2013/REC-prov-n-20130430/#expression-alternate"^^xsd:anyURI ;
  prov:category "expanded" ;
  prov:component "alternate" ;
  prov:constraints "http://www.w3.org/TR/2013/REC-prov-constraints-20130430/#prov-dm-constraints-fig"^^xsd:anyURI ;
  prov:definition "Two alternate entities present aspects of the same thing. These aspects may be the same or different, and the alternate entities may or may not overlap in time."@en ;
  prov:dm "http://www.w3.org/TR/2013/REC-prov-dm-20130430/#term-alternate"^^xsd:anyURI ;
  prov:inverse "alternateOf" ;
  prov:n "http://www.w3.org/TR/2013/REC-prov-n-20130430/#expression-alternate"^^xsd:anyURI ;
.
prov:aq
  rdf:type owl:AnnotationProperty ;
  rdfs:isDefinedBy <http://www.w3.org/ns/prov-o#> ;
  rdfs:subPropertyOf rdfs:seeAlso ;
.
prov:atLocation
  rdf:type owl:ObjectProperty ;
  rdfs:comment "The Location of any resource."@en ;
  rdfs:comment "This property has multiple RDFS domains to suit multiple OWL Profiles. See <a href=\"#owl-profile\">PROV-O OWL Profile</a>." ;
  rdfs:domain owl:Thing ;
  rdfs:domain _:b897711 ;
  rdfs:isDefinedBy <http://www.w3.org/ns/prov-o#> ;
  rdfs:label "atLocation" ;
  rdfs:range owl:Thing ;
  rdfs:range prov:Location ;
  rdfs:seeAlso prov:Location ;
  prov:category "expanded" ;
  prov:editorialNote "The naming of prov:atLocation parallels prov:atTime, and is not named prov:hadLocation to avoid conflicting with the convention that prov:had* properties are used on prov:Influence classes."@en ;
  prov:editorialNote "This property is not functional because the many values could be at a variety of granularies (In this building, in this room, in that chair)."@en ;
  prov:inverse "locationOf" ;
  prov:sharesDefinitionWith prov:Location ;
.
prov:atTime
  rdf:type owl:DatatypeProperty ;
  rdfs:comment "The time at which an InstantaneousEvent occurred, in the form of xsd:dateTime."@en ;
  rdfs:domain owl:Thing ;
  rdfs:domain prov:InstantaneousEvent ;
  rdfs:domain _:b594637 ;
  rdfs:domain _:b897711 ;
  rdfs:isDefinedBy <http://www.w3.org/ns/prov-o#> ;
  rdfs:label "atTime" ;
  rdfs:range xsd:dateTime ;
  rdfs:range _:b115973 ;
  rdfs:range _:b148299 ;
  rdfs:range _:b671381 ;
  rdfs:range _:b719479 ;
  rdfs:seeAlso prov:InstantaneousEvent ;
  rdfs:seeAlso prov:endedAtTime ;
  rdfs:seeAlso prov:generatedAtTime ;
  rdfs:seeAlso prov:invalidatedAtTime ;
  rdfs:seeAlso prov:startedAtTime ;
  prov:category "qualified" ;
  prov:component "entities-activities" ;
  prov:sharesDefinitionWith prov:InstantaneousEvent ;
  prov:unqualifiedForm prov:endedAtTime ;
  prov:unqualifiedForm prov:generatedAtTime ;
  prov:unqualifiedForm prov:invalidatedAtTime ;
  prov:unqualifiedForm prov:startedAtTime ;
.
prov:category
  rdf:type owl:AnnotationProperty ;
  rdfs:comment "Classify prov-o terms into three categories, including 'starting-point', 'qualifed', and 'extended'. This classification is used by the prov-o html document to gently introduce prov-o terms to its users. "@en ;
  rdfs:isDefinedBy <http://www.w3.org/ns/prov-o#> ;
.
prov:component
  rdf:type owl:AnnotationProperty ;
  rdfs:comment "Classify prov-o terms into six components according to prov-dm, including 'agents-responsibility', 'alternate', 'annotations', 'collections', 'derivations', and 'entities-activities'. This classification is used so that readers of prov-o specification can find its correspondence with the prov-dm specification."@en ;
  rdfs:isDefinedBy <http://www.w3.org/ns/prov-o#> ;
.
prov:constraints
  rdf:type owl:AnnotationProperty ;
  rdfs:comment "A reference to the principal section of the PROV-CONSTRAINTS document that describes this concept."@en ;
  rdfs:isDefinedBy <http://www.w3.org/ns/prov-o#> ;
  rdfs:subPropertyOf rdfs:seeAlso ;
.
prov:definition
  rdf:type owl:AnnotationProperty ;
  rdfs:comment "A definition quoted from PROV-DM or PROV-CONSTRAINTS that describes the concept expressed with this OWL term."@en ;
  rdfs:isDefinedBy <http://www.w3.org/ns/prov-o#> ;
.
prov:dm
  rdf:type owl:AnnotationProperty ;
  rdfs:comment "A reference to the principal section of the PROV-DM document that describes this concept."@en ;
  rdfs:isDefinedBy <http://www.w3.org/ns/prov-o#> ;
  rdfs:subPropertyOf rdfs:seeAlso ;
.
prov:editorialNote
  rdf:type owl:AnnotationProperty ;
  rdfs:comment "A note by the OWL development team about how this term expresses the PROV-DM concept, or how it should be used in context of semantic web or linked data."@en ;
  rdfs:isDefinedBy <http://www.w3.org/ns/prov-o#> ;
.
prov:editorsDefinition
  rdf:type owl:AnnotationProperty ;
  rdfs:comment "When the prov-o term does not have a definition drawn from prov-dm, and the prov-o editor provides one."@en ;
  rdfs:isDefinedBy <http://www.w3.org/ns/prov-o#> ;
  rdfs:subPropertyOf prov:definition ;
.
prov:endedAtTime
  rdf:type owl:DatatypeProperty ;
  rdfs:comment "The time at which an activity ended. See also prov:startedAtTime."@en ;
  rdfs:domain owl:Thing ;
  rdfs:domain prov:Activity ;
  rdfs:domain _:b53184 ;
  rdfs:domain _:b170340 ;
  rdfs:domain _:b399839 ;
  rdfs:domain _:b715640 ;
  rdfs:domain _:b895567 ;
  rdfs:domain _:b897711 ;
  rdfs:isDefinedBy <http://www.w3.org/ns/prov-o#> ;
  rdfs:label "endedAtTime" ;
  rdfs:range xsd:dateTime ;
  rdfs:range _:b115973 ;
  rdfs:range _:b148299 ;
  rdfs:range _:b671381 ;
  rdfs:range _:b719479 ;
  rdfs:seeAlso prov:End ;
  rdfs:seeAlso prov:atTime ;
  prov:category "starting-point" ;
  prov:component "entities-activities" ;
  prov:editorialNote "It is the intent that the property chain holds: (prov:qualifiedEnd o prov:atTime) rdfs:subPropertyOf prov:endedAtTime."@en ;
  prov:qualifiedForm prov:End ;
  prov:qualifiedForm prov:atTime ;
.
prov:entity
  rdf:type owl:ObjectProperty ;
  rdfs:domain owl:Thing ;
  rdfs:domain prov:EntityInfluence ;
  rdfs:domain prov:Influence ;
  rdfs:isDefinedBy <http://www.w3.org/ns/prov-o#> ;
  rdfs:label "entity" ;
  rdfs:range owl:Thing ;
  rdfs:range prov:Entity ;
  rdfs:range _:b53184 ;
  rdfs:range _:b170340 ;
  rdfs:range _:b399839 ;
  rdfs:range _:b715640 ;
  rdfs:range _:b895567 ;
  rdfs:range _:b897711 ;
  rdfs:subPropertyOf prov:influencer ;
  prov:category "qualified" ;
  prov:definition "The prov:entity property references an prov:Entity which influenced a resource. This property applies to an prov:EntityInfluence, which is given by a subproperty of prov:qualifiedInfluence from the influenced prov:Entity, prov:Activity or prov:Agent." ;
  prov:editorialNote "This property behaves in spirit like rdf:object; it references the object of a prov:wasInfluencedBy triple."@en ;
  prov:editorsDefinition "The prov:entity property references an prov:Entity which influenced a resource. This property applies to an prov:EntityInfluence, which is given by a subproperty of prov:qualifiedInfluence from the influenced prov:Entity, prov:Activity or prov:Agent." ;
  prov:inverse "entityOfInfluence" ;
.
prov:generated
  rdf:type owl:ObjectProperty ;
  rdfs:domain owl:Thing ;
  rdfs:domain prov:Activity ;
  rdfs:domain _:b53184 ;
  rdfs:domain _:b170340 ;
  rdfs:domain _:b399839 ;
  rdfs:domain _:b715640 ;
  rdfs:domain _:b895567 ;
  rdfs:domain _:b897711 ;
  rdfs:isDefinedBy <http://www.w3.org/ns/prov-o#> ;
  rdfs:label "generated" ;
  rdfs:range owl:Thing ;
  rdfs:range prov:Entity ;
  rdfs:range _:b53184 ;
  rdfs:range _:b170340 ;
  rdfs:range _:b399839 ;
  rdfs:range _:b715640 ;
  rdfs:range _:b895567 ;
  rdfs:range _:b897711 ;
  rdfs:seeAlso prov:Generation ;
  rdfs:subPropertyOf prov:influenced ;
  owl:inverseOf prov:wasGeneratedBy ;
  prov:category "expanded" ;
  prov:component "entities-activities" ;
  prov:editorialNote "prov:generated is one of few inverse property defined, to allow Activity-oriented assertions in addition to Entity-oriented assertions."@en ;
  prov:inverse "wasGeneratedBy" ;
  prov:sharesDefinitionWith prov:Generation ;
.
prov:generatedAtTime
  rdf:type owl:DatatypeProperty ;
  rdfs:comment "The time at which an entity was completely created and is available for use."@en ;
  rdfs:domain owl:Thing ;
  rdfs:domain prov:Entity ;
  rdfs:domain _:b53184 ;
  rdfs:domain _:b170340 ;
  rdfs:domain _:b399839 ;
  rdfs:domain _:b715640 ;
  rdfs:domain _:b895567 ;
  rdfs:domain _:b897711 ;
  rdfs:isDefinedBy <http://www.w3.org/ns/prov-o#> ;
  rdfs:label "generatedAtTime" ;
  rdfs:range xsd:dateTime ;
  rdfs:range _:b115973 ;
  rdfs:range _:b148299 ;
  rdfs:range _:b671381 ;
  rdfs:range _:b719479 ;
  rdfs:seeAlso prov:Generation ;
  rdfs:seeAlso prov:atTime ;
  prov:category "expanded" ;
  prov:component "entities-activities" ;
  prov:editorialNote "It is the intent that the property chain holds: (prov:qualifiedGeneration o prov:atTime) rdfs:subPropertyOf prov:generatedAtTime."@en ;
  prov:qualifiedForm prov:Generation ;
  prov:qualifiedForm prov:atTime ;
.
prov:hadActivity
  rdf:type owl:ObjectProperty ;
  rdfs:comment "The _optional_ Activity of an Influence, which used, generated, invalidated, or was the responsibility of some Entity. This property is _not_ used by ActivityInfluence (use prov:activity instead)."@en ;
  rdfs:comment "This property has multiple RDFS domains to suit multiple OWL Profiles. See <a href=\"#owl-profile\">PROV-O OWL Profile</a>." ;
  rdfs:domain owl:Thing ;
  rdfs:domain prov:Influence ;
  rdfs:domain _:b275344 ;
  rdfs:isDefinedBy <http://www.w3.org/ns/prov-o#> ;
  rdfs:label "hadActivity" ;
  rdfs:range owl:Thing ;
  rdfs:range prov:Activity ;
  rdfs:range _:b53184 ;
  rdfs:range _:b170340 ;
  rdfs:range _:b399839 ;
  rdfs:range _:b715640 ;
  rdfs:range _:b895567 ;
  rdfs:range _:b897711 ;
  rdfs:seeAlso prov:Activity ;
  prov:category "qualified" ;
  prov:component "derivations" ;
  prov:editorialNote "The multiple rdfs:domain assertions are intended. One is simpler and works for OWL-RL, the union is more specific but is not recognized by OWL-RL."@en ;
  prov:inverse "wasActivityOfInfluence" ;
  prov:sharesDefinitionWith prov:Activity ;
.
prov:hadGeneration
  rdf:type owl:ObjectProperty ;
  rdfs:comment "The _optional_ Generation involved in an Entity's Derivation."@en ;
  rdfs:domain owl:Thing ;
  rdfs:domain prov:Derivation ;
  rdfs:domain prov:EntityInfluence ;
  rdfs:domain prov:Influence ;
  rdfs:domain _:b275344 ;
  rdfs:isDefinedBy <http://www.w3.org/ns/prov-o#> ;
  rdfs:label "hadGeneration" ;
  rdfs:range owl:Thing ;
  rdfs:range prov:ActivityInfluence ;
  rdfs:range prov:Generation ;
  rdfs:range prov:Influence ;
  rdfs:range prov:InstantaneousEvent ;
  rdfs:range _:b594637 ;
  rdfs:range _:b705303 ;
  rdfs:range _:b897711 ;
  rdfs:seeAlso prov:Generation ;
  prov:category "qualified" ;
  prov:component "derivations" ;
  prov:inverse "generatedAsDerivation" ;
  prov:sharesDefinitionWith prov:Generation ;
.
prov:hadMember
  rdf:type owl:ObjectProperty ;
  rdfs:domain owl:Thing ;
  rdfs:domain prov:Collection ;
  rdfs:domain prov:Entity ;
  rdfs:domain _:b53184 ;
  rdfs:domain _:b170340 ;
  rdfs:domain _:b399839 ;
  rdfs:domain _:b715640 ;
  rdfs:domain _:b895567 ;
  rdfs:domain _:b897711 ;
  rdfs:isDefinedBy <http://www.w3.org/ns/prov-o#> ;
  rdfs:label "hadMember" ;
  rdfs:range owl:Thing ;
  rdfs:range prov:Entity ;
  rdfs:range _:b53184 ;
  rdfs:range _:b170340 ;
  rdfs:range _:b399839 ;
  rdfs:range _:b715640 ;
  rdfs:range _:b895567 ;
  rdfs:range _:b897711 ;
  rdfs:seeAlso prov:Collection ;
  rdfs:subPropertyOf prov:wasInfluencedBy ;
  prov:category "expanded" ;
  prov:component "expanded" ;
  prov:inverse "wasMemberOf" ;
  prov:sharesDefinitionWith prov:Collection ;
.
prov:hadPlan
  rdf:type owl:ObjectProperty ;
  rdfs:comment "The _optional_ Plan adopted by an Agent in Association with some Activity. Plan specifications are out of the scope of this specification."@en ;
  rdfs:domain owl:Thing ;
  rdfs:domain prov:AgentInfluence ;
  rdfs:domain prov:Association ;
  rdfs:domain prov:Influence ;
  rdfs:domain _:b594637 ;
  rdfs:isDefinedBy <http://www.w3.org/ns/prov-o#> ;
  rdfs:label "hadPlan" ;
  rdfs:range owl:Thing ;
  rdfs:range prov:Entity ;
  rdfs:range prov:Plan ;
  rdfs:range _:b53184 ;
  rdfs:range _:b170340 ;
  rdfs:range _:b399839 ;
  rdfs:range _:b715640 ;
  rdfs:range _:b895567 ;
  rdfs:range _:b897711 ;
  rdfs:seeAlso prov:Plan ;
  prov:category "qualified" ;
  prov:component "agents-responsibility" ;
  prov:inverse "wasPlanOf" ;
  prov:sharesDefinitionWith prov:Plan ;
.
prov:hadPrimarySource
  rdf:type owl:ObjectProperty ;
  rdfs:domain owl:Thing ;
  rdfs:domain prov:Entity ;
  rdfs:domain _:b53184 ;
  rdfs:domain _:b170340 ;
  rdfs:domain _:b399839 ;
  rdfs:domain _:b715640 ;
  rdfs:domain _:b895567 ;
  rdfs:domain _:b897711 ;
  rdfs:isDefinedBy <http://www.w3.org/ns/prov-o#> ;
  rdfs:label "hadPrimarySource" ;
  rdfs:range owl:Thing ;
  rdfs:range prov:Entity ;
  rdfs:range _:b53184 ;
  rdfs:range _:b170340 ;
  rdfs:range _:b399839 ;
  rdfs:range _:b715640 ;
  rdfs:range _:b895567 ;
  rdfs:range _:b897711 ;
  rdfs:seeAlso prov:PrimarySource ;
  rdfs:seeAlso prov:qualifiedPrimarySource ;
  rdfs:subPropertyOf prov:wasDerivedFrom ;
  rdfs:subPropertyOf prov:wasInfluencedBy ;
  owl:propertyChainAxiom (
      prov:qualifiedPrimarySource
      prov:entity
    ) ;
  prov:category "expanded" ;
  prov:component "derivations" ;
  prov:inverse "wasPrimarySourceOf" ;
  prov:qualifiedForm prov:PrimarySource ;
  prov:qualifiedForm prov:qualifiedPrimarySource ;
.
prov:hadRole
  rdf:type owl:ObjectProperty ;
  rdfs:comment "The _optional_ Role that an Entity assumed in the context of an Activity. For example, :baking prov:used :spoon; prov:qualified [ a prov:Usage; prov:entity :spoon; prov:hadRole roles:mixing_implement ]."@en ;
  rdfs:comment "This property has multiple RDFS domains to suit multiple OWL Profiles. See <a href=\"#owl-profile\">PROV-O OWL Profile</a>." ;
  rdfs:domain owl:Thing ;
  rdfs:domain prov:Influence ;
  rdfs:domain _:b594637 ;
  rdfs:isDefinedBy <http://www.w3.org/ns/prov-o#> ;
  rdfs:label "hadRole" ;
  rdfs:range owl:Thing ;
  rdfs:range prov:Role ;
  rdfs:seeAlso prov:Role ;
  prov:category "qualified" ;
  prov:component "agents-responsibility" ;
  prov:definition "prov:hadRole references the Role (i.e. the function of an entity with respect to an activity), in the context of an instantaneous usage, generation, association, start, and end."@en ;
  prov:editorsDefinition "prov:hadRole references the Role (i.e. the function of an entity with respect to an activity), in the context of an instantaneous usage, generation, association, start, and end."@en ;
  prov:inverse "wasRoleIn" ;
  prov:sharesDefinitionWith prov:Role ;
.
prov:hadUsage
  rdf:type owl:ObjectProperty ;
  rdfs:comment "The _optional_ Usage involved in an Entity's Derivation."@en ;
  rdfs:domain owl:Thing ;
  rdfs:domain prov:Derivation ;
  rdfs:domain prov:EntityInfluence ;
  rdfs:domain prov:Influence ;
  rdfs:domain _:b275344 ;
  rdfs:isDefinedBy <http://www.w3.org/ns/prov-o#> ;
  rdfs:label "hadUsage" ;
  rdfs:range owl:Thing ;
  rdfs:range prov:EntityInfluence ;
  rdfs:range prov:Influence ;
  rdfs:range prov:InstantaneousEvent ;
  rdfs:range prov:Usage ;
  rdfs:range _:b594637 ;
  rdfs:range _:b897711 ;
  rdfs:seeAlso prov:Usage ;
  prov:category "qualified" ;
  prov:component "derivations" ;
  prov:inverse "wasUsedInDerivation" ;
  prov:sharesDefinitionWith prov:Usage ;
.
prov:influenced
  rdf:type owl:ObjectProperty ;
  rdfs:isDefinedBy <http://www.w3.org/ns/prov-o#> ;
  rdfs:label "influenced" ;
  rdfs:seeAlso prov:Influence ;
  owl:inverseOf prov:wasInfluencedBy ;
  prov:category "expanded" ;
  prov:component "agents-responsibility" ;
  prov:inverse "wasInfluencedBy" ;
  prov:sharesDefinitionWith prov:Influence ;
.
prov:influencer
  rdf:type owl:ObjectProperty ;
  rdfs:comment "Subproperties of prov:influencer are used to cite the object of an unqualified PROV-O triple whose predicate is a subproperty of prov:wasInfluencedBy (e.g. prov:used, prov:wasGeneratedBy). prov:influencer is used much like rdf:object is used."@en ;
  rdfs:domain owl:Thing ;
  rdfs:domain prov:Influence ;
  rdfs:isDefinedBy <http://www.w3.org/ns/prov-o#> ;
  rdfs:label "influencer" ;
  rdfs:range owl:Thing ;
  rdfs:seeAlso "http://www.w3.org/TR/2013/REC-prov-dm-20130430/#term-influence"^^xsd:anyURI ;
  prov:category "qualified" ;
  prov:definition "This property is used as part of the qualified influence pattern. Subclasses of prov:Influence use these subproperties to reference the resource (Entity, Agent, or Activity) whose influence is being qualified."@en ;
  prov:dm "http://www.w3.org/TR/2013/REC-prov-dm-20130430/#term-influence"^^xsd:anyURI ;
  prov:editorialNote "This property and its subproperties are used in the same way as the rdf:object property, i.e. to reference the object of an unqualified prov:wasInfluencedBy or prov:influenced triple."@en ;
  prov:editorsDefinition "This property is used as part of the qualified influence pattern. Subclasses of prov:Influence use these subproperties to reference the resource (Entity, Agent, or Activity) whose influence is being qualified."@en ;
  prov:inverse "hadInfluence" ;
.
prov:invalidated
  rdf:type owl:ObjectProperty ;
  rdfs:domain owl:Thing ;
  rdfs:domain prov:Activity ;
  rdfs:domain _:b53184 ;
  rdfs:domain _:b170340 ;
  rdfs:domain _:b399839 ;
  rdfs:domain _:b715640 ;
  rdfs:domain _:b895567 ;
  rdfs:domain _:b897711 ;
  rdfs:isDefinedBy <http://www.w3.org/ns/prov-o#> ;
  rdfs:label "invalidated" ;
  rdfs:range owl:Thing ;
  rdfs:range prov:Entity ;
  rdfs:range _:b53184 ;
  rdfs:range _:b170340 ;
  rdfs:range _:b399839 ;
  rdfs:range _:b715640 ;
  rdfs:range _:b895567 ;
  rdfs:range _:b897711 ;
  rdfs:seeAlso prov:Invalidation ;
  rdfs:subPropertyOf prov:influenced ;
  owl:inverseOf prov:wasInvalidatedBy ;
  prov:category "expanded" ;
  prov:component "entities-activities" ;
  prov:editorialNote "prov:invalidated is one of few inverse property defined, to allow Activity-oriented assertions in addition to Entity-oriented assertions."@en ;
  prov:inverse "wasInvalidatedBy" ;
  prov:sharesDefinitionWith prov:Invalidation ;
.
prov:invalidatedAtTime
  rdf:type owl:DatatypeProperty ;
  rdfs:comment "The time at which an entity was invalidated (i.e., no longer usable)."@en ;
  rdfs:domain owl:Thing ;
  rdfs:domain prov:Entity ;
  rdfs:domain _:b53184 ;
  rdfs:domain _:b170340 ;
  rdfs:domain _:b399839 ;
  rdfs:domain _:b715640 ;
  rdfs:domain _:b895567 ;
  rdfs:domain _:b897711 ;
  rdfs:isDefinedBy <http://www.w3.org/ns/prov-o#> ;
  rdfs:label "invalidatedAtTime" ;
  rdfs:range xsd:dateTime ;
  rdfs:range _:b115973 ;
  rdfs:range _:b148299 ;
  rdfs:range _:b671381 ;
  rdfs:range _:b719479 ;
  rdfs:seeAlso prov:Invalidation ;
  rdfs:seeAlso prov:atTime ;
  prov:category "expanded" ;
  prov:component "entities-activities" ;
  prov:editorialNote "It is the intent that the property chain holds: (prov:qualifiedInvalidation o prov:atTime) rdfs:subPropertyOf prov:invalidatedAtTime."@en ;
  prov:qualifiedForm prov:Invalidation ;
  prov:qualifiedForm prov:atTime ;
.
prov:inverse
  rdf:type owl:AnnotationProperty ;
  rdfs:comment "PROV-O does not define all property inverses. The directionalities defined in PROV-O should be given preference over those not defined. However, if users wish to name the inverse of a PROV-O property, the local name given by prov:inverse should be used."@en ;
  rdfs:isDefinedBy <http://www.w3.org/ns/prov-o#> ;
  rdfs:seeAlso <http://www.w3.org/TR/prov-o/#names-of-inverse-properties> ;
.
prov:n
  rdf:type owl:AnnotationProperty ;
  rdfs:comment "A reference to the principal section of the PROV-DM document that describes this concept."@en ;
  rdfs:isDefinedBy <http://www.w3.org/ns/prov-o#> ;
  rdfs:subPropertyOf rdfs:seeAlso ;
.
prov:order
  rdf:type owl:AnnotationProperty ;
  rdfs:comment "The position that this OWL term should be listed within documentation. The scope of the documentation (e.g., among all terms, among terms within a prov:category, among properties applying to a particular class, etc.) is unspecified."@en ;
  rdfs:isDefinedBy <http://www.w3.org/ns/prov-o#> ;
.
prov:qualifiedAssociation
  rdf:type owl:ObjectProperty ;
  rdfs:comment "If this Activity prov:wasAssociatedWith Agent :ag, then it can qualify the Association using prov:qualifiedAssociation [ a prov:Association;  prov:agent :ag; :foo :bar ]."@en ;
  rdfs:domain owl:Thing ;
  rdfs:domain prov:Activity ;
  rdfs:domain _:b53184 ;
  rdfs:domain _:b170340 ;
  rdfs:domain _:b399839 ;
  rdfs:domain _:b715640 ;
  rdfs:domain _:b895567 ;
  rdfs:domain _:b897711 ;
  rdfs:isDefinedBy <http://www.w3.org/ns/prov-o#> ;
  rdfs:label "qualifiedAssociation" ;
  rdfs:range owl:Thing ;
  rdfs:range prov:AgentInfluence ;
  rdfs:range prov:Association ;
  rdfs:range prov:Influence ;
  rdfs:range _:b594637 ;
  rdfs:seeAlso prov:Association ;
  rdfs:seeAlso prov:wasAssociatedWith ;
  rdfs:subPropertyOf prov:qualifiedInfluence ;
  prov:category "qualified" ;
  prov:component "agents-responsibility" ;
  prov:inverse "qualifiedAssociationOf" ;
  prov:sharesDefinitionWith prov:Association ;
  prov:unqualifiedForm prov:wasAssociatedWith ;
.
prov:qualifiedAttribution
  rdf:type owl:ObjectProperty ;
  rdfs:comment "If this Entity prov:wasAttributedTo Agent :ag, then it can qualify how it was influenced using prov:qualifiedAttribution [ a prov:Attribution;  prov:agent :ag; :foo :bar ]."@en ;
  rdfs:domain owl:Thing ;
  rdfs:domain prov:Entity ;
  rdfs:domain _:b53184 ;
  rdfs:domain _:b170340 ;
  rdfs:domain _:b399839 ;
  rdfs:domain _:b715640 ;
  rdfs:domain _:b895567 ;
  rdfs:domain _:b897711 ;
  rdfs:isDefinedBy <http://www.w3.org/ns/prov-o#> ;
  rdfs:label "qualifiedAttribution" ;
  rdfs:range owl:Thing ;
  rdfs:range prov:AgentInfluence ;
  rdfs:range prov:Attribution ;
  rdfs:range prov:Influence ;
  rdfs:seeAlso prov:Attribution ;
  rdfs:seeAlso prov:wasAttributedTo ;
  rdfs:subPropertyOf prov:qualifiedInfluence ;
  prov:category "qualified" ;
  prov:component "agents-responsibility" ;
  prov:inverse "qualifiedAttributionOf" ;
  prov:sharesDefinitionWith prov:Attribution ;
  prov:unqualifiedForm prov:wasAttributedTo ;
.
prov:qualifiedCommunication
  rdf:type owl:ObjectProperty ;
  rdfs:comment "If this Activity prov:wasInformedBy Activity :a, then it can qualify how it was influenced using prov:qualifiedCommunication [ a prov:Communication;  prov:activity :a; :foo :bar ]."@en ;
  rdfs:domain owl:Thing ;
  rdfs:domain prov:Activity ;
  rdfs:domain _:b53184 ;
  rdfs:domain _:b170340 ;
  rdfs:domain _:b399839 ;
  rdfs:domain _:b715640 ;
  rdfs:domain _:b895567 ;
  rdfs:domain _:b897711 ;
  rdfs:isDefinedBy <http://www.w3.org/ns/prov-o#> ;
  rdfs:label "qualifiedCommunication" ;
  rdfs:range owl:Thing ;
  rdfs:range prov:ActivityInfluence ;
  rdfs:range prov:Communication ;
  rdfs:range prov:Influence ;
  rdfs:range _:b705303 ;
  rdfs:seeAlso prov:Communication ;
  rdfs:subPropertyOf prov:qualifiedInfluence ;
  prov:category "qualified" ;
  prov:component "entities-activities" ;
  prov:inverse "qualifiedCommunicationOf" ;
  prov:qualifiedForm prov:Communication ;
  prov:sharesDefinitionWith prov:Communication ;
.
prov:qualifiedDelegation
  rdf:type owl:ObjectProperty ;
  rdfs:comment "If this Agent prov:actedOnBehalfOf Agent :ag, then it can qualify how with prov:qualifiedResponsibility [ a prov:Responsibility;  prov:agent :ag; :foo :bar ]."@en ;
  rdfs:domain owl:Thing ;
  rdfs:domain prov:Agent ;
  rdfs:domain _:b53184 ;
  rdfs:domain _:b170340 ;
  rdfs:domain _:b399839 ;
  rdfs:domain _:b715640 ;
  rdfs:domain _:b895567 ;
  rdfs:domain _:b897711 ;
  rdfs:isDefinedBy <http://www.w3.org/ns/prov-o#> ;
  rdfs:label "qualifiedDelegation" ;
  rdfs:range owl:Thing ;
  rdfs:range prov:AgentInfluence ;
  rdfs:range prov:Delegation ;
  rdfs:range prov:Influence ;
  rdfs:range _:b275344 ;
  rdfs:seeAlso prov:Delegation ;
  rdfs:seeAlso prov:actedOnBehalfOf ;
  rdfs:subPropertyOf prov:qualifiedInfluence ;
  prov:category "qualified" ;
  prov:component "agents-responsibility" ;
  prov:inverse "qualifiedDelegationOf" ;
  prov:sharesDefinitionWith prov:Delegation ;
  prov:unqualifiedForm prov:actedOnBehalfOf ;
.
prov:qualifiedDerivation
  rdf:type owl:ObjectProperty ;
  rdfs:comment "If this Entity prov:wasDerivedFrom Entity :e, then it can qualify how it was derived using prov:qualifiedDerivation [ a prov:Derivation;  prov:entity :e; :foo :bar ]."@en ;
  rdfs:domain owl:Thing ;
  rdfs:domain prov:Entity ;
  rdfs:domain _:b53184 ;
  rdfs:domain _:b170340 ;
  rdfs:domain _:b399839 ;
  rdfs:domain _:b715640 ;
  rdfs:domain _:b895567 ;
  rdfs:domain _:b897711 ;
  rdfs:isDefinedBy <http://www.w3.org/ns/prov-o#> ;
  rdfs:label "qualifiedDerivation" ;
  rdfs:range owl:Thing ;
  rdfs:range prov:Derivation ;
  rdfs:range prov:EntityInfluence ;
  rdfs:range prov:Influence ;
  rdfs:range _:b275344 ;
  rdfs:seeAlso prov:Derivation ;
  rdfs:seeAlso prov:wasDerivedFrom ;
  rdfs:subPropertyOf prov:qualifiedInfluence ;
  prov:category "qualified" ;
  prov:component "derivations" ;
  prov:inverse "qualifiedDerivationOf" ;
  prov:sharesDefinitionWith prov:Derivation ;
  prov:unqualifiedForm prov:wasDerivedFrom ;
.
prov:qualifiedEnd
  rdf:type owl:ObjectProperty ;
  rdfs:comment "If this Activity prov:wasEndedBy Entity :e1, then it can qualify how it was ended using prov:qualifiedEnd [ a prov:End;  prov:entity :e1; :foo :bar ]."@en ;
  rdfs:domain owl:Thing ;
  rdfs:domain prov:Activity ;
  rdfs:domain _:b53184 ;
  rdfs:domain _:b170340 ;
  rdfs:domain _:b399839 ;
  rdfs:domain _:b715640 ;
  rdfs:domain _:b895567 ;
  rdfs:domain _:b897711 ;
  rdfs:isDefinedBy <http://www.w3.org/ns/prov-o#> ;
  rdfs:label "qualifiedEnd" ;
  rdfs:range owl:Thing ;
  rdfs:range prov:End ;
  rdfs:range prov:EntityInfluence ;
  rdfs:range prov:Influence ;
  rdfs:range prov:InstantaneousEvent ;
  rdfs:range _:b275344 ;
  rdfs:range _:b594637 ;
  rdfs:range _:b897711 ;
  rdfs:seeAlso prov:End ;
  rdfs:seeAlso prov:wasEndedBy ;
  rdfs:subPropertyOf prov:qualifiedInfluence ;
  prov:category "qualified" ;
  prov:component "entities-activities" ;
  prov:inverse "qualifiedEndOf" ;
  prov:sharesDefinitionWith prov:End ;
  prov:unqualifiedForm prov:wasEndedBy ;
.
prov:qualifiedForm
  rdf:type owl:AnnotationProperty ;
  rdfs:comment """This annotation property links a subproperty of prov:wasInfluencedBy with the subclass of prov:Influence and the qualifying property that are used to qualify it. 

Example annotation:

    prov:wasGeneratedBy prov:qualifiedForm prov:qualifiedGeneration, prov:Generation .

Then this unqualified assertion:

    :entity1 prov:wasGeneratedBy :activity1 .

can be qualified by adding:

   :entity1 prov:qualifiedGeneration :entity1Gen .
   :entity1Gen 
       a prov:Generation, prov:Influence;
       prov:activity :activity1;
       :customValue 1337 .

Note how the value of the unqualified influence (prov:wasGeneratedBy :activity1) is mirrored as the value of the prov:activity (or prov:entity, or prov:agent) property on the influence class."""@en ;
  rdfs:isDefinedBy <http://www.w3.org/ns/prov-o#> ;
  rdfs:subPropertyOf rdfs:seeAlso ;
.
prov:qualifiedGeneration
  rdf:type owl:ObjectProperty ;
  rdfs:comment "If this Activity prov:generated Entity :e, then it can qualify how it performed the Generation using prov:qualifiedGeneration [ a prov:Generation;  prov:entity :e; :foo :bar ]."@en ;
  rdfs:domain owl:Thing ;
  rdfs:domain prov:Entity ;
  rdfs:domain _:b53184 ;
  rdfs:domain _:b170340 ;
  rdfs:domain _:b399839 ;
  rdfs:domain _:b715640 ;
  rdfs:domain _:b895567 ;
  rdfs:domain _:b897711 ;
  rdfs:isDefinedBy <http://www.w3.org/ns/prov-o#> ;
  rdfs:label "qualifiedGeneration" ;
  rdfs:range owl:Thing ;
  rdfs:range prov:ActivityInfluence ;
  rdfs:range prov:Generation ;
  rdfs:range prov:Influence ;
  rdfs:range prov:InstantaneousEvent ;
  rdfs:range _:b594637 ;
  rdfs:range _:b705303 ;
  rdfs:range _:b897711 ;
  rdfs:seeAlso prov:Generation ;
  rdfs:seeAlso prov:wasGeneratedBy ;
  rdfs:subPropertyOf prov:qualifiedInfluence ;
  prov:category "qualified" ;
  prov:component "entities-activities" ;
  prov:inverse "qualifiedGenerationOf" ;
  prov:sharesDefinitionWith prov:Generation ;
  prov:unqualifiedForm prov:wasGeneratedBy ;
.
prov:qualifiedInfluence
  rdf:type owl:ObjectProperty ;
  rdfs:comment "Because prov:qualifiedInfluence is a broad relation, the more specific relations (qualifiedCommunication, qualifiedDelegation, qualifiedEnd, etc.) should be used when applicable."@en ;
  rdfs:domain owl:Thing ;
  rdfs:domain _:b170340 ;
  rdfs:isDefinedBy <http://www.w3.org/ns/prov-o#> ;
  rdfs:label "qualifiedInfluence" ;
  rdfs:range owl:Thing ;
  rdfs:range prov:Influence ;
  rdfs:seeAlso prov:Influence ;
  rdfs:seeAlso prov:wasInfluencedBy ;
  prov:category "qualified" ;
  prov:component "derivations" ;
  prov:inverse "qualifiedInfluenceOf" ;
  prov:sharesDefinitionWith prov:Influence ;
  prov:unqualifiedForm prov:wasInfluencedBy ;
.
prov:qualifiedInvalidation
  rdf:type owl:ObjectProperty ;
  rdfs:comment "If this Entity prov:wasInvalidatedBy Activity :a, then it can qualify how it was invalidated using prov:qualifiedInvalidation [ a prov:Invalidation;  prov:activity :a; :foo :bar ]."@en ;
  rdfs:domain owl:Thing ;
  rdfs:domain prov:Entity ;
  rdfs:domain _:b53184 ;
  rdfs:domain _:b170340 ;
  rdfs:domain _:b399839 ;
  rdfs:domain _:b715640 ;
  rdfs:domain _:b895567 ;
  rdfs:domain _:b897711 ;
  rdfs:isDefinedBy <http://www.w3.org/ns/prov-o#> ;
  rdfs:label "qualifiedInvalidation" ;
  rdfs:range owl:Thing ;
  rdfs:range prov:ActivityInfluence ;
  rdfs:range prov:Influence ;
  rdfs:range prov:InstantaneousEvent ;
  rdfs:range prov:Invalidation ;
  rdfs:range _:b594637 ;
  rdfs:range _:b705303 ;
  rdfs:range _:b897711 ;
  rdfs:seeAlso prov:Invalidation ;
  rdfs:seeAlso prov:wasInvalidatedBy ;
  rdfs:subPropertyOf prov:qualifiedInfluence ;
  prov:category "qualified" ;
  prov:component "entities-activities" ;
  prov:inverse "qualifiedInvalidationOf" ;
  prov:sharesDefinitionWith prov:Invalidation ;
  prov:unqualifiedForm prov:wasInvalidatedBy ;
.
prov:qualifiedPrimarySource
  rdf:type owl:ObjectProperty ;
  rdfs:comment "If this Entity prov:hadPrimarySource Entity :e, then it can qualify how using prov:qualifiedPrimarySource [ a prov:PrimarySource; prov:entity :e; :foo :bar ]."@en ;
  rdfs:domain owl:Thing ;
  rdfs:domain prov:Entity ;
  rdfs:domain _:b53184 ;
  rdfs:domain _:b170340 ;
  rdfs:domain _:b399839 ;
  rdfs:domain _:b715640 ;
  rdfs:domain _:b895567 ;
  rdfs:domain _:b897711 ;
  rdfs:isDefinedBy <http://www.w3.org/ns/prov-o#> ;
  rdfs:label "qualifiedPrimarySource" ;
  rdfs:range owl:Thing ;
  rdfs:range prov:Derivation ;
  rdfs:range prov:EntityInfluence ;
  rdfs:range prov:Influence ;
  rdfs:range prov:PrimarySource ;
  rdfs:range _:b275344 ;
  rdfs:seeAlso prov:PrimarySource ;
  rdfs:seeAlso prov:hadPrimarySource ;
  rdfs:subPropertyOf prov:qualifiedInfluence ;
  prov:category "qualified" ;
  prov:component "derivations" ;
  prov:inverse "qualifiedSourceOf" ;
  prov:sharesDefinitionWith prov:PrimarySource ;
  prov:unqualifiedForm prov:hadPrimarySource ;
.
prov:qualifiedQuotation
  rdf:type owl:ObjectProperty ;
  rdfs:comment "If this Entity prov:wasQuotedFrom Entity :e, then it can qualify how using prov:qualifiedQuotation [ a prov:Quotation;  prov:entity :e; :foo :bar ]."@en ;
  rdfs:domain owl:Thing ;
  rdfs:domain prov:Entity ;
  rdfs:domain _:b53184 ;
  rdfs:domain _:b170340 ;
  rdfs:domain _:b399839 ;
  rdfs:domain _:b715640 ;
  rdfs:domain _:b895567 ;
  rdfs:domain _:b897711 ;
  rdfs:isDefinedBy <http://www.w3.org/ns/prov-o#> ;
  rdfs:label "qualifiedQuotation" ;
  rdfs:range owl:Thing ;
  rdfs:range prov:Derivation ;
  rdfs:range prov:EntityInfluence ;
  rdfs:range prov:Influence ;
  rdfs:range prov:Quotation ;
  rdfs:range _:b275344 ;
  rdfs:seeAlso prov:Quotation ;
  rdfs:seeAlso prov:wasQuotedFrom ;
  rdfs:subPropertyOf prov:qualifiedInfluence ;
  prov:category "qualified" ;
  prov:component "derivations" ;
  prov:inverse "qualifiedQuotationOf" ;
  prov:sharesDefinitionWith prov:Quotation ;
  prov:unqualifiedForm prov:wasQuotedFrom ;
.
prov:qualifiedRevision
  rdf:type owl:ObjectProperty ;
  rdfs:comment "If this Entity prov:wasRevisionOf Entity :e, then it can qualify how it was revised using prov:qualifiedRevision [ a prov:Revision;  prov:entity :e; :foo :bar ]."@en ;
  rdfs:domain owl:Thing ;
  rdfs:domain prov:Entity ;
  rdfs:domain _:b53184 ;
  rdfs:domain _:b170340 ;
  rdfs:domain _:b399839 ;
  rdfs:domain _:b715640 ;
  rdfs:domain _:b895567 ;
  rdfs:domain _:b897711 ;
  rdfs:isDefinedBy <http://www.w3.org/ns/prov-o#> ;
  rdfs:label "qualifiedRevision" ;
  rdfs:range owl:Thing ;
  rdfs:range prov:Derivation ;
  rdfs:range prov:EntityInfluence ;
  rdfs:range prov:Influence ;
  rdfs:range prov:Revision ;
  rdfs:range _:b275344 ;
  rdfs:seeAlso prov:Revision ;
  rdfs:seeAlso prov:wasRevisionOf ;
  rdfs:subPropertyOf prov:qualifiedInfluence ;
  prov:category "qualified" ;
  prov:component "derivations" ;
  prov:inverse "revisedEntity" ;
  prov:sharesDefinitionWith prov:Revision ;
  prov:unqualifiedForm prov:wasRevisionOf ;
.
prov:qualifiedStart
  rdf:type owl:ObjectProperty ;
  rdfs:comment "If this Activity prov:wasStartedBy Entity :e1, then it can qualify how it was started using prov:qualifiedStart [ a prov:Start;  prov:entity :e1; :foo :bar ]."@en ;
  rdfs:domain owl:Thing ;
  rdfs:domain prov:Activity ;
  rdfs:domain _:b53184 ;
  rdfs:domain _:b170340 ;
  rdfs:domain _:b399839 ;
  rdfs:domain _:b715640 ;
  rdfs:domain _:b895567 ;
  rdfs:domain _:b897711 ;
  rdfs:isDefinedBy <http://www.w3.org/ns/prov-o#> ;
  rdfs:label "qualifiedStart" ;
  rdfs:range owl:Thing ;
  rdfs:range prov:EntityInfluence ;
  rdfs:range prov:Influence ;
  rdfs:range prov:InstantaneousEvent ;
  rdfs:range prov:Start ;
  rdfs:range _:b275344 ;
  rdfs:range _:b594637 ;
  rdfs:range _:b897711 ;
  rdfs:seeAlso prov:Start ;
  rdfs:seeAlso prov:wasStartedBy ;
  rdfs:subPropertyOf prov:qualifiedInfluence ;
  prov:category "qualified" ;
  prov:component "entities-activities" ;
  prov:inverse "qualifiedStartOf" ;
  prov:sharesDefinitionWith prov:Start ;
  prov:unqualifiedForm prov:wasStartedBy ;
.
prov:qualifiedUsage
  rdf:type owl:ObjectProperty ;
  rdfs:comment "If this Activity prov:used Entity :e, then it can qualify how it used it using prov:qualifiedUsage [ a prov:Usage; prov:entity :e; :foo :bar ]."@en ;
  rdfs:domain owl:Thing ;
  rdfs:domain prov:Activity ;
  rdfs:domain _:b53184 ;
  rdfs:domain _:b170340 ;
  rdfs:domain _:b399839 ;
  rdfs:domain _:b715640 ;
  rdfs:domain _:b895567 ;
  rdfs:domain _:b897711 ;
  rdfs:isDefinedBy <http://www.w3.org/ns/prov-o#> ;
  rdfs:label "qualifiedUsage" ;
  rdfs:range owl:Thing ;
  rdfs:range prov:EntityInfluence ;
  rdfs:range prov:Influence ;
  rdfs:range prov:InstantaneousEvent ;
  rdfs:range prov:Usage ;
  rdfs:range _:b594637 ;
  rdfs:range _:b897711 ;
  rdfs:seeAlso prov:Usage ;
  rdfs:seeAlso prov:used ;
  rdfs:subPropertyOf prov:qualifiedInfluence ;
  prov:category "qualified" ;
  prov:component "entities-activities" ;
  prov:inverse "qualifiedUsingActivity" ;
  prov:sharesDefinitionWith prov:Usage ;
  prov:unqualifiedForm prov:used ;
.
prov:sharesDefinitionWith
  rdf:type owl:AnnotationProperty ;
  rdfs:isDefinedBy <http://www.w3.org/ns/prov-o#> ;
  rdfs:subPropertyOf rdfs:seeAlso ;
.
prov:specializationOf
  rdf:type owl:AnnotationProperty ;
  rdf:type owl:ObjectProperty ;
  rdfs:domain owl:Thing ;
  rdfs:domain prov:Entity ;
  rdfs:domain _:b53184 ;
  rdfs:domain _:b170340 ;
  rdfs:domain _:b399839 ;
  rdfs:domain _:b715640 ;
  rdfs:domain _:b895567 ;
  rdfs:domain _:b897711 ;
  rdfs:isDefinedBy <http://www.w3.org/ns/prov-o#> ;
  rdfs:label "specializationOf" ;
  rdfs:range owl:Thing ;
  rdfs:range prov:Entity ;
  rdfs:range _:b53184 ;
  rdfs:range _:b170340 ;
  rdfs:range _:b399839 ;
  rdfs:range _:b715640 ;
  rdfs:range _:b895567 ;
  rdfs:range _:b897711 ;
  rdfs:seeAlso prov:alternateOf ;
  rdfs:seeAlso "http://www.w3.org/TR/2013/REC-prov-constraints-20130430/#prov-dm-constraints-fig"^^xsd:anyURI ;
  rdfs:seeAlso "http://www.w3.org/TR/2013/REC-prov-dm-20130430/#term-specialization"^^xsd:anyURI ;
  rdfs:seeAlso "http://www.w3.org/TR/2013/REC-prov-n-20130430/#expression-specialization"^^xsd:anyURI ;
  rdfs:subPropertyOf prov:alternateOf ;
  prov:category "expanded" ;
  prov:component "alternate" ;
  prov:constraints "http://www.w3.org/TR/2013/REC-prov-constraints-20130430/#prov-dm-constraints-fig"^^xsd:anyURI ;
  prov:definition "An entity that is a specialization of another shares all aspects of the latter, and additionally presents more specific aspects of the same thing as the latter. In particular, the lifetime of the entity being specialized contains that of any specialization. Examples of aspects include a time period, an abstraction, and a context associated with the entity."@en ;
  prov:dm "http://www.w3.org/TR/2013/REC-prov-dm-20130430/#term-specialization"^^xsd:anyURI ;
  prov:inverse "generalizationOf" ;
  prov:n "http://www.w3.org/TR/2013/REC-prov-n-20130430/#expression-specialization"^^xsd:anyURI ;
.
prov:startedAtTime
  rdf:type owl:DatatypeProperty ;
  rdfs:comment "The time at which an activity started. See also prov:endedAtTime."@en ;
  rdfs:domain owl:Thing ;
  rdfs:domain prov:Activity ;
  rdfs:domain _:b53184 ;
  rdfs:domain _:b170340 ;
  rdfs:domain _:b399839 ;
  rdfs:domain _:b715640 ;
  rdfs:domain _:b895567 ;
  rdfs:domain _:b897711 ;
  rdfs:isDefinedBy <http://www.w3.org/ns/prov-o#> ;
  rdfs:label "startedAtTime" ;
  rdfs:range xsd:dateTime ;
  rdfs:range _:b115973 ;
  rdfs:range _:b148299 ;
  rdfs:range _:b671381 ;
  rdfs:range _:b719479 ;
  rdfs:seeAlso prov:Start ;
  rdfs:seeAlso prov:atTime ;
  prov:category "starting-point" ;
  prov:component "entities-activities" ;
  prov:editorialNote "It is the intent that the property chain holds: (prov:qualifiedStart o prov:atTime) rdfs:subPropertyOf prov:startedAtTime."@en ;
  prov:qualifiedForm prov:Start ;
  prov:qualifiedForm prov:atTime ;
.
prov:todo
  rdf:type owl:AnnotationProperty ;
.
prov:unqualifiedForm
  rdf:type owl:AnnotationProperty ;
  rdfs:comment "Classes and properties used to qualify relationships are annotated with prov:unqualifiedForm to indicate the property used to assert an unqualified provenance relation."@en ;
  rdfs:isDefinedBy <http://www.w3.org/ns/prov-o#> ;
  rdfs:subPropertyOf rdfs:seeAlso ;
.
prov:used
  rdf:type owl:ObjectProperty ;
  rdfs:comment "A prov:Entity that was used by this prov:Activity. For example, :baking prov:used :spoon, :egg, :oven ."@en ;
  rdfs:domain owl:Thing ;
  rdfs:domain prov:Activity ;
  rdfs:domain _:b53184 ;
  rdfs:domain _:b170340 ;
  rdfs:domain _:b399839 ;
  rdfs:domain _:b715640 ;
  rdfs:domain _:b895567 ;
  rdfs:domain _:b897711 ;
  rdfs:isDefinedBy <http://www.w3.org/ns/prov-o#> ;
  rdfs:label "used" ;
  rdfs:range owl:Thing ;
  rdfs:range prov:Entity ;
  rdfs:range _:b53184 ;
  rdfs:range _:b170340 ;
  rdfs:range _:b399839 ;
  rdfs:range _:b715640 ;
  rdfs:range _:b895567 ;
  rdfs:range _:b897711 ;
  rdfs:seeAlso prov:Usage ;
  rdfs:seeAlso prov:qualifiedUsage ;
  rdfs:subPropertyOf prov:wasInfluencedBy ;
  owl:propertyChainAxiom (
      prov:qualifiedUsage
      prov:entity
    ) ;
  prov:category "starting-point" ;
  prov:component "entities-activities" ;
  prov:inverse "wasUsedBy" ;
  prov:qualifiedForm prov:Usage ;
  prov:qualifiedForm prov:qualifiedUsage ;
.
prov:value
  rdf:type owl:DatatypeProperty ;
  rdfs:domain owl:Thing ;
  rdfs:domain prov:Entity ;
  rdfs:domain _:b53184 ;
  rdfs:domain _:b170340 ;
  rdfs:domain _:b399839 ;
  rdfs:domain _:b715640 ;
  rdfs:domain _:b895567 ;
  rdfs:domain _:b897711 ;
  rdfs:isDefinedBy <http://www.w3.org/ns/prov-o#> ;
  rdfs:label "value" ;
  rdfs:seeAlso "http://www.w3.org/TR/2013/REC-prov-dm-20130430/#term-attribute-value"^^xsd:anyURI ;
  prov:category "expanded" ;
  prov:component "entities-activities" ;
  prov:definition "Provides a value that is a direct representation of an entity."@en ;
  prov:dm "http://www.w3.org/TR/2013/REC-prov-dm-20130430/#term-attribute-value"^^xsd:anyURI ;
  prov:editorialNote "The editor's definition comes from http://www.w3.org/TR/rdf-primer/#rdfvalue" ;
  prov:editorialNote "This property serves the same purpose as rdf:value, but has been reintroduced to avoid some of the definitional ambiguity in the RDF specification (specifically, 'may be used in describing structured values')."@en ;
.
prov:wasAssociatedWith
  rdf:type owl:ObjectProperty ;
  rdfs:comment "An prov:Agent that had some (unspecified) responsibility for the occurrence of this prov:Activity."@en ;
  rdfs:domain owl:Thing ;
  rdfs:domain prov:Activity ;
  rdfs:domain _:b53184 ;
  rdfs:domain _:b170340 ;
  rdfs:domain _:b399839 ;
  rdfs:domain _:b715640 ;
  rdfs:domain _:b895567 ;
  rdfs:domain _:b897711 ;
  rdfs:isDefinedBy <http://www.w3.org/ns/prov-o#> ;
  rdfs:label "wasAssociatedWith" ;
  rdfs:range owl:Thing ;
  rdfs:range prov:Agent ;
  rdfs:range _:b53184 ;
  rdfs:range _:b170340 ;
  rdfs:range _:b399839 ;
  rdfs:range _:b715640 ;
  rdfs:range _:b895567 ;
  rdfs:range _:b897711 ;
  rdfs:seeAlso prov:Association ;
  rdfs:seeAlso prov:qualifiedAssociation ;
  rdfs:subPropertyOf prov:wasInfluencedBy ;
  owl:propertyChainAxiom (
      prov:qualifiedAssociation
      prov:agent
    ) ;
  prov:category "starting-point" ;
  prov:component "agents-responsibility" ;
  prov:inverse "wasAssociateFor" ;
  prov:qualifiedForm prov:Association ;
  prov:qualifiedForm prov:qualifiedAssociation ;
.
prov:wasAttributedTo
  rdf:type owl:ObjectProperty ;
  rdfs:comment "Attribution is the ascribing of an entity to an agent."@en ;
  rdfs:domain owl:Thing ;
  rdfs:domain prov:Entity ;
  rdfs:domain _:b53184 ;
  rdfs:domain _:b170340 ;
  rdfs:domain _:b399839 ;
  rdfs:domain _:b715640 ;
  rdfs:domain _:b895567 ;
  rdfs:domain _:b897711 ;
  rdfs:isDefinedBy <http://www.w3.org/ns/prov-o#> ;
  rdfs:label "wasAttributedTo" ;
  rdfs:range owl:Thing ;
  rdfs:range prov:Agent ;
  rdfs:range _:b53184 ;
  rdfs:range _:b170340 ;
  rdfs:range _:b399839 ;
  rdfs:range _:b715640 ;
  rdfs:range _:b895567 ;
  rdfs:range _:b897711 ;
  rdfs:seeAlso prov:Attribution ;
  rdfs:seeAlso prov:qualifiedAttribution ;
  rdfs:subPropertyOf prov:wasInfluencedBy ;
  owl:propertyChainAxiom (
      prov:qualifiedAttribution
      prov:agent
    ) ;
  prov:category "starting-point" ;
  prov:component "agents-responsibility" ;
  prov:definition "Attribution is the ascribing of an entity to an agent."@en ;
  prov:inverse "contributed" ;
  prov:qualifiedForm prov:Attribution ;
  prov:qualifiedForm prov:qualifiedAttribution ;
.
prov:wasDerivedFrom
  rdf:type owl:ObjectProperty ;
  rdfs:comment "The more specific subproperties of prov:wasDerivedFrom (i.e., prov:wasQuotedFrom, prov:wasRevisionOf, prov:hadPrimarySource) should be used when applicable."@en ;
  rdfs:domain owl:Thing ;
  rdfs:domain prov:Entity ;
  rdfs:domain _:b53184 ;
  rdfs:domain _:b170340 ;
  rdfs:domain _:b399839 ;
  rdfs:domain _:b715640 ;
  rdfs:domain _:b895567 ;
  rdfs:domain _:b897711 ;
  rdfs:isDefinedBy <http://www.w3.org/ns/prov-o#> ;
  rdfs:label "wasDerivedFrom" ;
  rdfs:range owl:Thing ;
  rdfs:range prov:Entity ;
  rdfs:range _:b53184 ;
  rdfs:range _:b170340 ;
  rdfs:range _:b399839 ;
  rdfs:range _:b715640 ;
  rdfs:range _:b895567 ;
  rdfs:range _:b897711 ;
  rdfs:seeAlso prov:Derivation ;
  rdfs:seeAlso prov:qualifiedDerivation ;
  rdfs:subPropertyOf prov:wasInfluencedBy ;
  owl:propertyChainAxiom (
      org:resultedFrom
      org:originalOrganization
    ) ;
  owl:propertyChainAxiom (
      org:resultedFrom
      org:originalOrganization
    ) ;
  owl:propertyChainAxiom (
      org:resultedFrom
      org:originalOrganization
    ) ;
  owl:propertyChainAxiom (
      prov:qualifiedDerivation
      prov:entity
    ) ;
  prov:category "starting-point" ;
  prov:component "derivations" ;
  prov:definition "A derivation is a transformation of an entity into another, an update of an entity resulting in a new one, or the construction of a new entity based on a pre-existing entity."@en ;
  prov:inverse "hadDerivation" ;
  prov:qualifiedForm prov:Derivation ;
  prov:qualifiedForm prov:qualifiedDerivation ;
.
prov:wasEndedBy
  rdf:type owl:ObjectProperty ;
  rdfs:comment "End is when an activity is deemed to have ended. An end may refer to an entity, known as trigger, that terminated the activity."@en ;
  rdfs:domain owl:Thing ;
  rdfs:domain prov:Activity ;
  rdfs:domain _:b53184 ;
  rdfs:domain _:b170340 ;
  rdfs:domain _:b399839 ;
  rdfs:domain _:b715640 ;
  rdfs:domain _:b895567 ;
  rdfs:domain _:b897711 ;
  rdfs:isDefinedBy <http://www.w3.org/ns/prov-o#> ;
  rdfs:label "wasEndedBy" ;
  rdfs:range owl:Thing ;
  rdfs:range prov:Entity ;
  rdfs:range _:b53184 ;
  rdfs:range _:b170340 ;
  rdfs:range _:b399839 ;
  rdfs:range _:b715640 ;
  rdfs:range _:b895567 ;
  rdfs:range _:b897711 ;
  rdfs:seeAlso prov:End ;
  rdfs:seeAlso prov:qualifiedEnd ;
  rdfs:subPropertyOf prov:wasInfluencedBy ;
  owl:propertyChainAxiom (
      prov:qualifiedEnd
      prov:entity
    ) ;
  prov:category "expanded" ;
  prov:component "entities-activities" ;
  prov:inverse "ended" ;
  prov:qualifiedForm prov:End ;
  prov:qualifiedForm prov:qualifiedEnd ;
.
prov:wasGeneratedBy
  rdf:type owl:ObjectProperty ;
  rdfs:domain owl:Thing ;
  rdfs:domain prov:Entity ;
  rdfs:domain _:b53184 ;
  rdfs:domain _:b170340 ;
  rdfs:domain _:b399839 ;
  rdfs:domain _:b715640 ;
  rdfs:domain _:b895567 ;
  rdfs:domain _:b897711 ;
  rdfs:isDefinedBy <http://www.w3.org/ns/prov-o#> ;
  rdfs:label "wasGeneratedBy" ;
  rdfs:range owl:Thing ;
  rdfs:range prov:Activity ;
  rdfs:range _:b53184 ;
  rdfs:range _:b170340 ;
  rdfs:range _:b399839 ;
  rdfs:range _:b715640 ;
  rdfs:range _:b895567 ;
  rdfs:range _:b897711 ;
  rdfs:seeAlso prov:Generation ;
  rdfs:seeAlso prov:qualifiedGeneration ;
  rdfs:subPropertyOf prov:wasInfluencedBy ;
  owl:propertyChainAxiom (
      prov:qualifiedGeneration
      prov:activity
    ) ;
  prov:category "starting-point" ;
  prov:component "entities-activities" ;
  prov:inverse "generated" ;
  prov:qualifiedForm prov:Generation ;
  prov:qualifiedForm prov:qualifiedGeneration ;
.
prov:wasInfluencedBy
  rdf:type owl:ObjectProperty ;
  rdfs:comment "Because prov:wasInfluencedBy is a broad relation, its more specific subproperties (e.g. prov:wasInformedBy, prov:actedOnBehalfOf, prov:wasEndedBy, etc.) should be used when applicable."@en ;
  rdfs:comment "This property has multiple RDFS domains to suit multiple OWL Profiles. See <a href=\"#owl-profile\">PROV-O OWL Profile</a>." ;
  rdfs:domain owl:Thing ;
  rdfs:domain _:b399839 ;
  rdfs:isDefinedBy <http://www.w3.org/ns/prov-o#> ;
  rdfs:label "wasInfluencedBy" ;
  rdfs:range owl:Thing ;
  rdfs:range _:b715640 ;
  rdfs:seeAlso prov:Influence ;
  rdfs:seeAlso prov:qualifiedInfluence ;
  prov:category "qualified" ;
  prov:component "agents-responsibility" ;
  prov:editorialNote """The sub-properties of prov:wasInfluencedBy can be elaborated in more detail using the Qualification Pattern. For example, the binary relation :baking prov:used :spoon can be qualified by asserting :baking prov:qualifiedUsage [ a prov:Usage; prov:entity :spoon; prov:atLocation :kitchen ] .

Subproperties of prov:wasInfluencedBy may also be asserted directly without being qualified.

prov:wasInfluencedBy should not be used without also using one of its subproperties. 
"""@en ;
  prov:inverse "influenced" ;
  prov:qualifiedForm prov:Influence ;
  prov:qualifiedForm prov:qualifiedInfluence ;
  prov:sharesDefinitionWith prov:Influence ;
.
prov:wasInformedBy
  rdf:type owl:ObjectProperty ;
  rdfs:comment "An activity a2 is dependent on or informed by another activity a1, by way of some unspecified entity that is generated by a1 and used by a2."@en ;
  rdfs:domain owl:Thing ;
  rdfs:domain prov:Activity ;
  rdfs:domain _:b53184 ;
  rdfs:domain _:b170340 ;
  rdfs:domain _:b399839 ;
  rdfs:domain _:b715640 ;
  rdfs:domain _:b895567 ;
  rdfs:domain _:b897711 ;
  rdfs:isDefinedBy <http://www.w3.org/ns/prov-o#> ;
  rdfs:label "wasInformedBy" ;
  rdfs:range owl:Thing ;
  rdfs:range prov:Activity ;
  rdfs:range _:b53184 ;
  rdfs:range _:b170340 ;
  rdfs:range _:b399839 ;
  rdfs:range _:b715640 ;
  rdfs:range _:b895567 ;
  rdfs:range _:b897711 ;
  rdfs:seeAlso prov:Communication ;
  rdfs:seeAlso prov:qualifiedCommunication ;
  rdfs:subPropertyOf prov:wasInfluencedBy ;
  owl:propertyChainAxiom (
      prov:qualifiedCommunication
      prov:activity
    ) ;
  prov:category "starting-point" ;
  prov:component "entities-activities" ;
  prov:inverse "informed" ;
  prov:qualifiedForm prov:Communication ;
  prov:qualifiedForm prov:qualifiedCommunication ;
.
prov:wasInvalidatedBy
  rdf:type owl:ObjectProperty ;
  rdfs:domain owl:Thing ;
  rdfs:domain prov:Entity ;
  rdfs:domain _:b53184 ;
  rdfs:domain _:b170340 ;
  rdfs:domain _:b399839 ;
  rdfs:domain _:b715640 ;
  rdfs:domain _:b895567 ;
  rdfs:domain _:b897711 ;
  rdfs:isDefinedBy <http://www.w3.org/ns/prov-o#> ;
  rdfs:label "wasInvalidatedBy" ;
  rdfs:range owl:Thing ;
  rdfs:range prov:Activity ;
  rdfs:range _:b53184 ;
  rdfs:range _:b170340 ;
  rdfs:range _:b399839 ;
  rdfs:range _:b715640 ;
  rdfs:range _:b895567 ;
  rdfs:range _:b897711 ;
  rdfs:seeAlso prov:Invalidation ;
  rdfs:seeAlso prov:qualifiedInvalidation ;
  rdfs:subPropertyOf prov:wasInfluencedBy ;
  owl:propertyChainAxiom (
      prov:qualifiedInvalidation
      prov:activity
    ) ;
  prov:category "expanded" ;
  prov:component "entities-activities" ;
  prov:inverse "invalidated" ;
  prov:qualifiedForm prov:Invalidation ;
  prov:qualifiedForm prov:qualifiedInvalidation ;
.
prov:wasQuotedFrom
  rdf:type owl:ObjectProperty ;
  rdfs:comment "An entity is derived from an original entity by copying, or 'quoting', some or all of it."@en ;
  rdfs:domain owl:Thing ;
  rdfs:domain prov:Entity ;
  rdfs:domain _:b53184 ;
  rdfs:domain _:b170340 ;
  rdfs:domain _:b399839 ;
  rdfs:domain _:b715640 ;
  rdfs:domain _:b895567 ;
  rdfs:domain _:b897711 ;
  rdfs:isDefinedBy <http://www.w3.org/ns/prov-o#> ;
  rdfs:label "wasQuotedFrom" ;
  rdfs:range owl:Thing ;
  rdfs:range prov:Entity ;
  rdfs:range _:b53184 ;
  rdfs:range _:b170340 ;
  rdfs:range _:b399839 ;
  rdfs:range _:b715640 ;
  rdfs:range _:b895567 ;
  rdfs:range _:b897711 ;
  rdfs:seeAlso prov:Quotation ;
  rdfs:seeAlso prov:qualifiedQuotation ;
  rdfs:subPropertyOf prov:wasDerivedFrom ;
  rdfs:subPropertyOf prov:wasInfluencedBy ;
  owl:propertyChainAxiom (
      prov:qualifiedQuotation
      prov:entity
    ) ;
  prov:category "expanded" ;
  prov:component "derivations" ;
  prov:inverse "quotedAs" ;
  prov:qualifiedForm prov:Quotation ;
  prov:qualifiedForm prov:qualifiedQuotation ;
.
prov:wasRevisionOf
  rdf:type owl:AnnotationProperty ;
  rdf:type owl:ObjectProperty ;
  rdfs:comment "A revision is a derivation that revises an entity into a revised version."@en ;
  rdfs:domain owl:Thing ;
  rdfs:domain prov:Entity ;
  rdfs:domain _:b53184 ;
  rdfs:domain _:b170340 ;
  rdfs:domain _:b399839 ;
  rdfs:domain _:b715640 ;
  rdfs:domain _:b895567 ;
  rdfs:domain _:b897711 ;
  rdfs:isDefinedBy <http://www.w3.org/ns/prov-o#> ;
  rdfs:label "wasRevisionOf" ;
  rdfs:range owl:Thing ;
  rdfs:range prov:Entity ;
  rdfs:range _:b53184 ;
  rdfs:range _:b170340 ;
  rdfs:range _:b399839 ;
  rdfs:range _:b715640 ;
  rdfs:range _:b895567 ;
  rdfs:range _:b897711 ;
  rdfs:seeAlso prov:Revision ;
  rdfs:seeAlso prov:qualifiedRevision ;
  rdfs:subPropertyOf prov:wasDerivedFrom ;
  rdfs:subPropertyOf prov:wasInfluencedBy ;
  owl:propertyChainAxiom (
      prov:qualifiedRevision
      prov:entity
    ) ;
  prov:category "expanded" ;
  prov:component "derivations" ;
  prov:inverse "hadRevision" ;
  prov:qualifiedForm prov:Revision ;
  prov:qualifiedForm prov:qualifiedRevision ;
.
prov:wasStartedBy
  rdf:type owl:ObjectProperty ;
  rdfs:comment "Start is when an activity is deemed to have started. A start may refer to an entity, known as trigger, that initiated the activity."@en ;
  rdfs:domain owl:Thing ;
  rdfs:domain prov:Activity ;
  rdfs:domain _:b53184 ;
  rdfs:domain _:b170340 ;
  rdfs:domain _:b399839 ;
  rdfs:domain _:b715640 ;
  rdfs:domain _:b895567 ;
  rdfs:domain _:b897711 ;
  rdfs:isDefinedBy <http://www.w3.org/ns/prov-o#> ;
  rdfs:label "wasStartedBy" ;
  rdfs:range owl:Thing ;
  rdfs:range prov:Entity ;
  rdfs:range _:b53184 ;
  rdfs:range _:b170340 ;
  rdfs:range _:b399839 ;
  rdfs:range _:b715640 ;
  rdfs:range _:b895567 ;
  rdfs:range _:b897711 ;
  rdfs:seeAlso prov:Start ;
  rdfs:seeAlso prov:qualifiedStart ;
  rdfs:subPropertyOf prov:wasInfluencedBy ;
  owl:propertyChainAxiom (
      prov:qualifiedStart
      prov:entity
    ) ;
  prov:category "expanded" ;
  prov:component "entities-activities" ;
  prov:inverse "started" ;
  prov:qualifiedForm prov:Start ;
  prov:qualifiedForm prov:qualifiedStart ;
.
<http://www.w3.org/ns/prov-o>
  rdf:type prov:Entity ;
  rdf:type _:b53184 ;
  rdf:type _:b170340 ;
  rdf:type _:b399839 ;
  rdf:type _:b715640 ;
  rdf:type _:b895567 ;
  rdf:type _:b897711 ;
.
<http://www.w3.org/ns/prov-o#>
  rdf:type prov:Entity ;
  rdf:type _:b53184 ;
  rdf:type _:b170340 ;
  rdf:type _:b399839 ;
  rdf:type _:b715640 ;
  rdf:type _:b895567 ;
  rdf:type _:b897711 ;
  rdfs:comment """This document is published by the Provenance Working Group (http://www.w3.org/2011/prov/wiki/Main_Page). 

If you wish to make comments regarding this document, please send them to public-prov-comments@w3.org (subscribe public-prov-comments-request@w3.org, archives http://lists.w3.org/Archives/Public/public-prov-comments/). All feedback is welcome."""@en ;
  rdfs:label "W3C PROVenance Interchange Ontology (PROV-O)"@en ;
  rdfs:seeAlso <http://www.w3.org/TR/prov-o/> ;
  rdfs:seeAlso <http://www.w3.org/ns/prov> ;
  owl:versionIRI <http://www.w3.org/ns/prov-o-20130430> ;
  owl:versionInfo "Recommendation version 2013-04-30"@en ;
  prov:alternateOf <http://www.w3.org/ns/prov-o> ;
  prov:specializationOf <http://www.w3.org/ns/prov-o> ;
  prov:wasDerivedFrom <http://www.w3.org/ns/prov-o-20130312> ;
  prov:wasInfluencedBy <http://www.w3.org/ns/prov-o-20130312> ;
  prov:wasRevisionOf <http://www.w3.org/ns/prov-o-20130312> ;
.
<http://www.w3.org/ns/prov-o-20130312>
  rdf:type prov:Entity ;
  rdf:type _:b53184 ;
  rdf:type _:b170340 ;
  rdf:type _:b399839 ;
  rdf:type _:b715640 ;
  rdf:type _:b895567 ;
  rdf:type _:b897711 ;
  prov:influenced <http://www.w3.org/ns/prov-o#> ;
.
<http://www.w3.org/ns/regorg>
  rdf:type elobr:EloniaBusinessCode ;
  rdf:type freebr:FreedoniaBusinessCode ;
  rdf:type voaf:Vocabulary ;
  elobr:EloniaRegistrationAuthority _:b11589 ;
  elobr:EloniaRegistrationAuthority _:b251823 ;
  elobr:EloniaRegistrationAuthority _:b421602 ;
  elobr:EloniaRegistrationAuthority _:b421866 ;
  elobr:EloniaRegistrationAuthority _:b421897 ;
  elobr:EloniaRegistrationAuthority _:b937319 ;
  elobr:EloniaRegistrationAuthority _:b937381 ;
  elobr:EloniaRegistrationAuthority _:b937505 ;
  elobr:EloniaRegistrationAuthority _:b937610 ;
  elobr:EloniaRegistrationAuthority _:b937939 ;
  elobr:EloniaRegistrationAuthority _:b937970 ;
  elobr:EloniaRegistrationAuthority _:b938203 ;
  elobr:EloniaRegistrationAuthority _:b938234 ;
  elobr:EloniaRegistrationAuthority _:b938246 ;
  freebr:FreedoniaRegistrationAuthority _:b11589 ;
  freebr:FreedoniaRegistrationAuthority _:b251823 ;
  freebr:FreedoniaRegistrationAuthority _:b421602 ;
  freebr:FreedoniaRegistrationAuthority _:b421866 ;
  freebr:FreedoniaRegistrationAuthority _:b421897 ;
  freebr:FreedoniaRegistrationAuthority _:b937319 ;
  freebr:FreedoniaRegistrationAuthority _:b937381 ;
  freebr:FreedoniaRegistrationAuthority _:b937505 ;
  freebr:FreedoniaRegistrationAuthority _:b937610 ;
  freebr:FreedoniaRegistrationAuthority _:b937939 ;
  freebr:FreedoniaRegistrationAuthority _:b937970 ;
  freebr:FreedoniaRegistrationAuthority _:b938203 ;
  freebr:FreedoniaRegistrationAuthority _:b938234 ;
  freebr:FreedoniaRegistrationAuthority _:b938246 ;
  dc:contributor _:b11589 ;
  dc:contributor _:b251823 ;
  dc:contributor _:b421602 ;
  dc:contributor _:b421866 ;
  dc:contributor _:b421897 ;
  dc:contributor _:b937319 ;
  dc:contributor _:b937381 ;
  dc:contributor _:b937505 ;
  dc:contributor _:b937610 ;
  dc:contributor _:b937939 ;
  dc:contributor _:b937970 ;
  dc:contributor _:b938203 ;
  dc:contributor _:b938234 ;
  dc:contributor _:b938246 ;
  dc:creator _:b11589 ;
  dc:creator _:b251823 ;
  dc:creator _:b421602 ;
  dc:creator _:b421866 ;
  dc:creator _:b421897 ;
  dc:creator _:b937319 ;
  dc:creator _:b937381 ;
  dc:creator _:b937505 ;
  dc:creator _:b937610 ;
  dc:creator _:b937939 ;
  dc:creator _:b937970 ;
  dc:creator _:b938203 ;
  dc:creator _:b938234 ;
  dc:creator _:b938246 ;
  dc:date "2013-05-24"^^xsd:date ;
  dc:date "2013-12-21"^^xsd:date ;
  dc:description "The Registered Organization Vocabulary is a profile of the Organization Ontology for describing organizations that have gained legal entity status through a formal registration process, typically in a national or regional register." ;
  dc:description "The Registered Organization Vocabulary is a profile of the Organization Ontology for describing organizations that have gained legal entity status through a formal registration process, typically in a national or regional register."@en ;
  dc:description "This is the RDF encoding of the Legal Entity vocabulary, originally developed under the European Commission's ISA Programme." ;
  dc:description "This is the RDF encoding of the Legal Entity vocabulary, originally developed under the European Commission's ISA Programme."@en ;
  dc:title "Registered Organization Vocabulary"@en ;
  dcterms:abstract "The Registered Organization Vocabulary is a profile of the Organization Ontology for describing organizations that have gained legal entity status through a formal registration process, typically in a national or regional register." ;
  dcterms:abstract "The Registered Organization Vocabulary is a profile of the Organization Ontology for describing organizations that have gained legal entity status through a formal registration process, typically in a national or regional register."@en ;
  dcterms:contributor _:b11589 ;
  dcterms:contributor _:b251823 ;
  dcterms:contributor _:b421602 ;
  dcterms:contributor _:b421866 ;
  dcterms:contributor _:b421897 ;
  dcterms:contributor _:b937319 ;
  dcterms:contributor _:b937381 ;
  dcterms:contributor _:b937505 ;
  dcterms:contributor _:b937610 ;
  dcterms:contributor _:b937939 ;
  dcterms:contributor _:b937970 ;
  dcterms:contributor _:b938203 ;
  dcterms:contributor _:b938234 ;
  dcterms:contributor _:b938246 ;
  dcterms:creator _:b11589 ;
  dcterms:creator _:b251823 ;
  dcterms:creator _:b421602 ;
  dcterms:creator _:b421866 ;
  dcterms:creator _:b421897 ;
  dcterms:creator _:b937319 ;
  dcterms:creator _:b937381 ;
  dcterms:creator _:b937505 ;
  dcterms:creator _:b937610 ;
  dcterms:creator _:b937939 ;
  dcterms:creator _:b937970 ;
  dcterms:creator _:b938203 ;
  dcterms:creator _:b938234 ;
  dcterms:creator _:b938246 ;
  dcterms:date "2013-05-24"^^xsd:date ;
  dcterms:date "2013-12-21"^^xsd:date ;
  dcterms:description "The Registered Organization Vocabulary is a profile of the Organization Ontology for describing organizations that have gained legal entity status through a formal registration process, typically in a national or regional register." ;
  dcterms:description "The Registered Organization Vocabulary is a profile of the Organization Ontology for describing organizations that have gained legal entity status through a formal registration process, typically in a national or regional register."@en ;
  dcterms:description "This is the RDF encoding of the Legal Entity vocabulary, originally developed under the European Commission's ISA Programme." ;
  dcterms:description "This is the RDF encoding of the Legal Entity vocabulary, originally developed under the European Commission's ISA Programme."@en ;
  dcterms:modified "2013-05-24"^^xsd:date ;
  dcterms:modified "2013-12-21"^^xsd:date ;
  dcterms:title "Registered Organization Vocabulary"@en ;
  vann:preferredNamespacePrefix "rov" ;
  vann:preferredNamespaceUri "http://www.w3.org/ns/regorg#" ;
  voaf:specializes <http://www.w3.org/ns/org> ;
  voaf:specializes <http://www.w3.org/org> ;
  toop:registrationAuthority _:b11589 ;
  toop:registrationAuthority _:b251823 ;
  toop:registrationAuthority _:b421602 ;
  toop:registrationAuthority _:b421866 ;
  toop:registrationAuthority _:b421897 ;
  toop:registrationAuthority _:b937319 ;
  toop:registrationAuthority _:b937381 ;
  toop:registrationAuthority _:b937505 ;
  toop:registrationAuthority _:b937610 ;
  toop:registrationAuthority _:b937939 ;
  toop:registrationAuthority _:b937970 ;
  toop:registrationAuthority _:b938203 ;
  toop:registrationAuthority _:b938234 ;
  toop:registrationAuthority _:b938246 ;
  rdfs:comment "This file specifies the set of RDF classes and properties used in the Registered Organization Vocabulary vocabulary"@en ;
  rdfs:comment "This file specifies the set of RDF classes and properties used in the Registered Organization Vocabulary"@en ;
  rdfs:label "Registered Organization Vocabulary"@en ;
  owl:versionInfo "Second version in w3.org/ns" ;
  owl:versionInfo "Second version in w3.org/ns"@en ;
  wdrs:describedby <http://www.w3.org/TR/2013/NOTE-vocab-regorg-20130528/> ;
  wdrs:describedby <http://www.w3.org/TR/vocab-regorg/> ;
  foaf:depiction <http://www.w3.org/TR/2013/NOTE-vocab-regorg-20130528/regorg20130508.png> ;
  foaf:maker _:b11589 ;
  foaf:maker _:b251823 ;
  foaf:maker _:b421602 ;
  foaf:maker _:b421866 ;
  foaf:maker _:b421897 ;
  foaf:maker _:b937319 ;
  foaf:maker _:b937381 ;
  foaf:maker _:b937505 ;
  foaf:maker _:b937610 ;
  foaf:maker _:b937939 ;
  foaf:maker _:b937970 ;
  foaf:maker _:b938203 ;
  foaf:maker _:b938234 ;
  foaf:maker _:b938246 ;
.
rov:RegisteredOrganization
  rdf:type rdfs:Class ;
  rdf:type owl:Class ;
  dc:identifier "rov:RegisteredOrganization" ;
  dcterms:identifier "rov:RegisteredOrganization" ;
  rdfs:comment """<p xmlns=\"http://www.w3.org/ns/regorg#\">rov:RegisteredOrganization is the key class for the Registered Organization vocabulary and represents an organization that is legally registered. In many countries there is a single registry although in others, such as Spain and Germany, multiple registries exist. A Registered Organization is able to trade, is legally liable for its actions, accounts, tax affairs etc. Legal entity status is conferred by the act of registration cf. org:FormalOrganization that applies to any legal entity, including those created by other legal means.</p>
    <p xmlns=\"http://www.w3.org/ns/regorg#\">This makes registered organizations distinct from the broader concept of organizations, groups or, in some jurisdictions, sole traders. Many organizations exist that are not legal entities yet to the outside world they have staff, hierarchies, locations etc. Other organizations exist that are an umbrella for several legal entities (universities are often good examples of this). This vocabulary is concerned solely with registered organizations.</p>
    <p xmlns=\"http://www.w3.org/ns/regorg#\">In RDF, Registered Organization is a sub class of the Organization Ontology's org:FormalOrganization which is itself a sub class of the more general 'Agent' class found in FOAF and Dublin Core that does encompass organizations, natural persons, groups etc. - i.e. an Agent is any entity that is able to carry out actions.</p>"""^^rdf:XMLLiteral ;
  rdfs:comment """rov:RegisteredOrganization is the key class for the Registered Organization vocabulary and represents 
    an organization that is legally registered. In many countries there is a single registry although in others, such 
    as Spain and Germany, multiple registries exist. A Registered Organization is able to trade, is legally liable for 
    its actions, accounts, tax affairs etc. Legal entity status is conferred by the act of registration cf. 
    org:FormalOrganization that applies to any legal entity, including those created by other legal means.
    This makes registered organizations distinct from the broader concept of organizations, groups or, in 
    some jurisdictions, sole traders. Many organizations exist that are not legal entities yet to the outside world 
    they have staff, hierarchies, locations etc. Other organizations exist that are an umbrella for several legal entities 
    (universities are often good examples of this). This vocabulary is concerned solely with registered organizations.
    In RDF, Registered Organization is a sub class of the Organization Ontology's org:FormalOrganization which is itself a 
    sub class of the more general 'Agent' class found in FOAF and Dublin Core that does encompass organizations, 
    natural persons, groups etc. - i.e. an Agent is any entity that is able to carry out actions.</p>"""@en ;
  rdfs:isDefinedBy <http://www.w3.org/TR/vocab-regorg/> ;
  rdfs:label "Registered Organization"@en ;
  rdfs:subClassOf org:FormalOrganization ;
.
rov:hasRegisteredOrganization
  rdf:type rdf:Property ;
  rdf:type owl:ObjectProperty ;
  dc:identifier "rov:hasRegisteredOrganization" ;
  dcterms:identifier "rov:hasRegisteredOrganization" ;
  rdfs:comment """The has registered organization relationship can be used to link any dcterms:Agent (equivalent class foaf:Agent)
    to a Registered Organization that in some way acts as a registered legal entity for it. This is useful, for example, 
    where an organization includes one or more legal entities, or where a natural person is also registered as a legal entity.
    rov:hasRegisteredOrganization has a range of rov:RegisteredOrganization."""@en ;
  rdfs:comment "The has registered organization relationship can be used to link any dcterms:Agent (equivalent class foaf:Agent) to a Registered Organization that in some way acts as a registered legal entity for it. This is useful, for example, where an organization includes one or more legal entities, or where a natural person is also registered as a legal entity. rov:hasRegisteredOrganization has a range of rov:RegisteredOrganization."@en ;
  rdfs:domain dcterms:Agent ;
  rdfs:domain owl:Thing ;
  rdfs:domain foaf:Agent ;
  rdfs:domain _:b420951 ;
  rdfs:domain _:b421075 ;
  rdfs:domain _:b421664 ;
  rdfs:domain _:b421928 ;
  rdfs:domain _:b937877 ;
  rdfs:domain _:b938265 ;
  rdfs:isDefinedBy <http://www.w3.org/TR/vocab-regorg/> ;
  rdfs:label "registered organization"@en ;
  rdfs:range dcterms:Agent ;
  rdfs:range owl:Thing ;
  rdfs:range org:FormalOrganization ;
  rdfs:range org:Organization ;
  rdfs:range rov:RegisteredOrganization ;
  rdfs:range foaf:Agent ;
  rdfs:range foaf:Organization ;
  rdfs:range _:b420951 ;
  rdfs:range _:b421075 ;
  rdfs:range _:b421664 ;
  rdfs:range _:b421928 ;
  rdfs:range _:b937877 ;
  rdfs:range _:b938265 ;
.
rov:legalName
  rdf:type rdf:Property ;
  rdf:type owl:DatatypeProperty ;
  dc:identifier "rov:legalName" ;
  dcterms:identifier "rov:legalName" ;
  rdfs:comment """The legal name of the business. A business might have more than one 
    legal name, particularly in countries with more than one official language. In such cases the 
    language of the string should be identified."""@en ;
  rdfs:comment "The legal name of the business. A business might have more than one legal name, particularly in countries with more than one official language. In such cases the language of the string should be identified."@en ;
  rdfs:domain dcterms:Agent ;
  rdfs:domain owl:Thing ;
  rdfs:domain org:FormalOrganization ;
  rdfs:domain org:Organization ;
  rdfs:domain foaf:Agent ;
  rdfs:domain foaf:Organization ;
  rdfs:domain _:b420951 ;
  rdfs:domain _:b421075 ;
  rdfs:domain _:b421664 ;
  rdfs:domain _:b421928 ;
  rdfs:domain _:b937877 ;
  rdfs:domain _:b938265 ;
  rdfs:isDefinedBy <http://www.w3.org/TR/vocab-regorg/> ;
  rdfs:label "legal name"@en ;
  rdfs:range rdfs:Literal ;
.
rov:orgActivity
  rdf:type rdf:Property ;
  rdf:type owl:ObjectProperty ;
  dc:identifier "rov:orgActivity" ;
  dcterms:identifier "rov:orgActivity" ;
  rdfs:comment """The activity of a company should be 
    recorded using a controlled vocabulary expressed as a SKOS concept scheme. Several such 
    vocabularies exist, many of which map to the UN's ISIC codes. Where a particular controlled vocabulary is in use 
    within a given context, such as SIC codes in the UK, it is acceptable to use these, however, the preferred 
    choice for European interoperability is NACE. rov:orgActivity is a sub class of org:classification which has a range of skos:Concept."""@en ;
  rdfs:comment "The activity of a company should be recorded using a controlled vocabulary expressed as a SKOS concept scheme. Several such vocabularies exist, many of which map to the UN's ISIC codes. Where a particular controlled vocabulary is in use within a given context, such as SIC codes in the UK, it is acceptable to use these, however, the preferred choice for European interoperability is NACE. rov:orgActivity is a sub class of org:classification which has a range of skos:Concept."@en ;
  rdfs:domain dcterms:Agent ;
  rdfs:domain owl:Thing ;
  rdfs:domain org:Organization ;
  rdfs:domain foaf:Agent ;
  rdfs:domain foaf:Organization ;
  rdfs:domain _:b420951 ;
  rdfs:domain _:b421075 ;
  rdfs:domain _:b421664 ;
  rdfs:domain _:b421928 ;
  rdfs:domain _:b937877 ;
  rdfs:domain _:b938265 ;
  rdfs:isDefinedBy <http://www.w3.org/TR/vocab-regorg/> ;
  rdfs:label "company activity"@en ;
  rdfs:range owl:Thing ;
  rdfs:range skos:Concept ;
  rdfs:range _:b327858 ;
  rdfs:subPropertyOf org:classification ;
.
rov:orgStatus
  rdf:type rdf:Property ;
  rdf:type owl:ObjectProperty ;
  dc:identifier "rov:orgStatus" ;
  dcterms:identifier "rov:orgStatus" ;
  rdfs:comment """Terms like insolvent, bankrupt and in receivership are likely to have 
    different legal implications in different jurisdictions. Best Practice for recording various 
    other status levels is to use the relevant jurisdiction's terms and to do so in a 
    consistent manner using a SKOS Concept Scheme. rov:orgStatus is a sub class of org:classification
    which has a range of skos:Concept."""@en ;
  rdfs:comment "Terms like insolvent, bankrupt and in receivership are likely to have different legal implications in different jurisdictions. Best Practice for recording various other status levels is to use the relevant jurisdiction's terms and to do so in a consistent manner using a SKOS Concept Scheme. rov:orgStatus is a sub class of org:classification which has a range of skos:Concept."@en ;
  rdfs:domain elobr:Company ;
  rdfs:domain elobr:EloniaBusinessCode ;
  rdfs:domain freebr:Company ;
  rdfs:domain freebr:FreedoniaBusinessCode ;
  rdfs:domain dcterms:Agent ;
  rdfs:domain toop:CompanyCode ;
  rdfs:domain owl:Thing ;
  rdfs:domain skos:Concept ;
  rdfs:domain adms:Identifier ;
  rdfs:domain org:Organization ;
  rdfs:domain foaf:Agent ;
  rdfs:domain foaf:Organization ;
  rdfs:domain _:b156576 ;
  rdfs:domain _:b213787 ;
  rdfs:domain _:b327858 ;
  rdfs:domain _:b420951 ;
  rdfs:domain _:b421075 ;
  rdfs:domain _:b421664 ;
  rdfs:domain _:b421928 ;
  rdfs:domain _:b772676 ;
  rdfs:domain _:b883411 ;
  rdfs:domain _:b937877 ;
  rdfs:domain _:b938265 ;
  rdfs:isDefinedBy <http://www.w3.org/TR/vocab-regorg/> ;
  rdfs:label "company status"@en ;
  rdfs:range owl:Thing ;
  rdfs:range skos:Concept ;
  rdfs:range _:b327858 ;
  rdfs:subPropertyOf org:classification ;
  owl:equivalentProperty elobr:EloniaLegalStatus ;
  owl:equivalentProperty freebr:FreedoniaLegalStatus ;
  owl:equivalentProperty toop:legalStatus ;
.
rov:orgType
  rdf:type rdf:Property ;
  rdf:type owl:ObjectProperty ;
  dc:identifier "rov:orgType" ;
  dcterms:identifier "rov:orgType" ;
  rdfs:comment """This property records the type of organization. Familiar types are SA, PLC, LLC, GmbH etc. Each 
    jurisdiction will have a limited set of recognized company types and these should be used in a consistent manner
    using a SKOS Concept Scheme. rov:orgType is a sub class of org:classification which has a range of skos:Concept."""@en ;
  rdfs:comment "This property records the type of organization. Familiar types are SA, PLC, LLC, GmbH etc. Each jurisdiction will have a limited set of recognized company types and these should be used in a consistent manner using a SKOS Concept Scheme. rov:orgType is a sub class of org:classification which has a range of skos:Concept."@en ;
  rdfs:domain elobr:Company ;
  rdfs:domain freebr:Company ;
  rdfs:domain dcterms:Agent ;
  rdfs:domain toop:RegisteredOrganization ;
  rdfs:domain owl:Thing ;
  rdfs:domain skos:Concept ;
  rdfs:domain org:FormalOrganization ;
  rdfs:domain org:Organization ;
  rdfs:domain rov:RegisteredOrganization ;
  rdfs:domain foaf:Agent ;
  rdfs:domain foaf:Organization ;
  rdfs:domain _:b156576 ;
  rdfs:domain _:b180769 ;
  rdfs:domain _:b213787 ;
  rdfs:domain _:b254570 ;
  rdfs:domain _:b327858 ;
  rdfs:domain _:b420951 ;
  rdfs:domain _:b421075 ;
  rdfs:domain _:b421664 ;
  rdfs:domain _:b421928 ;
  rdfs:domain _:b454254 ;
  rdfs:domain _:b772676 ;
  rdfs:domain _:b826282 ;
  rdfs:domain _:b826680 ;
  rdfs:domain _:b883411 ;
  rdfs:domain _:b937877 ;
  rdfs:domain _:b938265 ;
  rdfs:isDefinedBy <http://www.w3.org/TR/vocab-regorg/> ;
  rdfs:label "company type"@en ;
  rdfs:range owl:Thing ;
  rdfs:range skos:Concept ;
  rdfs:range _:b327858 ;
  rdfs:range _:b875853 ;
  rdfs:subPropertyOf org:classification ;
  owl:equivalentProperty elobr:EloniaCompanyType ;
  owl:equivalentProperty freebr:FreedoniaCompanyType ;
  owl:equivalentProperty toop:companyType ;
.
rov:registration
  rdf:type rdf:Property ;
  rdf:type owl:ObjectProperty ;
  dc:identifier "rov:registration" ;
  dcterms:identifier "rov:registration" ;
  rdfs:comment """The registration is a fundamental relationship between a legal entity and the 
    authority with which it is registered and that confers legal status upon it. rov:registration is 
    a sub property of adms:identifier which has a range of adms:Identifier. rov:registration has a domain of rov:RegisteredOrganization."""@en ;
  rdfs:comment "The registration is a fundamental relationship between a legal entity and the authority with which it is registered and that confers legal status upon it. rov:registration is a sub property of adms:identifier which has a range of adms:Identifier. rov:registration has a domain of rov:RegisteredOrganization."@en ;
  rdfs:domain dcterms:Agent ;
  rdfs:domain owl:Thing ;
  rdfs:domain org:FormalOrganization ;
  rdfs:domain org:Organization ;
  rdfs:domain rov:RegisteredOrganization ;
  rdfs:domain foaf:Agent ;
  rdfs:domain foaf:Organization ;
  rdfs:domain _:b420951 ;
  rdfs:domain _:b421075 ;
  rdfs:domain _:b421664 ;
  rdfs:domain _:b421928 ;
  rdfs:domain _:b937877 ;
  rdfs:domain _:b938265 ;
  rdfs:isDefinedBy <http://www.w3.org/TR/vocab-regorg/> ;
  rdfs:isDefinedBy rov: ;
  rdfs:label "registration"@en ;
  rdfs:range adms:Identifier ;
  rdfs:subPropertyOf adms:identifier ;
.
foaf:
  dc:description "The Friend of a Friend (FOAF) RDF vocabulary, described using W3C RDF Schema and the Web Ontology Language." ;
  dc:title "Friend of a Friend (FOAF) vocabulary" ;
.
foaf:Agent
  rdf:type rdfs:Class ;
  rdf:type owl:Class ;
  rdfs:comment "An agent (eg. person, group, software or physical artifact)." ;
  rdfs:label "Agent" ;
  rdfs:subClassOf dcterms:Agent ;
  owl:equivalentClass dcterms:Agent ;
  vs:term_status "stable" ;
.
foaf:Document
  rdf:type rdfs:Class ;
  rdf:type owl:Class ;
  rdfs:comment "A document." ;
  rdfs:isDefinedBy foaf: ;
  rdfs:label "Document" ;
  rdfs:subClassOf schema:CreativeWork ;
  rdfs:subClassOf owl:Thing ;
  owl:disjointWith foaf:Organization ;
  owl:disjointWith foaf:Project ;
  owl:equivalentClass schema:CreativeWork ;
  vs:term_status "stable" ;
.
foaf:Group
  rdf:type rdfs:Class ;
  rdf:type owl:Class ;
  rdfs:comment "A class of Agents." ;
  rdfs:label "Group" ;
  rdfs:subClassOf foaf:Agent ;
  vs:term_status "stable" ;
.
foaf:Image
  rdf:type rdfs:Class ;
  rdf:type owl:Class ;
  rdfs:comment "An image." ;
  rdfs:isDefinedBy foaf: ;
  rdfs:label "Image" ;
  rdfs:subClassOf schema:ImageObject ;
  rdfs:subClassOf foaf:Document ;
  owl:equivalentClass schema:ImageObject ;
  vs:term_status "stable" ;
.
foaf:LabelProperty
  rdf:type rdfs:Class ;
  rdf:type owl:Class ;
  rdfs:comment "A foaf:LabelProperty is any RDF property with texual values that serve as labels." ;
  rdfs:isDefinedBy foaf: ;
  rdfs:label "Label Property" ;
  rdfs:subClassOf owl:Thing ;
  vs:term_status "unstable" ;
.
foaf:OnlineAccount
  rdf:type rdfs:Class ;
  rdf:type owl:Class ;
  rdfs:comment "An online account." ;
  rdfs:isDefinedBy foaf: ;
  rdfs:label "Online Account" ;
  rdfs:subClassOf owl:Thing ;
  vs:term_status "testing" ;
.
foaf:OnlineChatAccount
  rdf:type rdfs:Class ;
  rdf:type owl:Class ;
  rdfs:comment "An online chat account." ;
  rdfs:isDefinedBy foaf: ;
  rdfs:label "Online Chat Account" ;
  rdfs:subClassOf foaf:OnlineAccount ;
  vs:term_status "unstable" ;
.
foaf:OnlineEcommerceAccount
  rdf:type rdfs:Class ;
  rdf:type owl:Class ;
  rdfs:comment "An online e-commerce account." ;
  rdfs:isDefinedBy foaf: ;
  rdfs:label "Online E-commerce Account" ;
  rdfs:subClassOf foaf:OnlineAccount ;
  vs:term_status "unstable" ;
.
foaf:OnlineGamingAccount
  rdf:type rdfs:Class ;
  rdf:type owl:Class ;
  rdfs:comment "An online gaming account." ;
  rdfs:isDefinedBy foaf: ;
  rdfs:label "Online Gaming Account" ;
  rdfs:subClassOf foaf:OnlineAccount ;
  vs:term_status "unstable" ;
.
foaf:Organization
  rdf:type rdfs:Class ;
  rdf:type owl:Class ;
  rdfs:comment "An organization." ;
  rdfs:isDefinedBy foaf: ;
  rdfs:label "Organization" ;
  rdfs:subClassOf org:Organization ;
  rdfs:subClassOf foaf:Agent ;
  owl:disjointWith foaf:Document ;
  owl:disjointWith foaf:Person ;
  owl:equivalentClass org:Organization ;
  vs:term_status "stable" ;
.
foaf:Person
  rdf:type rdfs:Class ;
  rdf:type owl:Class ;
  rdfs:comment "A person." ;
  rdfs:isDefinedBy foaf: ;
  rdfs:label "Person" ;
  rdfs:subClassOf wgs:SpatialThing ;
  rdfs:subClassOf foaf:Agent ;
  owl:disjointWith foaf:Organization ;
  owl:disjointWith foaf:Project ;
  owl:equivalentClass schema:Person ;
  owl:equivalentClass toop:Person ;
  owl:equivalentClass <http://www.w3.org/2000/10/swap/pim/contact#Person> ;
  vs:term_status "stable" ;
.
foaf:PersonalProfileDocument
  rdf:type rdfs:Class ;
  rdf:type owl:Class ;
  rdfs:comment "A personal profile RDF document." ;
  rdfs:label "PersonalProfileDocument" ;
  rdfs:subClassOf foaf:Document ;
  vs:term_status "testing" ;
.
foaf:Project
  rdf:type rdfs:Class ;
  rdf:type owl:Class ;
  rdfs:comment "A project (a collective endeavour of some kind)." ;
  rdfs:isDefinedBy foaf: ;
  rdfs:label "Project" ;
  rdfs:subClassOf owl:Thing ;
  owl:disjointWith foaf:Document ;
  owl:disjointWith foaf:Person ;
  vs:term_status "testing" ;
.
foaf:account
  rdf:type rdf:Property ;
  rdf:type owl:ObjectProperty ;
  rdfs:comment "Indicates an account held by this agent." ;
  rdfs:domain dcterms:Agent ;
  rdfs:domain owl:Thing ;
  rdfs:domain foaf:Agent ;
  rdfs:domain _:b420951 ;
  rdfs:domain _:b421075 ;
  rdfs:domain _:b421664 ;
  rdfs:domain _:b421928 ;
  rdfs:domain _:b937877 ;
  rdfs:domain _:b938265 ;
  rdfs:isDefinedBy foaf: ;
  rdfs:label "account" ;
  rdfs:range owl:Thing ;
  rdfs:range foaf:OnlineAccount ;
  vs:term_status "testing" ;
.
foaf:accountName
  rdf:type rdf:Property ;
  rdf:type owl:DatatypeProperty ;
  rdfs:comment "Indicates the name (identifier) associated with this online account." ;
  rdfs:domain owl:Thing ;
  rdfs:domain foaf:OnlineAccount ;
  rdfs:isDefinedBy foaf: ;
  rdfs:label "account name" ;
  rdfs:range rdfs:Literal ;
  vs:term_status "testing" ;
.
foaf:accountServiceHomepage
  rdf:type rdf:Property ;
  rdf:type owl:ObjectProperty ;
  rdfs:comment "Indicates a homepage of the service provide for this online account." ;
  rdfs:domain owl:Thing ;
  rdfs:domain foaf:OnlineAccount ;
  rdfs:isDefinedBy foaf: ;
  rdfs:label "account service homepage" ;
  rdfs:range schema:CreativeWork ;
  rdfs:range owl:Thing ;
  rdfs:range foaf:Document ;
  vs:term_status "testing" ;
.
foaf:age
  rdf:type rdf:Property ;
  rdf:type owl:DatatypeProperty ;
  rdf:type owl:FunctionalProperty ;
  rdfs:comment "The age in years of some agent." ;
  rdfs:domain dcterms:Agent ;
  rdfs:domain schema:Person ;
  rdfs:domain toop:Person ;
  rdfs:domain <http://www.w3.org/2000/10/swap/pim/contact#Person> ;
  rdfs:domain owl:Thing ;
  rdfs:domain wgs:SpatialThing ;
  rdfs:domain foaf:Agent ;
  rdfs:domain foaf:Person ;
  rdfs:domain _:b420951 ;
  rdfs:domain _:b421075 ;
  rdfs:domain _:b421664 ;
  rdfs:domain _:b421928 ;
  rdfs:domain _:b937877 ;
  rdfs:domain _:b938265 ;
  rdfs:isDefinedBy foaf: ;
  rdfs:label "age" ;
  rdfs:range rdfs:Literal ;
  owl:equivalentProperty toop:age ;
  vs:term_status "unstable" ;
.
foaf:aimChatID
  rdf:type rdf:Property ;
  rdf:type owl:DatatypeProperty ;
  rdf:type owl:InverseFunctionalProperty ;
  rdfs:comment "An AIM chat ID" ;
  rdfs:domain dcterms:Agent ;
  rdfs:domain owl:Thing ;
  rdfs:domain foaf:Agent ;
  rdfs:domain _:b420951 ;
  rdfs:domain _:b421075 ;
  rdfs:domain _:b421664 ;
  rdfs:domain _:b421928 ;
  rdfs:domain _:b937877 ;
  rdfs:domain _:b938265 ;
  rdfs:isDefinedBy foaf: ;
  rdfs:label "AIM chat ID" ;
  rdfs:range rdfs:Literal ;
  rdfs:subPropertyOf foaf:nick ;
  vs:term_status "testing" ;
.
foaf:based_near
  rdf:type rdf:Property ;
  rdf:type owl:ObjectProperty ;
  rdfs:comment "A location that something is based near, for some broadly human notion of near." ;
  rdfs:domain owl:Thing ;
  rdfs:domain wgs:SpatialThing ;
  rdfs:isDefinedBy foaf: ;
  rdfs:label "based near" ;
  rdfs:range owl:Thing ;
  rdfs:range wgs:SpatialThing ;
  vs:term_status "testing" ;
.
foaf:birthday
  rdf:type rdf:Property ;
  rdf:type owl:DatatypeProperty ;
  rdf:type owl:FunctionalProperty ;
  rdfs:comment "The birthday of this Agent, represented in mm-dd string form, eg. '12-31'." ;
  rdfs:domain dcterms:Agent ;
  rdfs:domain schema:Person ;
  rdfs:domain toop:Person ;
  rdfs:domain <http://www.w3.org/2000/10/swap/pim/contact#Person> ;
  rdfs:domain owl:Thing ;
  rdfs:domain wgs:SpatialThing ;
  rdfs:domain foaf:Agent ;
  rdfs:domain foaf:Person ;
  rdfs:domain _:b420951 ;
  rdfs:domain _:b421075 ;
  rdfs:domain _:b421664 ;
  rdfs:domain _:b421928 ;
  rdfs:domain _:b937877 ;
  rdfs:domain _:b938265 ;
  rdfs:isDefinedBy foaf: ;
  rdfs:label "birthday" ;
  rdfs:range rdfs:Literal ;
  owl:equivalentProperty toop:birthday ;
  vs:term_status "unstable" ;
.
foaf:currentProject
  rdf:type rdf:Property ;
  rdf:type owl:ObjectProperty ;
  rdfs:comment "A current project this person works on." ;
  rdfs:domain dcterms:Agent ;
  rdfs:domain schema:Person ;
  rdfs:domain toop:Person ;
  rdfs:domain <http://www.w3.org/2000/10/swap/pim/contact#Person> ;
  rdfs:domain owl:Thing ;
  rdfs:domain wgs:SpatialThing ;
  rdfs:domain foaf:Agent ;
  rdfs:domain foaf:Person ;
  rdfs:domain _:b420951 ;
  rdfs:domain _:b421075 ;
  rdfs:domain _:b421664 ;
  rdfs:domain _:b421928 ;
  rdfs:domain _:b937877 ;
  rdfs:domain _:b938265 ;
  rdfs:isDefinedBy foaf: ;
  rdfs:label "current project" ;
  rdfs:range owl:Thing ;
  vs:term_status "testing" ;
.
foaf:depiction
  rdf:type rdf:Property ;
  rdf:type owl:ObjectProperty ;
  rdfs:comment "A depiction of some thing." ;
  rdfs:domain owl:Thing ;
  rdfs:isDefinedBy foaf: ;
  rdfs:label "depiction" ;
  rdfs:range schema:CreativeWork ;
  rdfs:range schema:ImageObject ;
  rdfs:range owl:Thing ;
  rdfs:range foaf:Document ;
  rdfs:range foaf:Image ;
  owl:inverseOf foaf:depicts ;
  vs:term_status "testing" ;
.
foaf:depicts
  rdf:type rdf:Property ;
  rdf:type owl:ObjectProperty ;
  rdfs:comment "A thing depicted in this representation." ;
  rdfs:domain schema:CreativeWork ;
  rdfs:domain schema:ImageObject ;
  rdfs:domain owl:Thing ;
  rdfs:domain foaf:Document ;
  rdfs:domain foaf:Image ;
  rdfs:isDefinedBy foaf: ;
  rdfs:label "depicts" ;
  rdfs:range owl:Thing ;
  owl:inverseOf foaf:depiction ;
  vs:term_status "testing" ;
.
foaf:dnaChecksum
  rdf:type rdf:Property ;
  rdf:type owl:DatatypeProperty ;
  rdfs:comment "A checksum for the DNA of some thing. Joke." ;
  rdfs:isDefinedBy foaf: ;
  rdfs:label "DNA checksum" ;
  rdfs:range rdfs:Literal ;
  vs:term_status "archaic" ;
.
foaf:familyName
  rdf:type rdf:Property ;
  rdf:type owl:DatatypeProperty ;
  rdfs:comment "The family name of some person." ;
  rdfs:domain dcterms:Agent ;
  rdfs:domain schema:Person ;
  rdfs:domain toop:Person ;
  rdfs:domain <http://www.w3.org/2000/10/swap/pim/contact#Person> ;
  rdfs:domain owl:Thing ;
  rdfs:domain wgs:SpatialThing ;
  rdfs:domain foaf:Agent ;
  rdfs:domain foaf:Person ;
  rdfs:domain _:b420951 ;
  rdfs:domain _:b421075 ;
  rdfs:domain _:b421664 ;
  rdfs:domain _:b421928 ;
  rdfs:domain _:b937877 ;
  rdfs:domain _:b938265 ;
  rdfs:isDefinedBy foaf: ;
  rdfs:label "familyName" ;
  rdfs:range rdfs:Literal ;
  owl:equivalentProperty toop:familyName ;
  vs:term_status "testing" ;
.
foaf:family_name
  rdf:type rdf:Property ;
  rdf:type owl:DatatypeProperty ;
  rdfs:comment "The family name of some person." ;
  rdfs:domain dcterms:Agent ;
  rdfs:domain schema:Person ;
  rdfs:domain toop:Person ;
  rdfs:domain <http://www.w3.org/2000/10/swap/pim/contact#Person> ;
  rdfs:domain owl:Thing ;
  rdfs:domain wgs:SpatialThing ;
  rdfs:domain foaf:Agent ;
  rdfs:domain foaf:Person ;
  rdfs:domain _:b420951 ;
  rdfs:domain _:b421075 ;
  rdfs:domain _:b421664 ;
  rdfs:domain _:b421928 ;
  rdfs:domain _:b937877 ;
  rdfs:domain _:b938265 ;
  rdfs:isDefinedBy foaf: ;
  rdfs:label "family_name" ;
  rdfs:range rdfs:Literal ;
  vs:term_status "archaic" ;
.
foaf:firstName
  rdf:type rdf:Property ;
  rdf:type owl:DatatypeProperty ;
  rdfs:comment "The first name of a person." ;
  rdfs:domain dcterms:Agent ;
  rdfs:domain schema:Person ;
  rdfs:domain toop:Person ;
  rdfs:domain <http://www.w3.org/2000/10/swap/pim/contact#Person> ;
  rdfs:domain owl:Thing ;
  rdfs:domain wgs:SpatialThing ;
  rdfs:domain foaf:Agent ;
  rdfs:domain foaf:Person ;
  rdfs:domain _:b420951 ;
  rdfs:domain _:b421075 ;
  rdfs:domain _:b421664 ;
  rdfs:domain _:b421928 ;
  rdfs:domain _:b937877 ;
  rdfs:domain _:b938265 ;
  rdfs:isDefinedBy foaf: ;
  rdfs:label "firstName" ;
  rdfs:range rdfs:Literal ;
  vs:term_status "testing" ;
.
foaf:focus
  rdf:type rdf:Property ;
  rdf:type owl:ObjectProperty ;
  rdfs:comment "The underlying or 'focal' entity associated with some SKOS-described concept." ;
  rdfs:domain owl:Thing ;
  rdfs:domain skos:Concept ;
  rdfs:domain _:b327858 ;
  rdfs:isDefinedBy foaf: ;
  rdfs:label "focus" ;
  rdfs:range owl:Thing ;
  vs:term_status "testing" ;
.
foaf:fundedBy
  rdf:type rdf:Property ;
  rdf:type owl:ObjectProperty ;
  rdfs:comment "An organization funding a project or person." ;
  rdfs:domain owl:Thing ;
  rdfs:isDefinedBy foaf: ;
  rdfs:label "funded by" ;
  rdfs:range owl:Thing ;
  vs:term_status "archaic" ;
.
foaf:geekcode
  rdf:type rdf:Property ;
  rdf:type owl:DatatypeProperty ;
  rdfs:comment "A textual geekcode for this person, see http://www.geekcode.com/geek.html" ;
  rdfs:domain dcterms:Agent ;
  rdfs:domain schema:Person ;
  rdfs:domain toop:Person ;
  rdfs:domain <http://www.w3.org/2000/10/swap/pim/contact#Person> ;
  rdfs:domain owl:Thing ;
  rdfs:domain wgs:SpatialThing ;
  rdfs:domain foaf:Agent ;
  rdfs:domain foaf:Person ;
  rdfs:domain _:b420951 ;
  rdfs:domain _:b421075 ;
  rdfs:domain _:b421664 ;
  rdfs:domain _:b421928 ;
  rdfs:domain _:b937877 ;
  rdfs:domain _:b938265 ;
  rdfs:isDefinedBy foaf: ;
  rdfs:label "geekcode" ;
  rdfs:range rdfs:Literal ;
  vs:term_status "archaic" ;
.
foaf:gender
  rdf:type rdf:Property ;
  rdf:type owl:DatatypeProperty ;
  rdf:type owl:FunctionalProperty ;
  rdfs:comment "The gender of this Agent (typically but not necessarily 'male' or 'female')." ;
  rdfs:domain dcterms:Agent ;
  rdfs:domain owl:Thing ;
  rdfs:domain foaf:Agent ;
  rdfs:domain _:b420951 ;
  rdfs:domain _:b421075 ;
  rdfs:domain _:b421664 ;
  rdfs:domain _:b421928 ;
  rdfs:domain _:b937877 ;
  rdfs:domain _:b938265 ;
  rdfs:isDefinedBy foaf: ;
  rdfs:label "gender" ;
  rdfs:range rdfs:Literal ;
  vs:term_status "testing" ;
.
foaf:givenName
  rdf:type rdf:Property ;
  rdf:type owl:DatatypeProperty ;
  rdfs:comment "The given name of some person." ;
  rdfs:domain dcterms:Agent ;
  rdfs:domain schema:Person ;
  rdfs:domain toop:Person ;
  rdfs:domain <http://www.w3.org/2000/10/swap/pim/contact#Person> ;
  rdfs:domain owl:Thing ;
  rdfs:domain wgs:SpatialThing ;
  rdfs:domain foaf:Agent ;
  rdfs:domain foaf:Person ;
  rdfs:domain _:b420951 ;
  rdfs:domain _:b421075 ;
  rdfs:domain _:b421664 ;
  rdfs:domain _:b421928 ;
  rdfs:domain _:b937877 ;
  rdfs:domain _:b938265 ;
  rdfs:isDefinedBy foaf: ;
  rdfs:label "Given name" ;
  owl:equivalentProperty toop:givenName ;
  vs:term_status "testing" ;
.
foaf:givenname
  rdf:type rdf:Property ;
  rdf:type owl:DatatypeProperty ;
  rdfs:comment "The given name of some person." ;
  rdfs:isDefinedBy foaf: ;
  rdfs:label "Given name" ;
  vs:term_status "archaic" ;
.
foaf:holdsAccount
  rdf:type rdf:Property ;
  rdf:type owl:ObjectProperty ;
  rdfs:comment "Indicates an account held by this agent." ;
  rdfs:domain dcterms:Agent ;
  rdfs:domain owl:Thing ;
  rdfs:domain foaf:Agent ;
  rdfs:domain _:b420951 ;
  rdfs:domain _:b421075 ;
  rdfs:domain _:b421664 ;
  rdfs:domain _:b421928 ;
  rdfs:domain _:b937877 ;
  rdfs:domain _:b938265 ;
  rdfs:isDefinedBy foaf: ;
  rdfs:label "account" ;
  rdfs:range owl:Thing ;
  rdfs:range foaf:OnlineAccount ;
  vs:term_status "archaic" ;
.
foaf:homepage
  rdf:type rdf:Property ;
  rdf:type owl:InverseFunctionalProperty ;
  rdf:type owl:ObjectProperty ;
  rdfs:comment "A homepage for some thing." ;
  rdfs:domain owl:Thing ;
  rdfs:isDefinedBy foaf: ;
  rdfs:label "homepage" ;
  rdfs:range schema:CreativeWork ;
  rdfs:range owl:Thing ;
  rdfs:range foaf:Document ;
  rdfs:subPropertyOf foaf:isPrimaryTopicOf ;
  rdfs:subPropertyOf foaf:page ;
  vs:term_status "stable" ;
.
foaf:icqChatID
  rdf:type rdf:Property ;
  rdf:type owl:DatatypeProperty ;
  rdf:type owl:InverseFunctionalProperty ;
  rdfs:comment "An ICQ chat ID" ;
  rdfs:domain dcterms:Agent ;
  rdfs:domain owl:Thing ;
  rdfs:domain foaf:Agent ;
  rdfs:domain _:b420951 ;
  rdfs:domain _:b421075 ;
  rdfs:domain _:b421664 ;
  rdfs:domain _:b421928 ;
  rdfs:domain _:b937877 ;
  rdfs:domain _:b938265 ;
  rdfs:isDefinedBy foaf: ;
  rdfs:label "ICQ chat ID" ;
  rdfs:range rdfs:Literal ;
  rdfs:subPropertyOf foaf:nick ;
  vs:term_status "testing" ;
.
foaf:img
  rdf:type rdf:Property ;
  rdf:type owl:ObjectProperty ;
  rdfs:comment "An image that can be used to represent some thing (ie. those depictions which are particularly representative of something, eg. one's photo on a homepage)." ;
  rdfs:domain dcterms:Agent ;
  rdfs:domain schema:Person ;
  rdfs:domain toop:Person ;
  rdfs:domain <http://www.w3.org/2000/10/swap/pim/contact#Person> ;
  rdfs:domain owl:Thing ;
  rdfs:domain wgs:SpatialThing ;
  rdfs:domain foaf:Agent ;
  rdfs:domain foaf:Person ;
  rdfs:domain _:b420951 ;
  rdfs:domain _:b421075 ;
  rdfs:domain _:b421664 ;
  rdfs:domain _:b421928 ;
  rdfs:domain _:b937877 ;
  rdfs:domain _:b938265 ;
  rdfs:isDefinedBy foaf: ;
  rdfs:label "image" ;
  rdfs:range schema:CreativeWork ;
  rdfs:range schema:ImageObject ;
  rdfs:range owl:Thing ;
  rdfs:range foaf:Document ;
  rdfs:range foaf:Image ;
  rdfs:subPropertyOf foaf:depiction ;
  vs:term_status "testing" ;
.
foaf:interest
  rdf:type rdf:Property ;
  rdf:type owl:ObjectProperty ;
  rdfs:comment "A page about a topic of interest to this person." ;
  rdfs:domain dcterms:Agent ;
  rdfs:domain owl:Thing ;
  rdfs:domain foaf:Agent ;
  rdfs:domain _:b420951 ;
  rdfs:domain _:b421075 ;
  rdfs:domain _:b421664 ;
  rdfs:domain _:b421928 ;
  rdfs:domain _:b937877 ;
  rdfs:domain _:b938265 ;
  rdfs:isDefinedBy foaf: ;
  rdfs:label "interest" ;
  rdfs:range schema:CreativeWork ;
  rdfs:range owl:Thing ;
  rdfs:range foaf:Document ;
  vs:term_status "testing" ;
.
foaf:isPrimaryTopicOf
  rdf:type rdf:Property ;
  rdf:type owl:InverseFunctionalProperty ;
  rdfs:comment "A document that this thing is the primary topic of." ;
  rdfs:domain owl:Thing ;
  rdfs:isDefinedBy foaf: ;
  rdfs:label "is primary topic of" ;
  rdfs:range schema:CreativeWork ;
  rdfs:range owl:Thing ;
  rdfs:range foaf:Document ;
  rdfs:subPropertyOf foaf:page ;
  owl:inverseOf foaf:primaryTopic ;
  vs:term_status "stable" ;
.
foaf:jabberID
  rdf:type rdf:Property ;
  rdf:type owl:DatatypeProperty ;
  rdf:type owl:InverseFunctionalProperty ;
  rdfs:comment "A jabber ID for something." ;
  rdfs:domain dcterms:Agent ;
  rdfs:domain owl:Thing ;
  rdfs:domain foaf:Agent ;
  rdfs:domain _:b420951 ;
  rdfs:domain _:b421075 ;
  rdfs:domain _:b421664 ;
  rdfs:domain _:b421928 ;
  rdfs:domain _:b937877 ;
  rdfs:domain _:b938265 ;
  rdfs:isDefinedBy foaf: ;
  rdfs:label "jabber ID" ;
  rdfs:range rdfs:Literal ;
  vs:term_status "testing" ;
.
foaf:knows
  rdf:type rdf:Property ;
  rdf:type owl:ObjectProperty ;
  rdfs:comment "A person known by this person (indicating some level of reciprocated interaction between the parties)." ;
  rdfs:domain dcterms:Agent ;
  rdfs:domain schema:Person ;
  rdfs:domain toop:Person ;
  rdfs:domain <http://www.w3.org/2000/10/swap/pim/contact#Person> ;
  rdfs:domain owl:Thing ;
  rdfs:domain wgs:SpatialThing ;
  rdfs:domain foaf:Agent ;
  rdfs:domain foaf:Person ;
  rdfs:domain _:b420951 ;
  rdfs:domain _:b421075 ;
  rdfs:domain _:b421664 ;
  rdfs:domain _:b421928 ;
  rdfs:domain _:b937877 ;
  rdfs:domain _:b938265 ;
  rdfs:isDefinedBy foaf: ;
  rdfs:label "knows" ;
  rdfs:range dcterms:Agent ;
  rdfs:range schema:Person ;
  rdfs:range toop:Person ;
  rdfs:range <http://www.w3.org/2000/10/swap/pim/contact#Person> ;
  rdfs:range owl:Thing ;
  rdfs:range wgs:SpatialThing ;
  rdfs:range foaf:Agent ;
  rdfs:range foaf:Person ;
  rdfs:range _:b420951 ;
  rdfs:range _:b421075 ;
  rdfs:range _:b421664 ;
  rdfs:range _:b421928 ;
  rdfs:range _:b937877 ;
  rdfs:range _:b938265 ;
  vs:term_status "stable" ;
.
foaf:lastName
  rdf:type rdf:Property ;
  rdf:type owl:DatatypeProperty ;
  rdfs:comment "The last name of a person." ;
  rdfs:domain dcterms:Agent ;
  rdfs:domain schema:Person ;
  rdfs:domain toop:Person ;
  rdfs:domain <http://www.w3.org/2000/10/swap/pim/contact#Person> ;
  rdfs:domain owl:Thing ;
  rdfs:domain wgs:SpatialThing ;
  rdfs:domain foaf:Agent ;
  rdfs:domain foaf:Person ;
  rdfs:domain _:b420951 ;
  rdfs:domain _:b421075 ;
  rdfs:domain _:b421664 ;
  rdfs:domain _:b421928 ;
  rdfs:domain _:b937877 ;
  rdfs:domain _:b938265 ;
  rdfs:isDefinedBy foaf: ;
  rdfs:label "lastName" ;
  rdfs:range rdfs:Literal ;
  vs:term_status "testing" ;
.
foaf:logo
  rdf:type rdf:Property ;
  rdf:type owl:InverseFunctionalProperty ;
  rdf:type owl:ObjectProperty ;
  rdfs:comment "A logo representing some thing." ;
  rdfs:domain owl:Thing ;
  rdfs:isDefinedBy foaf: ;
  rdfs:label "logo" ;
  rdfs:range owl:Thing ;
  vs:term_status "testing" ;
.
foaf:made
  rdf:type rdf:Property ;
  rdf:type owl:ObjectProperty ;
  rdfs:comment "Something that was made by this agent." ;
  rdfs:domain dcterms:Agent ;
  rdfs:domain owl:Thing ;
  rdfs:domain foaf:Agent ;
  rdfs:domain _:b420951 ;
  rdfs:domain _:b421075 ;
  rdfs:domain _:b421664 ;
  rdfs:domain _:b421928 ;
  rdfs:domain _:b937877 ;
  rdfs:domain _:b938265 ;
  rdfs:isDefinedBy foaf: ;
  rdfs:label "made" ;
  rdfs:range owl:Thing ;
  owl:inverseOf foaf:maker ;
  vs:term_status "stable" ;
.
foaf:maker
  rdf:type rdf:Property ;
  rdf:type owl:ObjectProperty ;
  rdfs:comment "An agent that  made this thing." ;
  rdfs:domain elobr:EloniaBusinessCode ;
  rdfs:domain freebr:FreedoniaBusinessCode ;
  rdfs:domain toop:CompanyCode ;
  rdfs:domain owl:Thing ;
  rdfs:domain adms:Identifier ;
  rdfs:isDefinedBy foaf: ;
  rdfs:label "maker" ;
  rdfs:range dcterms:Agent ;
  rdfs:range owl:Thing ;
  rdfs:range foaf:Agent ;
  rdfs:range _:b420951 ;
  rdfs:range _:b421075 ;
  rdfs:range _:b421664 ;
  rdfs:range _:b421928 ;
  rdfs:range _:b937877 ;
  rdfs:range _:b938265 ;
  rdfs:subPropertyOf dc:contributor ;
  rdfs:subPropertyOf dc:creator ;
  rdfs:subPropertyOf dcterms:contributor ;
  rdfs:subPropertyOf dcterms:creator ;
  owl:equivalentProperty elobr:EloniaRegistrationAuthority ;
  owl:equivalentProperty freebr:FreedoniaRegistrationAuthority ;
  owl:equivalentProperty dcterms:creator ;
  owl:equivalentProperty toop:registrationAuthority ;
  owl:inverseOf foaf:made ;
  vs:term_status "stable" ;
.
foaf:mbox
  rdf:type rdf:Property ;
  rdf:type owl:InverseFunctionalProperty ;
  rdf:type owl:ObjectProperty ;
  rdfs:comment "A  personal mailbox, ie. an Internet mailbox associated with exactly one owner, the first owner of this mailbox. This is a 'static inverse functional property', in that  there is (across time and change) at most one individual that ever has any particular value for foaf:mbox." ;
  rdfs:domain dcterms:Agent ;
  rdfs:domain owl:Thing ;
  rdfs:domain foaf:Agent ;
  rdfs:domain _:b420951 ;
  rdfs:domain _:b421075 ;
  rdfs:domain _:b421664 ;
  rdfs:domain _:b421928 ;
  rdfs:domain _:b937877 ;
  rdfs:domain _:b938265 ;
  rdfs:isDefinedBy foaf: ;
  rdfs:label "personal mailbox" ;
  rdfs:range owl:Thing ;
  vs:term_status "stable" ;
.
foaf:mbox_sha1sum
  rdf:type rdf:Property ;
  rdf:type owl:DatatypeProperty ;
  rdf:type owl:InverseFunctionalProperty ;
  rdfs:comment "The sha1sum of the URI of an Internet mailbox associated with exactly one owner, the  first owner of the mailbox." ;
  rdfs:domain dcterms:Agent ;
  rdfs:domain owl:Thing ;
  rdfs:domain foaf:Agent ;
  rdfs:domain _:b420951 ;
  rdfs:domain _:b421075 ;
  rdfs:domain _:b421664 ;
  rdfs:domain _:b421928 ;
  rdfs:domain _:b937877 ;
  rdfs:domain _:b938265 ;
  rdfs:isDefinedBy foaf: ;
  rdfs:label "sha1sum of a personal mailbox URI name" ;
  rdfs:range rdfs:Literal ;
  vs:term_status "testing" ;
.
foaf:member
  rdf:type rdf:Property ;
  rdf:type owl:ObjectProperty ;
  rdfs:comment "Indicates a member of a Group" ;
  rdfs:domain dcterms:Agent ;
  rdfs:domain owl:Thing ;
  rdfs:domain org:Organization ;
  rdfs:domain foaf:Agent ;
  rdfs:domain foaf:Group ;
  rdfs:domain foaf:Organization ;
  rdfs:domain _:b420951 ;
  rdfs:domain _:b421075 ;
  rdfs:domain _:b421664 ;
  rdfs:domain _:b421928 ;
  rdfs:domain _:b937877 ;
  rdfs:domain _:b938265 ;
  rdfs:isDefinedBy foaf: ;
  rdfs:label "member" ;
  rdfs:range dcterms:Agent ;
  rdfs:range owl:Thing ;
  rdfs:range foaf:Agent ;
  rdfs:range _:b420951 ;
  rdfs:range _:b421075 ;
  rdfs:range _:b421664 ;
  rdfs:range _:b421928 ;
  rdfs:range _:b937877 ;
  rdfs:range _:b938265 ;
  owl:equivalentProperty org:hasMember ;
  vs:term_status "stable" ;
.
foaf:membershipClass
  rdf:type rdf:Property ;
  rdf:type owl:AnnotationProperty ;
  rdfs:comment "Indicates the class of individuals that are a member of a Group" ;
  rdfs:isDefinedBy foaf: ;
  rdfs:label "membershipClass" ;
  vs:term_status "unstable" ;
.
foaf:msnChatID
  rdf:type rdf:Property ;
  rdf:type owl:DatatypeProperty ;
  rdf:type owl:InverseFunctionalProperty ;
  rdfs:comment "An MSN chat ID" ;
  rdfs:domain dcterms:Agent ;
  rdfs:domain owl:Thing ;
  rdfs:domain foaf:Agent ;
  rdfs:domain _:b420951 ;
  rdfs:domain _:b421075 ;
  rdfs:domain _:b421664 ;
  rdfs:domain _:b421928 ;
  rdfs:domain _:b937877 ;
  rdfs:domain _:b938265 ;
  rdfs:isDefinedBy foaf: ;
  rdfs:label "MSN chat ID" ;
  rdfs:range rdfs:Literal ;
  rdfs:subPropertyOf foaf:nick ;
  vs:term_status "testing" ;
.
foaf:myersBriggs
  rdf:type rdf:Property ;
  rdf:type owl:DatatypeProperty ;
  rdfs:comment "A Myers Briggs (MBTI) personality classification." ;
  rdfs:domain dcterms:Agent ;
  rdfs:domain schema:Person ;
  rdfs:domain toop:Person ;
  rdfs:domain <http://www.w3.org/2000/10/swap/pim/contact#Person> ;
  rdfs:domain owl:Thing ;
  rdfs:domain wgs:SpatialThing ;
  rdfs:domain foaf:Agent ;
  rdfs:domain foaf:Person ;
  rdfs:domain _:b420951 ;
  rdfs:domain _:b421075 ;
  rdfs:domain _:b421664 ;
  rdfs:domain _:b421928 ;
  rdfs:domain _:b937877 ;
  rdfs:domain _:b938265 ;
  rdfs:isDefinedBy foaf: ;
  rdfs:label "myersBriggs" ;
  rdfs:range rdfs:Literal ;
  vs:term_status "testing" ;
.
foaf:name
  rdf:type rdf:Property ;
  rdf:type owl:DatatypeProperty ;
  rdfs:comment "A name for some thing." ;
  rdfs:domain owl:Thing ;
  rdfs:isDefinedBy foaf: ;
  rdfs:label "name" ;
  rdfs:range rdfs:Literal ;
  rdfs:subPropertyOf rdfs:label ;
  vs:term_status "testing" ;
.
foaf:nick
  rdf:type rdf:Property ;
  rdf:type owl:DatatypeProperty ;
  rdfs:comment "A short informal nickname characterising an agent (includes login identifiers, IRC and other chat nicknames)." ;
  rdfs:isDefinedBy foaf: ;
  rdfs:label "nickname" ;
  vs:term_status "testing" ;
.
foaf:openid
  rdf:type rdf:Property ;
  rdf:type owl:InverseFunctionalProperty ;
  rdf:type owl:ObjectProperty ;
  rdfs:comment "An OpenID for an Agent." ;
  rdfs:domain dcterms:Agent ;
  rdfs:domain owl:Thing ;
  rdfs:domain foaf:Agent ;
  rdfs:domain _:b420951 ;
  rdfs:domain _:b421075 ;
  rdfs:domain _:b421664 ;
  rdfs:domain _:b421928 ;
  rdfs:domain _:b937877 ;
  rdfs:domain _:b938265 ;
  rdfs:isDefinedBy foaf: ;
  rdfs:label "openid" ;
  rdfs:range schema:CreativeWork ;
  rdfs:range owl:Thing ;
  rdfs:range foaf:Document ;
  rdfs:subPropertyOf foaf:isPrimaryTopicOf ;
  rdfs:subPropertyOf foaf:page ;
  vs:term_status "testing" ;
.
foaf:page
  rdf:type rdf:Property ;
  rdf:type owl:ObjectProperty ;
  rdfs:comment "A page or document about this thing." ;
  rdfs:domain owl:Thing ;
  rdfs:isDefinedBy foaf: ;
  rdfs:label "page" ;
  rdfs:range schema:CreativeWork ;
  rdfs:range owl:Thing ;
  rdfs:range foaf:Document ;
  owl:inverseOf foaf:topic ;
  vs:term_status "stable" ;
.
foaf:pastProject
  rdf:type rdf:Property ;
  rdf:type owl:ObjectProperty ;
  rdfs:comment "A project this person has previously worked on." ;
  rdfs:domain dcterms:Agent ;
  rdfs:domain schema:Person ;
  rdfs:domain toop:Person ;
  rdfs:domain <http://www.w3.org/2000/10/swap/pim/contact#Person> ;
  rdfs:domain owl:Thing ;
  rdfs:domain wgs:SpatialThing ;
  rdfs:domain foaf:Agent ;
  rdfs:domain foaf:Person ;
  rdfs:domain _:b420951 ;
  rdfs:domain _:b421075 ;
  rdfs:domain _:b421664 ;
  rdfs:domain _:b421928 ;
  rdfs:domain _:b937877 ;
  rdfs:domain _:b938265 ;
  rdfs:isDefinedBy foaf: ;
  rdfs:label "past project" ;
  rdfs:range owl:Thing ;
  vs:term_status "testing" ;
.
foaf:phone
  rdf:type rdf:Property ;
  rdf:type owl:ObjectProperty ;
  rdfs:comment "A phone,  specified using fully qualified tel: URI scheme (refs: http://www.w3.org/Addressing/schemes.html#tel)." ;
  rdfs:isDefinedBy foaf: ;
  rdfs:label "phone" ;
  vs:term_status "testing" ;
.
foaf:plan
  rdf:type rdf:Property ;
  rdf:type owl:DatatypeProperty ;
  rdfs:comment "A .plan comment, in the tradition of finger and '.plan' files." ;
  rdfs:domain dcterms:Agent ;
  rdfs:domain schema:Person ;
  rdfs:domain toop:Person ;
  rdfs:domain <http://www.w3.org/2000/10/swap/pim/contact#Person> ;
  rdfs:domain owl:Thing ;
  rdfs:domain wgs:SpatialThing ;
  rdfs:domain foaf:Agent ;
  rdfs:domain foaf:Person ;
  rdfs:domain _:b420951 ;
  rdfs:domain _:b421075 ;
  rdfs:domain _:b421664 ;
  rdfs:domain _:b421928 ;
  rdfs:domain _:b937877 ;
  rdfs:domain _:b938265 ;
  rdfs:isDefinedBy foaf: ;
  rdfs:label "plan" ;
  rdfs:range rdfs:Literal ;
  vs:term_status "testing" ;
.
foaf:primaryTopic
  rdf:type rdf:Property ;
  rdf:type owl:FunctionalProperty ;
  rdf:type owl:ObjectProperty ;
  rdfs:comment "The primary topic of some page or document." ;
  rdfs:domain schema:CreativeWork ;
  rdfs:domain owl:Thing ;
  rdfs:domain foaf:Document ;
  rdfs:isDefinedBy foaf: ;
  rdfs:label "primary topic" ;
  rdfs:range owl:Thing ;
  owl:inverseOf foaf:isPrimaryTopicOf ;
  vs:term_status "stable" ;
.
foaf:publications
  rdf:type rdf:Property ;
  rdf:type owl:ObjectProperty ;
  rdfs:comment "A link to the publications of this person." ;
  rdfs:domain dcterms:Agent ;
  rdfs:domain schema:Person ;
  rdfs:domain toop:Person ;
  rdfs:domain <http://www.w3.org/2000/10/swap/pim/contact#Person> ;
  rdfs:domain owl:Thing ;
  rdfs:domain wgs:SpatialThing ;
  rdfs:domain foaf:Agent ;
  rdfs:domain foaf:Person ;
  rdfs:domain _:b420951 ;
  rdfs:domain _:b421075 ;
  rdfs:domain _:b421664 ;
  rdfs:domain _:b421928 ;
  rdfs:domain _:b937877 ;
  rdfs:domain _:b938265 ;
  rdfs:isDefinedBy foaf: ;
  rdfs:label "publications" ;
  rdfs:range schema:CreativeWork ;
  rdfs:range owl:Thing ;
  rdfs:range foaf:Document ;
  vs:term_status "testing" ;
.
foaf:schoolHomepage
  rdf:type rdf:Property ;
  rdf:type owl:ObjectProperty ;
  rdfs:comment "A homepage of a school attended by the person." ;
  rdfs:domain dcterms:Agent ;
  rdfs:domain schema:Person ;
  rdfs:domain toop:Person ;
  rdfs:domain <http://www.w3.org/2000/10/swap/pim/contact#Person> ;
  rdfs:domain owl:Thing ;
  rdfs:domain wgs:SpatialThing ;
  rdfs:domain foaf:Agent ;
  rdfs:domain foaf:Person ;
  rdfs:domain _:b420951 ;
  rdfs:domain _:b421075 ;
  rdfs:domain _:b421664 ;
  rdfs:domain _:b421928 ;
  rdfs:domain _:b937877 ;
  rdfs:domain _:b938265 ;
  rdfs:isDefinedBy foaf: ;
  rdfs:label "schoolHomepage" ;
  rdfs:range schema:CreativeWork ;
  rdfs:range owl:Thing ;
  rdfs:range foaf:Document ;
  vs:term_status "testing" ;
.
foaf:sha1
  rdf:type rdf:Property ;
  rdf:type owl:DatatypeProperty ;
  rdfs:comment "A sha1sum hash, in hex." ;
  rdfs:domain schema:CreativeWork ;
  rdfs:domain owl:Thing ;
  rdfs:domain foaf:Document ;
  rdfs:isDefinedBy foaf: ;
  rdfs:label "sha1sum (hex)" ;
  vs:term_status "unstable" ;
.
foaf:skypeID
  rdf:type rdf:Property ;
  rdf:type owl:DatatypeProperty ;
  rdfs:comment "A Skype ID" ;
  rdfs:domain dcterms:Agent ;
  rdfs:domain owl:Thing ;
  rdfs:domain foaf:Agent ;
  rdfs:domain _:b420951 ;
  rdfs:domain _:b421075 ;
  rdfs:domain _:b421664 ;
  rdfs:domain _:b421928 ;
  rdfs:domain _:b937877 ;
  rdfs:domain _:b938265 ;
  rdfs:isDefinedBy foaf: ;
  rdfs:label "Skype ID" ;
  rdfs:range rdfs:Literal ;
  rdfs:subPropertyOf foaf:nick ;
  vs:term_status "testing" ;
.
foaf:status
  rdf:type rdf:Property ;
  rdf:type owl:DatatypeProperty ;
  rdfs:comment "A string expressing what the user is happy for the general public (normally) to know about their current activity." ;
  rdfs:domain dcterms:Agent ;
  rdfs:domain owl:Thing ;
  rdfs:domain foaf:Agent ;
  rdfs:domain _:b420951 ;
  rdfs:domain _:b421075 ;
  rdfs:domain _:b421664 ;
  rdfs:domain _:b421928 ;
  rdfs:domain _:b937877 ;
  rdfs:domain _:b938265 ;
  rdfs:isDefinedBy foaf: ;
  rdfs:label "status" ;
  rdfs:range rdfs:Literal ;
  vs:term_status "unstable" ;
.
foaf:surname
  rdf:type rdf:Property ;
  rdf:type owl:DatatypeProperty ;
  rdfs:comment "The surname of some person." ;
  rdfs:domain dcterms:Agent ;
  rdfs:domain schema:Person ;
  rdfs:domain toop:Person ;
  rdfs:domain <http://www.w3.org/2000/10/swap/pim/contact#Person> ;
  rdfs:domain owl:Thing ;
  rdfs:domain wgs:SpatialThing ;
  rdfs:domain foaf:Agent ;
  rdfs:domain foaf:Person ;
  rdfs:domain _:b420951 ;
  rdfs:domain _:b421075 ;
  rdfs:domain _:b421664 ;
  rdfs:domain _:b421928 ;
  rdfs:domain _:b937877 ;
  rdfs:domain _:b938265 ;
  rdfs:isDefinedBy foaf: ;
  rdfs:label "Surname" ;
  rdfs:range rdfs:Literal ;
  vs:term_status "archaic" ;
.
foaf:theme
  rdf:type rdf:Property ;
  rdf:type owl:ObjectProperty ;
  rdfs:comment "A theme." ;
  rdfs:domain owl:Thing ;
  rdfs:isDefinedBy foaf: ;
  rdfs:label "theme" ;
  rdfs:range owl:Thing ;
  vs:term_status "archaic" ;
.
foaf:thumbnail
  rdf:type rdf:Property ;
  rdf:type owl:ObjectProperty ;
  rdfs:comment "A derived thumbnail image." ;
  rdfs:domain schema:CreativeWork ;
  rdfs:domain schema:ImageObject ;
  rdfs:domain owl:Thing ;
  rdfs:domain foaf:Document ;
  rdfs:domain foaf:Image ;
  rdfs:isDefinedBy foaf: ;
  rdfs:label "thumbnail" ;
  rdfs:range schema:CreativeWork ;
  rdfs:range schema:ImageObject ;
  rdfs:range owl:Thing ;
  rdfs:range foaf:Document ;
  rdfs:range foaf:Image ;
  vs:term_status "testing" ;
.
foaf:tipjar
  rdf:type rdf:Property ;
  rdf:type owl:ObjectProperty ;
  rdfs:comment "A tipjar document for this agent, describing means for payment and reward." ;
  rdfs:domain dcterms:Agent ;
  rdfs:domain owl:Thing ;
  rdfs:domain foaf:Agent ;
  rdfs:domain _:b420951 ;
  rdfs:domain _:b421075 ;
  rdfs:domain _:b421664 ;
  rdfs:domain _:b421928 ;
  rdfs:domain _:b937877 ;
  rdfs:domain _:b938265 ;
  rdfs:isDefinedBy foaf: ;
  rdfs:label "tipjar" ;
  rdfs:range schema:CreativeWork ;
  rdfs:range owl:Thing ;
  rdfs:range foaf:Document ;
  rdfs:subPropertyOf foaf:page ;
  vs:term_status "testing" ;
.
foaf:title
  rdf:type rdf:Property ;
  rdf:type owl:DatatypeProperty ;
  rdfs:comment "Title (Mr, Mrs, Ms, Dr. etc)" ;
  rdfs:isDefinedBy foaf: ;
  rdfs:label "title" ;
  vs:term_status "testing" ;
.
foaf:topic
  rdf:type rdf:Property ;
  rdf:type owl:ObjectProperty ;
  rdfs:comment "A topic of some page or document." ;
  rdfs:domain schema:CreativeWork ;
  rdfs:domain owl:Thing ;
  rdfs:domain foaf:Document ;
  rdfs:isDefinedBy foaf: ;
  rdfs:label "topic" ;
  rdfs:range owl:Thing ;
  owl:inverseOf foaf:page ;
  vs:term_status "testing" ;
.
foaf:topic_interest
  rdf:type rdf:Property ;
  rdf:type owl:ObjectProperty ;
  rdfs:comment "A thing of interest to this person." ;
  rdfs:domain dcterms:Agent ;
  rdfs:domain owl:Thing ;
  rdfs:domain foaf:Agent ;
  rdfs:domain _:b420951 ;
  rdfs:domain _:b421075 ;
  rdfs:domain _:b421664 ;
  rdfs:domain _:b421928 ;
  rdfs:domain _:b937877 ;
  rdfs:domain _:b938265 ;
  rdfs:isDefinedBy foaf: ;
  rdfs:label "topic_interest" ;
  rdfs:range owl:Thing ;
  vs:term_status "testing" ;
.
foaf:weblog
  rdf:type rdf:Property ;
  rdf:type owl:InverseFunctionalProperty ;
  rdf:type owl:ObjectProperty ;
  rdfs:comment "A weblog of some thing (whether person, group, company etc.)." ;
  rdfs:domain dcterms:Agent ;
  rdfs:domain owl:Thing ;
  rdfs:domain foaf:Agent ;
  rdfs:domain _:b420951 ;
  rdfs:domain _:b421075 ;
  rdfs:domain _:b421664 ;
  rdfs:domain _:b421928 ;
  rdfs:domain _:b937877 ;
  rdfs:domain _:b938265 ;
  rdfs:isDefinedBy foaf: ;
  rdfs:label "weblog" ;
  rdfs:range schema:CreativeWork ;
  rdfs:range owl:Thing ;
  rdfs:range foaf:Document ;
  rdfs:subPropertyOf foaf:page ;
  vs:term_status "stable" ;
.
foaf:workInfoHomepage
  rdf:type rdf:Property ;
  rdf:type owl:ObjectProperty ;
  rdfs:comment "A work info homepage of some person; a page about their work for some organization." ;
  rdfs:domain dcterms:Agent ;
  rdfs:domain schema:Person ;
  rdfs:domain toop:Person ;
  rdfs:domain <http://www.w3.org/2000/10/swap/pim/contact#Person> ;
  rdfs:domain owl:Thing ;
  rdfs:domain wgs:SpatialThing ;
  rdfs:domain foaf:Agent ;
  rdfs:domain foaf:Person ;
  rdfs:domain _:b420951 ;
  rdfs:domain _:b421075 ;
  rdfs:domain _:b421664 ;
  rdfs:domain _:b421928 ;
  rdfs:domain _:b937877 ;
  rdfs:domain _:b938265 ;
  rdfs:isDefinedBy foaf: ;
  rdfs:label "work info homepage" ;
  rdfs:range schema:CreativeWork ;
  rdfs:range owl:Thing ;
  rdfs:range foaf:Document ;
  vs:term_status "testing" ;
.
foaf:workplaceHomepage
  rdf:type rdf:Property ;
  rdf:type owl:ObjectProperty ;
  rdfs:comment "A workplace homepage of some person; the homepage of an organization they work for." ;
  rdfs:domain dcterms:Agent ;
  rdfs:domain schema:Person ;
  rdfs:domain toop:Person ;
  rdfs:domain <http://www.w3.org/2000/10/swap/pim/contact#Person> ;
  rdfs:domain owl:Thing ;
  rdfs:domain wgs:SpatialThing ;
  rdfs:domain foaf:Agent ;
  rdfs:domain foaf:Person ;
  rdfs:domain _:b420951 ;
  rdfs:domain _:b421075 ;
  rdfs:domain _:b421664 ;
  rdfs:domain _:b421928 ;
  rdfs:domain _:b937877 ;
  rdfs:domain _:b938265 ;
  rdfs:isDefinedBy foaf: ;
  rdfs:label "workplace homepage" ;
  rdfs:range schema:CreativeWork ;
  rdfs:range owl:Thing ;
  rdfs:range foaf:Document ;
  vs:term_status "testing" ;
.
foaf:yahooChatID
  rdf:type rdf:Property ;
  rdf:type owl:DatatypeProperty ;
  rdf:type owl:InverseFunctionalProperty ;
  rdfs:comment "A Yahoo chat ID" ;
  rdfs:domain dcterms:Agent ;
  rdfs:domain owl:Thing ;
  rdfs:domain foaf:Agent ;
  rdfs:domain _:b420951 ;
  rdfs:domain _:b421075 ;
  rdfs:domain _:b421664 ;
  rdfs:domain _:b421928 ;
  rdfs:domain _:b937877 ;
  rdfs:domain _:b938265 ;
  rdfs:isDefinedBy foaf: ;
  rdfs:label "Yahoo chat ID" ;
  rdfs:range rdfs:Literal ;
  rdfs:subPropertyOf foaf:nick ;
  vs:term_status "testing" ;
.
wot:assurance
  rdf:type owl:AnnotationProperty ;
.
wot:src_assurance
  rdf:type owl:AnnotationProperty ;
.
_:b11589
  rdf:type dcterms:Agent ;
  rdf:type foaf:Agent ;
  rdf:type _:b420951 ;
  rdf:type _:b421075 ;
  rdf:type _:b421664 ;
  rdf:type _:b421928 ;
  rdf:type _:b937877 ;
  rdf:type _:b938265 ;
  rdfs:label "Government Linked Data WG, based on output from the ADMS Working Group" ;
  foaf:homepage <http://www.w3.org/2011/gld/> ;
  foaf:isPrimaryTopicOf <http://www.w3.org/2011/gld/> ;
  foaf:made <http://www.w3.org/ns/regorg> ;
  foaf:name "Government Linked Data WG, based on output from the ADMS Working Group" ;
  foaf:page <http://www.w3.org/2011/gld/> ;
.
_:b18002
  rdf:type owl:Restriction ;
  owl:cardinality "1"^^xsd:nonNegativeInteger ;
  owl:onProperty nhr:toegangscodeCommunicatienummer ;
.
_:b29166
  rdf:type owl:Restriction ;
  owl:minQualifiedCardinality "1"^^xsd:nonNegativeInteger ;
  owl:onClass vcard:Kind ;
  owl:onProperty vcard:hasMember ;
.
_:b49042
  rdf:type owl:Class ;
  owl:equivalentClass elobr:EloniaAddress ;
  owl:equivalentClass freebr:FreedoniaAddress ;
  owl:equivalentClass toop:Address ;
  owl:equivalentClass vcard:Address ;
  owl:unionOf (
      [
        rdf:type owl:Class ;
        owl:intersectionOf (
            [
              rdf:type owl:Restriction ;
              owl:onProperty vcard:country-name ;
              owl:someValuesFrom xsd:string ;
            ]
            [
              rdf:type owl:Restriction ;
              owl:maxCardinality "1"^^xsd:nonNegativeInteger ;
              owl:onProperty vcard:country-name ;
            ]
          ) ;
      ]
      [
        rdf:type owl:Class ;
        owl:intersectionOf (
            [
              rdf:type owl:Restriction ;
              owl:onProperty vcard:locality ;
              owl:someValuesFrom xsd:string ;
            ]
            [
              rdf:type owl:Restriction ;
              owl:maxCardinality "1"^^xsd:nonNegativeInteger ;
              owl:onProperty vcard:locality ;
            ]
          ) ;
      ]
      [
        rdf:type owl:Class ;
        owl:intersectionOf (
            [
              rdf:type owl:Restriction ;
              owl:onProperty vcard:postal-code ;
              owl:someValuesFrom xsd:string ;
            ]
            [
              rdf:type owl:Restriction ;
              owl:maxCardinality "1"^^xsd:nonNegativeInteger ;
              owl:onProperty vcard:postal-code ;
            ]
          ) ;
      ]
      [
        rdf:type owl:Class ;
        owl:intersectionOf (
            [
              rdf:type owl:Restriction ;
              owl:onProperty vcard:region ;
              owl:someValuesFrom xsd:string ;
            ]
            [
              rdf:type owl:Restriction ;
              owl:maxCardinality "1"^^xsd:nonNegativeInteger ;
              owl:onProperty vcard:region ;
            ]
          ) ;
      ]
      [
        rdf:type owl:Class ;
        owl:intersectionOf (
            [
              rdf:type owl:Restriction ;
              owl:onProperty vcard:street-address ;
              owl:someValuesFrom xsd:string ;
            ]
            [
              rdf:type owl:Restriction ;
              owl:maxCardinality "1"^^xsd:nonNegativeInteger ;
              owl:onProperty vcard:street-address ;
            ]
          ) ;
      ]
    ) ;
.
_:b53184
  rdf:type owl:Class ;
  owl:unionOf (
      prov:Activity
      prov:Agent
      prov:Entity
    ) ;
.
_:b57053
  rdf:type owl:Restriction ;
  owl:equivalentClass vcard:Kind ;
  owl:equivalentClass vcard:VCard ;
  owl:minQualifiedCardinality "1"^^xsd:nonNegativeInteger ;
  owl:onDataRange xsd:string ;
  owl:onProperty vcard:fn ;
.
_:b83024
  rdf:type owl:Class ;
  owl:unionOf (
      vcard:Address
      vcard:Label
    ) ;
.
_:b115973
  rdf:type rdfs:Datatype ;
  owl:unionOf (
      xsd:date
      xsd:dateTime
    ) ;
.
_:b148299
  rdf:type rdfs:Datatype ;
  owl:unionOf (
      xsd:date
      xsd:dateTime
    ) ;
.
_:b156576
  rdf:type owl:Restriction ;
  owl:cardinality "1"^^xsd:nonNegativeInteger ;
  owl:onProperty freebr:FreedoniaCompanyName ;
.
_:b157701
  rdf:type owl:Restriction ;
  owl:onProperty vcard:country-name ;
  owl:someValuesFrom rdfs:Literal ;
.
_:b168676
  rdf:type owl:Restriction ;
  owl:onProperty vcard:extended-address ;
  owl:someValuesFrom rdfs:Literal ;
.
_:b170340
  rdf:type owl:Class ;
  owl:unionOf (
      prov:Activity
      prov:Agent
      prov:Entity
    ) ;
.
_:b180769
  rdf:type owl:Restriction ;
  owl:cardinality "1"^^xsd:nonNegativeInteger ;
  owl:onProperty toop:companyName ;
.
_:b213787
  rdf:type owl:Restriction ;
  owl:cardinality "1"^^xsd:nonNegativeInteger ;
  owl:onProperty elobr:EloniaCompanyName ;
.
_:b218915
  rdf:type owl:Restriction ;
  owl:onProperty vcard:additional-name ;
  owl:someValuesFrom rdfs:Literal ;
.
_:b229905
  rdf:type owl:Restriction ;
  owl:cardinality "1"^^xsd:nonNegativeInteger ;
  owl:onProperty nhr:land ;
.
_:b251823
  rdf:type dcterms:Agent ;
  rdf:type foaf:Agent ;
  rdf:type _:b420951 ;
  rdf:type _:b421075 ;
  rdf:type _:b421664 ;
  rdf:type _:b421928 ;
  rdf:type _:b937877 ;
  rdf:type _:b938265 ;
  rdfs:label "Government Linked Data WG, based on output from the ADMS Working Group" ;
  foaf:made <http://www.w3.org/ns/regorg> ;
  foaf:name "Government Linked Data WG, based on output from the ADMS Working Group" ;
  foaf:page <http://www.w3.org/2011/gld/> ;
.
_:b254570
  rdf:type owl:Restriction ;
  owl:onProperty toop:hasRegistration ;
  owl:someValuesFrom toop:Registration ;
.
_:b269191
  rdf:type owl:Restriction ;
  owl:onProperty vcard:honorific-suffix ;
  owl:someValuesFrom rdfs:Literal ;
.
_:b275344
  rdf:type owl:Class ;
  owl:unionOf (
      prov:Delegation
      prov:Derivation
      prov:End
      prov:Start
    ) ;
.
_:b302287
  rdf:type owl:Restriction ;
  owl:cardinality "1"^^xsd:nonNegativeInteger ;
  owl:onProperty nhr:postcodeWoonplaats ;
.
_:b313826
  rdf:type owl:Restriction ;
  owl:onProperty vcard:longitude ;
  owl:someValuesFrom rdfs:Literal ;
.
_:b327858
  rdf:type owl:Class ;
  owl:unionOf (
      skos:Concept
      skos:Collection
    ) ;
.
_:b329657
  rdf:type owl:Restriction ;
  owl:cardinality "1"^^xsd:nonNegativeInteger ;
  owl:onProperty nhr:plaats ;
.
_:b333528
  rdf:type owl:Restriction ;
  owl:onDataRange nhr:RechtsvormRechtspersoon ;
  owl:onProperty nhr:heeftRechtsvorm ;
  owl:qualifiedCardinality "1"^^xsd:nonNegativeInteger ;
.
_:b396249
  rdf:type owl:Restriction ;
  owl:onProperty vcard:street-address ;
  owl:someValuesFrom rdfs:Literal ;
.
_:b399839
  rdf:type owl:Class ;
  owl:unionOf (
      prov:Activity
      prov:Agent
      prov:Entity
    ) ;
.
_:b401324
  rdf:type owl:Class ;
  owl:unionOf (
      vcard:Address
      vcard:Label
    ) ;
.
_:b405470
  rdf:type owl:Restriction ;
  owl:onProperty vcard:latitude ;
  owl:someValuesFrom rdfs:Literal ;
.
_:b407513
  rdf:type owl:Restriction ;
  owl:cardinality "1"^^xsd:nonNegativeInteger ;
  owl:onProperty nhr:kvkNummer ;
.
_:b420951
  rdf:type owl:Class ;
  <http://www.topbraid.org/c14n#true> "36"^^xsd:long ;
  owl:unionOf (
      foaf:Agent
      org:Post
    ) ;
.
_:b420982
  rdf:type owl:Class ;
  <http://www.topbraid.org/c14n#true> "34"^^xsd:long ;
  owl:unionOf (
      org:Membership
      org:Post
    ) ;
.
_:b421013
  rdf:type dcterms:Agent ;
  rdf:type foaf:Agent ;
  rdf:type _:b420951 ;
  rdf:type _:b421075 ;
  rdf:type _:b421664 ;
  rdf:type _:b421928 ;
  rdf:type _:b937877 ;
  rdf:type _:b938265 ;
  <http://www.topbraid.org/c14n#true> "40"^^xsd:long ;
  rdfs:label "Dominique Guardiola" ;
  owl:sameAs _:b421013 ;
  owl:sameAs _:b937548 ;
  owl:sameAs _:b937769 ;
  foaf:mbox "dguardiola@quinode.fr" ;
  foaf:name "Dominique Guardiola" ;
.
_:b421044
  rdf:type dcterms:Agent ;
  rdf:type foaf:Agent ;
  rdf:type _:b420951 ;
  rdf:type _:b421075 ;
  rdf:type _:b421664 ;
  rdf:type _:b421928 ;
  rdf:type _:b937877 ;
  rdf:type _:b938265 ;
  <http://www.topbraid.org/c14n#true> "38"^^xsd:long ;
  rdfs:label "Olga Ximena Giraldo" ;
  owl:sameAs _:b421044 ;
  owl:sameAs _:b938032 ;
  owl:sameAs _:b938141 ;
  foaf:mbox "ogiraldo@fi.upm.es" ;
  foaf:name "Olga Ximena Giraldo" ;
.
_:b421075
  rdf:type owl:Class ;
  <http://www.topbraid.org/c14n#true> "44"^^xsd:long ;
  owl:unionOf (
      foaf:Agent
      org:Post
    ) ;
.
_:b421106
  rdf:type dcterms:Agent ;
  rdf:type foaf:Agent ;
  rdf:type _:b420951 ;
  rdf:type _:b421075 ;
  rdf:type _:b421664 ;
  rdf:type _:b421928 ;
  rdf:type _:b937877 ;
  rdf:type _:b938265 ;
  <http://www.topbraid.org/c14n#true> "42"^^xsd:long ;
  rdfs:label "Elena Montiel Ponsoda" ;
  owl:sameAs _:b421106 ;
  owl:sameAs _:b937284 ;
  owl:sameAs _:b938001 ;
  foaf:mbox "emontiel@fi.upm.es" ;
  foaf:name "Elena Montiel Ponsoda" ;
.
_:b421137
  <http://www.topbraid.org/c14n#true> "48"^^xsd:long ;
  rdfs:label "W3C/ERCIM" ;
  owl:sameAs _:b421137 ;
  owl:sameAs _:b421711 ;
  owl:sameAs _:b421804 ;
  foaf:homepage <http://www.w3.org/> ;
  foaf:isPrimaryTopicOf <http://www.w3.org/> ;
  foaf:name "W3C/ERCIM" ;
  foaf:page <http://www.w3.org/> ;
.
_:b421168
  rdf:type owl:Class ;
  <http://www.topbraid.org/c14n#true> "46"^^xsd:long ;
  owl:unionOf (
      nhr:NatuurlijkPersoon
      nhr:NietNatuurlijkPersoon
    ) ;
.
_:b421215
  rdf:type dcterms:Agent ;
  rdf:type foaf:Agent ;
  rdf:type _:b420951 ;
  rdf:type _:b421075 ;
  rdf:type _:b421664 ;
  rdf:type _:b421928 ;
  rdf:type _:b937877 ;
  rdf:type _:b938265 ;
  <http://www.topbraid.org/c14n#true> "52"^^xsd:long ;
  rdfs:label "Shuji Kamitsuna" ;
  owl:sameAs _:b421215 ;
  owl:sameAs _:b937583 ;
  owl:sameAs _:b938110 ;
  foaf:homepage <http://www.asahi-net.or.jp/~ax2s-kmtn/> ;
  foaf:isPrimaryTopicOf <http://www.asahi-net.or.jp/~ax2s-kmtn/> ;
  foaf:name "Shuji Kamitsuna" ;
  foaf:page <http://www.asahi-net.or.jp/~ax2s-kmtn/> ;
.
_:b421246
  rdf:type owl:Class ;
  <http://www.topbraid.org/c14n#true> "50"^^xsd:long ;
  owl:equivalentClass org:OrganizationalCollaboration ;
  owl:equivalentClass _:b937707 ;
  owl:equivalentClass _:b938296 ;
  owl:intersectionOf (
      org:Organization
      _:b421432
    ) ;
.
_:b421277
  rdf:type dcterms:Agent ;
  rdf:type foaf:Agent ;
  rdf:type _:b420951 ;
  rdf:type _:b421075 ;
  rdf:type _:b421664 ;
  rdf:type _:b421928 ;
  rdf:type _:b937877 ;
  rdf:type _:b938265 ;
  <http://www.topbraid.org/c14n#true> "56"^^xsd:long ;
  rdfs:label "María Poveda Villalón" ;
  owl:sameAs _:b421277 ;
  owl:sameAs _:b937486 ;
  owl:sameAs _:b937908 ;
  foaf:mbox "mpoveda@fi.upm.es" ;
  foaf:name "María Poveda Villalón" ;
.
_:b421308
  rdf:type dcterms:Agent ;
  rdf:type foaf:Agent ;
  rdf:type _:b420951 ;
  rdf:type _:b421075 ;
  rdf:type _:b421664 ;
  rdf:type _:b421928 ;
  rdf:type _:b937877 ;
  rdf:type _:b938265 ;
  <http://www.topbraid.org/c14n#true> "54"^^xsd:long ;
  rdfs:label "Dave Reynolds" ;
  owl:sameAs _:b421308 ;
  owl:sameAs _:b421401 ;
  owl:sameAs _:b421497 ;
  foaf:mbox "dave@epimorphics.com" ;
  foaf:name "Dave Reynolds" ;
.
_:b421339
  rdf:type dcterms:Agent ;
  rdf:type foaf:Agent ;
  rdf:type _:b420951 ;
  rdf:type _:b421075 ;
  rdf:type _:b421664 ;
  rdf:type _:b421928 ;
  rdf:type _:b937877 ;
  rdf:type _:b938265 ;
  <http://www.topbraid.org/c14n#true> "60"^^xsd:long ;
  rdfs:label "Giorgia Lodi" ;
  owl:sameAs _:b421339 ;
  owl:sameAs _:b937346 ;
  owl:sameAs _:b937408 ;
  foaf:mbox "giorgia.lodi@agid.gov.it" ;
  foaf:name "Giorgia Lodi" ;
.
_:b421370
  rdf:type owl:Class ;
  <http://www.topbraid.org/c14n#true> "58"^^xsd:long ;
  owl:unionOf (
      org:Membership
      org:Post
    ) ;
.
_:b421401
  rdf:type dcterms:Agent ;
  rdf:type foaf:Agent ;
  rdf:type _:b420951 ;
  rdf:type _:b421075 ;
  rdf:type _:b421664 ;
  rdf:type _:b421928 ;
  rdf:type _:b937877 ;
  rdf:type _:b938265 ;
  <http://www.topbraid.org/c14n#true> "64"^^xsd:long ;
  rdfs:label "Dave Reynolds" ;
  owl:sameAs _:b421308 ;
  owl:sameAs _:b421401 ;
  owl:sameAs _:b421497 ;
  foaf:mbox "dave@epimorphics.com" ;
  foaf:name "Dave Reynolds" ;
.
_:b421432
  rdf:type owl:Restriction ;
  <http://www.topbraid.org/c14n#true> "62"^^xsd:long ;
  owl:allValuesFrom org:Organization ;
  owl:equivalentClass _:b421742 ;
  owl:equivalentClass _:b937846 ;
  owl:onProperty org:hasMember ;
.
_:b421447
  rdf:type owl:Class ;
  <http://www.topbraid.org/c14n#true> "4"^^xsd:long ;
  owl:unionOf (
      nhr:NatuurlijkPersoon
      nhr:NietNatuurlijkPersoon
    ) ;
.
_:b421478
  <http://www.topbraid.org/c14n#true> "2"^^xsd:long ;
  rdfs:label "European Commission, Joint Research Centre " ;
  owl:sameAs _:b421478 ;
  owl:sameAs _:b937645 ;
  owl:sameAs _:b937815 ;
  owl:sameAs _:b938079 ;
  foaf:homepage <http://ies.jrc.ec.europa.eu/DE> ;
  foaf:isPrimaryTopicOf <http://ies.jrc.ec.europa.eu/DE> ;
  foaf:name "European Commission, Joint Research Centre " ;
  foaf:page <http://ies.jrc.ec.europa.eu/DE> ;
.
_:b421497
  rdf:type dcterms:Agent ;
  rdf:type foaf:Agent ;
  rdf:type _:b420951 ;
  rdf:type _:b421075 ;
  rdf:type _:b421664 ;
  rdf:type _:b421928 ;
  rdf:type _:b937877 ;
  rdf:type _:b938265 ;
  <http://www.topbraid.org/c14n#true> "0"^^xsd:long ;
  rdfs:label "Dave Reynolds" ;
  owl:sameAs _:b421308 ;
  owl:sameAs _:b421401 ;
  owl:sameAs _:b421497 ;
  foaf:mbox "dave@epimorphics.com" ;
  foaf:name "Dave Reynolds" ;
.
_:b421509
  rdf:type dcterms:Agent ;
  rdf:type foaf:Agent ;
  rdf:type _:b420951 ;
  rdf:type _:b421075 ;
  rdf:type _:b421664 ;
  rdf:type _:b421928 ;
  rdf:type _:b937877 ;
  rdf:type _:b938265 ;
  <http://www.topbraid.org/c14n#true> "8"^^xsd:long ;
  rdfs:label "Government Linked Data WG, based on output from the ADMS Working Group" ;
  foaf:made <http://www.w3.org/ns/adms> ;
  foaf:name "Government Linked Data WG, based on output from the ADMS Working Group" ;
  foaf:page <http://www.w3.org/2011/gld/> ;
.
_:b421540
  rdf:type dcterms:Agent ;
  rdf:type foaf:Agent ;
  rdf:type _:b420951 ;
  rdf:type _:b421075 ;
  rdf:type _:b421664 ;
  rdf:type _:b421928 ;
  rdf:type _:b937877 ;
  rdf:type _:b938265 ;
  <http://www.topbraid.org/c14n#true> "6"^^xsd:long ;
  rdfs:label "Guadalupe Aguado de Cea" ;
  owl:sameAs _:b421540 ;
  owl:sameAs _:b421633 ;
  owl:sameAs _:b421835 ;
  foaf:mbox "lupe@fi.upm.es" ;
  foaf:name "Guadalupe Aguado de Cea" ;
.
_:b421571
  rdf:type dcterms:Agent ;
  rdf:type foaf:Agent ;
  rdf:type _:b420951 ;
  rdf:type _:b421075 ;
  rdf:type _:b421664 ;
  rdf:type _:b421928 ;
  rdf:type _:b937877 ;
  rdf:type _:b938265 ;
  <http://www.topbraid.org/c14n#true> "12"^^xsd:long ;
  rdfs:label "Antonio Maccioni" ;
  owl:sameAs _:b421571 ;
  owl:sameAs _:b937672 ;
  owl:sameAs _:b938172 ;
  foaf:mbox "antonio.maccioni@agid.gov.it" ;
  foaf:name "Antonio Maccioni" ;
.
_:b421602
  rdf:type dcterms:Agent ;
  rdf:type foaf:Agent ;
  rdf:type _:b420951 ;
  rdf:type _:b421075 ;
  rdf:type _:b421664 ;
  rdf:type _:b421928 ;
  rdf:type _:b937877 ;
  rdf:type _:b938265 ;
  <http://www.topbraid.org/c14n#true> "10"^^xsd:long ;
  rdfs:label "Makx Dekkers" ;
  rdfs:seeAlso <http://makxdekkers.com/makxdekkers.rdf#me> ;
  owl:sameAs _:b421602 ;
  owl:sameAs _:b937939 ;
  owl:sameAs _:b938203 ;
  owl:sameAs _:b938246 ;
  foaf:homepage <http://makxdekkers.com/> ;
  foaf:isPrimaryTopicOf <http://makxdekkers.com/> ;
  foaf:made <http://www.w3.org/ns/adms> ;
  foaf:made <http://www.w3.org/ns/regorg> ;
  foaf:name "Makx Dekkers" ;
  foaf:page <http://makxdekkers.com/> ;
.
_:b421633
  rdf:type dcterms:Agent ;
  rdf:type foaf:Agent ;
  rdf:type _:b420951 ;
  rdf:type _:b421075 ;
  rdf:type _:b421664 ;
  rdf:type _:b421928 ;
  rdf:type _:b937877 ;
  rdf:type _:b938265 ;
  <http://www.topbraid.org/c14n#true> "16"^^xsd:long ;
  rdfs:label "Guadalupe Aguado de Cea" ;
  owl:sameAs _:b421540 ;
  owl:sameAs _:b421633 ;
  owl:sameAs _:b421835 ;
  foaf:mbox "lupe@fi.upm.es" ;
  foaf:name "Guadalupe Aguado de Cea" ;
.
_:b421664
  rdf:type owl:Class ;
  <http://www.topbraid.org/c14n#true> "14"^^xsd:long ;
  owl:unionOf (
      foaf:Agent
      org:Post
    ) ;
.
_:b421711
  <http://www.topbraid.org/c14n#true> "20"^^xsd:long ;
  rdfs:label "W3C/ERCIM" ;
  owl:sameAs _:b421137 ;
  owl:sameAs _:b421711 ;
  owl:sameAs _:b421804 ;
  foaf:homepage <http://www.w3.org/> ;
  foaf:isPrimaryTopicOf <http://www.w3.org/> ;
  foaf:name "W3C/ERCIM" ;
  foaf:page <http://www.w3.org/> ;
.
_:b421742
  rdf:type owl:Restriction ;
  <http://www.topbraid.org/c14n#true> "18"^^xsd:long ;
  owl:allValuesFrom org:Organization ;
  owl:equivalentClass _:b421432 ;
  owl:equivalentClass _:b937846 ;
  owl:onProperty org:hasMember ;
.
_:b421773
  rdf:type dcterms:Agent ;
  rdf:type foaf:Agent ;
  rdf:type _:b420951 ;
  rdf:type _:b421075 ;
  rdf:type _:b421664 ;
  rdf:type _:b421928 ;
  rdf:type _:b937877 ;
  rdf:type _:b938265 ;
  <http://www.topbraid.org/c14n#true> "24"^^xsd:long ;
  rdfs:label "Government Linked Data WG, based on output from the ADMS Working Group" ;
  foaf:made <http://www.w3.org/ns/adms> ;
  foaf:name "Government Linked Data WG, based on output from the ADMS Working Group" ;
  foaf:page <http://www.w3.org/2011/gld/> ;
.
_:b421804
  <http://www.topbraid.org/c14n#true> "22"^^xsd:long ;
  rdfs:label "W3C/ERCIM" ;
  owl:sameAs _:b421137 ;
  owl:sameAs _:b421711 ;
  owl:sameAs _:b421804 ;
  foaf:homepage <http://www.w3.org/> ;
  foaf:isPrimaryTopicOf <http://www.w3.org/> ;
  foaf:name "W3C/ERCIM" ;
  foaf:page <http://www.w3.org/> ;
.
_:b421835
  rdf:type dcterms:Agent ;
  rdf:type foaf:Agent ;
  rdf:type _:b420951 ;
  rdf:type _:b421075 ;
  rdf:type _:b421664 ;
  rdf:type _:b421928 ;
  rdf:type _:b937877 ;
  rdf:type _:b938265 ;
  <http://www.topbraid.org/c14n#true> "28"^^xsd:long ;
  rdfs:label "Guadalupe Aguado de Cea" ;
  owl:sameAs _:b421540 ;
  owl:sameAs _:b421633 ;
  owl:sameAs _:b421835 ;
  foaf:mbox "lupe@fi.upm.es" ;
  foaf:name "Guadalupe Aguado de Cea" ;
.
_:b421866
  rdf:type dcterms:Agent ;
  rdf:type foaf:Agent ;
  rdf:type _:b420951 ;
  rdf:type _:b421075 ;
  rdf:type _:b421664 ;
  rdf:type _:b421928 ;
  rdf:type _:b937877 ;
  rdf:type _:b938265 ;
  schema:affiliation <http://www.w3.org/data#W3C> ;
  schema:affiliation _:b421137 ;
  schema:affiliation _:b421711 ;
  schema:affiliation _:b421804 ;
  <http://www.topbraid.org/c14n#true> "26"^^xsd:long ;
  rdfs:label "Phil Archer" ;
  rdfs:seeAlso <http://philarcher.org/foaf.rdf#me> ;
  owl:sameAs _:b421866 ;
  owl:sameAs _:b421897 ;
  owl:sameAs _:b937319 ;
  owl:sameAs _:b937970 ;
  foaf:homepage <http://www.w3.org/People/all#phila> ;
  foaf:isPrimaryTopicOf <http://www.w3.org/People/all#phila> ;
  foaf:made <http://www.w3.org/ns/adms> ;
  foaf:made <http://www.w3.org/ns/regorg> ;
  foaf:name "Phil Archer" ;
  foaf:page <http://www.w3.org/People/all#phila> ;
.
_:b421897
  rdf:type dcterms:Agent ;
  rdf:type foaf:Agent ;
  rdf:type _:b420951 ;
  rdf:type _:b421075 ;
  rdf:type _:b421664 ;
  rdf:type _:b421928 ;
  rdf:type _:b937877 ;
  rdf:type _:b938265 ;
  schema:affiliation <http://www.w3.org/data#W3C> ;
  schema:affiliation _:b421137 ;
  schema:affiliation _:b421711 ;
  schema:affiliation _:b421804 ;
  <http://www.topbraid.org/c14n#true> "32"^^xsd:long ;
  rdfs:label "Phil Archer" ;
  rdfs:seeAlso <http://philarcher.org/foaf.rdf#me> ;
  owl:sameAs _:b421866 ;
  owl:sameAs _:b421897 ;
  owl:sameAs _:b937319 ;
  owl:sameAs _:b937970 ;
  foaf:homepage <http://www.w3.org/People/all#phila> ;
  foaf:isPrimaryTopicOf <http://www.w3.org/People/all#phila> ;
  foaf:made <http://www.w3.org/ns/adms> ;
  foaf:made <http://www.w3.org/ns/regorg> ;
  foaf:name "Phil Archer" ;
  foaf:page <http://www.w3.org/People/all#phila> ;
.
_:b421928
  rdf:type owl:Class ;
  <http://www.topbraid.org/c14n#true> "30"^^xsd:long ;
  owl:unionOf (
      foaf:Agent
      org:Post
    ) ;
.
_:b454254
  rdf:type owl:Restriction ;
  owl:onProperty toop:hasMainSite ;
  owl:someValuesFrom toop:MainSite ;
.
_:b481819
  rdf:type owl:Restriction ;
  owl:minCardinality "1"^^xsd:nonNegativeInteger ;
  owl:onProperty skosxl:literalForm ;
.
_:b499218
  rdf:type owl:Restriction ;
  owl:onProperty vcard:region ;
  owl:someValuesFrom rdfs:Literal ;
.
_:b541374
  rdf:type owl:Class ;
  owl:unionOf (
      vcard:Address
      vcard:Label
    ) ;
.
_:b546250
  rdf:type owl:Restriction ;
  owl:cardinality "1"^^xsd:nonNegativeInteger ;
  owl:onProperty nhr:geslachtsnaam ;
.
_:b568769
  rdf:type owl:Class ;
  owl:equivalentClass vcard:Name ;
  owl:unionOf (
      [
        rdf:type owl:Class ;
        owl:intersectionOf (
            [
              rdf:type owl:Restriction ;
              owl:onProperty vcard:additional-name ;
              owl:someValuesFrom xsd:string ;
            ]
            [
              rdf:type owl:Restriction ;
              owl:minCardinality "0"^^xsd:nonNegativeInteger ;
              owl:onProperty vcard:additional-name ;
            ]
          ) ;
      ]
      [
        rdf:type owl:Class ;
        owl:intersectionOf (
            [
              rdf:type owl:Restriction ;
              owl:onProperty vcard:family-name ;
              owl:someValuesFrom xsd:string ;
            ]
            [
              rdf:type owl:Restriction ;
              owl:maxCardinality "1"^^xsd:nonNegativeInteger ;
              owl:onProperty vcard:family-name ;
            ]
          ) ;
      ]
      [
        rdf:type owl:Class ;
        owl:intersectionOf (
            [
              rdf:type owl:Restriction ;
              owl:onProperty vcard:given-name ;
              owl:someValuesFrom xsd:string ;
            ]
            [
              rdf:type owl:Restriction ;
              owl:maxCardinality "1"^^xsd:nonNegativeInteger ;
              owl:onProperty vcard:given-name ;
            ]
          ) ;
      ]
      [
        rdf:type owl:Class ;
        owl:intersectionOf (
            [
              rdf:type owl:Restriction ;
              owl:onProperty vcard:honorific-prefix ;
              owl:someValuesFrom xsd:string ;
            ]
            [
              rdf:type owl:Restriction ;
              owl:minCardinality "0"^^xsd:nonNegativeInteger ;
              owl:onProperty vcard:honorific-prefix ;
            ]
          ) ;
      ]
      [
        rdf:type owl:Class ;
        owl:intersectionOf (
            [
              rdf:type owl:Restriction ;
              owl:onProperty vcard:honorific-suffix ;
              owl:someValuesFrom xsd:string ;
            ]
            [
              rdf:type owl:Restriction ;
              owl:minCardinality "0"^^xsd:nonNegativeInteger ;
              owl:onProperty vcard:honorific-suffix ;
            ]
          ) ;
      ]
    ) ;
.
_:b583853
  rdf:type owl:Class ;
  owl:unionOf (
      vcard:Address
      vcard:Email
      vcard:Label
      vcard:Tel
    ) ;
.
_:b593574
  rdf:type owl:Restriction ;
  owl:cardinality "1"^^xsd:nonNegativeInteger ;
  owl:onProperty nhr:postcode ;
.
_:b594637
  rdf:type owl:Class ;
  owl:unionOf (
      prov:Association
      prov:InstantaneousEvent
    ) ;
.
_:b623638
  rdf:type owl:Restriction ;
  owl:onProperty vcard:given-name ;
  owl:someValuesFrom rdfs:Literal ;
.
_:b627138
  rdf:type owl:Restriction ;
  owl:cardinality "1"^^xsd:nonNegativeInteger ;
  owl:onProperty nhr:naamDomeinnaam ;
.
_:b642226
  rdf:type owl:Class ;
  owl:unionOf (
      nhr:NatuurlijkPersoon
      nhr:NietNatuurlijkPersoon
    ) ;
.
_:b652026
  rdf:type owl:Class ;
  owl:unionOf (
      vcard:Address
      vcard:Email
      vcard:Label
      vcard:Tel
    ) ;
.
_:b671381
  rdf:type rdfs:Datatype ;
  owl:unionOf (
      xsd:dateTime
      xsd:gYear
    ) ;
.
_:b671776
  rdf:type owl:Restriction ;
  owl:onProperty vcard:family-name ;
  owl:someValuesFrom rdfs:Literal ;
.
_:b705303
  rdf:type owl:Restriction ;
  owl:maxCardinality "0"^^xsd:nonNegativeInteger ;
  owl:onProperty prov:hadActivity ;
.
_:b715640
  rdf:type owl:Class ;
  owl:unionOf (
      prov:Activity
      prov:Agent
      prov:Entity
    ) ;
.
_:b719479
  rdf:type rdfs:Datatype ;
  owl:unionOf (
      xsd:dateTime
      xsd:dateTimeStamp
      xsd:gYear
    ) ;
.
_:b726818
  rdf:type owl:Restriction ;
  owl:onProperty vcard:postal-code ;
  owl:someValuesFrom rdfs:Literal ;
.
_:b757317
  rdf:type owl:Restriction ;
  owl:onProperty vcard:organization-unit ;
  owl:someValuesFrom rdfs:Literal ;
.
_:b763315
  rdf:type owl:Class ;
  owl:unionOf (
      vcard:Address
      vcard:Label
      vcard:Tel
    ) ;
.
_:b767375
  rdf:type owl:Restriction ;
  owl:cardinality "1"^^xsd:nonNegativeInteger ;
  owl:onProperty nhr:soortCommunicatienummer ;
.
_:b770826
  rdf:type owl:Restriction ;
  owl:cardinality "1"^^xsd:nonNegativeInteger ;
  owl:onProperty nhr:nummerCommunicatienummer ;
.
_:b772676
  rdf:type owl:Restriction ;
  owl:onDataRange elobr:EloniaBusinessCode ;
  owl:onProperty elobr:hasBusinessCode ;
  owl:qualifiedCardinality "1"^^xsd:nonNegativeInteger ;
.
_:b780263
  rdf:type owl:Restriction ;
  owl:onProperty vcard:hasMember ;
  owl:someValuesFrom vcard:Kind ;
.
_:b787338
  rdf:type owl:Restriction ;
  owl:onProperty vcard:locality ;
  owl:someValuesFrom rdfs:Literal ;
.
_:b789349
  rdf:type owl:Class ;
  owl:equivalentClass vcard:Group ;
  owl:intersectionOf (
      _:b780263
      _:b29166
    ) ;
.
_:b794039
  rdf:type owl:Restriction ;
  owl:onProperty vcard:honorific-prefix ;
  owl:someValuesFrom rdfs:Literal ;
.
_:b809403
  rdf:type owl:Restriction ;
  owl:onDataRange _:b642226 ;
  owl:onProperty nhr:isActiviteitVan ;
  owl:qualifiedCardinality "1"^^xsd:nonNegativeInteger ;
.
_:b813138
  rdf:type owl:Restriction ;
  owl:cardinality "1"^^xsd:nonNegativeInteger ;
  owl:onProperty nhr:adresEmailAdres ;
.
_:b826282
  rdf:type owl:Restriction ;
  owl:onProperty toop:hasCompanyCode ;
  owl:someValuesFrom toop:CompanyCode ;
.
_:b826680
  rdf:type owl:Restriction ;
  owl:cardinality "1"^^xsd:nonNegativeInteger ;
  owl:onProperty toop:companyType ;
.
_:b839515
  rdf:type owl:Restriction ;
  owl:cardinality "1"^^xsd:nonNegativeInteger ;
  owl:onProperty nhr:geboortedatum ;
.
_:b875853
  rdf:type owl:Restriction ;
  owl:onProperty skos:inScheme ;
  owl:someValuesFrom toop:CompanyTypeScheme ;
.
_:b883411
  rdf:type owl:Restriction ;
  owl:onDataRange freebr:FreedoniaBusinessCode ;
  owl:onProperty freebr:hasBusinessCode ;
  owl:qualifiedCardinality "1"^^xsd:nonNegativeInteger ;
.
_:b895567
  rdf:type owl:Class ;
  owl:unionOf (
      prov:Activity
      prov:Agent
      prov:Entity
    ) ;
.
_:b897711
  rdf:type owl:Class ;
  owl:unionOf (
      prov:Activity
      prov:Agent
      prov:Entity
      prov:InstantaneousEvent
    ) ;
.
_:b918886
  rdf:type owl:Restriction ;
  owl:cardinality "1"^^xsd:nonNegativeInteger ;
  owl:onProperty nhr:straatHuisnummer ;
.
_:b926654
  rdf:type owl:Restriction ;
  owl:onProperty vcard:post-office-box ;
  owl:someValuesFrom rdfs:Literal ;
.
_:b937284
  rdf:type dcterms:Agent ;
  rdf:type foaf:Agent ;
  rdf:type _:b420951 ;
  rdf:type _:b421075 ;
  rdf:type _:b421664 ;
  rdf:type _:b421928 ;
  rdf:type _:b937877 ;
  rdf:type _:b938265 ;
  <http://www.topbraid.org/c14n#true> "37"^^xsd:long ;
  rdfs:label "Elena Montiel Ponsoda" ;
  owl:sameAs _:b421106 ;
  owl:sameAs _:b937284 ;
  owl:sameAs _:b938001 ;
  foaf:mbox "emontiel@fi.upm.es" ;
  foaf:name "Elena Montiel Ponsoda" ;
.
_:b937319
  rdf:type dcterms:Agent ;
  rdf:type foaf:Agent ;
  rdf:type _:b420951 ;
  rdf:type _:b421075 ;
  rdf:type _:b421664 ;
  rdf:type _:b421928 ;
  rdf:type _:b937877 ;
  rdf:type _:b938265 ;
  schema:affiliation <http://www.w3.org/data#W3C> ;
  schema:affiliation _:b421137 ;
  schema:affiliation _:b421711 ;
  schema:affiliation _:b421804 ;
  <http://www.topbraid.org/c14n#true> "35"^^xsd:long ;
  rdfs:label "Phil Archer" ;
  rdfs:seeAlso <http://philarcher.org/foaf.rdf#me> ;
  owl:sameAs _:b421866 ;
  owl:sameAs _:b421897 ;
  owl:sameAs _:b937319 ;
  owl:sameAs _:b937970 ;
  foaf:homepage <http://www.w3.org/People/all#phila> ;
  foaf:isPrimaryTopicOf <http://www.w3.org/People/all#phila> ;
  foaf:made <http://www.w3.org/ns/adms> ;
  foaf:made <http://www.w3.org/ns/regorg> ;
  foaf:name "Phil Archer" ;
  foaf:page <http://www.w3.org/People/all#phila> ;
.
_:b937346
  rdf:type dcterms:Agent ;
  rdf:type foaf:Agent ;
  rdf:type _:b420951 ;
  rdf:type _:b421075 ;
  rdf:type _:b421664 ;
  rdf:type _:b421928 ;
  rdf:type _:b937877 ;
  rdf:type _:b938265 ;
  <http://www.topbraid.org/c14n#true> "41"^^xsd:long ;
  rdfs:label "Giorgia Lodi" ;
  owl:sameAs _:b421339 ;
  owl:sameAs _:b937346 ;
  owl:sameAs _:b937408 ;
  foaf:mbox "giorgia.lodi@agid.gov.it" ;
  foaf:name "Giorgia Lodi" ;
.
_:b937381
  rdf:type dcterms:Agent ;
  rdf:type foaf:Agent ;
  rdf:type _:b420951 ;
  rdf:type _:b421075 ;
  rdf:type _:b421664 ;
  rdf:type _:b421928 ;
  rdf:type _:b937877 ;
  rdf:type _:b938265 ;
  schema:affiliation _:b421478 ;
  schema:affiliation _:b937645 ;
  schema:affiliation _:b937815 ;
  schema:affiliation _:b938079 ;
  <http://www.topbraid.org/c14n#true> "39"^^xsd:long ;
  rdfs:label "Andrea Perego" ;
  rdfs:seeAlso <http://andrea-perego.name/foaf/#me> ;
  owl:sameAs _:b937381 ;
  owl:sameAs _:b937505 ;
  owl:sameAs _:b937610 ;
  owl:sameAs _:b938234 ;
  foaf:homepage <http://andrea-perego.name/> ;
  foaf:isPrimaryTopicOf <http://andrea-perego.name/> ;
  foaf:made <http://www.w3.org/ns/adms> ;
  foaf:made <http://www.w3.org/ns/regorg> ;
  foaf:name "Andrea Perego" ;
  foaf:page <http://andrea-perego.name/> ;
.
_:b937408
  rdf:type dcterms:Agent ;
  rdf:type foaf:Agent ;
  rdf:type _:b420951 ;
  rdf:type _:b421075 ;
  rdf:type _:b421664 ;
  rdf:type _:b421928 ;
  rdf:type _:b937877 ;
  rdf:type _:b938265 ;
  <http://www.topbraid.org/c14n#true> "45"^^xsd:long ;
  rdfs:label "Giorgia Lodi" ;
  owl:sameAs _:b421339 ;
  owl:sameAs _:b937346 ;
  owl:sameAs _:b937408 ;
  foaf:mbox "giorgia.lodi@agid.gov.it" ;
  foaf:name "Giorgia Lodi" ;
.
_:b937443
  rdf:type owl:Class ;
  <http://www.topbraid.org/c14n#true> "43"^^xsd:long ;
  owl:unionOf (
      org:Membership
      org:Post
    ) ;
.
_:b937486
  rdf:type dcterms:Agent ;
  rdf:type foaf:Agent ;
  rdf:type _:b420951 ;
  rdf:type _:b421075 ;
  rdf:type _:b421664 ;
  rdf:type _:b421928 ;
  rdf:type _:b937877 ;
  rdf:type _:b938265 ;
  <http://www.topbraid.org/c14n#true> "49"^^xsd:long ;
  rdfs:label "María Poveda Villalón" ;
  owl:sameAs _:b421277 ;
  owl:sameAs _:b937486 ;
  owl:sameAs _:b937908 ;
  foaf:mbox "mpoveda@fi.upm.es" ;
  foaf:name "María Poveda Villalón" ;
.
_:b937505
  rdf:type dcterms:Agent ;
  rdf:type foaf:Agent ;
  rdf:type _:b420951 ;
  rdf:type _:b421075 ;
  rdf:type _:b421664 ;
  rdf:type _:b421928 ;
  rdf:type _:b937877 ;
  rdf:type _:b938265 ;
  schema:affiliation _:b421478 ;
  schema:affiliation _:b937645 ;
  schema:affiliation _:b937815 ;
  schema:affiliation _:b938079 ;
  <http://www.topbraid.org/c14n#true> "47"^^xsd:long ;
  rdfs:label "Andrea Perego" ;
  rdfs:seeAlso <http://andrea-perego.name/foaf/#me> ;
  owl:sameAs _:b937381 ;
  owl:sameAs _:b937505 ;
  owl:sameAs _:b937610 ;
  owl:sameAs _:b938234 ;
  foaf:homepage <http://andrea-perego.name/> ;
  foaf:isPrimaryTopicOf <http://andrea-perego.name/> ;
  foaf:made <http://www.w3.org/ns/adms> ;
  foaf:made <http://www.w3.org/ns/regorg> ;
  foaf:name "Andrea Perego" ;
  foaf:page <http://andrea-perego.name/> ;
.
_:b937548
  rdf:type dcterms:Agent ;
  rdf:type foaf:Agent ;
  rdf:type _:b420951 ;
  rdf:type _:b421075 ;
  rdf:type _:b421664 ;
  rdf:type _:b421928 ;
  rdf:type _:b937877 ;
  rdf:type _:b938265 ;
  <http://www.topbraid.org/c14n#true> "53"^^xsd:long ;
  rdfs:label "Dominique Guardiola" ;
  owl:sameAs _:b421013 ;
  owl:sameAs _:b937548 ;
  owl:sameAs _:b937769 ;
  foaf:mbox "dguardiola@quinode.fr" ;
  foaf:name "Dominique Guardiola" ;
.
_:b937583
  rdf:type dcterms:Agent ;
  rdf:type foaf:Agent ;
  rdf:type _:b420951 ;
  rdf:type _:b421075 ;
  rdf:type _:b421664 ;
  rdf:type _:b421928 ;
  rdf:type _:b937877 ;
  rdf:type _:b938265 ;
  <http://www.topbraid.org/c14n#true> "51"^^xsd:long ;
  rdfs:label "Shuji Kamitsuna" ;
  owl:sameAs _:b421215 ;
  owl:sameAs _:b937583 ;
  owl:sameAs _:b938110 ;
  foaf:homepage <http://www.asahi-net.or.jp/~ax2s-kmtn/> ;
  foaf:isPrimaryTopicOf <http://www.asahi-net.or.jp/~ax2s-kmtn/> ;
  foaf:name "Shuji Kamitsuna" ;
  foaf:page <http://www.asahi-net.or.jp/~ax2s-kmtn/> ;
.
_:b937610
  rdf:type dcterms:Agent ;
  rdf:type foaf:Agent ;
  rdf:type _:b420951 ;
  rdf:type _:b421075 ;
  rdf:type _:b421664 ;
  rdf:type _:b421928 ;
  rdf:type _:b937877 ;
  rdf:type _:b938265 ;
  schema:affiliation _:b421478 ;
  schema:affiliation _:b937645 ;
  schema:affiliation _:b937815 ;
  schema:affiliation _:b938079 ;
  <http://www.topbraid.org/c14n#true> "57"^^xsd:long ;
  rdfs:label "Andrea Perego" ;
  rdfs:seeAlso <http://andrea-perego.name/foaf/#me> ;
  owl:sameAs _:b937381 ;
  owl:sameAs _:b937505 ;
  owl:sameAs _:b937610 ;
  owl:sameAs _:b938234 ;
  foaf:homepage <http://andrea-perego.name/> ;
  foaf:isPrimaryTopicOf <http://andrea-perego.name/> ;
  foaf:made <http://www.w3.org/ns/adms> ;
  foaf:made <http://www.w3.org/ns/regorg> ;
  foaf:name "Andrea Perego" ;
  foaf:page <http://andrea-perego.name/> ;
.
_:b937645
  <http://www.topbraid.org/c14n#true> "55"^^xsd:long ;
  rdfs:label "European Commission, Joint Research Centre " ;
  owl:sameAs _:b421478 ;
  owl:sameAs _:b937645 ;
  owl:sameAs _:b937815 ;
  owl:sameAs _:b938079 ;
  foaf:homepage <http://ies.jrc.ec.europa.eu/DE> ;
  foaf:isPrimaryTopicOf <http://ies.jrc.ec.europa.eu/DE> ;
  foaf:name "European Commission, Joint Research Centre " ;
  foaf:page <http://ies.jrc.ec.europa.eu/DE> ;
.
_:b937672
  rdf:type dcterms:Agent ;
  rdf:type foaf:Agent ;
  rdf:type _:b420951 ;
  rdf:type _:b421075 ;
  rdf:type _:b421664 ;
  rdf:type _:b421928 ;
  rdf:type _:b937877 ;
  rdf:type _:b938265 ;
  <http://www.topbraid.org/c14n#true> "61"^^xsd:long ;
  rdfs:label "Antonio Maccioni" ;
  owl:sameAs _:b421571 ;
  owl:sameAs _:b937672 ;
  owl:sameAs _:b938172 ;
  foaf:mbox "antonio.maccioni@agid.gov.it" ;
  foaf:name "Antonio Maccioni" ;
.
_:b937707
  rdf:type owl:Class ;
  <http://www.topbraid.org/c14n#true> "59"^^xsd:long ;
  owl:equivalentClass org:OrganizationalCollaboration ;
  owl:equivalentClass _:b421246 ;
  owl:equivalentClass _:b938296 ;
  owl:intersectionOf (
      org:Organization
      _:b421742
    ) ;
.
_:b937769
  rdf:type dcterms:Agent ;
  rdf:type foaf:Agent ;
  rdf:type _:b420951 ;
  rdf:type _:b421075 ;
  rdf:type _:b421664 ;
  rdf:type _:b421928 ;
  rdf:type _:b937877 ;
  rdf:type _:b938265 ;
  <http://www.topbraid.org/c14n#true> "63"^^xsd:long ;
  rdfs:label "Dominique Guardiola" ;
  owl:sameAs _:b421013 ;
  owl:sameAs _:b937548 ;
  owl:sameAs _:b937769 ;
  foaf:mbox "dguardiola@quinode.fr" ;
  foaf:name "Dominique Guardiola" ;
.
_:b937815
  <http://www.topbraid.org/c14n#true> "3"^^xsd:long ;
  rdfs:label "European Commission, Joint Research Centre " ;
  owl:sameAs _:b421478 ;
  owl:sameAs _:b937645 ;
  owl:sameAs _:b937815 ;
  owl:sameAs _:b938079 ;
  foaf:homepage <http://ies.jrc.ec.europa.eu/DE> ;
  foaf:isPrimaryTopicOf <http://ies.jrc.ec.europa.eu/DE> ;
  foaf:name "European Commission, Joint Research Centre " ;
  foaf:page <http://ies.jrc.ec.europa.eu/DE> ;
.
_:b937846
  rdf:type owl:Restriction ;
  <http://www.topbraid.org/c14n#true> "1"^^xsd:long ;
  owl:allValuesFrom org:Organization ;
  owl:equivalentClass _:b421432 ;
  owl:equivalentClass _:b421742 ;
  owl:onProperty org:hasMember ;
.
_:b937877
  rdf:type owl:Class ;
  <http://www.topbraid.org/c14n#true> "7"^^xsd:long ;
  owl:unionOf (
      foaf:Agent
      org:Post
    ) ;
.
_:b937908
  rdf:type dcterms:Agent ;
  rdf:type foaf:Agent ;
  rdf:type _:b420951 ;
  rdf:type _:b421075 ;
  rdf:type _:b421664 ;
  rdf:type _:b421928 ;
  rdf:type _:b937877 ;
  rdf:type _:b938265 ;
  <http://www.topbraid.org/c14n#true> "5"^^xsd:long ;
  rdfs:label "María Poveda Villalón" ;
  owl:sameAs _:b421277 ;
  owl:sameAs _:b937486 ;
  owl:sameAs _:b937908 ;
  foaf:mbox "mpoveda@fi.upm.es" ;
  foaf:name "María Poveda Villalón" ;
.
_:b937939
  rdf:type dcterms:Agent ;
  rdf:type foaf:Agent ;
  rdf:type _:b420951 ;
  rdf:type _:b421075 ;
  rdf:type _:b421664 ;
  rdf:type _:b421928 ;
  rdf:type _:b937877 ;
  rdf:type _:b938265 ;
  <http://www.topbraid.org/c14n#true> "11"^^xsd:long ;
  rdfs:label "Makx Dekkers" ;
  rdfs:seeAlso <http://makxdekkers.com/makxdekkers.rdf#me> ;
  owl:sameAs _:b421602 ;
  owl:sameAs _:b937939 ;
  owl:sameAs _:b938203 ;
  owl:sameAs _:b938246 ;
  foaf:homepage <http://makxdekkers.com/> ;
  foaf:isPrimaryTopicOf <http://makxdekkers.com/> ;
  foaf:made <http://www.w3.org/ns/adms> ;
  foaf:made <http://www.w3.org/ns/regorg> ;
  foaf:name "Makx Dekkers" ;
  foaf:page <http://makxdekkers.com/> ;
.
_:b937970
  rdf:type dcterms:Agent ;
  rdf:type foaf:Agent ;
  rdf:type _:b420951 ;
  rdf:type _:b421075 ;
  rdf:type _:b421664 ;
  rdf:type _:b421928 ;
  rdf:type _:b937877 ;
  rdf:type _:b938265 ;
  schema:affiliation <http://www.w3.org/data#W3C> ;
  schema:affiliation _:b421137 ;
  schema:affiliation _:b421711 ;
  schema:affiliation _:b421804 ;
  <http://www.topbraid.org/c14n#true> "9"^^xsd:long ;
  rdfs:label "Phil Archer" ;
  rdfs:seeAlso <http://philarcher.org/foaf.rdf#me> ;
  owl:sameAs _:b421866 ;
  owl:sameAs _:b421897 ;
  owl:sameAs _:b937319 ;
  owl:sameAs _:b937970 ;
  foaf:homepage <http://www.w3.org/People/all#phila> ;
  foaf:isPrimaryTopicOf <http://www.w3.org/People/all#phila> ;
  foaf:made <http://www.w3.org/ns/adms> ;
  foaf:made <http://www.w3.org/ns/regorg> ;
  foaf:name "Phil Archer" ;
  foaf:page <http://www.w3.org/People/all#phila> ;
.
_:b938001
  rdf:type dcterms:Agent ;
  rdf:type foaf:Agent ;
  rdf:type _:b420951 ;
  rdf:type _:b421075 ;
  rdf:type _:b421664 ;
  rdf:type _:b421928 ;
  rdf:type _:b937877 ;
  rdf:type _:b938265 ;
  <http://www.topbraid.org/c14n#true> "15"^^xsd:long ;
  rdfs:label "Elena Montiel Ponsoda" ;
  owl:sameAs _:b421106 ;
  owl:sameAs _:b937284 ;
  owl:sameAs _:b938001 ;
  foaf:mbox "emontiel@fi.upm.es" ;
  foaf:name "Elena Montiel Ponsoda" ;
.
_:b938032
  rdf:type dcterms:Agent ;
  rdf:type foaf:Agent ;
  rdf:type _:b420951 ;
  rdf:type _:b421075 ;
  rdf:type _:b421664 ;
  rdf:type _:b421928 ;
  rdf:type _:b937877 ;
  rdf:type _:b938265 ;
  <http://www.topbraid.org/c14n#true> "13"^^xsd:long ;
  rdfs:label "Olga Ximena Giraldo" ;
  owl:sameAs _:b421044 ;
  owl:sameAs _:b938032 ;
  owl:sameAs _:b938141 ;
  foaf:mbox "ogiraldo@fi.upm.es" ;
  foaf:name "Olga Ximena Giraldo" ;
.
_:b938079
  <http://www.topbraid.org/c14n#true> "19"^^xsd:long ;
  rdfs:label "European Commission, Joint Research Centre " ;
  owl:sameAs _:b421478 ;
  owl:sameAs _:b937645 ;
  owl:sameAs _:b937815 ;
  owl:sameAs _:b938079 ;
  foaf:homepage <http://ies.jrc.ec.europa.eu/DE> ;
  foaf:isPrimaryTopicOf <http://ies.jrc.ec.europa.eu/DE> ;
  foaf:name "European Commission, Joint Research Centre " ;
  foaf:page <http://ies.jrc.ec.europa.eu/DE> ;
.
_:b938110
  rdf:type dcterms:Agent ;
  rdf:type foaf:Agent ;
  rdf:type _:b420951 ;
  rdf:type _:b421075 ;
  rdf:type _:b421664 ;
  rdf:type _:b421928 ;
  rdf:type _:b937877 ;
  rdf:type _:b938265 ;
  <http://www.topbraid.org/c14n#true> "17"^^xsd:long ;
  rdfs:label "Shuji Kamitsuna" ;
  owl:sameAs _:b421215 ;
  owl:sameAs _:b937583 ;
  owl:sameAs _:b938110 ;
  foaf:homepage <http://www.asahi-net.or.jp/~ax2s-kmtn/> ;
  foaf:isPrimaryTopicOf <http://www.asahi-net.or.jp/~ax2s-kmtn/> ;
  foaf:name "Shuji Kamitsuna" ;
  foaf:page <http://www.asahi-net.or.jp/~ax2s-kmtn/> ;
.
_:b938141
  rdf:type dcterms:Agent ;
  rdf:type foaf:Agent ;
  rdf:type _:b420951 ;
  rdf:type _:b421075 ;
  rdf:type _:b421664 ;
  rdf:type _:b421928 ;
  rdf:type _:b937877 ;
  rdf:type _:b938265 ;
  <http://www.topbraid.org/c14n#true> "23"^^xsd:long ;
  rdfs:label "Olga Ximena Giraldo" ;
  owl:sameAs _:b421044 ;
  owl:sameAs _:b938032 ;
  owl:sameAs _:b938141 ;
  foaf:mbox "ogiraldo@fi.upm.es" ;
  foaf:name "Olga Ximena Giraldo" ;
.
_:b938172
  rdf:type dcterms:Agent ;
  rdf:type foaf:Agent ;
  rdf:type _:b420951 ;
  rdf:type _:b421075 ;
  rdf:type _:b421664 ;
  rdf:type _:b421928 ;
  rdf:type _:b937877 ;
  rdf:type _:b938265 ;
  <http://www.topbraid.org/c14n#true> "21"^^xsd:long ;
  rdfs:label "Antonio Maccioni" ;
  owl:sameAs _:b421571 ;
  owl:sameAs _:b937672 ;
  owl:sameAs _:b938172 ;
  foaf:mbox "antonio.maccioni@agid.gov.it" ;
  foaf:name "Antonio Maccioni" ;
.
_:b938203
  rdf:type dcterms:Agent ;
  rdf:type foaf:Agent ;
  rdf:type _:b420951 ;
  rdf:type _:b421075 ;
  rdf:type _:b421664 ;
  rdf:type _:b421928 ;
  rdf:type _:b937877 ;
  rdf:type _:b938265 ;
  <http://www.topbraid.org/c14n#true> "27"^^xsd:long ;
  rdfs:label "Makx Dekkers" ;
  rdfs:seeAlso <http://makxdekkers.com/makxdekkers.rdf#me> ;
  owl:sameAs _:b421602 ;
  owl:sameAs _:b937939 ;
  owl:sameAs _:b938203 ;
  owl:sameAs _:b938246 ;
  foaf:homepage <http://makxdekkers.com/> ;
  foaf:isPrimaryTopicOf <http://makxdekkers.com/> ;
  foaf:made <http://www.w3.org/ns/adms> ;
  foaf:made <http://www.w3.org/ns/regorg> ;
  foaf:name "Makx Dekkers" ;
  foaf:page <http://makxdekkers.com/> ;
.
_:b938234
  rdf:type dcterms:Agent ;
  rdf:type foaf:Agent ;
  rdf:type _:b420951 ;
  rdf:type _:b421075 ;
  rdf:type _:b421664 ;
  rdf:type _:b421928 ;
  rdf:type _:b937877 ;
  rdf:type _:b938265 ;
  schema:affiliation _:b421478 ;
  schema:affiliation _:b937645 ;
  schema:affiliation _:b937815 ;
  schema:affiliation _:b938079 ;
  <http://www.topbraid.org/c14n#true> "25"^^xsd:long ;
  rdfs:label "Andrea Perego" ;
  rdfs:seeAlso <http://andrea-perego.name/foaf/#me> ;
  owl:sameAs _:b937381 ;
  owl:sameAs _:b937505 ;
  owl:sameAs _:b937610 ;
  owl:sameAs _:b938234 ;
  foaf:homepage <http://andrea-perego.name/> ;
  foaf:isPrimaryTopicOf <http://andrea-perego.name/> ;
  foaf:made <http://www.w3.org/ns/adms> ;
  foaf:made <http://www.w3.org/ns/regorg> ;
  foaf:name "Andrea Perego" ;
  foaf:page <http://andrea-perego.name/> ;
.
_:b938246
  rdf:type dcterms:Agent ;
  rdf:type foaf:Agent ;
  rdf:type _:b420951 ;
  rdf:type _:b421075 ;
  rdf:type _:b421664 ;
  rdf:type _:b421928 ;
  rdf:type _:b937877 ;
  rdf:type _:b938265 ;
  <http://www.topbraid.org/c14n#true> "33"^^xsd:long ;
  rdfs:label "Makx Dekkers" ;
  rdfs:seeAlso <http://makxdekkers.com/makxdekkers.rdf#me> ;
  owl:sameAs _:b421602 ;
  owl:sameAs _:b937939 ;
  owl:sameAs _:b938203 ;
  owl:sameAs _:b938246 ;
  foaf:homepage <http://makxdekkers.com/> ;
  foaf:isPrimaryTopicOf <http://makxdekkers.com/> ;
  foaf:made <http://www.w3.org/ns/adms> ;
  foaf:made <http://www.w3.org/ns/regorg> ;
  foaf:name "Makx Dekkers" ;
  foaf:page <http://makxdekkers.com/> ;
.
_:b938265
  rdf:type owl:Class ;
  <http://www.topbraid.org/c14n#true> "31"^^xsd:long ;
  owl:unionOf (
      foaf:Agent
      org:Post
    ) ;
.
_:b938296
  rdf:type owl:Class ;
  <http://www.topbraid.org/c14n#true> "29"^^xsd:long ;
  owl:equivalentClass org:OrganizationalCollaboration ;
  owl:equivalentClass _:b421246 ;
  owl:equivalentClass _:b937707 ;
  owl:intersectionOf (
      org:Organization
      _:b937846
    ) ;
.
_:b938985
  rdf:type owl:Restriction ;
  owl:onProperty vcard:organization-name ;
  owl:someValuesFrom rdfs:Literal ;
.
_:b955705
  rdf:type owl:Class ;
  owl:unionOf (
      vcard:Address
      vcard:Label
    ) ;
.
[
  rdf:type owl:Axiom ;
  rdfs:comment "A collection is an entity that provides a structure to some constituents, which are themselves entities. These constituents are said to be member of the collections."@en ;
  rdfs:seeAlso "http://www.w3.org/TR/2013/REC-prov-dm-20130430/#term-collection" ;
  owl:annotatedProperty rdfs:range ;
  owl:annotatedSource prov:hadMember ;
  owl:annotatedTarget prov:Entity ;
  prov:dm "http://www.w3.org/TR/2013/REC-prov-dm-20130430/#term-collection" ;
].
[
  rdf:type owl:Axiom ;
  rdfs:comment "Attribution is a particular case of trace (see http://www.w3.org/TR/prov-dm/#concept-trace), in the sense that it links an entity to the agent that ascribed it." ;
  owl:annotatedProperty rdfs:subPropertyOf ;
  owl:annotatedSource prov:wasAttributedTo ;
  owl:annotatedTarget prov:wasInfluencedBy ;
  prov:definition "IF wasAttributedTo(e2,ag1,aAttr) holds, THEN wasInfluencedBy(e2,ag1) also holds. " ;
].
[
  rdf:type owl:Axiom ;
  rdfs:comment "Derivation is a particular case of trace (see http://www.w3.org/TR/prov-dm/#term-trace), since it links an entity to another entity that contributed to its existence." ;
  owl:annotatedProperty rdfs:subPropertyOf ;
  owl:annotatedSource prov:wasDerivedFrom ;
  owl:annotatedTarget prov:wasInfluencedBy ;
].
[
  rdf:type owl:Axiom ;
  rdfs:comment "Quotation is a particular case of derivation (see http://www.w3.org/TR/prov-dm/#term-quotation) in which an entity is derived from an original entity by copying, or \"quoting\", some or all of it. " ;
  owl:annotatedProperty rdfs:subPropertyOf ;
  owl:annotatedSource prov:wasQuotedFrom ;
  owl:annotatedTarget prov:wasDerivedFrom ;
].
[
  rdf:type owl:Axiom ;
  rdfs:comment """Revision is a derivation (see http://www.w3.org/TR/prov-dm/#term-Revision). Moreover, according to 
http://www.w3.org/TR/2013/REC-prov-constraints-20130430/#term-Revision 23 April 2012 'wasRevisionOf is a strict sub-relation of wasDerivedFrom since two entities e2 and e1 may satisfy wasDerivedFrom(e2,e1) without being a variant of each other.'""" ;
  owl:annotatedProperty rdfs:subPropertyOf ;
  owl:annotatedSource prov:wasRevisionOf ;
  owl:annotatedTarget prov:wasDerivedFrom ;
].
[
  rdf:type owl:Axiom ;
  rdfs:comment "hadPrimarySource property is a particular case of wasDerivedFrom (see http://www.w3.org/TR/prov-dm/#term-original-source) that aims to give credit to the source that originated some information." ;
  owl:annotatedProperty rdfs:subPropertyOf ;
  owl:annotatedSource prov:hadPrimarySource ;
  owl:annotatedTarget prov:wasDerivedFrom ;
].
[
  rdf:type owl:Axiom ;
  rdfs:seeAlso "http://www.w3.org/TR/2013/REC-prov-dm-20130430/#term-influence" ;
  owl:annotatedProperty rdfs:domain ;
  owl:annotatedSource prov:wasInfluencedBy ;
  owl:annotatedTarget _:b895567 ;
  prov:definition "influencee: an identifier (o2) for an entity, activity, or agent; " ;
  prov:dm "http://www.w3.org/TR/2013/REC-prov-dm-20130430/#term-influence" ;
].
[
  rdf:type owl:Axiom ;
  rdfs:seeAlso "http://www.w3.org/TR/2013/REC-prov-dm-20130430/#term-influence" ;
  owl:annotatedProperty rdfs:range ;
  owl:annotatedSource prov:wasInfluencedBy ;
  owl:annotatedTarget _:b53184 ;
  prov:definition "influencer: an identifier (o1) for an ancestor entity, activity, or agent that the former depends on;" ;
  prov:dm "http://www.w3.org/TR/2013/REC-prov-dm-20130430/#term-influence" ;
].
